# baseURI: http://anzsoil.org/def/au/asls/soil-profile
# imports: http://anzsoil.org/def/au/asls/land-surface
# imports: http://anzsoil.org/def/au/asls/substrate
# imports: http://purl.org/dc/elements/1.1/

@prefix asls: <http://anzsoil.org/def/au/asls/> .
@prefix dc: <http://purl.org/dc/elements/1.1/> .
@prefix dcterms: <http://purl.org/dc/terms/> .
@prefix foaf: <http://xmlns.com/foaf/0.1/> .
@prefix ls: <http://anzsoil.org/def/au/asls/land-surface/> .
@prefix owl: <http://www.w3.org/2002/07/owl#> .
@prefix rdf: <http://www.w3.org/1999/02/22-rdf-syntax-ns#> .
@prefix rdfs: <http://www.w3.org/2000/01/rdf-schema#> .
@prefix schema: <https://schema.org/> .
@prefix skos: <http://www.w3.org/2004/02/skos/core#> .
@prefix sosa: <http://www.w3.org/ns/sosa/> .
@prefix sp: <http://anzsoil.org/def/au/asls/soil-profile/> .
@prefix subst: <http://anzsoil.org/def/au/asls/substrate/> .
@prefix xsd: <http://www.w3.org/2001/XMLSchema#> .

ls:Coarse-fragments-abundance
  a owl:Class ;
  a skos:Collection ;
  rdfs:isDefinedBy asls:soil-profile ;
  skos:inScheme asls:soil-profile ;
  rdfs:subClassOf skos:Concept ;
  skos:definition "The percentage of coarse fragments."@en ;
  skos:member ls:coarse-fragments-abundance-0 ;
  skos:member ls:coarse-fragments-abundance-1 ;
  skos:member ls:coarse-fragments-abundance-2 ;
  skos:member ls:coarse-fragments-abundance-3 ;
  skos:member ls:coarse-fragments-abundance-4 ;
  skos:member ls:coarse-fragments-abundance-5 ;
  skos:member ls:coarse-fragments-abundance-6 ;
  skos:note "The percentage is estimated by eye using the charts in the yellow book for comparison. N_CF_ABUN"@en ;
  skos:prefLabel "Abundance of coarse fragments - enumeration"@en ;
.
ls:Coarse-fragments-shape
  a owl:Class ;
  a skos:Collection ;
  rdfs:isDefinedBy asls:soil-profile ;
  skos:inScheme asls:soil-profile ;
  rdfs:comment "C_CF_SHAPE" ;
  rdfs:subClassOf skos:Concept ;
  skos:definition "The shape of coarse fragments is determined by referencing the chart that captures the roundness and sphericity. (Figure 12)"@en ;
  skos:member ls:coarse-fragments-shape-A ;
  skos:member ls:coarse-fragments-shape-AP ;
  skos:member ls:coarse-fragments-shape-AT ;
  skos:member ls:coarse-fragments-shape-R ;
  skos:member ls:coarse-fragments-shape-RP ;
  skos:member ls:coarse-fragments-shape-RT ;
  skos:member ls:coarse-fragments-shape-S ;
  skos:member ls:coarse-fragments-shape-SP ;
  skos:member ls:coarse-fragments-shape-ST ;
  skos:member ls:coarse-fragments-shape-U ;
  skos:member ls:coarse-fragments-shape-UP ;
  skos:member ls:coarse-fragments-shape-UT ;
  skos:prefLabel "Shape of coarse fragments - enumeration"@en ;
.
ls:Coarse-fragments-size
  a owl:Class ;
  a skos:Collection ;
  rdfs:isDefinedBy asls:soil-profile ;
  skos:inScheme asls:soil-profile ;
  rdfs:subClassOf skos:Concept ;
  skos:definition "The scale adopted employs class boundaries at (2 × 10n/2) mm, where n is an integer. This system is an extension of that used for particles smaller than 2 mm both in the scheme of the British Standards Institution and the Massachusetts Institute of Technology and the original Atterberg (1905) scheme on which the International Scheme was based. It is thus compatible with both the International Scheme referred to in the field texture section and the grain size criteria for substrate materials."@en ;
  skos:member ls:coarse-fragments-size-1 ;
  skos:member ls:coarse-fragments-size-2 ;
  skos:member ls:coarse-fragments-size-3 ;
  skos:member ls:coarse-fragments-size-4 ;
  skos:member ls:coarse-fragments-size-5 ;
  skos:member ls:coarse-fragments-size-6 ;
  skos:member ls:coarse-fragments-size-7 ;
  skos:note "Note that in preparing soils for laboratory analysis, the greater than 2mm size fraction is commonly recorded as 'gravel'."@en ;
  skos:note "The terms used to describe size apply to fragments of any shape: The average maximum dimension of fragments is used to determine the class interval. N_CF_SIZE"@en ;
  skos:prefLabel "Size of coarse fragments -enumeration"@en ;
.
ls:Coarse-fragments-strength
  a owl:Class ;
  a skos:Collection ;
  rdfs:isDefinedBy asls:soil-profile ;
  skos:inScheme asls:soil-profile ;
  rdfs:comment "C_CF_STRENGTH"@en ;
  rdfs:subClassOf skos:Concept ;
  owl:equivalentClass subst:Material-strength ;
  skos:altLabel "Strength of material"@en ;
  skos:definition "Strength of coarse fragments is the same as for 'Strength of material'. The strength of a specimen of soil substrate material may be crudely estimated in the field by striking it with the head-end or the pick-end of a geological hammer or by trying to cut it with a knife, and then referring to Table 32 (ASLS Field Handbook). These estimates refer to the unconfined (or uniaxial) compressive strength. The strength is that of the intact material rather than that of the mass, the strength of which has generally been reduced by the development of fractures and other phenomena."@en ;
  skos:member subst:material-strength-M ;
  skos:member subst:material-strength-S ;
  skos:member subst:material-strength-VS ;
  skos:member subst:material-strength-VW ;
  skos:member subst:material-strength-W ;
  skos:prefLabel "Strength of coarse fragments - enumeration"@en ;
.
ls:Lithology-coarse-fragments
  a owl:Class ;
  a skos:Collection ;
  rdfs:isDefinedBy asls:soil-profile ;
  skos:inScheme asls:soil-profile ;
  rdfs:subClassOf skos:Concept ;
  skos:definition "The lithology of the coarse fragments is usually identified as coming from the substrate or from rock outcrop. Where the lithology of the coarse fragments is different from that of the substrate material and/or rock outcrop, describe it as for lithology of substrate material only where the rock type is definitely known or is confidently presumed. Some coarse fragments are commonly encountered that are not directly related to the substrate material.    "@en ;
  skos:member ls:lithology-CC ;
  skos:member ls:lithology-IS ;
  skos:member ls:lithology-M ;
  skos:member ls:lithology-OT ;
  skos:member ls:lithology-OW ;
  skos:member ls:lithology-PU ;
  skos:member ls:lithology-R ;
  skos:member ls:lithology-SS ;
  skos:member subst:lithology-AC ;
  skos:member subst:lithology-AD ;
  skos:member subst:lithology-AF ;
  skos:member subst:lithology-AG ;
  skos:member subst:lithology-AH ;
  skos:member subst:lithology-AM ;
  skos:member subst:lithology-AN ;
  skos:member subst:lithology-AP ;
  skos:member subst:lithology-AR ;
  skos:member subst:lithology-AS ;
  skos:member subst:lithology-BA ;
  skos:member subst:lithology-BB ;
  skos:member subst:lithology-BO ;
  skos:member subst:lithology-BR ;
  skos:member subst:lithology-C ;
  skos:member subst:lithology-CB ;
  skos:member subst:lithology-CG ;
  skos:member subst:lithology-CH ;
  skos:member subst:lithology-CO ;
  skos:member subst:lithology-CU ;
  skos:member subst:lithology-DI ;
  skos:member subst:lithology-DM ;
  skos:member subst:lithology-DR ;
  skos:member subst:lithology-FC ;
  skos:member subst:lithology-GA ;
  skos:member subst:lithology-GD ;
  skos:member subst:lithology-GE ;
  skos:member subst:lithology-GN ;
  skos:member subst:lithology-GR ;
  skos:member subst:lithology-GS ;
  skos:member subst:lithology-GV ;
  skos:member subst:lithology-GW ;
  skos:member subst:lithology-GY ;
  skos:member subst:lithology-HA ;
  skos:member subst:lithology-HO ;
  skos:member subst:lithology-IG ;
  skos:member subst:lithology-JA ;
  skos:member subst:lithology-KA ;
  skos:member subst:lithology-KC ;
  skos:member subst:lithology-KL ;
  skos:member subst:lithology-KM ;
  skos:member subst:lithology-KR ;
  skos:member subst:lithology-KS ;
  skos:member subst:lithology-LC ;
  skos:member subst:lithology-LI ;
  skos:member subst:lithology-M ;
  skos:member subst:lithology-MB ;
  skos:member subst:lithology-MD ;
  skos:member subst:lithology-ME ;
  skos:member subst:lithology-MG ;
  skos:member subst:lithology-MI ;
  skos:member subst:lithology-ML ;
  skos:member subst:lithology-MS ;
  skos:member subst:lithology-MU ;
  skos:member subst:lithology-MY ;
  skos:member subst:lithology-PC ;
  skos:member subst:lithology-PE ;
  skos:member subst:lithology-PG ;
  skos:member subst:lithology-PH ;
  skos:member subst:lithology-PL ;
  skos:member subst:lithology-PO ;
  skos:member subst:lithology-PY ;
  skos:member subst:lithology-QP ;
  skos:member subst:lithology-QS ;
  skos:member subst:lithology-QU ;
  skos:member subst:lithology-QZ ;
  skos:member subst:lithology-R ;
  skos:member subst:lithology-RB ;
  skos:member subst:lithology-RH ;
  skos:member subst:lithology-S ;
  skos:member subst:lithology-SA ;
  skos:member subst:lithology-SD ;
  skos:member subst:lithology-SH ;
  skos:member subst:lithology-SK ;
  skos:member subst:lithology-SL ;
  skos:member subst:lithology-SN ;
  skos:member subst:lithology-SR ;
  skos:member subst:lithology-ST ;
  skos:member subst:lithology-SY ;
  skos:member subst:lithology-TR ;
  skos:member subst:lithology-TU ;
  skos:member subst:lithology-UC ;
  skos:member subst:lithology-VB ;
  skos:member subst:lithology-VG ;
  skos:member subst:lithology-Z ;
  skos:member subst:lithology-ZS ;
  skos:note "C_LITHOLOGY" ;
  skos:prefLabel "Lithology of coarse fragments - enumeration"@en ;
.
ls:coarse-fragments-abundance-0
  a skos:Concept ;
  skos:prefLabel "No coarse fragments"@en ;
.
ls:coarse-fragments-abundance-1
  a skos:Concept ;
  skos:prefLabel "Very slightly or very few"@en ;
.
ls:coarse-fragments-abundance-2
  a skos:Concept ;
  skos:prefLabel "Slightly or few"@en ;
.
ls:coarse-fragments-abundance-3
  a skos:Concept ;
  skos:prefLabel "No qualifier or common"@en ;
.
ls:coarse-fragments-abundance-4
  a skos:Concept ;
  skos:prefLabel "Moderately or many"@en ;
.
ls:coarse-fragments-abundance-5
  a skos:Concept ;
  skos:prefLabel "Very or abundant"@en ;
.
ls:coarse-fragments-abundance-6
  a skos:Concept ;
  skos:prefLabel "Extremely or very abundant"@en ;
.
ls:coarse-fragments-shape-A
  a skos:Concept ;
  skos:prefLabel "Angular"@en ;
.
ls:coarse-fragments-shape-AP
  a skos:Concept ;
  skos:prefLabel "Angular platy"@en ;
.
ls:coarse-fragments-shape-AT
  a skos:Concept ;
  skos:prefLabel "Angular tabular"@en ;
.
ls:coarse-fragments-shape-R
  a skos:Concept ;
  skos:prefLabel "Rounded"@en ;
.
ls:coarse-fragments-shape-RP
  a skos:Concept ;
  skos:prefLabel "Rounded platy"@en ;
.
ls:coarse-fragments-shape-RT
  a skos:Concept ;
  skos:prefLabel "Rounded tabular"@en ;
.
ls:coarse-fragments-shape-S
  a skos:Concept ;
  skos:prefLabel "Subangular"@en ;
.
ls:coarse-fragments-shape-SP
  a skos:Concept ;
  skos:prefLabel "Subangular platy"@en ;
.
ls:coarse-fragments-shape-ST
  a skos:Concept ;
  skos:prefLabel "Subangular tabular"@en ;
.
ls:coarse-fragments-shape-U
  a skos:Concept ;
  skos:prefLabel "Subrounded"@en ;
.
ls:coarse-fragments-shape-UP
  a skos:Concept ;
  skos:prefLabel "Subrounded platy"@en ;
.
ls:coarse-fragments-shape-UT
  a skos:Concept ;
  skos:prefLabel "Subrounded tabular"@en ;
.
ls:coarse-fragments-size-1
  a skos:Concept ;
  skos:prefLabel "Fine gravelly or small pebbles"@en ;
.
ls:coarse-fragments-size-2
  a skos:Concept ;
  skos:prefLabel "Medium gravelly or medium pebbles"@en ;
.
ls:coarse-fragments-size-3
  a skos:Concept ;
  skos:prefLabel "Coarse gravelly or large pebbles"@en ;
.
ls:coarse-fragments-size-4
  a skos:Concept ;
  skos:prefLabel "Cobbly or cobbles"@en ;
.
ls:coarse-fragments-size-5
  a skos:Concept ;
  skos:prefLabel "Stony or stones"@en ;
.
ls:coarse-fragments-size-6
  a skos:Concept ;
  skos:prefLabel "Bouldery or boulders"@en ;
.
ls:coarse-fragments-size-7
  a skos:Concept ;
  skos:prefLabel "Large boulders"@en ;
.
ls:lithology-CC
  a skos:Concept ;
  skos:prefLabel "Charcoal"@en ;
.
ls:lithology-IS
  a skos:Concept ;
  skos:prefLabel "Ironstone"@en ;
.
ls:lithology-M
  a skos:Concept ;
  skos:prefLabel "Same as substrate material"@en ;
.
ls:lithology-OT
  a skos:Concept ;
  skos:prefLabel "Other"@en ;
.
ls:lithology-OW
  a skos:Concept ;
  skos:prefLabel "Opalised wood"@en ;
.
ls:lithology-PU
  a skos:Concept ;
  skos:prefLabel "Pumice"@en ;
.
ls:lithology-R
  a skos:Concept ;
  skos:prefLabel "Same as rock outcrop"@en ;
.
ls:lithology-SS
  a skos:Concept ;
  skos:prefLabel "Shells"@en ;
.
asls:soil-profile
  a owl:Ontology ;
  a skos:ConceptScheme ;
  dcterms:contributor <https://orcid.org/0000-0002-0693-1899> ;
  dcterms:contributor <https://orcid.org/0000-0002-3884-3420> ;
  dcterms:created "2017-10-26"^^xsd:date ;
  dcterms:creator [
      a schema:Person ;
      schema:name "R.C. McDonald" ;
      schema:email ""^^xsd:anyURI ;
    ] ;
  dcterms:creator [
      a schema:Person ;
      schema:name "R.F. Isbell" ;
      schema:email ""^^xsd:anyURI ;
    ] ;
  skos:definition """This vocabulary is a machine-readable representation of the classifiers described in chapter 8 Soil Profile, by R.C. McDonald and R.F. Isbell, in Australian soil and land survey field handbook (3rd edn).
A soil profile is a vertical section of a soil from the soil surface through all its horizons to parent material, other consolidated substrate material or selected depth in unconsolidated material.""" ;
  dcterms:isFormatOf <https://catalogue.nla.gov.au/Record/4273240> ;
  schema:license <http://purl.org/NET/rdflicense/cc-by4.0> ;
  dcterms:modified "2025-06-07"^^xsd:date ;
  dcterms:publisher <https://linked.data.gov.au/org/csiro> ;
  dcterms:rights "copyright CSIRO 2009, 2021. All rights reserved."@en ;
  dcterms:source "National Committee on Soil and Terrain (2009), 'Australian soil and land survey field handbook (3rd edn).' (CSIRO Publishing: Melbourne)"@en ;
  dcterms:title "Soil Profile classifiers"@en ;
  rdfs:seeAlso <http://www.publish.csiro.au/nid/22/pid/5230.htm> ;
  owl:imports asls:land-surface ;
  owl:imports asls:substrate ;
  skos:changeNote "2025-06-07 - made VocPub conformant; used prefLabels for missing definitions" ;
  skos:changeNote "2020-09-16 - Added skos:inScheme and skos:topConceptOf links to asls:soil-profile; removed redundant owl:sameAs links" ;
  skos:changeNote "2021-04-07 - replace local lithology concepts with common lithology concepts from Substrate and Land-surface" ;
  skos:changeNote "2021-04-08 - replace local material strength concepts with common material strength concepts from Substrate" ;
  skos:changeNote "2022-02-25 - remove reg, ui, ldp components; remove top-concept links" ;
  skos:changeNote "2022-03-03	- minor clean up of structure, remove inScheme links; remove duplicate labels and descriptions in favour of skos prefLabel and definition" ;
  skos:changeNote "2022-07-27 - delete duplicate comment & label annotations" ;
  skos:changeNote "2022-07-28 - minor refactoring of Horizon collections" ;
  skos:changeNote "2022-07-29 - replace `sosa:ObservableProperty , skos:Concept` type on enumerations with `skos:related` link to the OP in the domain model" ;
  skos:changeNote "2022-11-23 - Rename collections for consistency with ANSIS" ;
  skos:changeNote "2022-12-07 - remove observable-properties collection" ;
  skos:historyNote "The data was converted from the print representation to this linked-data form by Linda Gregory assisted by Simon J D Cox" ;
  skos:notation "soil-profile"@en ;
  skos:prefLabel "Soil Profile classifiers"@en ;
.
sp:Artificial-aggregates-structure
  a owl:Class ;
  a skos:Collection ;
  rdfs:isDefinedBy asls:soil-profile ;
  skos:inScheme asls:soil-profile ;
  rdfs:subClassOf skos:Concept ;
  skos:definition "Cultivated horizons (Ap horizons) often consist of artificial aggregates formed by cultivation or work being done on the soil. The distinction between artificial aggregates and peds can be difficult. In cultivated horizons, where the pedologist is confident the aggregates are natural peds they should be recorded as such. If the pedologist is doubtful, or the aggregates are obviously artificial, they should be recorded as clods or fragments."@en ;
  skos:member sp:structure-artificial-CL ;
  skos:member sp:structure-artificial-FR ;
  skos:prefLabel "Structure of artificial aggregates"@en ;
.
sp:Boundary-distinctness
  a owl:Class ;
  a skos:Collection ;
  rdfs:isDefinedBy asls:soil-profile ;
  skos:inScheme asls:soil-profile ;
  dcterms:description "Distinctness of the boundaries between horizons"@en ;
  rdfs:comment "N_H_BOUND_DISTINCT" ;
  rdfs:subClassOf skos:Concept ;
  skos:definition "Distinctness of the boundaries between horizons"@en ;
  skos:member sp:horizon-boundary-distinctness-A ;
  skos:member sp:horizon-boundary-distinctness-C ;
  skos:member sp:horizon-boundary-distinctness-D ;
  skos:member sp:horizon-boundary-distinctness-G ;
  skos:member sp:horizon-boundary-distinctness-S ;
  skos:prefLabel "Boundary distinctness - enumeration"@en ;
.
sp:Boundary-shape
  a owl:Class ;
  a skos:Collection ;
  rdfs:isDefinedBy asls:soil-profile ;
  skos:inScheme asls:soil-profile ;
  dcterms:description "Shape of boundary between horizons"@en ;
  rdfs:comment "H_BOUND_SHAPE" ;
  rdfs:subClassOf skos:Concept ;
  skos:definition "Shape of boundary between horizons"@en ;
  skos:member sp:horizon-boundary-shape-B ;
  skos:member sp:horizon-boundary-shape-I ;
  skos:member sp:horizon-boundary-shape-S ;
  skos:member sp:horizon-boundary-shape-T ;
  skos:member sp:horizon-boundary-shape-W ;
  skos:prefLabel "Boundary shape - enumeration"@en ;
.
sp:Carbonate-effervescence
  a owl:Class ;
  a skos:Collection ;
  rdfs:isDefinedBy asls:soil-profile ;
  skos:inScheme asls:soil-profile ;
  rdfs:comment "C_H_CARBONATE_EFF" ;
  rdfs:subClassOf skos:Concept ;
  skos:definition "Effervescence of carbonate in fine earth using two or three drops of 1-molar HCl."@en ;
  skos:member sp:effervescence-H ;
  skos:member sp:effervescence-M ;
  skos:member sp:effervescence-N ;
  skos:member sp:effervescence-S ;
  skos:member sp:effervescence-V ;
  skos:prefLabel "Effervescence of carbonate in fine earth - enumeration"@en ;
.
sp:Coarse-fragments-distribution
  a owl:Class ;
  a skos:Collection ;
  rdfs:isDefinedBy asls:soil-profile ;
  skos:inScheme asls:soil-profile ;
  rdfs:comment "C_CF_DISTRIBUTION" ;
  rdfs:subClassOf skos:Concept ;
  skos:definition "Coarse fragments may occur throughout the profile."@en ;
  skos:member sp:coarse-fragments-distribution-D ;
  skos:member sp:coarse-fragments-distribution-R ;
  skos:member sp:coarse-fragments-distribution-S ;
  skos:member sp:coarse-fragments-distribution-U ;
  skos:prefLabel "Distribution of coarse fragments - enumeration"@en ;
.
sp:Colour-moisture-status
  a owl:Class ;
  a skos:Collection ;
  rdfs:isDefinedBy asls:soil-profile ;
  skos:inScheme asls:soil-profile ;
  rdfs:comment "C_MOISTURE_STAT"@en ;
  rdfs:subClassOf skos:Concept ;
  skos:definition "Moisture status for colour description"@en ;
  skos:member sp:colour-stat-D ;
  skos:member sp:colour-stat-M ;
  skos:prefLabel "Moisture status for colour description - enumeration"@en ;
.
sp:Consistence-plasticity-degree
  a owl:Class ;
  a skos:Collection ;
  rdfs:isDefinedBy asls:soil-profile ;
  skos:inScheme asls:soil-profile ;
  rdfs:comment "C_H_PLASTICITY_DEGREE" ;
  rdfs:subClassOf skos:Concept ;
  skos:definition "Plasticity is the ability to change shape and retain the new shape after the stress is removed. The degree of plasticity given below applies only to normal plasticity. The degree of plasticity is determined at the soil moisture content used for field texturing, that is, just below sticky point. The soil is rolled between the palms of the hand and, if possible, 40 mm long rolls are formed. The rolls are dangled from the thumb and forefinger. Plasticity is determined on the behaviour of rolls of varying thickness."@en ;
  skos:member sp:consistence-plasticity-degree-0 ;
  skos:member sp:consistence-plasticity-degree-1 ;
  skos:member sp:consistence-plasticity-degree-2 ;
  skos:member sp:consistence-plasticity-degree-3 ;
  skos:prefLabel "Plasticity Degree - enumeration"@en ;
.
sp:Consistence-plasticity-type
  a owl:Class ;
  a skos:Collection ;
  rdfs:isDefinedBy asls:soil-profile ;
  skos:inScheme asls:soil-profile ;
  rdfs:comment "C_H_PLASTICITY_TYPE" ;
  rdfs:subClassOf skos:Concept ;
  skos:definition "The type of plasticity refers to the degree to which either the consistence, field texture or both properties of a soil suggest the amount of clay-sized particles it contains (Butler 1955). It may be identified by determining two field textures: one after an initial 1 to 2 minute working of the soil sample, and another after a prolonged 10 minute kneading. The change in field texture from the initial to the prolonged working of the soil sample indicates the type of plasticity."@en ;
  skos:member sp:consistence-plasticity-type-N ;
  skos:member sp:consistence-plasticity-type-S ;
  skos:member sp:consistence-plasticity-type-T ;
  skos:member sp:consistence-plasticity-type-U ;
  skos:prefLabel "Plasticity Type - enumeration"@en ;
.
sp:Consistence-stickiness
  a owl:Class ;
  a skos:Collection ;
  rdfs:isDefinedBy asls:soil-profile ;
  skos:inScheme asls:soil-profile ;
  rdfs:comment "C_H_STICKINESS" ;
  rdfs:subClassOf skos:Concept ;
  skos:definition "Stickiness is determined on wet soil by pressing the wet sample between thumb and forefinger and then observing the adherence of the soil to the fingers."@en ;
  skos:member sp:consistence-stickiness-0 ;
  skos:member sp:consistence-stickiness-1 ;
  skos:member sp:consistence-stickiness-2 ;
  skos:member sp:consistence-stickiness-3 ;
  skos:prefLabel "Stickiness - enumeration"@en ;
.
sp:Consistence-strength
  a owl:Class ;
  a skos:Collection ;
  rdfs:isDefinedBy asls:soil-profile ;
  skos:inScheme asls:soil-profile ;
  rdfs:comment "C_STRG_CLASS" ;
  rdfs:subClassOf skos:Concept ;
  skos:definition """Strength of soil is the resistance to breaking or deformation. Strength is determined by the force just sufficient to break or deform a 20 mm diameter piece of soil when a compressive shearing force is applied between thumb and forefinger. The 20 mm piece of soil may be a ped, part of a ped, a compound ped or a fragment.

Forces 0 to 5 are equivalent to the following dry consistence classes in the ‘USDA Soil Survey Manual’ (Soil Survey Staff 1951):
0	Loose
1	Soft
2	Slightly hard
3	Hard
4	Very hard
5	Extremely hard"""@en ;
  skos:member sp:consistence-strength-0 ;
  skos:member sp:consistence-strength-1 ;
  skos:member sp:consistence-strength-2 ;
  skos:member sp:consistence-strength-3 ;
  skos:member sp:consistence-strength-4 ;
  skos:member sp:consistence-strength-5 ;
  skos:member sp:consistence-strength-6 ;
  skos:member sp:consistence-strength-7 ;
  skos:prefLabel "Strength - enumeration"@en ;
.
sp:Cracks-width
  a owl:Class ;
  a skos:Collection ;
  rdfs:isDefinedBy asls:soil-profile ;
  skos:inScheme asls:soil-profile ;
  rdfs:subClassOf skos:Concept ;
  skos:definition "Width of planar voids"@en ;
  skos:member sp:voids-cracks-1 ;
  skos:member sp:voids-cracks-2 ;
  skos:member sp:voids-cracks-3 ;
  skos:member sp:voids-cracks-4 ;
  skos:member sp:voids-cracks-5 ;
  skos:prefLabel "Width of cracks"@en ;
.
sp:Cutans-abundance
  a owl:Class ;
  a skos:Collection ;
  rdfs:isDefinedBy asls:soil-profile ;
  skos:inScheme asls:soil-profile ;
  rdfs:comment "N_CUTAN_ABUN" ;
  rdfs:subClassOf skos:Concept ;
  skos:definition "Abundance of cutans"@en ;
  skos:member sp:cutans-abundance-0 ;
  skos:member sp:cutans-abundance-1 ;
  skos:member sp:cutans-abundance-2 ;
  skos:member sp:cutans-abundance-3 ;
  skos:prefLabel "Abundance of cutans - enumeration"@en ;
.
sp:Cutans-distinctness
  a owl:Class ;
  a skos:Collection ;
  rdfs:isDefinedBy asls:soil-profile ;
  skos:inScheme asls:soil-profile ;
  rdfs:comment "C_CUTAN_DISTINCT" ;
  rdfs:subClassOf skos:Concept ;
  skos:definition "This refers to the ease and certainty with which a cutan is identified. Distinctness relates to thickness and to the colour contrast with the adjacent material; it may change markedly with moisture content."@en ;
  skos:member sp:cutans-distinctness-D ;
  skos:member sp:cutans-distinctness-F ;
  skos:member sp:cutans-distinctness-P ;
  skos:prefLabel "Distinctness of cutans - enumeration"@en ;
.
sp:Cutans-type
  a owl:Class ;
  a skos:Collection ;
  rdfs:isDefinedBy asls:soil-profile ;
  skos:inScheme asls:soil-profile ;
  rdfs:comment "C_CUTAN_TYPE" ;
  rdfs:subClassOf skos:Concept ;
  skos:definition "Types of cutans"@en ;
  skos:member sp:cutans-type-C ;
  skos:member sp:cutans-type-K ;
  skos:member sp:cutans-type-M ;
  skos:member sp:cutans-type-O ;
  skos:member sp:cutans-type-S ;
  skos:member sp:cutans-type-U ;
  skos:member sp:cutans-type-Z ;
  skos:prefLabel "Types of cutans - enumeration"@en ;
.
sp:Fabric-type
  a owl:Class ;
  a skos:Collection ;
  rdfs:isDefinedBy asls:soil-profile ;
  skos:inScheme asls:soil-profile ;
  rdfs:comment "C_FAB_TYPE" ;
  rdfs:subClassOf skos:Concept ;
  skos:definition """The definition of soil fabric in Australia is incomplete. The following description is adapted from Northcote (1979).
Fabric describes the appearance of the soil material (under ×10 hand lens). Differences in fabric are associated with the presence or absence of peds, the lustre or lack of lustre of the ped surfaces, and the presence, size and arrangement of pores (voids) in the soil mass. The descriptions given below apply primarily to B horizons."""@en ;
  skos:member sp:fabric-E ;
  skos:member sp:fabric-G ;
  skos:member sp:fabric-R ;
  skos:member sp:fabric-S ;
  skos:prefLabel "Fabric - enumeration"@en ;
.
sp:Field-texture-mineral
  a owl:Class ;
  a skos:Collection ;
  rdfs:isDefinedBy asls:soil-profile ;
  skos:inScheme asls:soil-profile ;
  dcterms:description """<p><img src=\"http://anzsoil.org/resources/yellowbook/Figure16.png\" /></p> 
<p> Figure 16 Triangular texture diagram based on International fractions (Marshall 1947). </p>"""^^rdf:HTML ;
  rdfs:subClassOf skos:Concept ;
  skos:definition """The following description of determination of field texture is adapted from Northcote (1979).
Field texture is a measure of the behaviour of a small handful of soil when moistened and kneaded into a ball and then pressed out between thumb and forefinger.
Take a sample of soil sufficient to fit comfortably into the palm of the hand. Moisten the soil with water, a little at a time, and knead until the ball of soil, so formed, just fails to stick to the fingers. Add more soil or water to attain this condition, known as the sticky point, which approximates field capacity for that soil. Continue kneading and moistening until there is no apparent change in the soil ball, usually a working time of 1–2 minutes. The soil ball, or bolus, is now ready for shearing manipulation, but the behaviour of the soil during bolus formation is also indicative of its field texture. The behaviour of the bolus and of the ribbon produced by shearing (pressing out) between thumb and forefinger characterises the field texture. Do not assess field texture grade solely on the length of ribbon.
The recommended field texture grades as characterised by the behaviour of the moist bolus are described. The approximate percentage content of clay (particles less than 0.002 mm in diameter) and silt (particles between 0.02 and 0.002 mm in diameter) are given as a guide. These percentages must not be used to determine a field texture, that is, do not use them to convert a laboratory particle size value to a field texture grade. Similarly, do not adjust a field texture grade when laboratory particle size data become available.""" ;
  skos:member sp:field-texture-CL ;
  skos:member sp:field-texture-CLS ;
  skos:member sp:field-texture-CS ;
  skos:member sp:field-texture-HC ;
  skos:member sp:field-texture-L ;
  skos:member sp:field-texture-LC ;
  skos:member sp:field-texture-LMC ;
  skos:member sp:field-texture-LS ;
  skos:member sp:field-texture-MC ;
  skos:member sp:field-texture-MHC ;
  skos:member sp:field-texture-S ;
  skos:member sp:field-texture-SCL ;
  skos:member sp:field-texture-SL ;
  skos:member sp:field-texture-ZCL ;
  skos:member sp:field-texture-ZL ;
  skos:prefLabel "Mineral soils field texture grade - enumeration"@en ;
.
sp:Field-texture-organic
  a owl:Class ;
  a skos:Collection ;
  rdfs:isDefinedBy asls:soil-profile ;
  skos:inScheme asls:soil-profile ;
  rdfs:subClassOf skos:Concept ;
  skos:definition "Organic soils do not have textural grades, as soil texture is determined by the size of mineral particles finer than 2 mm (NCST). In a sense, organic soils do have a texture related to the plant materials from which they formed and the degree of decomposition, exposure and drying. These field texture names may be used to characterise materials that on field examination are considered to be clearly dominated by organic matter. Peats may be assessed by examining the degree of decomposition and distinctness of plant remains. This work is adapted from Soil Survey Staff (1975) and Avery (1980)."@en ;
  skos:member sp:field-texture-AP ;
  skos:member sp:field-texture-CP ;
  skos:member sp:field-texture-GP ;
  skos:member sp:field-texture-HP ;
  skos:member sp:field-texture-IP ;
  skos:member sp:field-texture-LP ;
  skos:member sp:field-texture-SP ;
  skos:prefLabel "Organic soils field texture - enumeration"@en ;
.
sp:Field-texture-qualifier
  a owl:Class ;
  a skos:Collection ;
  rdfs:isDefinedBy asls:soil-profile ;
  skos:inScheme asls:soil-profile ;
  rdfs:subClassOf skos:Concept ;
  skos:definition """The non-clay field texture grades (clay loams and coarser) may be qualified according to whether they are at, or near, the light (lower clay content) or heavy (higher clay content) end of the range for that 
particular field texture grade. Note that clay field texture grades provide for light and heavy qualifiers in the clays and hence – and + are not required. 
If the soils are appreciably organic, they are qualified as Sapric or Fibric.
These codes are given after the field texture. For example, light sandy clay loam is coded SCL–, heavy sandy clay loam is coded SCL+, and fibric sandy loam is coded SLI.
It is strongly recommended that qualifiers only be used where considered essential. If too freely used, it can lead to excessive, unnecessary detail of doubtful usefulness."""@en ;
  skos:member sp:field-texture-qualifier-fibric ;
  skos:member sp:field-texture-qualifier-heavy ;
  skos:member sp:field-texture-qualifier-light ;
  skos:member sp:field-texture-qualifier-sapric ;
  skos:prefLabel "Field texture qualifier - enumeration"@en ;
.
sp:Horizon-code
  a owl:Class ;
  a skos:Collection ;
  rdfs:isDefinedBy asls:soil-profile ;
  skos:inScheme asls:soil-profile ;
  rdfs:subClassOf skos:Concept ;
  skos:definition """A soil horizon is a layer of soil, approximately parallel to the land surface, with morphological properties different from layers below and/or above it. Tongues of material from one horizon may penetrate into adjacent horizons. Give horizon notation as described below.

As horizon notation is deduced from the profile description data (Northcote 1979) and in some instances laboratory data, record it after the profile is described. Horizons may be difficult to name, but should be named in the field. Opinions formed at the time of description are useful for later reference.

With regard to horizon notation, the long-established usage in horizon designation is adopted. Emphasis is on factual objective notation rather than assumed genesis, as genetic implications are often uncertain and difficult to establish. Thus the notation E indicating eluvial horizon (International Society of Soil Science 1967) has not been used, even though this has been adopted by a number of overseas organisations, for example Hodgson (1974), Soil Survey Staff (1990).""" ;
  skos:member sp:horizons-A ;
  skos:member sp:horizons-B ;
  skos:member sp:horizons-C ;
  skos:member sp:horizons-D ;
  skos:member sp:horizons-O ;
  skos:member sp:horizons-P ;
  skos:member sp:horizons-R ;
  skos:prefLabel "Type of soil horizon - enumeration"@en ;
.
sp:Horizon-suffix
  a owl:Class ;
  a skos:Collection ;
  rdfs:isDefinedBy asls:soil-profile ;
  skos:inScheme asls:soil-profile ;
  rdfs:subClassOf skos:Concept ;
  skos:definition "The horizon's alphabetic suffix is used to further define the horizon. It always comes after the numeric subdivision except for suffix p, where the number always follows the letter (e.g. Ap2)."@en ;
  skos:member sp:horizon-suffix-b ;
  skos:member sp:horizon-suffix-c ;
  skos:member sp:horizon-suffix-d ;
  skos:member sp:horizon-suffix-e ;
  skos:member sp:horizon-suffix-f ;
  skos:member sp:horizon-suffix-g ;
  skos:member sp:horizon-suffix-h ;
  skos:member sp:horizon-suffix-j ;
  skos:member sp:horizon-suffix-k ;
  skos:member sp:horizon-suffix-m ;
  skos:member sp:horizon-suffix-p ;
  skos:member sp:horizon-suffix-q ;
  skos:member sp:horizon-suffix-r ;
  skos:member sp:horizon-suffix-s ;
  skos:member sp:horizon-suffix-t ;
  skos:member sp:horizon-suffix-w ;
  skos:member sp:horizon-suffix-x ;
  skos:member sp:horizon-suffix-y ;
  skos:member sp:horizon-suffix-z ;
  skos:prefLabel "Horizon suffixes"@en ;
.
sp:Mottle-abundance
  a owl:Class ;
  a skos:Collection ;
  rdfs:isDefinedBy asls:soil-profile ;
  skos:inScheme asls:soil-profile ;
  rdfs:comment "N_MOTT_ABUN" ;
  rdfs:subClassOf skos:Concept ;
  skos:definition "The percentage of mottles is estimated by eye using the chart in Figure 11 (ASLSFH3Ed) for comparison. "@en ;
  skos:member sp:mottle-abundance-0 ;
  skos:member sp:mottle-abundance-1 ;
  skos:member sp:mottle-abundance-2 ;
  skos:member sp:mottle-abundance-3 ;
  skos:member sp:mottle-abundance-4 ;
  skos:prefLabel "Mottle abundance - enumeration"@en ;
.
sp:Mottle-colour
  a owl:Class ;
  a skos:Collection ;
  rdfs:isDefinedBy asls:soil-profile ;
  skos:inScheme asls:soil-profile ;
  rdfs:comment "C_MOTT_COLOUR" ;
  rdfs:subClassOf skos:Concept ;
  skos:definition "This should be described in terms of Munsell or Revised Standard Soil colours, but abbreviated forms can be used"@en ;
  skos:member sp:mottle-colour-B ;
  skos:member sp:mottle-colour-D ;
  skos:member sp:mottle-colour-G ;
  skos:member sp:mottle-colour-L ;
  skos:member sp:mottle-colour-O ;
  skos:member sp:mottle-colour-P ;
  skos:member sp:mottle-colour-R ;
  skos:member sp:mottle-colour-Y ;
  skos:prefLabel "Mottle colour - enumeration"@en ;
.
sp:Mottle-contrast
  a owl:Class ;
  a skos:Collection ;
  rdfs:isDefinedBy asls:soil-profile ;
  skos:inScheme asls:soil-profile ;
  rdfs:comment "C_CONTRAST" ;
  rdfs:subClassOf skos:Concept ;
  skos:definition "Mottle contrast"@en ;
  skos:member sp:mottle-contrast-D ;
  skos:member sp:mottle-contrast-F ;
  skos:member sp:mottle-contrast-P ;
  skos:prefLabel "Mottle contrast - enumeration"@en ;
.
sp:Mottle-distinctness
  a owl:Class ;
  a skos:Collection ;
  rdfs:isDefinedBy asls:soil-profile ;
  skos:inScheme asls:soil-profile ;
  rdfs:comment "C_MOTT_BOUN_DISTINCT" ;
  rdfs:subClassOf skos:Concept ;
  skos:definition "Mottle distinctness of boundaries"@en ;
  skos:member sp:mottle-boundary-C ;
  skos:member sp:mottle-boundary-D ;
  skos:member sp:mottle-boundary-S ;
  skos:prefLabel "Mottle distinctness of boundaries - enumeration"@en ;
.
sp:Mottle-size
  a owl:Class ;
  a skos:Collection ;
  rdfs:isDefinedBy asls:soil-profile ;
  skos:inScheme asls:soil-profile ;
  rdfs:comment "N_MOTT_SIZE" ;
  rdfs:subClassOf skos:Concept ;
  skos:definition "Measure mottle size (mm) along the greatest dimension, except in streaks or linear forms where width is measured."@en ;
  skos:member sp:mottle-size-1 ;
  skos:member sp:mottle-size-2 ;
  skos:member sp:mottle-size-3 ;
  skos:member sp:mottle-size-4 ;
  skos:prefLabel "Mottle size - enumeration"@en ;
.
sp:Mottle-type
  a owl:Class ;
  a skos:Collection ;
  rdfs:isDefinedBy asls:soil-profile ;
  skos:inScheme asls:soil-profile ;
  rdfs:comment "C_MOTT_TYPE" ;
  rdfs:subClassOf skos:Concept ;
  skos:definition "The type of mottle can suggest the origin of the mottles."@en ;
  skos:member sp:mottle-type-M ;
  skos:member sp:mottle-type-X ;
  skos:member sp:mottle-type-Y ;
  skos:member sp:mottle-type-Z ;
  skos:prefLabel "Mottle or colour pattern type - enumeration"@en ;
.
sp:Pans-cementation
  a owl:Class ;
  a skos:Collection ;
  rdfs:isDefinedBy asls:soil-profile ;
  skos:inScheme asls:soil-profile ;
  rdfs:comment "C_PAN_CEMENTATION" ;
  rdfs:subClassOf skos:Concept ;
  skos:definition "Place a 30 mm diameter piece of the pan in water for 1 hour. If it slakes, it is uncemented; if not, it is cemented. The degree of cementation is assessed on the following scale after the 1 hour soaking in water."@en ;
  skos:member sp:pans-cementation-0 ;
  skos:member sp:pans-cementation-1 ;
  skos:member sp:pans-cementation-2 ;
  skos:member sp:pans-cementation-3 ;
  skos:member sp:pans-cementation-4 ;
  skos:prefLabel "Cementation of pan - enumeration"@en ;
.
sp:Pans-continuity
  a owl:Class ;
  a skos:Collection ;
  rdfs:isDefinedBy asls:soil-profile ;
  skos:inScheme asls:soil-profile ;
  rdfs:comment "C_PAN_CONTINUITY" ;
  rdfs:subClassOf skos:Concept ;
  skos:definition "Continuity of pan"@en ;
  skos:member sp:pans-continuity-B ;
  skos:member sp:pans-continuity-C ;
  skos:member sp:pans-continuity-D ;
  skos:prefLabel "Continuity of pan - enumeration"@en ;
.
sp:Pans-structure
  a owl:Class ;
  a skos:Collection ;
  rdfs:isDefinedBy asls:soil-profile ;
  skos:inScheme asls:soil-profile ;
  rdfs:comment "C_PAN_STRUCTURE" ;
  rdfs:subClassOf skos:Concept ;
  skos:definition "Structure of pan"@en ;
  skos:member sp:pans-structure-C ;
  skos:member sp:pans-structure-L ;
  skos:member sp:pans-structure-N ;
  skos:member sp:pans-structure-R ;
  skos:member sp:pans-structure-S ;
  skos:member sp:pans-structure-V ;
  skos:prefLabel "Structure of pan - enumeration"@en ;
.
sp:Pans-type
  a owl:Class ;
  a skos:Collection ;
  rdfs:isDefinedBy asls:soil-profile ;
  skos:inScheme asls:soil-profile ;
  rdfs:comment "C_PAN_TYPE" ;
  rdfs:subClassOf skos:Concept ;
  skos:definition "Type of pan"@en ;
  skos:member sp:pans-type-A ;
  skos:member sp:pans-type-C ;
  skos:member sp:pans-type-D ;
  skos:member sp:pans-type-E ;
  skos:member sp:pans-type-F ;
  skos:member sp:pans-type-I ;
  skos:member sp:pans-type-K ;
  skos:member sp:pans-type-L ;
  skos:member sp:pans-type-M ;
  skos:member sp:pans-type-N ;
  skos:member sp:pans-type-O ;
  skos:member sp:pans-type-R ;
  skos:member sp:pans-type-T ;
  skos:member sp:pans-type-V ;
  skos:member sp:pans-type-Z ;
  skos:prefLabel "Type of pan - enumeration"@en ;
.
sp:Particle-size-fractions
  a owl:Class ;
  a skos:Collection ;
  rdfs:isDefinedBy asls:soil-profile ;
  skos:inScheme asls:soil-profile ;
  dcterms:description """<p><img src=\"http://anzsoil.org/resources/yellowbook/Figure15.png\" /></p> 
<p> Figure 15 Size fractions in several major classification systems. </p>"""^^rdf:HTML ;
  rdfs:subClassOf skos:Concept ;
  skos:definition "Particle size is measured in the laboratory. The recommended scale in Australia uses these class boundaries for particle diameters, given in millimetres."@en ;
  skos:member sp:particle-size-fraction-boulders ;
  skos:member sp:particle-size-fraction-clay ;
  skos:member sp:particle-size-fraction-coarse-gravel ;
  skos:member sp:particle-size-fraction-coarse-sand ;
  skos:member sp:particle-size-fraction-cobbles ;
  skos:member sp:particle-size-fraction-fine-clay ;
  skos:member sp:particle-size-fraction-fine-gravel ;
  skos:member sp:particle-size-fraction-fine-sand ;
  skos:member sp:particle-size-fraction-medium-gravel ;
  skos:member sp:particle-size-fraction-sand ;
  skos:member sp:particle-size-fraction-silt ;
  skos:member sp:particle-size-fraction-stones ;
  skos:prefLabel "Particle size fractions (Australia)"@en ;
.
sp:Pedality-grade-apedal
  a owl:Class ;
  a skos:Collection ;
  rdfs:isDefinedBy asls:soil-profile ;
  skos:inScheme asls:soil-profile ;
  rdfs:subClassOf skos:Concept ;
  skos:definition "Apedal soils have no observable peds and are divided into:" ;
  skos:member sp:structure-pedality-grade-G ;
  skos:member sp:structure-pedality-grade-V ;
  skos:prefLabel "Apedal soil grades" ;
.
sp:Pedality-grade-pedal
  a owl:Class ;
  a skos:Collection ;
  rdfs:isDefinedBy asls:soil-profile ;
  skos:inScheme asls:soil-profile ;
  rdfs:subClassOf skos:Concept ;
  skos:definition "Pedal soils have observable peds and are divided into:" ;
  skos:member sp:structure-pedality-grade-M ;
  skos:member sp:structure-pedality-grade-S ;
  skos:member sp:structure-pedality-grade-W ;
  skos:prefLabel "Pedal soil grades - enumeration" ;
.
sp:Pedality-size
  a owl:Class ;
  a skos:Collection ;
  rdfs:isDefinedBy asls:soil-profile ;
  skos:inScheme asls:soil-profile ;
  rdfs:comment "N_STR_PED_SIZE" ;
  rdfs:subClassOf skos:Concept ;
  skos:definition "The average least dimension of peds is used to determine the class interval. Use figure 17. The least dimension is the vertical dimension for platy structure; the horizontal dimension for prismatic, columnar, blocky and polyhedral peds; the maximum separation of convex faces for lenticular peds; and the diameter for granular peds."@en ;
  skos:member sp:structure-pedality-size-1 ;
  skos:member sp:structure-pedality-size-2 ;
  skos:member sp:structure-pedality-size-3 ;
  skos:member sp:structure-pedality-size-4 ;
  skos:member sp:structure-pedality-size-5 ;
  skos:member sp:structure-pedality-size-6 ;
  skos:member sp:structure-pedality-size-7 ;
  skos:member sp:structure-pedality-size-8 ;
  skos:member sp:structure-pedality-size-9 ;
  skos:note "<p>Figure 17	Ped size. <img src=\"http://anzsoil.org/resources/yellowbook/Figure17.png\" alt=\"Ped Size\"/> </p>"^^rdf:HTML ;
  skos:prefLabel "Size of peds"@en ;
.
sp:Pedality-type
  a owl:Class ;
  a skos:Collection ;
  rdfs:isDefinedBy asls:soil-profile ;
  skos:inScheme asls:soil-profile ;
  rdfs:comment "C_STR_PED_TYPE" ;
  rdfs:subClassOf skos:Concept ;
  skos:definition "The types of structure are illustrated in diagrammatic form. See figure 17."@en ;
  skos:member sp:structure-pedality-type-AB ;
  skos:member sp:structure-pedality-type-CA ;
  skos:member sp:structure-pedality-type-CO ;
  skos:member sp:structure-pedality-type-GR ;
  skos:member sp:structure-pedality-type-LE ;
  skos:member sp:structure-pedality-type-PL ;
  skos:member sp:structure-pedality-type-PO ;
  skos:member sp:structure-pedality-type-PR ;
  skos:member sp:structure-pedality-type-SB ;
  skos:note "<p>Figure 17	Ped size. <img src=\"http://anzsoil.org/resources/yellowbook/Figure17.png\" alt=\"Ped Size\"/> </p>"^^rdf:HTML ;
  skos:prefLabel "Type of pedality"@en ;
.
sp:Pore-abundance-coarse
  a owl:Class ;
  a skos:Collection ;
  rdfs:isDefinedBy asls:soil-profile ;
  skos:inScheme asls:soil-profile ;
  rdfs:subClassOf skos:Concept ;
  skos:definition "Abundance of medium and coarse macropores (greater than 2 mm diameter)" ;
  skos:member sp:voids-macropores-abundance-0 ;
  skos:member sp:voids-macropores-abundance-4 ;
  skos:member sp:voids-macropores-abundance-5 ;
  skos:member sp:voids-macropores-abundance-6 ;
  skos:prefLabel "Abundance of medium and coarse macropores" ;
.
sp:Pore-abundance-fine
  a owl:Class ;
  a skos:Collection ;
  rdfs:isDefinedBy asls:soil-profile ;
  skos:inScheme asls:soil-profile ;
  rdfs:subClassOf skos:Concept ;
  skos:definition "Abundance of very fine and fine macropores (less than 2mm diameter)" ;
  skos:member sp:voids-macropores-abundance-0 ;
  skos:member sp:voids-macropores-abundance-1 ;
  skos:member sp:voids-macropores-abundance-2 ;
  skos:member sp:voids-macropores-abundance-3 ;
  skos:prefLabel "Abundance of very fine and fine macropores" ;
.
sp:Pore-diameter
  a owl:Class ;
  a skos:Collection ;
  rdfs:isDefinedBy asls:soil-profile ;
  skos:inScheme asls:soil-profile ;
  dcterms:description "<p>Figure 18	Size of macropores.<img src=\"http://anzsoil.org/resources/yellowbook/Figure18.png\" /></p>"^^rdf:HTML ;
  rdfs:comment "N_PORE_DIAMETER" ;
  rdfs:subClassOf skos:Concept ;
  skos:definition "Diameter of macropores Use Figure 18 as a guide to average diameter"@en ;
  skos:member sp:voids-macropores-diameter-1 ;
  skos:member sp:voids-macropores-diameter-2 ;
  skos:member sp:voids-macropores-diameter-3 ;
  skos:member sp:voids-macropores-diameter-4 ;
  skos:prefLabel "Diameter of macropores"@en ;
.
sp:Profile-construction
  a owl:Class ;
  a skos:Collection ;
  rdfs:isDefinedBy asls:soil-profile ;
  skos:inScheme asls:soil-profile ;
  rdfs:comment "C_O_TYPE" ;
  rdfs:subClassOf skos:Concept ;
  skos:definition "The soil profile may be described using several types of observation."@en ;
  skos:member sp:observation-type-A ;
  skos:member sp:observation-type-C ;
  skos:member sp:observation-type-E ;
  skos:member sp:observation-type-P ;
  skos:prefLabel "Type of soil observation - enumeration"@en ;
.
sp:Root-abundance
  a owl:Class ;
  a skos:Collection ;
  rdfs:isDefinedBy asls:soil-profile ;
  skos:inScheme asls:soil-profile ;
  dcterms:description "<p>Number of roots per 0.01 m<sup>2</sup> (100 mm × 100 mm)</p>"^^rdf:HTML ;
  rdfs:comment "N_ROOT_ABUN" ;
  rdfs:subClassOf skos:Concept ;
  skos:definition "Number of roots per 0.01 m2 (100 mm × 100 mm)"@en ;
  skos:member sp:roots-abundance-0 ;
  skos:member sp:roots-abundance-1 ;
  skos:member sp:roots-abundance-2 ;
  skos:member sp:roots-abundance-3 ;
  skos:member sp:roots-abundance-4 ;
  skos:prefLabel "Root abundance - enumeration"@en ;
.
sp:Root-size
  a owl:Class ;
  a skos:Collection ;
  rdfs:isDefinedBy asls:soil-profile ;
  skos:inScheme asls:soil-profile ;
  rdfs:comment "N_ROOT_SIZE" ;
  rdfs:subClassOf skos:Concept ;
  skos:definition "The size (diameter) of roots observed in the horizon in mm"@en ;
  skos:member sp:roots-size-1 ;
  skos:member sp:roots-size-2 ;
  skos:member sp:roots-size-3 ;
  skos:member sp:roots-size-4 ;
  skos:prefLabel "Root size - enumeration"@en ;
.
sp:Segregations-abundance
  a owl:Class ;
  a skos:Collection ;
  rdfs:isDefinedBy asls:soil-profile ;
  skos:inScheme asls:soil-profile ;
  dcterms:description "<p>Use Figure 11 as a guide <img src=\"http://anzsoil.org/resources/yellowbook/Figure11.png\" /></p>"^^rdf:HTML ;
  rdfs:comment "N_SEG_ABUN" ;
  rdfs:subClassOf skos:Concept ;
  skos:definition "Abundance of segregations. Use figure 11 as a guide."@en ;
  skos:member sp:segregations-abundance-0 ;
  skos:member sp:segregations-abundance-1 ;
  skos:member sp:segregations-abundance-2 ;
  skos:member sp:segregations-abundance-3 ;
  skos:member sp:segregations-abundance-4 ;
  skos:member sp:segregations-abundance-5 ;
  skos:prefLabel "Abundance of segregations - enumeration"@en ;
.
sp:Segregations-form
  a owl:Class ;
  a skos:Collection ;
  rdfs:isDefinedBy asls:soil-profile ;
  skos:inScheme asls:soil-profile ;
  rdfs:comment "C_SEG_FORM" ;
  rdfs:subClassOf skos:Concept ;
  skos:definition "Form of segregations"@en ;
  skos:member sp:segregations-form-C ;
  skos:member sp:segregations-form-F ;
  skos:member sp:segregations-form-L ;
  skos:member sp:segregations-form-N ;
  skos:member sp:segregations-form-R ;
  skos:member sp:segregations-form-S ;
  skos:member sp:segregations-form-T ;
  skos:member sp:segregations-form-V ;
  skos:member sp:segregations-form-X ;
  skos:prefLabel "Form of segregations - enumeration"@en ;
.
sp:Segregations-magnetic-attributes
  a owl:Class ;
  a skos:Collection ;
  rdfs:isDefinedBy asls:soil-profile ;
  skos:inScheme asls:soil-profile ;
  rdfs:comment "C_SEG_MAGNETIC_ATTR" ;
  rdfs:subClassOf skos:Concept ;
  skos:definition "attraction to surface of hand-held magnet"@en ;
  skos:member sp:segregations-magnetic-M ;
  skos:member sp:segregations-magnetic-N ;
  skos:prefLabel "Magnetic attributes of segregations - enumeration"@en ;
.
sp:Segregations-nature
  a owl:Class ;
  a skos:Collection ;
  rdfs:isDefinedBy asls:soil-profile ;
  skos:inScheme asls:soil-profile ;
  rdfs:comment "C_SEG_NATURE" ;
  rdfs:subClassOf skos:Concept ;
  skos:definition "Nature of segregations"@en ;
  skos:member sp:segregations-nature-A ;
  skos:member sp:segregations-nature-E ;
  skos:member sp:segregations-nature-F ;
  skos:member sp:segregations-nature-G ;
  skos:member sp:segregations-nature-H ;
  skos:member sp:segregations-nature-K ;
  skos:member sp:segregations-nature-L ;
  skos:member sp:segregations-nature-M ;
  skos:member sp:segregations-nature-N ;
  skos:member sp:segregations-nature-O ;
  skos:member sp:segregations-nature-S ;
  skos:member sp:segregations-nature-U ;
  skos:member sp:segregations-nature-Y ;
  skos:member sp:segregations-nature-Z ;
  skos:prefLabel "Nature of segregations - enumeration"@en ;
.
sp:Segregations-size
  a owl:Class ;
  a skos:Collection ;
  rdfs:isDefinedBy asls:soil-profile ;
  skos:inScheme asls:soil-profile ;
  rdfs:comment "N_SEG_SIZE" ;
  rdfs:subClassOf skos:Concept ;
  skos:definition "Approximately equidimensional segregations (concretions, nodules) are measured in the greatest dimension. Segregations where one dimension is much greater than the other two (tubules, root linings, veins, laminae) are measured in the least dimension"@en ;
  skos:member sp:segregations-size-1 ;
  skos:member sp:segregations-size-2 ;
  skos:member sp:segregations-size-3 ;
  skos:member sp:segregations-size-4 ;
  skos:member sp:segregations-size-5 ;
  skos:prefLabel "Size of segregations - enumeration"@en ;
.
sp:Segregations-strength
  a owl:Class ;
  a skos:Collection ;
  rdfs:isDefinedBy asls:soil-profile ;
  skos:inScheme asls:soil-profile ;
  rdfs:comment "C_SEG_STRENGTH" ;
  rdfs:subClassOf skos:Concept ;
  skos:definition "Strength may be recorded where appropriate"@en ;
  skos:member sp:segregations-strength-1 ;
  skos:member sp:segregations-strength-2 ;
  skos:prefLabel "Strength of segregations - enumeration"@en ;
.
sp:Site-drainage
  a owl:Class ;
  a skos:Collection ;
  rdfs:isDefinedBy asls:soil-profile ;
  skos:inScheme asls:soil-profile ;
  rdfs:comment "C_O_DRAINAGE" ;
  rdfs:subClassOf skos:Concept ;
  skos:definition "Drainage is a useful term to summarise local soil wetness conditions, that is, it provides a statement about soil and site drainage likely to occur in most years. It is affected by a number of attributes, both internal and external, that may act separately or together. Internal attributes include soil structure, texture, porosity, hydraulic conductivity, and water-holding capacity, while external attributes are source and quality of water, evapotranspiration, gradient and length of slope, and position in the landscape."@en ;
  skos:member sp:soil-water-drainage-1 ;
  skos:member sp:soil-water-drainage-2 ;
  skos:member sp:soil-water-drainage-3 ;
  skos:member sp:soil-water-drainage-4 ;
  skos:member sp:soil-water-drainage-5 ;
  skos:member sp:soil-water-drainage-6 ;
  skos:prefLabel "Drainage - enumeration"@en ;
.
sp:Soil-permeability
  a owl:Class ;
  a skos:Collection ;
  rdfs:isDefinedBy asls:soil-profile ;
  skos:inScheme asls:soil-profile ;
  rdfs:comment "C_PERMEABILITY" ;
  rdfs:subClassOf skos:Concept ;
  skos:definition "Permeability is independent of climate and drainage, and – as applied to a soil – is controlled by the potential to transmit water (saturated hydraulic conductivity, Ks) of the least permeable layer in the soil. Therefore it is inferred from attributes of the soil such as structure, texture, porosity, cracks and shrink–swell properties. The rate of transmission of water in the profile is based on the assumption that loss by evapotranspiration is minimal. The Ks ranges are compatible with those of Nowland in Canada, as reported by McKeague et al. (1982)."@en ;
  skos:member sp:soil-water-permeability-1 ;
  skos:member sp:soil-water-permeability-2 ;
  skos:member sp:soil-water-permeability-3 ;
  skos:member sp:soil-water-permeability-4 ;
  skos:prefLabel "Permeability - enumeration"@en ;
.
sp:Soil-water-status
  a owl:Class ;
  a skos:Collection ;
  rdfs:isDefinedBy asls:soil-profile ;
  skos:inScheme asls:soil-profile ;
  rdfs:subClassOf skos:Concept ;
  skos:definition """Give soil water status of the soil at the time of description.
It may also be relevant to note the weather conditions immediately prior to examination of the soil if these are known, for example a soil may be wet because of local rain or from seepage.
The following guidelines may be used as a crude approximation of soil water status:

Dry is below wilting point. Material becomes darker or has lower colour value when moistened.
Moderately moist is the drier half of the available moisture range.
Moist is the wetter half of the available moisture range.
Wet is at, or exceeding, field capacity. Will wet and/or stick to fingers when moulded."""@en ;
  skos:member sp:soil-water-status-D ;
  skos:member sp:soil-water-status-M ;
  skos:member sp:soil-water-status-T ;
  skos:member sp:soil-water-status-W ;
  skos:prefLabel "Soil water status"@en ;
.
sp:Surface-condition
  a owl:Class ;
  a skos:Collection ;
  rdfs:isDefinedBy asls:soil-profile ;
  skos:inScheme asls:soil-profile ;
  rdfs:subClassOf skos:Concept ;
  skos:definition "Many surface soils have a characteristic appearance when dry. Because surface conditions are often relevant to the use of the soil and indicative of particular kinds of soil, every effort should be made to observe the surface condition in the dry state. The surface conditions are not necessarily mutually exclusive:"@en ;
  skos:member sp:surfacecondition-C ;
  skos:member sp:surfacecondition-F ;
  skos:member sp:surfacecondition-G ;
  skos:member sp:surfacecondition-H ;
  skos:member sp:surfacecondition-L ;
  skos:member sp:surfacecondition-M ;
  skos:member sp:surfacecondition-O ;
  skos:member sp:surfacecondition-P ;
  skos:member sp:surfacecondition-R ;
  skos:member sp:surfacecondition-S ;
  skos:member sp:surfacecondition-T ;
  skos:member sp:surfacecondition-X ;
  skos:member sp:surfacecondition-Y ;
  skos:member sp:surfacecondition-Z ;
  skos:prefLabel "Condition of surface soil when dry - enumeration"@en ;
.
sp:Water-repellence
  a owl:Class ;
  a skos:Collection ;
  rdfs:isDefinedBy asls:soil-profile ;
  skos:inScheme asls:soil-profile ;
  rdfs:subClassOf skos:Concept ;
  skos:definition "Water repellence of some soils, usually sandy, is caused by a series of long-chain polymethylene waxes, made up of acids, alcohols and esters, attached to the sand grains (Ma’shum et al. 1988). These soils occur Australia-wide but are more widespread in southern Australia (Wetherby 1984, McGhie and Posner 1980). Degree of repellence is assessed by determining the concentration of ethanol required to wet the sand in 10 seconds (King 1981). An abbreviated form of this method is recommended for routine field situations."@en ;
  skos:member sp:water-repellence-N ;
  skos:member sp:water-repellence-R ;
  skos:member sp:water-repellence-S ;
  skos:note "Soil temperature at testing should be between 15ºC and 25ºC. Higher temperatures will increase, and lower decrease, rates of absorption. Industrial-grade methylated spirits, available from chemists, at a concentration of 23.9 ml per 200 ml water can be substituted for the 2-molar ethanol to obtain approximate values."@en ;
  skos:prefLabel "Water repellence"@en ;
.
sp:coarse-fragments
  a skos:Collection ;
  rdfs:isDefinedBy asls:soil-profile ;
  skos:inScheme asls:soil-profile ;
  skos:definition "Coarse fragments are particles coarser than 2 mm. They include unattached rock fragments and other fragments such as charcoal and shells. Coarse fragments are distinguished from segregations of pedogenic origin in that they are not, or not considered to be, of pedogenic origin. Coarse fragments may occur throughout the profile. Their abundance, size, shape, lithology and strength are described in exactly the same way on the surface as throughout the profile where their distribution is also described."@en ;
  skos:member ls:Coarse-fragments-abundance ;
  skos:member ls:Coarse-fragments-shape ;
  skos:member ls:Coarse-fragments-size ;
  skos:member ls:Coarse-fragments-strength ;
  skos:member ls:Lithology-coarse-fragments ;
  skos:member sp:Coarse-fragments-distribution ;
  skos:prefLabel "Coarse fragments"@en ;
.
sp:coarse-fragments-distribution-D
  a sp:Coarse-fragments-distribution ;
  a skos:Concept ;
  rdfs:comment "C_CF_DISTRIBUTION" ;
  skos:definition "fragments are scattered randomly throughout the soil and may be of mixed origin."@en ;
  skos:notation "D" ;
  skos:prefLabel "Dispersed"@en ;
.
sp:coarse-fragments-distribution-R
  a sp:Coarse-fragments-distribution ;
  a skos:Concept ;
  rdfs:comment "C_CF_DISTRIBUTION" ;
  skos:definition "all fragments are remnants of the underlying bedrock but their orientation is not related to the joint or bedding planes of the bedrock."@en ;
  skos:notation "R" ;
  skos:prefLabel "Reoriented"@en ;
.
sp:coarse-fragments-distribution-S
  a sp:Coarse-fragments-distribution ;
  a skos:Concept ;
  rdfs:comment "C_CF_DISTRIBUTION" ;
  skos:definition "fragments occur in bands, usually parallel with the soil surface (excluding those parallel with joint or bedding planes of the bedrock). They may include materials other than those from the underlying bedrock."@en ;
  skos:notation "S" ;
  skos:prefLabel "Stratified"@en ;
.
sp:coarse-fragments-distribution-U
  a sp:Coarse-fragments-distribution ;
  a skos:Concept ;
  rdfs:comment "C_CF_DISTRIBUTION" ;
  skos:definition "all fragments are remnants of the underlying bedrock and their orientation closely parallels that of the joint or bedding planes of the bedrock."@en ;
  skos:notation "U" ;
  skos:prefLabel "Undisturbed"@en ;
.
sp:colour
  a owl:Class ;
  a skos:Collection ;
  rdfs:isDefinedBy asls:soil-profile ;
  skos:inScheme asls:soil-profile ;
  rdfs:subClassOf skos:Concept ;
  skos:definition """Record colours by comparing soils with colour charts using the Munsell Color system, for example the Munsell Soil Color Charts or the Revised Standard Soil Color Charts (Oyama and Takehara 1970).
Hue, value and chroma of the matrix colour are recorded, for example 10YR4/2.
Soil colours rarely match the chart colour chips perfectly. They should be matched to the chip closest in colour, or the nearest whole number in chroma where chips are not provided, for example chromas 5 and 7.
The soil colour is measured on the surface of a freshly broken aggregate of moist soil. Moisten the soil if it is dry. Record the colour when the visible moisture film disappears from the surface of the moistened broken aggregate. The aggregate should be held as close as possible to the colour chips. Take care not to smear the broken surface, as this can give an incorrect recording of the colour of the soil matrix.
Dry colours may also be recorded."""@en ;
  skos:member sp:Colour-moisture-status ;
  skos:member sp:colour-value ;
  skos:note "A moisture status must be recorded with the colour description"@en ;
  skos:prefLabel "Colour"@en ;
.
sp:colour-stat-D
  a sp:Colour-moisture-status ;
  a skos:Concept ;
  skos:definition "Dry"@en ;
  skos:notation "D" ;
  skos:prefLabel "Dry (colour status)"@en ;
.
sp:colour-stat-M
  a sp:Colour-moisture-status ;
  a skos:Concept ;
  skos:definition "Moist"@en ;
  skos:notation "M" ;
  skos:prefLabel "Moist"@en ;
.
sp:colour-value
  a sp:colour ;
  a skos:Concept ;
  skos:definition """Record colours by comparing soils with colour charts using the Munsell Color system, for example the Munsell Soil Color Charts or the Revised Standard Soil Color Charts (Oyama and Takehara 1970).
Hue, value and chroma of the matrix colour are recorded, for example 10YR4/2.
Soil colours rarely match the chart colour chips perfectly. They should be matched to the chip closest in colour, or the nearest whole number in chroma where chips are not provided, for example chromas 5 and 7.
The soil colour is measured on the surface of a freshly broken aggregate of moist soil. Moisten the soil if it is dry. Record the colour when the visible moisture film disappears from the surface of the moistened broken aggregate. The aggregate should be held as close as possible to the colour chips. Take care not to smear the broken surface, as this can give an incorrect recording of the colour of the soil matrix.
Dry colours may also be recorded."""@en ;
  skos:note "A moisture status must be recorded with the colour description"@en ;
  skos:prefLabel "Colour value"@en ;
.
sp:consistence
  a skos:Collection ;
  rdfs:isDefinedBy asls:soil-profile ;
  skos:inScheme asls:soil-profile ;
  skos:definition "Consistence refers to the strength of cohesion and adhesion in soil. Strength will vary according to soil water status. Note that soil water status must be recorded with strength."@en ;
  skos:member sp:Consistence-plasticity-degree ;
  skos:member sp:Consistence-plasticity-type ;
  skos:member sp:Consistence-stickiness ;
  skos:member sp:Consistence-strength ;
  skos:prefLabel "Consistence"@en ;
.
sp:consistence-plasticity-degree-0
  a sp:Consistence-plasticity-degree ;
  a skos:Concept ;
  rdfs:comment "C_H_PLASTICITY_DEGREE" ;
  skos:definition "Roll (40mm length x 6mm diameter) will not form."@en ;
  skos:notation "0" ;
  skos:prefLabel "Non-plastic"@en ;
.
sp:consistence-plasticity-degree-1
  a sp:Consistence-plasticity-degree ;
  a skos:Concept ;
  rdfs:comment "C_H_PLASTICITY_DEGREE" ;
  skos:definition """Roll (40mm length x 6mm diameter) will form and will support its own weight.
Roll (40mm length x 4mm diameter) will form but will not support its own weight."""@en ;
  skos:notation "1" ;
  skos:prefLabel "Slightly plastic"@en ;
.
sp:consistence-plasticity-degree-2
  a sp:Consistence-plasticity-degree ;
  a skos:Concept ;
  rdfs:comment "C_H_PLASTICITY_DEGREE" ;
  skos:definition """Roll (40mm length x 4mm diameter) will form and will support its own weight.
Roll (40mm length x 2mm diameter) will form but will not support its own weight."""@en ;
  skos:notation "2" ;
  skos:prefLabel "Moderately plastic"@en ;
.
sp:consistence-plasticity-degree-3
  a sp:Consistence-plasticity-degree ;
  a skos:Concept ;
  rdfs:comment "C_H_PLASTICITY_DEGREE" ;
  skos:definition "Roll (40mm length x 2mm diameter) will form and will support its own weight."@en ;
  skos:notation "3" ;
  skos:prefLabel "Very plastic"@en ;
.
sp:consistence-plasticity-type-N
  a sp:Consistence-plasticity-type ;
  a skos:Concept ;
  rdfs:comment "C_H_PLASTICITY_TYPE" ;
  skos:definition "negligible change."@en ;
  skos:notation "N" ;
  skos:prefLabel "Normal plasticity"@en ;
.
sp:consistence-plasticity-type-S
  a sp:Consistence-plasticity-type ;
  a skos:Concept ;
  rdfs:comment "C_H_PLASTICITY_TYPE" ;
  skos:definition "decreases one or more field texture groups of Northcote (1979)."@en ;
  skos:notation "S" ;
  skos:prefLabel "Superplastic"@en ;
.
sp:consistence-plasticity-type-T
  a sp:Consistence-plasticity-type ;
  a skos:Concept ;
  rdfs:comment "C_H_PLASTICITY_TYPE" ;
  skos:definition "increases two or more field texture groups."@en ;
  skos:notation "T" ;
  skos:prefLabel "Strongly subplastic"@en ;
.
sp:consistence-plasticity-type-U
  a sp:Consistence-plasticity-type ;
  a skos:Concept ;
  dcterms:description "ncreases one to two field texture groups."@en ;
  rdfs:comment "C_H_PLASTICITY_TYPE" ;
  skos:definition "increases one to two field texture groups."@en ;
  skos:notation "U" ;
  skos:prefLabel "Subplastic"@en ;
.
sp:consistence-stickiness-0
  a sp:Consistence-stickiness ;
  a skos:Concept ;
  rdfs:comment "C_H_STICKINESS" ;
  skos:definition "little or no soil adheres."@en ;
  skos:notation "0" ;
  skos:prefLabel "Non-sticky"@en ;
.
sp:consistence-stickiness-1
  a sp:Consistence-stickiness ;
  a skos:Concept ;
  rdfs:comment "C_H_STICKINESS" ;
  skos:definition "soil adheres to thumb and forefinger but is not stretched notably and comes off rather cleanly."@en ;
  skos:notation "1" ;
  skos:prefLabel "Slightly sticky"@en ;
.
sp:consistence-stickiness-2
  a sp:Consistence-stickiness ;
  a skos:Concept ;
  rdfs:comment "C_H_STICKINESS" ;
  skos:definition "soil adheres to thumb and forefinger and tends to stretch rather than pull free of fingers."@en ;
  skos:notation "2" ;
  skos:prefLabel "Moderately sticky"@en ;
.
sp:consistence-stickiness-3
  a sp:Consistence-stickiness ;
  a skos:Concept ;
  rdfs:comment "C_H_STICKINESS" ;
  skos:definition "soil adheres strongly to thumb and forefinger and stretches notably."@en ;
  skos:notation "3" ;
  skos:prefLabel "Very sticky"@en ;
.
sp:consistence-strength-0
  a sp:Consistence-strength ;
  a skos:Concept ;
  rdfs:comment "C_STRG_CLASS" ;
  skos:definition "no force required. Separate particles such as loose sands."@en ;
  skos:notation "0" ;
  skos:note "Equivalent '0 Loose' dry consistence class in the USDA soil survey manual (Soil Survey Staff 1951)" ;
  skos:prefLabel "Loose (consistence strength)"@en ;
.
sp:consistence-strength-1
  a sp:Consistence-strength ;
  a skos:Concept ;
  rdfs:comment "C_STRG_CLASS" ;
  skos:definition "very small force, almost nil."@en ;
  skos:notation "1" ;
  skos:note "Equivalent '1 Soft' dry consistence class in the USDA soil survey manual (Soil Survey Staff 1951)" ;
  skos:prefLabel "Very weak (consistence strength)"@en ;
.
sp:consistence-strength-2
  a sp:Consistence-strength ;
  a skos:Concept ;
  rdfs:comment "C_STRG_CLASS" ;
  skos:definition "small but significant force."@en ;
  skos:notation "2" ;
  skos:note "Equivalent '2 Slightly hard' dry consistence class in the USDA soil survey manual (Soil Survey Staff 1951)" ;
  skos:prefLabel "Weak (consistence strength)"@en ;
.
sp:consistence-strength-3
  a sp:Consistence-strength ;
  a skos:Concept ;
  rdfs:comment "C_STRG_CLASS" ;
  skos:definition "moderate or firm force."@en ;
  skos:notation "3" ;
  skos:note "Equivalent '3 Hard' dry consistence class in the USDA soil survey manual (Soil Survey Staff 1951)" ;
  skos:prefLabel "Firm (consistence strength)"@en ;
.
sp:consistence-strength-4
  a sp:Consistence-strength ;
  a skos:Concept ;
  rdfs:comment "C_STRG_CLASS" ;
  skos:definition "strong force but within power of thumb and forefinger."@en ;
  skos:notation "4" ;
  skos:note "Equivalent '4 Very hard' dry consistence class in the USDA soil survey manual (Soil Survey Staff 1951)" ;
  skos:prefLabel "Very Firm (consistence strength)"@en ;
.
sp:consistence-strength-5
  a sp:Consistence-strength ;
  a skos:Concept ;
  rdfs:comment "C_STRG_CLASS" ;
  skos:definition "beyond power of thumb and forefinger. Crushes underfoot on hard, flat surface with small force."@en ;
  skos:notation "5" ;
  skos:note "Equivalent '5 Extremely hard' dry consistence class in the USDA soil survey manual (Soil Survey Staff 1951)" ;
  skos:prefLabel "Strong (consistence strength)"@en ;
.
sp:consistence-strength-6
  a sp:Consistence-strength ;
  a skos:Concept ;
  rdfs:comment "C_STRG_CLASS" ;
  skos:definition "crushes underfoot on hard, flat surface with full body weight applied slowly."@en ;
  skos:notation "6" ;
  skos:prefLabel "Very Strong (consistence strength)"@en ;
.
sp:consistence-strength-7
  a sp:Consistence-strength ;
  a skos:Concept ;
  rdfs:comment "C_STRG_CLASS" ;
  skos:definition "cannot be crushed underfoot by full body weight applied slowly."@en ;
  skos:notation "7" ;
  skos:prefLabel "Rigid (consistence strength)"@en ;
.
sp:cutans
  a skos:Collection ;
  rdfs:isDefinedBy asls:soil-profile ;
  skos:inScheme asls:soil-profile ;
  skos:definition """A cutan is a modification of the texture, structure or fabric at natural surfaces in soil materials; it arises from concentration of particular soil constituents or in situ modification of the plasma. Cutans comprise any of the component substances of the soil material (Brewer 1964).

Cutans may be observed in the field (a ×10 hand lens is usually necessary) but their nature is often difficult to determine unless a thin section is made. Hence the following simple classification."""@en ;
  skos:member sp:Cutans-abundance ;
  skos:member sp:Cutans-distinctness ;
  skos:member sp:Cutans-type ;
  skos:prefLabel "Cutans"@en ;
.
sp:cutans-abundance-0
  a sp:Cutans-abundance ;
  a skos:Concept ;
  rdfs:comment "N_CUTAN_ABUN" ;
  skos:definition "0"@en ;
  skos:notation "0" ;
  skos:prefLabel "No cutans"@en ;
.
sp:cutans-abundance-1
  a sp:Cutans-abundance ;
  a skos:Concept ;
  rdfs:comment "N_CUTAN_ABUN" ;
  skos:definition "<10% of ped faces or pore walls with cutans."@en ;
  skos:notation "1" ;
  skos:prefLabel "Few (cutans abundance)"@en ;
.
sp:cutans-abundance-2
  a sp:Cutans-abundance ;
  a skos:Concept ;
  rdfs:comment "N_CUTAN_ABUN" ;
  skos:definition "10–50% of ped faces or pore walls with cutans."@en ;
  skos:notation "2" ;
  skos:prefLabel "Common (cutans abundance)"@en ;
.
sp:cutans-abundance-3
  a sp:Cutans-abundance ;
  a skos:Concept ;
  rdfs:comment "N_CUTAN_ABUN" ;
  skos:definition ">50% of ped faces or pore walls with cutans."@en ;
  skos:notation "3" ;
  skos:prefLabel "Many (cutans abundance)"@en ;
.
sp:cutans-distinctness-D
  a sp:Cutans-distinctness ;
  a skos:Concept ;
  rdfs:comment "C_CUTAN_DISTINCT" ;
  skos:definition "can be detected without magnification. Contrast with adjacent material is evident in colour, texture or other properties."@en ;
  skos:notation "D" ;
  skos:prefLabel "Distinct (cutans distinctness)"@en ;
.
sp:cutans-distinctness-F
  a sp:Cutans-distinctness ;
  a skos:Concept ;
  rdfs:comment "C_CUTAN_DISTINCT" ;
  skos:definition "evident only on close examination with ×10 magnification. Little contrast with adjacent material."@en ;
  skos:notation "F" ;
  skos:prefLabel "Faint (cutans distinctness)"@en ;
.
sp:cutans-distinctness-P
  a sp:Cutans-distinctness ;
  a skos:Concept ;
  rdfs:comment "C_CUTAN_DISTINCT" ;
  skos:definition "conspicuous without magnification when compared with a surface broken through the soil. Colour, texture or some other property contrasts sharply with properties of the adjacent material, or the feature is thick enough to be conspicuous."@en ;
  skos:notation "P" ;
  skos:prefLabel "Prominent (cutans distinctness)"@en ;
.
sp:cutans-type-C
  a sp:Cutans-type ;
  a skos:Concept ;
  rdfs:comment "C_CUTAN_TYPE" ;
  skos:definition "coatings of clay often different in colour from the matrix of the ped. They are frequently difficult to distinguish from stress cutans, which are not true coatings."@en ;
  skos:notation "C" ;
  skos:prefLabel "Clay skins"@en ;
.
sp:cutans-type-K
  a sp:Cutans-type ;
  a skos:Concept ;
  rdfs:comment "C_CUTAN_TYPE" ;
  skos:definition "stress cutans with smooth striations or grooves."@en ;
  skos:notation "K" ;
  skos:prefLabel "Slickensides"@en ;
.
sp:cutans-type-M
  a sp:Cutans-type ;
  a skos:Concept ;
  rdfs:comment "C_CUTAN_TYPE" ;
  skos:definition "coatings of manganese oxides or hydroxides. The material may have a glazed appearance and is very dark brown to black."@en ;
  skos:notation "M" ;
  skos:prefLabel "Mangans"@en ;
.
sp:cutans-type-O
  a sp:Cutans-type ;
  a skos:Concept ;
  rdfs:comment "C_CUTAN_TYPE" ;
  skos:definition "may be composed of iron oxides, organic matter, calcium carbonate or gypsum."@en ;
  skos:notation "O" ;
  skos:prefLabel "Other cutans"@en ;
.
sp:cutans-type-S
  a sp:Cutans-type ;
  a skos:Concept ;
  rdfs:comment "C_CUTAN_TYPE" ;
  skos:definition "in situ modifications of natural surfaces in soil materials due to differential forces such as shearing. They are not true coatings."@en ;
  skos:notation "S" ;
  skos:prefLabel "Stress cutans"@en ;
.
sp:cutans-type-U
  a sp:Cutans-type ;
  a skos:Concept ;
  rdfs:comment "C_CUTAN_TYPE" ;
  skos:definition "nature of cutans cannot be determined."@en ;
  skos:notation "U" ;
  skos:prefLabel "Unspecified"@en ;
.
sp:cutans-type-Z
  a sp:Cutans-type ;
  a skos:Concept ;
  rdfs:comment "C_CUTAN_TYPE" ;
  skos:definition "Zero or no cutans."@en ;
  skos:notation "Z" ;
  skos:prefLabel "Zero or no cutans"@en ;
.
sp:depth-of-horizon
  a sp:horizons ;
  a skos:Concept ;
  skos:definition """The upper and lower depths, in metres, of each horizon are measured from the soil surface, excluding O horizons. O horizon depths are measured above the mineral soil surface, for example O1 0.120.10 m, O2 0.10.0 m.
A scaled horizon diagram may be useful where horizons are irregular."""@en ;
  skos:narrower sp:depth-of-horizon-lower ;
  skos:narrower sp:depth-of-horizon-upper ;
  skos:prefLabel "Depth of Horizons"@en ;
.
sp:depth-of-horizon-lower
  a skos:Concept ;
  skos:prefLabel "Lower depth of soil horizon in metres" ;
.
sp:depth-of-horizon-upper
  a skos:Concept ;
  skos:prefLabel "Upper depth of soil horizon in metres" ;
.
sp:depth-to-r-horizon
  a sp:horizons ;
  a skos:Concept ;
  skos:definition """Give depth to R horizon or strongly cemented pan in metres.
The purpose of recording this depth is to include in the soil description those materials that may be relatively easily moved by earth-moving equipment or may be relatively easily penetrated by roots. Strong or very strong rock or pan that may require ripping or blasting to move, and/or has little or no root penetration, is excluded"""@en ;
  skos:prefLabel "Depth to R horizon or strongly cemented pan"@en ;
.
sp:effervescence-H
  a sp:Carbonate-effervescence ;
  a skos:Concept ;
  rdfs:comment "C_H_CARBONATE_EFF" ;
  skos:definition "moderate visible effervescence."@en ;
  skos:notation "H" ;
  skos:prefLabel "Highly calcareous"@en ;
.
sp:effervescence-M
  a sp:Carbonate-effervescence ;
  a skos:Concept ;
  rdfs:comment "C_H_CARBONATE_EFF" ;
  skos:definition "audible and slightly visible effervescence."@en ;
  skos:notation "M" ;
  skos:prefLabel "Moderately calcareous"@en ;
.
sp:effervescence-N
  a sp:Carbonate-effervescence ;
  a skos:Concept ;
  rdfs:comment "C_H_CARBONATE_EFF" ;
  skos:definition "no audible or visible effervescence."@en ;
  skos:notation "N" ;
  skos:prefLabel "Non-calcareous"@en ;
.
sp:effervescence-S
  a sp:Carbonate-effervescence ;
  a skos:Concept ;
  rdfs:comment "C_H_CARBONATE_EFF" ;
  skos:definition "slightly audible but no visible effervescence."@en ;
  skos:notation "S" ;
  skos:prefLabel "Slightly calcareous"@en ;
.
sp:effervescence-V
  a sp:Carbonate-effervescence ;
  a skos:Concept ;
  rdfs:comment "C_H_CARBONATE_EFF" ;
  skos:definition "strong visible effervescence."@en ;
  skos:notation "V" ;
  skos:prefLabel "Very highly calcareous"@en ;
.
sp:fabric-E
  a sp:Fabric-type ;
  a skos:Concept ;
  rdfs:comment "C_FAB_TYPE" ;
  skos:altLabel "Porous"@en ;
  skos:definition "The soil material is coherent and characterised by the presence of pores (voids) and few, if any, peds. Ultimate soil particles (sand grains, for example) are coated with oxides and/or clays and are arranged (clumped) around the pores."@en ;
  skos:notation "E" ;
  skos:prefLabel "Earthy (fabric)"@en ;
.
sp:fabric-G
  a sp:Fabric-type ;
  a skos:Concept ;
  rdfs:comment "C_FAB_TYPE" ;
  skos:definition "The soil material is coherent, with few, if any, peds. The closely packed sand grains provide the characteristic appearance of the soil mass."@en ;
  skos:notation "G" ;
  skos:prefLabel "Sandy (grains prominent)"@en ;
.
sp:fabric-R
  a sp:Fabric-type ;
  a skos:Concept ;
  rdfs:comment "C_FAB_TYPE" ;
  skos:definition "Peds are evident, and characteristically more than 50% of the peds are rough-faced, that is, they have relatively porous surfaces. (Rough-faced peds generally have less clearly defined faces than smooth-faced peds and the pedality of the soil may be questioned. However, if the soil mass is pressed gently, the characteristic size and shape of the soil aggregates will confirm its pedality.) Granular peds with common or many macropores are always rough-faced, but this condition varies in other ped forms."@en ;
  skos:notation "R" ;
  skos:prefLabel "Rough-ped"@en ;
.
sp:fabric-S
  a sp:Fabric-type ;
  a skos:Concept ;
  rdfs:comment "C_FAB_TYPE" ;
  skos:definition "Peds are evident, and characteristically more than 50% of them are dense and smooth-faced, although the degree of lustre may vary."@en ;
  skos:notation "S" ;
  skos:prefLabel "Smooth-ped"@en ;
.
sp:field-ph
  a skos:Concept ;
  skos:definition """pH is determined in the field using a field pH kit based on the specifications of Raupach and Tucker (1959). Estimate to 0.5 of a unit. Portable pH meters may also be used.

Record depth at which pH is determined, in metres.
pH may be measured either:

•	by horizons, or
•	where horizons are thick (greater than 0.5 m) and horizon boundaries are diffuse, at selected intervals down the profile. This system gives useful data in some soils when important pH changes may occur independently of visible horizon changes, for instance the change from alkaline to strongly acid conditions in some cracking clays."""@en ;
  skos:prefLabel "Field pH"@en ;
.
sp:field-texture-AP
  a sp:Field-texture-organic ;
  a skos:Concept ;
  skos:altLabel "humified peat"@en ;
  skos:definition "strongly to completely decomposed organic material. Plant remains vary from few being identifiable to completely amorphous."@en ;
  skos:notation "AP" ;
  skos:note "Organic soil"@en ;
  skos:prefLabel "Sapric peat"@en ;
.
sp:field-texture-C
  a skos:Concept ;
  skos:definition "."@en ;
  skos:narrower sp:field-texture-HC ;
  skos:narrower sp:field-texture-LC ;
  skos:narrower sp:field-texture-LMC ;
  skos:narrower sp:field-texture-MC ;
  skos:narrower sp:field-texture-MHC ;
  skos:notation "C" ;
  skos:note "Approximate clay content (%): 35% or more"@en ;
  skos:prefLabel "Clay"@en ;
.
sp:field-texture-CFS
  a skos:Concept ;
  skos:broader sp:field-texture-CS ;
  skos:definition "Behaviour of moist bolus: slight coherence; sand grains of medium size; sticky when wet; many sand grains stick to fingers; will form minimal ribbon of 5–15 mm; discolours fingers with clay stain. Fine sand can be felt and often heard when manipulated. Sand grains are clearly evident under a ×10 hand lens."@en ;
  skos:narrower sp:field-texture-CFS-heavy ;
  skos:narrower sp:field-texture-CFS-light ;
  skos:notation "CFS" ;
  skos:note "Approximate clay content (%): 5 - 10%"@en ;
  skos:prefLabel "Clayey fine sand"@en ;
.
sp:field-texture-CFS-heavy
  a skos:Concept ;
  skos:broader sp:field-texture-CFS ;
  skos:broader sp:field-texture-CS-heavy ;
  skos:definition "Behaviour of moist bolus: slight coherence; sand grains of medium size; sticky when wet; many sand grains stick to fingers; will form minimal ribbon of 5–15 mm; discolours fingers with clay stain. Fine sand can be felt and often heard when manipulated. Sand grains are clearly evident under a ×10 hand lens."@en ;
  skos:notation "CFS+"@en ;
  skos:note "Approximate clay content (%): 5 - 10%"@en ;
  skos:prefLabel "Heavy clayey fine sand"@en ;
.
sp:field-texture-CFS-light
  a skos:Concept ;
  skos:broader sp:field-texture-CFS ;
  skos:broader sp:field-texture-CS-light ;
  skos:definition "Behaviour of moist bolus: slight coherence; sand grains of medium size; sticky when wet; many sand grains stick to fingers; will form minimal ribbon of 5–15 mm; discolours fingers with clay stain. Fine sand can be felt and often heard when manipulated. Sand grains are clearly evident under a ×10 hand lens."@en ;
  skos:notation "CFS-"@en ;
  skos:note "Approximate clay content (%): 5 - 10%"@en ;
  skos:prefLabel "Light clayey fine sand"@en ;
.
sp:field-texture-CKS
  a skos:Concept ;
  skos:broader sp:field-texture-CS ;
  skos:definition "Behaviour of moist bolus: slight coherence; sand grains of medium size; sticky when wet; many sand grains stick to fingers; will form minimal ribbon of 5–15 mm; discolours fingers with clay stain. Coarse sand is obviously coarse to touch. Sand grains are very readily seen with the naked eye."@en ;
  skos:narrower sp:field-texture-CKS-heavy ;
  skos:narrower sp:field-texture-CKS-light ;
  skos:notation "CKS" ;
  skos:note "Approximate clay content (%): 5 - 10%"@en ;
  skos:prefLabel "Clayey coarse sand"@en ;
.
sp:field-texture-CKS-heavy
  a skos:Concept ;
  skos:broader sp:field-texture-CKS ;
  skos:broader sp:field-texture-CS-heavy ;
  skos:definition "Behaviour of moist bolus: slight coherence; sand grains of medium size; sticky when wet; many sand grains stick to fingers; will form minimal ribbon of 5–15 mm; discolours fingers with clay stain. Coarse sand is obviously coarse to touch. Sand grains are very readily seen with the naked eye."@en ;
  skos:notation "CKS+"@en ;
  skos:note "Approximate clay content (%): 5 - 10%"@en ;
  skos:prefLabel "Heavy clayey coarse sand"@en ;
.
sp:field-texture-CKS-light
  a skos:Concept ;
  skos:broader sp:field-texture-CKS ;
  skos:broader sp:field-texture-CS-light ;
  skos:definition "Behaviour of moist bolus: slight coherence; sand grains of medium size; sticky when wet; many sand grains stick to fingers; will form minimal ribbon of 5–15 mm; discolours fingers with clay stain. Coarse sand is obviously coarse to touch. Sand grains are very readily seen with the naked eye."@en ;
  skos:notation "CKS-"@en ;
  skos:note "Approximate clay content (%): 5 - 10%"@en ;
  skos:prefLabel "Light clayey coarse sand"@en ;
.
sp:field-texture-CL
  a sp:Field-texture-mineral ;
  a skos:Concept ;
  skos:definition "Behaviour of moist bolus: coherent plastic bolus, smooth to manipulate; will form ribbon of 40–50 mm."@en ;
  skos:narrower sp:field-texture-CL-A ;
  skos:narrower sp:field-texture-CL-I ;
  skos:narrower sp:field-texture-CL-heavy ;
  skos:narrower sp:field-texture-CL-light ;
  skos:notation "CL" ;
  skos:note "Approximate clay content (%): 30 - 35%"@en ;
  skos:prefLabel "Clay loam"@en ;
.
sp:field-texture-CL-A
  a skos:Concept ;
  skos:broader sp:field-texture-CL ;
  skos:definition "Behaviour of moist bolus: coherent plastic bolus, smooth to manipulate; will form ribbon of 40–50 mm."@en ;
  skos:notation "CLA" ;
  skos:note """Approximate clay content (%): 30 - 35%
Organic and non-fibrous; dark organic stain discolours fingers; greasy feel in clayey textures and coherence in sandy textures. Fibres (excluding living roots) or plant tissue remains are not visible to naked eye and little or none visible with ×10 hand lens."""@en ;
  skos:prefLabel "Sapric clay loam"@en ;
.
sp:field-texture-CL-I
  a skos:Concept ;
  skos:broader sp:field-texture-CL ;
  skos:definition "Behaviour of moist bolus: coherent plastic bolus, smooth to manipulate; will form ribbon of 40–50 mm."@en ;
  skos:notation "CLI" ;
  skos:note """Approximate clay content (%): 30 - 35%
Organic and fibrous; dark organic stain discolours fingers; greasy feel in clayey textures and coherence in sandy textures. Fibres (excluding living roots) or plant tissue remain visible to naked eye or easily visible with ×10 hand lens."""@en ;
  skos:prefLabel "Fibric clay loam"@en ;
.
sp:field-texture-CL-heavy
  a skos:Concept ;
  skos:broader sp:field-texture-CL ;
  skos:definition "Behaviour of moist bolus: coherent plastic bolus, smooth to manipulate; will form ribbon of 40–50 mm."@en ;
  skos:notation "CL+"@en ;
  skos:note "Approximate clay content (%): 30 - 35%"@en ;
  skos:prefLabel "Heavy clay loam"@en ;
.
sp:field-texture-CL-light
  a skos:Concept ;
  skos:broader sp:field-texture-CL ;
  skos:definition "Behaviour of moist bolus: coherent plastic bolus, smooth to manipulate; will form ribbon of 40–50 mm."@en ;
  skos:notation "CL-"@en ;
  skos:note "Approximate clay content (%): 30 - 35%"@en ;
  skos:prefLabel "Light clay loam"@en ;
.
sp:field-texture-CLFS
  a skos:Concept ;
  skos:broader sp:field-texture-CLS ;
  skos:definition "Behaviour of moist bolus: coherent plastic bolus; medium-size sand grains visible in finer matrix; will form ribbon of 40–50 mm. Fine sand can be felt and often heard when manipulated. Sand grains are clearly evident under a ×10 hand lens."@en ;
  skos:narrower sp:field-texture-CLFS-A ;
  skos:narrower sp:field-texture-CLFS-I ;
  skos:narrower sp:field-texture-CLFS-heavy ;
  skos:narrower sp:field-texture-CLFS-light ;
  skos:notation "CLFS" ;
  skos:note "Approximate clay content (%): 30 - 35%"@en ;
  skos:prefLabel "Clay loam, fine sandy"@en ;
.
sp:field-texture-CLFS-A
  a skos:Concept ;
  skos:broader sp:field-texture-CLFS ;
  skos:broader sp:field-texture-CLS-A ;
  skos:definition "Behaviour of moist bolus: coherent plastic bolus; medium-size sand grains visible in finer matrix; will form ribbon of 40–50 mm."@en ;
  skos:notation "CLFSA" ;
  skos:note """Approximate clay content (%): 30 - 35%
Organic and non-fibrous; dark organic stain discolours fingers; greasy feel in clayey textures and coherence in sandy textures. Fibres (excluding living roots) or plant tissue remains are not visible to naked eye and little or none visible with ×10 hand lens."""@en ;
  skos:prefLabel "Sapric clay loam, fine sandy"@en ;
.
sp:field-texture-CLFS-I
  a skos:Concept ;
  skos:broader sp:field-texture-CLFS ;
  skos:broader sp:field-texture-CLS-I ;
  skos:definition "Behaviour of moist bolus: coherent plastic bolus; medium-size sand grains visible in finer matrix; will form ribbon of 40–50 mm."@en ;
  skos:notation "CLFSI" ;
  skos:note """Approximate clay content (%): 30 - 35%
Organic and fibrous; dark organic stain discolours fingers; greasy feel in clayey textures and coherence in sandy textures. Fibres (excluding living roots) or plant tissue remain visible to naked eye or easily visible with ×10 hand lens."""@en ;
  skos:prefLabel "Fibric clay loam, fine sandy"@en ;
.
sp:field-texture-CLFS-heavy
  a skos:Concept ;
  skos:broader sp:field-texture-CLFS ;
  skos:broader sp:field-texture-CLS-heavy ;
  skos:definition "Behaviour of moist bolus: coherent plastic bolus; medium-size sand grains visible in finer matrix; will form ribbon of 40–50 mm. Fine sand can be felt and often heard when manipulated. Sand grains are clearly evident under a ×10 hand lens."@en ;
  skos:notation "CLFS+"@en ;
  skos:note "Approximate clay content (%): 30 - 35%"@en ;
  skos:prefLabel "Heavy clay loam, fine sandy"@en ;
.
sp:field-texture-CLFS-light
  a skos:Concept ;
  skos:broader sp:field-texture-CLFS ;
  skos:broader sp:field-texture-CLS-light ;
  skos:definition "Behaviour of moist bolus: coherent plastic bolus; medium-size sand grains visible in finer matrix; will form ribbon of 40–50 mm. Fine sand can be felt and often heard when manipulated. Sand grains are clearly evident under a ×10 hand lens."@en ;
  skos:notation "CLFS-"@en ;
  skos:note "Approximate clay content (%): 30 - 35%"@en ;
  skos:prefLabel "Light clay loam, fine sandy"@en ;
.
sp:field-texture-CLKS
  a skos:Concept ;
  skos:broader sp:field-texture-CLS ;
  skos:definition "Behaviour of moist bolus: coherent plastic bolus; medium-size sand grains visible in finer matrix; will form ribbon of 40–50 mm. Coarse sand is obviously coarse to touch. Sand grains are very readily seen with the naked eye."@en ;
  skos:narrower sp:field-texture-CLKS-A ;
  skos:narrower sp:field-texture-CLKS-I ;
  skos:narrower sp:field-texture-CLKS-heavy ;
  skos:narrower sp:field-texture-CLKS-light ;
  skos:notation "CLKS" ;
  skos:note "Approximate clay content (%): 30 - 35%"@en ;
  skos:prefLabel "Clay loam, coarse sandy"@en ;
.
sp:field-texture-CLKS-A
  a skos:Concept ;
  skos:broader sp:field-texture-CLKS ;
  skos:broader sp:field-texture-CLS-A ;
  skos:definition "Behaviour of moist bolus: coherent plastic bolus; medium-size sand grains visible in finer matrix; will form ribbon of 40–50 mm."@en ;
  skos:notation "CLKS-A"@en ;
  skos:note """Approximate clay content (%): 30 - 35%
Organic and non-fibrous; dark organic stain discolours fingers; greasy feel in clayey textures and coherence in sandy textures. Fibres (excluding living roots) or plant tissue remains are not visible to naked eye and little or none visible with ×10 hand lens."""@en ;
  skos:prefLabel "Sapric clay loam, coarse sandy"@en ;
.
sp:field-texture-CLKS-I
  a skos:Concept ;
  skos:broader sp:field-texture-CLKS ;
  skos:broader sp:field-texture-CLS-I ;
  skos:definition "Behaviour of moist bolus: coherent plastic bolus; medium-size sand grains visible in finer matrix; will form ribbon of 40–50 mm."@en ;
  skos:notation "CLKS-I"@en ;
  skos:note """Approximate clay content (%): 30 - 35%
Organic and fibrous; dark organic stain discolours fingers; greasy feel in clayey textures and coherence in sandy textures. Fibres (excluding living roots) or plant tissue remain visible to naked eye or easily visible with ×10 hand lens."""@en ;
  skos:prefLabel "Fibric clay loam, coarse sandy"@en ;
.
sp:field-texture-CLKS-heavy
  a skos:Concept ;
  skos:broader sp:field-texture-CLKS ;
  skos:broader sp:field-texture-CLS-heavy ;
  skos:definition "Behaviour of moist bolus: coherent plastic bolus; medium-size sand grains visible in finer matrix; will form ribbon of 40–50 mm. Coarse sand is obviously coarse to touch. Sand grains are very readily seen with the naked eye."@en ;
  skos:notation "CLKS+"@en ;
  skos:note "Approximate clay content (%): 30 - 35%"@en ;
  skos:prefLabel "Heavy clay loam, coarse sandy"@en ;
.
sp:field-texture-CLKS-light
  a skos:Concept ;
  skos:broader sp:field-texture-CLKS ;
  skos:broader sp:field-texture-CLS-light ;
  skos:definition "Behaviour of moist bolus: coherent plastic bolus; medium-size sand grains visible in finer matrix; will form ribbon of 40–50 mm. Coarse sand is obviously coarse to touch. Sand grains are very readily seen with the naked eye."@en ;
  skos:notation "CLKS-"@en ;
  skos:note "Approximate clay content (%): 30 - 35%"@en ;
  skos:prefLabel "Light clay loam, coarse sandy"@en ;
.
sp:field-texture-CLS
  a sp:Field-texture-mineral ;
  a skos:Concept ;
  skos:definition "Behaviour of moist bolus: coherent plastic bolus; medium-size sand grains visible in finer matrix; will form ribbon of 40–50 mm."@en ;
  skos:narrower sp:field-texture-CLFS ;
  skos:narrower sp:field-texture-CLKS ;
  skos:narrower sp:field-texture-CLS-A ;
  skos:narrower sp:field-texture-CLS-I ;
  skos:narrower sp:field-texture-CLS-heavy ;
  skos:narrower sp:field-texture-CLS-light ;
  skos:notation "CLS" ;
  skos:note "Approximate clay content (%): 30 - 35%"@en ;
  skos:prefLabel "Clay loam, sandy"@en ;
.
sp:field-texture-CLS-A
  a skos:Concept ;
  skos:broader sp:field-texture-CLS ;
  skos:definition "Behaviour of moist bolus: coherent plastic bolus; medium-size sand grains visible in finer matrix; will form ribbon of 40–50 mm."@en ;
  skos:narrower sp:field-texture-CLFS-A ;
  skos:narrower sp:field-texture-CLKS-A ;
  skos:notation "CLS-A"@en ;
  skos:note """Approximate clay content (%): 30 - 35%
Organic and non-fibrous; dark organic stain discolours fingers; greasy feel in clayey textures and coherence in sandy textures. Fibres (excluding living roots) or plant tissue remains are not visible to naked eye and little or none visible with ×10 hand lens."""@en ;
  skos:prefLabel "Sapric clay loam, sandy"@en ;
.
sp:field-texture-CLS-I
  a skos:Concept ;
  skos:broader sp:field-texture-CLS ;
  skos:definition "Behaviour of moist bolus: coherent plastic bolus; medium-size sand grains visible in finer matrix; will form ribbon of 40–50 mm."@en ;
  skos:narrower sp:field-texture-CLFS-I ;
  skos:narrower sp:field-texture-CLKS-I ;
  skos:notation "CLS-I"@en ;
  skos:note """Approximate clay content (%): 30 - 35%
Organic and fibrous; dark organic stain discolours fingers; greasy feel in clayey textures and coherence in sandy textures. Fibres (excluding living roots) or plant tissue remain visible to naked eye or easily visible with ×10 hand lens."""@en ;
  skos:prefLabel "Fibric clay loam, sandy"@en ;
.
sp:field-texture-CLS-heavy
  a skos:Concept ;
  skos:broader sp:field-texture-CLS ;
  skos:definition "Behaviour of moist bolus: coherent plastic bolus; medium-size sand grains visible in finer matrix; will form ribbon of 40–50 mm."@en ;
  skos:narrower sp:field-texture-CLFS-heavy ;
  skos:narrower sp:field-texture-CLKS-heavy ;
  skos:notation "CLS+"@en ;
  skos:note "Approximate clay content (%): 30 - 35%"@en ;
  skos:prefLabel "Heavy clay loam, sandy"@en ;
.
sp:field-texture-CLS-light
  a skos:Concept ;
  skos:broader sp:field-texture-CLS ;
  skos:definition "Behaviour of moist bolus: coherent plastic bolus; medium-size sand grains visible in finer matrix; will form ribbon of 40–50 mm."@en ;
  skos:narrower sp:field-texture-CLFS-light ;
  skos:narrower sp:field-texture-CLKS-light ;
  skos:notation "CLS-"@en ;
  skos:note "Approximate clay content (%): 30 - 35%"@en ;
  skos:prefLabel "Light clay loam, sandy"@en ;
.
sp:field-texture-CP
  a sp:Field-texture-organic ;
  a skos:Concept ;
  skos:definition "bolus has obvious fine mineral particle content, is sticky when wet, and is coherent."@en ;
  skos:notation "CP" ;
  skos:note "Organic soil"@en ;
  skos:prefLabel "Clayey peat"@en ;
.
sp:field-texture-CS
  a sp:Field-texture-mineral ;
  a skos:Concept ;
  skos:definition "Behaviour of moist bolus: slight coherence; sand grains of medium size; sticky when wet; many sand grains stick to fingers; will form minimal ribbon of 5–15 mm; discolours fingers with clay stain."@en ;
  skos:narrower sp:field-texture-CFS ;
  skos:narrower sp:field-texture-CKS ;
  skos:narrower sp:field-texture-CS-heavy ;
  skos:narrower sp:field-texture-CS-light ;
  skos:notation "CS" ;
  skos:note "Approximate clay content (%): 5 - 10%"@en ;
  skos:prefLabel "Clayey sand"@en ;
.
sp:field-texture-CS-heavy
  a skos:Concept ;
  skos:broader sp:field-texture-CS ;
  skos:definition "Behaviour of moist bolus: slight coherence; sand grains of medium size; sticky when wet; many sand grains stick to fingers; will form minimal ribbon of 5–15 mm; discolours fingers with clay stain."@en ;
  skos:narrower sp:field-texture-CFS-heavy ;
  skos:narrower sp:field-texture-CKS-heavy ;
  skos:notation "CS+"@en ;
  skos:note "Approximate clay content (%): 5 - 10%"@en ;
  skos:prefLabel "Heavy clayey sand"@en ;
.
sp:field-texture-CS-light
  a skos:Concept ;
  skos:broader sp:field-texture-CS ;
  skos:definition "Behaviour of moist bolus: slight coherence; sand grains of medium size; sticky when wet; many sand grains stick to fingers; will form minimal ribbon of 5–15 mm; discolours fingers with clay stain."@en ;
  skos:narrower sp:field-texture-CFS-light ;
  skos:narrower sp:field-texture-CKS-light ;
  skos:notation "CS-"@en ;
  skos:note "Approximate clay content (%): 5 - 10%"@en ;
  skos:prefLabel "Light clayey sand"@en ;
.
sp:field-texture-FS
  a skos:Concept ;
  skos:broader sp:field-texture-S ;
  skos:definition "Behaviour of moist bolus: coherence nil to very slight, cannot be moulded; sand grains of medium size; single sand grains adhere to fingers. Fine sand can be felt and often heard when manipulated. Sand grains are clearly evident under a ×10 hand lens."@en ;
  skos:narrower sp:field-texture-FS-A ;
  skos:narrower sp:field-texture-FS-I ;
  skos:notation "FS" ;
  skos:note "Approximate clay content (%): commonly less than 5%"@en ;
  skos:prefLabel "Fine sand (field texture)"@en ;
.
sp:field-texture-FS-A
  a skos:Concept ;
  skos:broader sp:field-texture-FS ;
  skos:broader sp:field-texture-S-A ;
  skos:definition "Behaviour of moist bolus: coherence nil to very slight, cannot be moulded; sand grains of medium size; single sand grains adhere to fingers. Fine sand can be felt and often heard when manipulated. Sand grains are clearly evident under a ×10 hand lens."@en ;
  skos:notation "FSA" ;
  skos:note "Approximate clay content (%): commonly less than 5%"@en ;
  skos:prefLabel "Sapric fine sand"@en ;
.
sp:field-texture-FS-I
  a skos:Concept ;
  skos:broader sp:field-texture-FS ;
  skos:broader sp:field-texture-S-I ;
  skos:definition "Behaviour of moist bolus: coherence nil to very slight, cannot be moulded; sand grains of medium size; single sand grains adhere to fingers. Fine sand can be felt and often heard when manipulated. Sand grains are clearly evident under a ×10 hand lens."@en ;
  skos:notation "FSI" ;
  skos:note "Approximate clay content (%): commonly less than 5%"@en ;
  skos:prefLabel "Fibric fine sand"@en ;
.
sp:field-texture-FSCL
  a skos:Concept ;
  skos:broader sp:field-texture-SCL ;
  skos:definition "Behaviour of moist bolus: strongly coherent bolus, sandy to touch; medium-size sand grains visible in finer matrix; will form ribbon of 25–40 mm. Fine sand can be felt and often heard when manipulated. Sand grains are clearly evident under a ×10 hand lens."@en ;
  skos:narrower sp:field-texture-FSCL-A ;
  skos:narrower sp:field-texture-FSCL-I ;
  skos:narrower sp:field-texture-FSCL-heavy ;
  skos:narrower sp:field-texture-FSCL-light ;
  skos:notation "FSCL" ;
  skos:note "Approximate clay content (%): 20 - 30%"@en ;
  skos:prefLabel "Fine sandy clay loam"@en ;
.
sp:field-texture-FSCL-A
  a skos:Concept ;
  skos:broader sp:field-texture-FSCL ;
  skos:broader sp:field-texture-SCL-A ;
  skos:definition "Behaviour of moist bolus: strongly coherent bolus, sandy to touch; medium-size sand grains visible in finer matrix; will form ribbon of 25–40 mm. Fine sand can be felt and often heard when manipulated. Sand grains are clearly evident under a ×10 hand lens."@en ;
  skos:notation "FSCLA" ;
  skos:note "Approximate clay content (%): 20 - 30%"@en ;
  skos:prefLabel "Sapric fine sandy clay loam"@en ;
.
sp:field-texture-FSCL-I
  a skos:Concept ;
  skos:broader sp:field-texture-FSCL ;
  skos:broader sp:field-texture-SCL-I ;
  skos:definition "Behaviour of moist bolus: strongly coherent bolus, sandy to touch; medium-size sand grains visible in finer matrix; will form ribbon of 25–40 mm. Fine sand can be felt and often heard when manipulated. Sand grains are clearly evident under a ×10 hand lens."@en ;
  skos:notation "FSCLI" ;
  skos:note "Approximate clay content (%): 20 - 30%"@en ;
  skos:prefLabel "Fibric fine sandy clay loam"@en ;
.
sp:field-texture-FSCL-heavy
  a skos:Concept ;
  skos:broader sp:field-texture-FSCL ;
  skos:broader sp:field-texture-SCL-heavy ;
  skos:definition "Behaviour of moist bolus: strongly coherent bolus, sandy to touch; medium-size sand grains visible in finer matrix; will form ribbon of 25–40 mm. Fine sand can be felt and often heard when manipulated. Sand grains are clearly evident under a ×10 hand lens."@en ;
  skos:notation "FSCL+"@en ;
  skos:note "Approximate clay content (%): 20 - 30%"@en ;
  skos:prefLabel "Heavy fine sandy clay loam"@en ;
.
sp:field-texture-FSCL-light
  a skos:Concept ;
  skos:broader sp:field-texture-FSCL ;
  skos:broader sp:field-texture-SCL-light ;
  skos:definition "Behaviour of moist bolus: strongly coherent bolus, sandy to touch; medium-size sand grains visible in finer matrix; will form ribbon of 25–40 mm. Fine sand can be felt and often heard when manipulated. Sand grains are clearly evident under a ×10 hand lens."@en ;
  skos:notation "FSCL-"@en ;
  skos:note "Approximate clay content (%): 20 - 30%"@en ;
  skos:prefLabel "Light fine sandy clay loam"@en ;
.
sp:field-texture-FSHC
  a skos:Concept ;
  skos:broader sp:field-texture-HC ;
  skos:definition "Behaviour of moist bolus: smooth plastic bolus; handles like stiff plasticine; can be moulded into rods without fracture; has firm resistance to ribboning shear; will form ribbon of 75 mm or more."@en ;
  skos:narrower sp:field-texture-FSHC-A ;
  skos:narrower sp:field-texture-FSHC-I ;
  skos:notation "FSHC" ;
  skos:note "Approximate clay content (%): 50% or more"@en ;
  skos:prefLabel "Fine sandy heavy clay"@en ;
.
sp:field-texture-FSHC-A
  a skos:Concept ;
  skos:broader sp:field-texture-FSHC ;
  skos:broader sp:field-texture-HC-A ;
  skos:definition "Behaviour of moist bolus: smooth plastic bolus; handles like stiff plasticine; can be moulded into rods without fracture; has firm resistance to ribboning shear; will form ribbon of 75 mm or more."@en ;
  skos:notation "FSHCA" ;
  skos:note "Approximate clay content (%): 50% or more"@en ;
  skos:prefLabel "Sapric fine sandy heavy clay"@en ;
.
sp:field-texture-FSHC-I
  a skos:Concept ;
  skos:broader sp:field-texture-FSHC ;
  skos:broader sp:field-texture-HC-I ;
  skos:definition "Behaviour of moist bolus: smooth plastic bolus; handles like stiff plasticine; can be moulded into rods without fracture; has firm resistance to ribboning shear; will form ribbon of 75 mm or more."@en ;
  skos:notation "FSHCI" ;
  skos:note "Approximate clay content (%): 50% or more"@en ;
  skos:prefLabel "Fibric fine sandy heavy clay"@en ;
.
sp:field-texture-FSL
  a skos:Concept ;
  skos:broader sp:field-texture-SL ;
  skos:definition "Behaviour of moist bolus: bolus coherent but very sandy to touch; will form ribbon of 15–25 mm; dominant sand grains are of medium size and are readily visible. Fine sand can be felt and often heard when manipulated. Sand grains are clearly evident under a ×10 hand lens."@en ;
  skos:narrower sp:field-texture-FSL-A ;
  skos:narrower sp:field-texture-FSL-I ;
  skos:notation "FSL" ;
  skos:note "Approximate clay content (%): 10 - 20%"@en ;
  skos:prefLabel "Fine sandy loam"@en ;
.
sp:field-texture-FSL-A
  a skos:Concept ;
  skos:broader sp:field-texture-FSL ;
  skos:broader sp:field-texture-SL-A ;
  skos:definition "Behaviour of moist bolus: bolus coherent but very sandy to touch; will form ribbon of 15–25 mm; dominant sand grains are of medium size and are readily visible. Fine sand can be felt and often heard when manipulated. Sand grains are clearly evident under a ×10 hand lens."@en ;
  skos:notation "FSLA" ;
  skos:note "Approximate clay content (%): 10 - 20%"@en ;
  skos:prefLabel "Sapric fine sandy loam"@en ;
.
sp:field-texture-FSL-I
  a skos:Concept ;
  skos:broader sp:field-texture-FSL ;
  skos:broader sp:field-texture-SL-I ;
  skos:definition "Behaviour of moist bolus: bolus coherent but very sandy to touch; will form ribbon of 15–25 mm; dominant sand grains are of medium size and are readily visible. Fine sand can be felt and often heard when manipulated. Sand grains are clearly evident under a ×10 hand lens."@en ;
  skos:notation "FSLI" ;
  skos:note "Approximate clay content (%): 10 - 20%"@en ;
  skos:prefLabel "Fibric fine sandy loam"@en ;
.
sp:field-texture-FSLC
  a skos:Concept ;
  skos:broader sp:field-texture-LC ;
  skos:definition "Behaviour of moist bolus: plastic bolus; smooth to touch; slight resistance to shearing between thumb and forefinger; will form ribbon of 50–75 mm."@en ;
  skos:narrower sp:field-texture-FSLC-A ;
  skos:narrower sp:field-texture-FSLC-I ;
  skos:notation "FSLC" ;
  skos:note "Approximate clay content (%): 35 - 40%"@en ;
  skos:prefLabel "Fine sandy light clay"@en ;
.
sp:field-texture-FSLC-A
  a skos:Concept ;
  skos:broader sp:field-texture-FSLC ;
  skos:broader sp:field-texture-LC-A ;
  skos:definition "Behaviour of moist bolus: plastic bolus; smooth to touch; slight resistance to shearing between thumb and forefinger; will form ribbon of 50–75 mm."@en ;
  skos:notation "FSLCA" ;
  skos:note "Approximate clay content (%): 35 - 40%"@en ;
  skos:prefLabel "Sapric fine sandy light clay"@en ;
.
sp:field-texture-FSLC-I
  a skos:Concept ;
  skos:broader sp:field-texture-FSLC ;
  skos:broader sp:field-texture-LC-I ;
  skos:definition "Behaviour of moist bolus: plastic bolus; smooth to touch; slight resistance to shearing between thumb and forefinger; will form ribbon of 50–75 mm."@en ;
  skos:notation "FSLCI" ;
  skos:note "Approximate clay content (%): 35 - 40%"@en ;
  skos:prefLabel "Fibric fine sandy light clay"@en ;
.
sp:field-texture-FSLMC
  a skos:Concept ;
  skos:broader sp:field-texture-LMC ;
  skos:definition "Behaviour of moist bolus: plastic bolus; smooth to touch; slight to moderate resistance to ribboning shear; will form ribbon of about 75 mm."@en ;
  skos:narrower sp:field-texture-FSLMC-A ;
  skos:narrower sp:field-texture-FSLMC-I ;
  skos:notation "FSLMC" ;
  skos:note "Approximate clay content (%): 40 - 45%"@en ;
  skos:prefLabel "Fine sandy light medium clay"@en ;
.
sp:field-texture-FSLMC-A
  a skos:Concept ;
  skos:broader sp:field-texture-FSLMC ;
  skos:broader sp:field-texture-LMC-A ;
  skos:definition "Behaviour of moist bolus: plastic bolus; smooth to touch; slight to moderate resistance to ribboning shear; will form ribbon of about 75 mm."@en ;
  skos:notation "FSLMCA" ;
  skos:note "Approximate clay content (%): 40 - 45%"@en ;
  skos:prefLabel "Sapric fine sandy light medium clay"@en ;
.
sp:field-texture-FSLMC-I
  a skos:Concept ;
  skos:broader sp:field-texture-FSLMC ;
  skos:broader sp:field-texture-LMC-I ;
  skos:definition "Behaviour of moist bolus: plastic bolus; smooth to touch; slight to moderate resistance to ribboning shear; will form ribbon of about 75 mm."@en ;
  skos:notation "FSLMCI" ;
  skos:note "Approximate clay content (%): 40 - 45%"@en ;
  skos:prefLabel "Fibric fine sandy light medium clay"@en ;
.
sp:field-texture-FSMC
  a skos:Concept ;
  skos:broader sp:field-texture-MC ;
  skos:definition "Behaviour of moist bolus: smooth plastic bolus; handles like plasticine and can be moulded into rods without fracture; has moderate resistance to ribboning shear; will form ribbon of 75 mm or more."@en ;
  skos:narrower sp:field-texture-FSMC-A ;
  skos:narrower sp:field-texture-FSMC-I ;
  skos:notation "FSMC" ;
  skos:note "Approximate clay content (%): 45 - 55%"@en ;
  skos:prefLabel "Fine sandy medium clay"@en ;
.
sp:field-texture-FSMC-A
  a skos:Concept ;
  skos:broader sp:field-texture-FSMC ;
  skos:broader sp:field-texture-MC-A ;
  skos:definition "Behaviour of moist bolus: smooth plastic bolus; handles like plasticine and can be moulded into rods without fracture; has moderate resistance to ribboning shear; will form ribbon of 75 mm or more."@en ;
  skos:notation "FSMCA" ;
  skos:note "Approximate clay content (%): 45 - 55%"@en ;
  skos:prefLabel "Sapric fine sandy medium clay"@en ;
.
sp:field-texture-FSMC-I
  a skos:Concept ;
  skos:broader sp:field-texture-FSMC ;
  skos:broader sp:field-texture-MC-I ;
  skos:definition "Behaviour of moist bolus: smooth plastic bolus; handles like plasticine and can be moulded into rods without fracture; has moderate resistance to ribboning shear; will form ribbon of 75 mm or more."@en ;
  skos:notation "FSMCI" ;
  skos:note "Approximate clay content (%): 45 - 55%"@en ;
  skos:prefLabel "Fibric fine sandy medium clay"@en ;
.
sp:field-texture-FSMHC
  a skos:Concept ;
  skos:broader sp:field-texture-MHC ;
  skos:definition "Behaviour of moist bolus: smooth plastic bolus; handles like plasticine; can be moulded into rods without fracture; has moderate to firm resistance to ribboning shear; will form ribbon of 75 mm or more."@en ;
  skos:narrower sp:field-texture-FSMHC-A ;
  skos:narrower sp:field-texture-FSMHC-I ;
  skos:notation "FSMHC" ;
  skos:note "Approximate clay content (%): 50% or more"@en ;
  skos:prefLabel "Fine sandy medium heavy clay"@en ;
.
sp:field-texture-FSMHC-A
  a skos:Concept ;
  skos:broader sp:field-texture-FSMHC ;
  skos:broader sp:field-texture-MHC-A ;
  skos:definition "Behaviour of moist bolus: smooth plastic bolus; handles like plasticine; can be moulded into rods without fracture; has moderate to firm resistance to ribboning shear; will form ribbon of 75 mm or more."@en ;
  skos:notation "FSMHCA" ;
  skos:note "Approximate clay content (%): 50% or more"@en ;
  skos:prefLabel "Sapric fine sandy medium heavy clay"@en ;
.
sp:field-texture-FSMHC-I
  a skos:Concept ;
  skos:broader sp:field-texture-FSMHC ;
  skos:broader sp:field-texture-MHC-I ;
  skos:definition "Behaviour of moist bolus: smooth plastic bolus; handles like plasticine; can be moulded into rods without fracture; has moderate to firm resistance to ribboning shear; will form ribbon of 75 mm or more."@en ;
  skos:notation "FSMHCI" ;
  skos:note "Approximate clay content (%): 50% or more"@en ;
  skos:prefLabel "Fibric fine sandy medium heavy clay"@en ;
.
sp:field-texture-GP
  a sp:Field-texture-organic ;
  a skos:Concept ;
  skos:definition "dominantly decomposed organic material, which has dried irreversibly to fine granules through exposure and drying and/or cultivation. Granules are approximately 1–2 mm in diameter and have granular or subangular blocky structure."@en ;
  skos:notation "GP" ;
  skos:note "Organic soil; On drying, peat may change irreversibly."@en ;
  skos:prefLabel "Granular peat"@en ;
.
sp:field-texture-HC
  a sp:Field-texture-mineral ;
  a skos:Concept ;
  skos:definition "Behaviour of moist bolus: smooth plastic bolus; handles like stiff plasticine; can be moulded into rods without fracture; has firm resistance to ribboning shear; will form ribbon of 75 mm or more."@en ;
  skos:narrower sp:field-texture-FSHC ;
  skos:narrower sp:field-texture-HC-A ;
  skos:narrower sp:field-texture-HC-I ;
  skos:narrower sp:field-texture-KSHC ;
  skos:narrower sp:field-texture-SHC ;
  skos:narrower sp:field-texture-ZHC ;
  skos:notation "HC" ;
  skos:note "Approximate clay content (%): 50% or more"@en ;
  skos:prefLabel "Heavy clay"@en ;
.
sp:field-texture-HC-A
  a skos:Concept ;
  skos:broader sp:field-texture-HC ;
  skos:definition "Behaviour of moist bolus: smooth plastic bolus; handles like stiff plasticine; can be moulded into rods without fracture; has firm resistance to ribboning shear; will form ribbon of 75 mm or more."@en ;
  skos:narrower sp:field-texture-FSHC-A ;
  skos:narrower sp:field-texture-KSHC-A ;
  skos:narrower sp:field-texture-SHC-A ;
  skos:narrower sp:field-texture-ZHC-A ;
  skos:notation "HCA" ;
  skos:note "Approximate clay content (%): 50% or more"@en ;
  skos:prefLabel "Sapric heavy clay"@en ;
.
sp:field-texture-HC-I
  a skos:Concept ;
  skos:broader sp:field-texture-HC ;
  skos:definition "Behaviour of moist bolus: smooth plastic bolus; handles like stiff plasticine; can be moulded into rods without fracture; has firm resistance to ribboning shear; will form ribbon of 75 mm or more."@en ;
  skos:narrower sp:field-texture-FSHC-I ;
  skos:narrower sp:field-texture-KSHC-I ;
  skos:narrower sp:field-texture-SHC-I ;
  skos:narrower sp:field-texture-ZHC-I ;
  skos:notation "HCI" ;
  skos:note "Approximate clay content (%): 50% or more"@en ;
  skos:prefLabel "Fibric heavy clay"@en ;
.
sp:field-texture-HP
  a sp:Field-texture-organic ;
  a skos:Concept ;
  skos:altLabel "Semi-fibrous peat"@en ;
  skos:definition "moderately to well decomposed organic material. Plant remains vary from most being difficult to identify to most being unidentifiable. It is intermediate in degree of decomposition between the less decomposed fibric peat and the more decomposed sapric peat."@en ;
  skos:notation "HP" ;
  skos:note "Organic soil"@en ;
  skos:prefLabel "Hemic peat"@en ;
.
sp:field-texture-IP
  a sp:Field-texture-organic ;
  a skos:Concept ;
  skos:altLabel "Fibrous peat"@en ;
  skos:definition "undecomposed or weakly decomposed organic material. Plant remains are distinct and readily identifiable."@en ;
  skos:notation "IP" ;
  skos:note "Organic soil"@en ;
  skos:prefLabel "Fibric peat"@en ;
.
sp:field-texture-KS
  a skos:Concept ;
  skos:broader sp:field-texture-S ;
  skos:definition "Behaviour of moist bolus: coherence nil to very slight, cannot be moulded; sand grains of medium size; single sand grains adhere to fingers. Coarse sand is obviously coarse to touch. Sand grains are very readily seen with the naked eye."@en ;
  skos:narrower sp:field-texture-KS-A ;
  skos:narrower sp:field-texture-KS-I ;
  skos:notation "KS" ;
  skos:note "Approximate clay content (%): commonly less than 5%"@en ;
  skos:prefLabel "Coarse sand (field texture)"@en ;
.
sp:field-texture-KS-A
  a skos:Concept ;
  skos:broader sp:field-texture-KS ;
  skos:broader sp:field-texture-S-A ;
  skos:definition "Behaviour of moist bolus: coherence nil to very slight, cannot be moulded; sand grains of medium size; single sand grains adhere to fingers. Coarse sand is obviously coarse to touch. Sand grains are very readily seen with the naked eye."@en ;
  skos:notation "KSA" ;
  skos:note "Approximate clay content (%): commonly less than 5%"@en ;
  skos:prefLabel "Sapric coarse sand"@en ;
.
sp:field-texture-KS-I
  a skos:Concept ;
  skos:broader sp:field-texture-KS ;
  skos:broader sp:field-texture-S-I ;
  skos:definition "Behaviour of moist bolus: coherence nil to very slight, cannot be moulded; sand grains of medium size; single sand grains adhere to fingers. Coarse sand is obviously coarse to touch. Sand grains are very readily seen with the naked eye."@en ;
  skos:notation "KSI" ;
  skos:note "Approximate clay content (%): commonly less than 5%"@en ;
  skos:prefLabel "Fibric coarse sand"@en ;
.
sp:field-texture-KSCL
  a skos:Concept ;
  skos:broader sp:field-texture-SCL ;
  skos:definition "Behaviour of moist bolus: strongly coherent bolus, sandy to touch; medium-size sand grains visible in finer matrix; will form ribbon of 25–40 mm. Coarse sand is obviously coarse to touch. Sand grains are very readily seen with the naked eye."@en ;
  skos:narrower sp:field-texture-KSCL-A ;
  skos:narrower sp:field-texture-KSCL-I ;
  skos:narrower sp:field-texture-KSCL-heavy ;
  skos:narrower sp:field-texture-KSCL-light ;
  skos:notation "KSCL" ;
  skos:note "Approximate clay content (%): 20 - 30%"@en ;
  skos:prefLabel "Coarse sandy clay loam"@en ;
.
sp:field-texture-KSCL-A
  a skos:Concept ;
  skos:broader sp:field-texture-KSCL ;
  skos:broader sp:field-texture-SCL-A ;
  skos:definition "Behaviour of moist bolus: strongly coherent bolus, sandy to touch; medium-size sand grains visible in finer matrix; will form ribbon of 25–40 mm. Coarse sand is obviously coarse to touch. Sand grains are very readily seen with the naked eye."@en ;
  skos:notation "KSCLA" ;
  skos:note "Approximate clay content (%): 20 - 30%"@en ;
  skos:prefLabel "Sapric coarse sandy clay loam"@en ;
.
sp:field-texture-KSCL-I
  a skos:Concept ;
  skos:broader sp:field-texture-KSCL ;
  skos:broader sp:field-texture-SCL-I ;
  skos:definition "Behaviour of moist bolus: strongly coherent bolus, sandy to touch; medium-size sand grains visible in finer matrix; will form ribbon of 25–40 mm. Coarse sand is obviously coarse to touch. Sand grains are very readily seen with the naked eye."@en ;
  skos:notation "KSCLI" ;
  skos:note "Approximate clay content (%): 20 - 30%"@en ;
  skos:prefLabel "Fibric coarse sandy clay loam"@en ;
.
sp:field-texture-KSCL-heavy
  a skos:Concept ;
  skos:broader sp:field-texture-KSCL ;
  skos:broader sp:field-texture-SCL-heavy ;
  skos:definition "Behaviour of moist bolus: strongly coherent bolus, sandy to touch; medium-size sand grains visible in finer matrix; will form ribbon of 25–40 mm. Coarse sand is obviously coarse to touch. Sand grains are very readily seen with the naked eye."@en ;
  skos:notation "KSCL+"@en ;
  skos:note "Approximate clay content (%): 20 - 30%"@en ;
  skos:prefLabel "Heavy coarse sandy clay loam"@en ;
.
sp:field-texture-KSCL-light
  a skos:Concept ;
  skos:broader sp:field-texture-KSCL ;
  skos:broader sp:field-texture-SCL-light ;
  skos:definition "Behaviour of moist bolus: strongly coherent bolus, sandy to touch; medium-size sand grains visible in finer matrix; will form ribbon of 25–40 mm. Coarse sand is obviously coarse to touch. Sand grains are very readily seen with the naked eye."@en ;
  skos:notation "KSCL-"@en ;
  skos:note "Approximate clay content (%): 20 - 30%"@en ;
  skos:prefLabel "Light coarse sandy clay loam"@en ;
.
sp:field-texture-KSHC
  a skos:Concept ;
  skos:broader sp:field-texture-HC ;
  skos:definition "Behaviour of moist bolus: smooth plastic bolus; handles like stiff plasticine; can be moulded into rods without fracture; has firm resistance to ribboning shear; will form ribbon of 75 mm or more."@en ;
  skos:narrower sp:field-texture-KSHC-A ;
  skos:narrower sp:field-texture-KSHC-I ;
  skos:notation "KSHC" ;
  skos:note "Approximate clay content (%): 50% or more"@en ;
  skos:prefLabel "Coarse sandy heavy clay"@en ;
.
sp:field-texture-KSHC-A
  a skos:Concept ;
  skos:broader sp:field-texture-HC-A ;
  skos:broader sp:field-texture-KSHC ;
  skos:definition "Behaviour of moist bolus: smooth plastic bolus; handles like stiff plasticine; can be moulded into rods without fracture; has firm resistance to ribboning shear; will form ribbon of 75 mm or more."@en ;
  skos:notation "KSHCA" ;
  skos:note "Approximate clay content (%): 50% or more"@en ;
  skos:prefLabel "Sapric coarse sandy heavy clay"@en ;
.
sp:field-texture-KSHC-I
  a skos:Concept ;
  skos:broader sp:field-texture-HC-I ;
  skos:broader sp:field-texture-KSHC ;
  skos:definition "Behaviour of moist bolus: smooth plastic bolus; handles like stiff plasticine; can be moulded into rods without fracture; has firm resistance to ribboning shear; will form ribbon of 75 mm or more."@en ;
  skos:notation "KSHCI" ;
  skos:note "Approximate clay content (%): 50% or more"@en ;
  skos:prefLabel "Fibric coarse sandy heavy clay"@en ;
.
sp:field-texture-KSL
  a skos:Concept ;
  skos:broader sp:field-texture-SL ;
  skos:definition "Behaviour of moist bolus: bolus coherent but very sandy to touch; will form ribbon of 15–25 mm; dominant sand grains are of medium size and are readily visible. Coarse sand is obviously coarse to touch. Sand grains are very readily seen with the naked eye."@en ;
  skos:narrower sp:field-texture-KSL-A ;
  skos:narrower sp:field-texture-KSL-I ;
  skos:notation "KSL" ;
  skos:note "Approximate clay content (%): 10 - 20%"@en ;
  skos:prefLabel "Coarse sandy loam"@en ;
.
sp:field-texture-KSL-A
  a skos:Concept ;
  skos:broader sp:field-texture-KSL ;
  skos:broader sp:field-texture-SL-A ;
  skos:definition "Behaviour of moist bolus: bolus coherent but very sandy to touch; will form ribbon of 15–25 mm; dominant sand grains are of medium size and are readily visible. Coarse sand is obviously coarse to touch. Sand grains are very readily seen with the naked eye."@en ;
  skos:notation "KSLA" ;
  skos:note "Approximate clay content (%): 10 - 20%"@en ;
  skos:prefLabel "Sapric coarse sandy loam"@en ;
.
sp:field-texture-KSL-I
  a skos:Concept ;
  skos:broader sp:field-texture-KSL ;
  skos:broader sp:field-texture-SL-I ;
  skos:definition "Behaviour of moist bolus: bolus coherent but very sandy to touch; will form ribbon of 15–25 mm; dominant sand grains are of medium size and are readily visible. Coarse sand is obviously coarse to touch. Sand grains are very readily seen with the naked eye."@en ;
  skos:notation "KSLI" ;
  skos:note "Approximate clay content (%): 10 - 20%"@en ;
  skos:prefLabel "Fibric coarse sandy loam"@en ;
.
sp:field-texture-KSLC
  a skos:Concept ;
  skos:broader sp:field-texture-LC ;
  skos:definition "Behaviour of moist bolus: plastic bolus; smooth to touch; slight resistance to shearing between thumb and forefinger; will form ribbon of 50–75 mm."@en ;
  skos:narrower sp:field-texture-KSLC-A ;
  skos:narrower sp:field-texture-KSLC-I ;
  skos:notation "KSLC" ;
  skos:note "Approximate clay content (%): 35 - 40%"@en ;
  skos:prefLabel "Coarse sandy light clay"@en ;
.
sp:field-texture-KSLC-A
  a skos:Concept ;
  skos:broader sp:field-texture-KSLC ;
  skos:broader sp:field-texture-LC-A ;
  skos:definition "Behaviour of moist bolus: plastic bolus; smooth to touch; slight resistance to shearing between thumb and forefinger; will form ribbon of 50–75 mm."@en ;
  skos:notation "KSLCA" ;
  skos:note "Approximate clay content (%): 35 - 40%"@en ;
  skos:prefLabel "Sapric coarse sandy light clay"@en ;
.
sp:field-texture-KSLC-I
  a skos:Concept ;
  skos:broader sp:field-texture-KSLC ;
  skos:broader sp:field-texture-LC-I ;
  skos:definition "Behaviour of moist bolus: plastic bolus; smooth to touch; slight resistance to shearing between thumb and forefinger; will form ribbon of 50–75 mm."@en ;
  skos:notation "KSLCI" ;
  skos:note "Approximate clay content (%): 35 - 40%"@en ;
  skos:prefLabel "Fibric coarse sandy light clay"@en ;
.
sp:field-texture-KSLMC
  a skos:Concept ;
  skos:broader sp:field-texture-LMC ;
  skos:definition "Behaviour of moist bolus: plastic bolus; smooth to touch; slight to moderate resistance to ribboning shear; will form ribbon of about 75 mm."@en ;
  skos:narrower sp:field-texture-KSLMC-A ;
  skos:narrower sp:field-texture-KSLMC-I ;
  skos:notation "KSLMC" ;
  skos:note "Approximate clay content (%): 40 - 45%"@en ;
  skos:prefLabel "Coarse sandy light medium clay"@en ;
.
sp:field-texture-KSLMC-A
  a skos:Concept ;
  skos:broader sp:field-texture-KSLMC ;
  skos:broader sp:field-texture-LMC-A ;
  skos:definition "Behaviour of moist bolus: plastic bolus; smooth to touch; slight to moderate resistance to ribboning shear; will form ribbon of about 75 mm."@en ;
  skos:notation "KSLMCA" ;
  skos:note "Approximate clay content (%): 40 - 45%"@en ;
  skos:prefLabel "Sapric coarse sandy light medium clay"@en ;
.
sp:field-texture-KSLMC-I
  a skos:Concept ;
  skos:broader sp:field-texture-KSLMC ;
  skos:broader sp:field-texture-LMC-I ;
  skos:definition "Behaviour of moist bolus: plastic bolus; smooth to touch; slight to moderate resistance to ribboning shear; will form ribbon of about 75 mm."@en ;
  skos:notation "KSLMCI" ;
  skos:note "Approximate clay content (%): 40 - 45%"@en ;
  skos:prefLabel "Fibric coarse sandy light medium clay"@en ;
.
sp:field-texture-KSMC
  a skos:Concept ;
  skos:broader sp:field-texture-MC ;
  skos:definition "Behaviour of moist bolus: smooth plastic bolus; handles like plasticine and can be moulded into rods without fracture; has moderate resistance to ribboning shear; will form ribbon of 75 mm or more."@en ;
  skos:narrower sp:field-texture-KSMC-A ;
  skos:narrower sp:field-texture-KSMC-I ;
  skos:notation "KSMC" ;
  skos:note "Approximate clay content (%): 45 - 55%"@en ;
  skos:prefLabel "Coarse sandy medium clay"@en ;
.
sp:field-texture-KSMC-A
  a skos:Concept ;
  skos:broader sp:field-texture-KSMC ;
  skos:broader sp:field-texture-MC-A ;
  skos:definition "Behaviour of moist bolus: smooth plastic bolus; handles like plasticine and can be moulded into rods without fracture; has moderate resistance to ribboning shear; will form ribbon of 75 mm or more."@en ;
  skos:notation "KSMCA" ;
  skos:note "Approximate clay content (%): 45 - 55%"@en ;
  skos:prefLabel "Sapric coarse sandy medium clay"@en ;
.
sp:field-texture-KSMC-I
  a skos:Concept ;
  skos:broader sp:field-texture-KSMC ;
  skos:broader sp:field-texture-MC-I ;
  skos:definition "Behaviour of moist bolus: smooth plastic bolus; handles like plasticine and can be moulded into rods without fracture; has moderate resistance to ribboning shear; will form ribbon of 75 mm or more."@en ;
  skos:notation "KSMCI" ;
  skos:note "Approximate clay content (%): 45 - 55%"@en ;
  skos:prefLabel "Fibric coarse sandy medium clay"@en ;
.
sp:field-texture-KSMHC
  a skos:Concept ;
  skos:broader sp:field-texture-MHC ;
  skos:definition "Behaviour of moist bolus: smooth plastic bolus; handles like plasticine; can be moulded into rods without fracture; has moderate to firm resistance to ribboning shear; will form ribbon of 75 mm or more."@en ;
  skos:narrower sp:field-texture-KSMHC-A ;
  skos:narrower sp:field-texture-KSMHC-I ;
  skos:notation "KSMHC" ;
  skos:note "Approximate clay content (%): 50% or more"@en ;
  skos:prefLabel "Coarse sandy medium heavy clay"@en ;
.
sp:field-texture-KSMHC-A
  a skos:Concept ;
  skos:broader sp:field-texture-KSMHC ;
  skos:broader sp:field-texture-MHC-A ;
  skos:definition "Behaviour of moist bolus: smooth plastic bolus; handles like plasticine; can be moulded into rods without fracture; has moderate to firm resistance to ribboning shear; will form ribbon of 75 mm or more."@en ;
  skos:notation "KSMHCA" ;
  skos:note "Approximate clay content (%): 50% or more"@en ;
  skos:prefLabel "Sapric coarse sandy medium heavy clay"@en ;
.
sp:field-texture-KSMHC-I
  a skos:Concept ;
  skos:broader sp:field-texture-KSMHC ;
  skos:broader sp:field-texture-MHC-I ;
  skos:definition "Behaviour of moist bolus: smooth plastic bolus; handles like plasticine; can be moulded into rods without fracture; has moderate to firm resistance to ribboning shear; will form ribbon of 75 mm or more."@en ;
  skos:notation "KSMHCI" ;
  skos:note "Approximate clay content (%): 50% or more"@en ;
  skos:prefLabel "Fibric coarse sandy medium heavy clay"@en ;
.
sp:field-texture-L
  a sp:Field-texture-mineral ;
  a skos:Concept ;
  skos:definition "Behaviour of moist bolus: bolus coherent and rather spongy; smooth feel when manipulated but with no obvious sandiness or ‘silkiness’; may be somewhat greasy to the touch if much organic matter present; will form ribbon of about 25 mm."@en ;
  skos:narrower sp:field-texture-L-A ;
  skos:narrower sp:field-texture-L-I ;
  skos:notation "L" ;
  skos:note "Approximate clay content (%): about 25%"@en ;
  skos:prefLabel "Loam"@en ;
.
sp:field-texture-L-A
  a skos:Concept ;
  skos:broader sp:field-texture-L ;
  skos:definition "Behaviour of moist bolus: bolus coherent and rather spongy; smooth feel when manipulated but with no obvious sandiness or ‘silkiness’; may be somewhat greasy to the touch if much organic matter present; will form ribbon of about 25 mm."@en ;
  skos:notation "LA" ;
  skos:note """Approximate clay content (%): about 25%
Organic and non-fibrous; dark organic stain discolours fingers; greasy feel in clayey textures and coherence in sandy textures. Fibres (excluding living roots) or plant tissue remains are not visible to naked eye and little or none visible with ×10 hand lens."""@en ;
  skos:prefLabel "Sapric loam"@en ;
.
sp:field-texture-L-I
  a skos:Concept ;
  skos:broader sp:field-texture-L ;
  skos:definition "Behaviour of moist bolus: bolus coherent and rather spongy; smooth feel when manipulated but with no obvious sandiness or ‘silkiness’; may be somewhat greasy to the touch if much organic matter present; will form ribbon of about 25 mm."@en ;
  skos:notation "LI" ;
  skos:note """Approximate clay content (%): about 25%
Organic and fibrous; dark organic stain discolours fingers; greasy feel in clayey textures and coherence in sandy textures. Fibres (excluding living roots) or plant tissue remain visible to naked eye or easily visible with ×10 hand lens."""@en ;
  skos:prefLabel "Fibric loam"@en ;
.
sp:field-texture-LC
  a sp:Field-texture-mineral ;
  a skos:Concept ;
  skos:definition "Behaviour of moist bolus: plastic bolus; smooth to touch; slight resistance to shearing between thumb and forefinger; will form ribbon of 50–75 mm."@en ;
  skos:narrower sp:field-texture-FSLC ;
  skos:narrower sp:field-texture-KSLC ;
  skos:narrower sp:field-texture-LC-A ;
  skos:narrower sp:field-texture-LC-I ;
  skos:narrower sp:field-texture-SLC ;
  skos:narrower sp:field-texture-ZLC ;
  skos:notation "LC" ;
  skos:note "Approximate clay content (%): 35 - 40%"@en ;
  skos:prefLabel "Light clay"@en ;
.
sp:field-texture-LC-A
  a skos:Concept ;
  skos:broader sp:field-texture-LC ;
  skos:definition "Behaviour of moist bolus: plastic bolus; smooth to touch; slight resistance to shearing between thumb and forefinger; will form ribbon of 50–75 mm."@en ;
  skos:narrower sp:field-texture-FSLC-A ;
  skos:narrower sp:field-texture-KSLC-A ;
  skos:narrower sp:field-texture-SLC-A ;
  skos:narrower sp:field-texture-ZLC-A ;
  skos:notation "LCA" ;
  skos:note "Approximate clay content (%): 35 - 40%"@en ;
  skos:prefLabel "Sapric light clay"@en ;
.
sp:field-texture-LC-I
  a skos:Concept ;
  skos:broader sp:field-texture-LC ;
  skos:definition "Behaviour of moist bolus: plastic bolus; smooth to touch; slight resistance to shearing between thumb and forefinger; will form ribbon of 50–75 mm."@en ;
  skos:narrower sp:field-texture-FSLC-I ;
  skos:narrower sp:field-texture-KSLC-I ;
  skos:narrower sp:field-texture-SLC-I ;
  skos:narrower sp:field-texture-ZLC-I ;
  skos:notation "LCI" ;
  skos:note "Approximate clay content (%): 35 - 40%"@en ;
  skos:prefLabel "Fibric light clay"@en ;
.
sp:field-texture-LFS
  a skos:Concept ;
  skos:broader sp:field-texture-LS ;
  skos:definition "Behaviour of moist bolus: slight coherence; sand grains of medium size; can be sheared between thumb and forefinger to give minimal ribbon of about 5 mm. Fine sand can be felt and often heard when manipulated. Sand grains are clearly evident under a ×10 hand lens."@en ;
  skos:narrower sp:field-texture-LFS-A ;
  skos:narrower sp:field-texture-LFS-I ;
  skos:notation "LFS" ;
  skos:note "Approximate clay content (%): about 5%"@en ;
  skos:prefLabel "Loamy fine sand"@en ;
.
sp:field-texture-LFS-A
  a skos:Concept ;
  skos:broader sp:field-texture-LFS ;
  skos:broader sp:field-texture-LS-A ;
  skos:definition "Behaviour of moist bolus: slight coherence; sand grains of medium size; can be sheared between thumb and forefinger to give minimal ribbon of about 5 mm."@en ;
  skos:notation "LFSA" ;
  skos:note """Approximate clay content (%): about 5%
Organic and non-fibrous; dark organic stain discolours fingers; greasy feel in clayey textures and coherence in sandy textures. Fibres (excluding living roots) or plant tissue remains are not visible to naked eye and little or none visible with ×10 hand lens."""@en ;
  skos:prefLabel "Sapric loamy fine sand"@en ;
.
sp:field-texture-LFS-I
  a skos:Concept ;
  skos:broader sp:field-texture-LFS ;
  skos:broader sp:field-texture-LS-I ;
  skos:definition "Behaviour of moist bolus: slight coherence; sand grains of medium size; can be sheared between thumb and forefinger to give minimal ribbon of about 5 mm."@en ;
  skos:notation "LFSI" ;
  skos:note """Approximate clay content (%): about 5%
Organic and fibrous; dark organic stain discolours fingers; greasy feel in clayey textures and coherence in sandy textures. Fibres (excluding living roots) or plant tissue remain visible to naked eye or easily visible with ×10 hand lens."""@en ;
  skos:prefLabel "Fibric loamy fine sand"@en ;
.
sp:field-texture-LKS
  a skos:Concept ;
  skos:broader sp:field-texture-LS ;
  skos:definition "Behaviour of moist bolus: slight coherence; sand grains of medium size; can be sheared between thumb and forefinger to give minimal ribbon of about 5 mm. Coarse sand is obviously coarse to touch. Sand grains are very readily seen with the naked eye."@en ;
  skos:narrower sp:field-texture-LKS-A ;
  skos:narrower sp:field-texture-LKS-I ;
  skos:notation "LKS" ;
  skos:note "Approximate clay content (%): about 5%"@en ;
  skos:prefLabel "Loamy coarse sand"@en ;
.
sp:field-texture-LKS-A
  a skos:Concept ;
  skos:broader sp:field-texture-LKS ;
  skos:broader sp:field-texture-LS-A ;
  skos:definition "Behaviour of moist bolus: slight coherence; sand grains of medium size; can be sheared between thumb and forefinger to give minimal ribbon of about 5 mm."@en ;
  skos:notation "LKSA" ;
  skos:note """Approximate clay content (%): about 5%
Organic and non-fibrous; dark organic stain discolours fingers; greasy feel in clayey textures and coherence in sandy textures. Fibres (excluding living roots) or plant tissue remains are not visible to naked eye and little or none visible with ×10 hand lens."""@en ;
  skos:prefLabel "Sapric loamy coarse sand"@en ;
.
sp:field-texture-LKS-I
  a skos:Concept ;
  skos:broader sp:field-texture-LKS ;
  skos:broader sp:field-texture-LS-I ;
  skos:definition "Behaviour of moist bolus: slight coherence; sand grains of medium size; can be sheared between thumb and forefinger to give minimal ribbon of about 5 mm."@en ;
  skos:notation "LKSI" ;
  skos:note """Approximate clay content (%): about 5%
Organic and fibrous; dark organic stain discolours fingers; greasy feel in clayey textures and coherence in sandy textures. Fibres (excluding living roots) or plant tissue remain visible to naked eye or easily visible with ×10 hand lens."""@en ;
  skos:prefLabel "Fibric loamy coarse sand"@en ;
.
sp:field-texture-LMC
  a sp:Field-texture-mineral ;
  a skos:Concept ;
  skos:definition "Behaviour of moist bolus: plastic bolus; smooth to touch; slight to moderate resistance to ribboning shear; will form ribbon of about 75 mm."@en ;
  skos:narrower sp:field-texture-FSLMC ;
  skos:narrower sp:field-texture-KSLMC ;
  skos:narrower sp:field-texture-LMC-A ;
  skos:narrower sp:field-texture-LMC-I ;
  skos:narrower sp:field-texture-SLMC ;
  skos:narrower sp:field-texture-ZLMC ;
  skos:notation "LMC" ;
  skos:note "Approximate clay content (%): 40 - 45%"@en ;
  skos:prefLabel "Light medium clay"@en ;
.
sp:field-texture-LMC-A
  a skos:Concept ;
  skos:broader sp:field-texture-LMC ;
  skos:definition "Behaviour of moist bolus: plastic bolus; smooth to touch; slight to moderate resistance to ribboning shear; will form ribbon of about 75 mm."@en ;
  skos:narrower sp:field-texture-FSLMC-A ;
  skos:narrower sp:field-texture-KSLMC-A ;
  skos:narrower sp:field-texture-SLMC-A ;
  skos:narrower sp:field-texture-ZLMC-A ;
  skos:notation "LMCA" ;
  skos:note "Approximate clay content (%): 40 - 45%"@en ;
  skos:prefLabel "Sapric light medium clay"@en ;
.
sp:field-texture-LMC-I
  a skos:Concept ;
  skos:broader sp:field-texture-LMC ;
  skos:definition "Behaviour of moist bolus: plastic bolus; smooth to touch; slight to moderate resistance to ribboning shear; will form ribbon of about 75 mm."@en ;
  skos:narrower sp:field-texture-FSLMC-I ;
  skos:narrower sp:field-texture-KSLMC-I ;
  skos:narrower sp:field-texture-SLMC-I ;
  skos:narrower sp:field-texture-ZLMC-I ;
  skos:notation "LMCI" ;
  skos:note "Approximate clay content (%): 40 - 45%"@en ;
  skos:prefLabel "Fibric light medium clay"@en ;
.
sp:field-texture-LP
  a sp:Field-texture-organic ;
  a skos:Concept ;
  skos:definition "bolus has obvious mineral particle content but no obvious sandiness to touch and is smooth, non-sticky when wet, and weakly coherent."@en ;
  skos:notation "LP" ;
  skos:note "Organic soil"@en ;
  skos:prefLabel "Loamy peat"@en ;
.
sp:field-texture-LS
  a sp:Field-texture-mineral ;
  a skos:Concept ;
  skos:definition "Behaviour of moist bolus: slight coherence; sand grains of medium size; can be sheared between thumb and forefinger to give minimal ribbon of about 5 mm."@en ;
  skos:narrower sp:field-texture-LFS ;
  skos:narrower sp:field-texture-LKS ;
  skos:narrower sp:field-texture-LS-A ;
  skos:narrower sp:field-texture-LS-I ;
  skos:notation "LS" ;
  skos:note "Approximate clay content (%): about 5%"@en ;
  skos:prefLabel "Loamy sand"@en ;
.
sp:field-texture-LS-A
  a skos:Concept ;
  skos:broader sp:field-texture-LS ;
  skos:definition "Behaviour of moist bolus: slight coherence; sand grains of medium size; can be sheared between thumb and forefinger to give minimal ribbon of about 5 mm."@en ;
  skos:narrower sp:field-texture-LFS-A ;
  skos:narrower sp:field-texture-LKS-A ;
  skos:notation "LSA" ;
  skos:note """Approximate clay content (%): about 5%
Organic and non-fibrous; dark organic stain discolours fingers; greasy feel in clayey textures and coherence in sandy textures. Fibres (excluding living roots) or plant tissue remains are not visible to naked eye and little or none visible with ×10 hand lens."""@en ;
  skos:prefLabel "Sapric loamy sand"@en ;
.
sp:field-texture-LS-I
  a skos:Concept ;
  skos:broader sp:field-texture-LS ;
  skos:definition "Behaviour of moist bolus: slight coherence; sand grains of medium size; can be sheared between thumb and forefinger to give minimal ribbon of about 5 mm."@en ;
  skos:narrower sp:field-texture-LFS-I ;
  skos:narrower sp:field-texture-LKS-I ;
  skos:notation "LSI" ;
  skos:note """Approximate clay content (%): about 5%
Organic and fibrous; dark organic stain discolours fingers; greasy feel in clayey textures and coherence in sandy textures. Fibres (excluding living roots) or plant tissue remain visible to naked eye or easily visible with ×10 hand lens."""@en ;
  skos:prefLabel "Fibric loamy sand"@en ;
.
sp:field-texture-MC
  a sp:Field-texture-mineral ;
  a skos:Concept ;
  skos:definition "Behaviour of moist bolus: smooth plastic bolus; handles like plasticine and can be moulded into rods without fracture; has moderate resistance to ribboning shear; will form ribbon of 75 mm or more."@en ;
  skos:narrower sp:field-texture-FSMC ;
  skos:narrower sp:field-texture-KSMC ;
  skos:narrower sp:field-texture-MC-A ;
  skos:narrower sp:field-texture-MC-I ;
  skos:narrower sp:field-texture-SMC ;
  skos:narrower sp:field-texture-ZMC ;
  skos:notation "MC" ;
  skos:note "Approximate clay content (%): 45 - 55%"@en ;
  skos:prefLabel "Medium clay"@en ;
.
sp:field-texture-MC-A
  a skos:Concept ;
  skos:broader sp:field-texture-MC ;
  skos:definition "Behaviour of moist bolus: smooth plastic bolus; handles like plasticine and can be moulded into rods without fracture; has moderate resistance to ribboning shear; will form ribbon of 75 mm or more."@en ;
  skos:narrower sp:field-texture-FSMC-A ;
  skos:narrower sp:field-texture-KSMC-A ;
  skos:narrower sp:field-texture-SMC-A ;
  skos:narrower sp:field-texture-ZMC-A ;
  skos:notation "MCA" ;
  skos:note "Approximate clay content (%): 45 - 55%"@en ;
  skos:prefLabel "Sapric medium clay"@en ;
.
sp:field-texture-MC-I
  a skos:Concept ;
  skos:broader sp:field-texture-MC ;
  skos:definition "Behaviour of moist bolus: smooth plastic bolus; handles like plasticine and can be moulded into rods without fracture; has moderate resistance to ribboning shear; will form ribbon of 75 mm or more."@en ;
  skos:narrower sp:field-texture-FSMC-I ;
  skos:narrower sp:field-texture-KSMC-I ;
  skos:narrower sp:field-texture-SMC-I ;
  skos:narrower sp:field-texture-ZMC-I ;
  skos:notation "MCI" ;
  skos:note "Approximate clay content (%): 45 - 55%"@en ;
  skos:prefLabel "Fibric medium clay"@en ;
.
sp:field-texture-MHC
  a sp:Field-texture-mineral ;
  a skos:Concept ;
  skos:definition "Behaviour of moist bolus: smooth plastic bolus; handles like plasticine; can be moulded into rods without fracture; has moderate to firm resistance to ribboning shear; will form ribbon of 75 mm or more."@en ;
  skos:narrower sp:field-texture-FSMHC ;
  skos:narrower sp:field-texture-KSMHC ;
  skos:narrower sp:field-texture-MHC-A ;
  skos:narrower sp:field-texture-MHC-I ;
  skos:narrower sp:field-texture-SMHC ;
  skos:narrower sp:field-texture-ZMHC ;
  skos:notation "MHC" ;
  skos:note "Approximate clay content (%): 50% or more"@en ;
  skos:prefLabel "Medium heavy clay"@en ;
.
sp:field-texture-MHC-A
  a skos:Concept ;
  skos:broader sp:field-texture-MHC ;
  skos:definition "Behaviour of moist bolus: smooth plastic bolus; handles like plasticine; can be moulded into rods without fracture; has moderate to firm resistance to ribboning shear; will form ribbon of 75 mm or more."@en ;
  skos:narrower sp:field-texture-FSMHC-A ;
  skos:narrower sp:field-texture-KSMHC-A ;
  skos:narrower sp:field-texture-SMHC-A ;
  skos:narrower sp:field-texture-ZMHC-A ;
  skos:notation "MHCA" ;
  skos:note "Approximate clay content (%): 50% or more"@en ;
  skos:prefLabel "Sapric medium heavy clay"@en ;
.
sp:field-texture-MHC-I
  a skos:Concept ;
  skos:broader sp:field-texture-MHC ;
  skos:definition "Behaviour of moist bolus: smooth plastic bolus; handles like plasticine; can be moulded into rods without fracture; has moderate to firm resistance to ribboning shear; will form ribbon of 75 mm or more."@en ;
  skos:narrower sp:field-texture-FSMHC-I ;
  skos:narrower sp:field-texture-KSMHC-I ;
  skos:narrower sp:field-texture-SMHC-I ;
  skos:narrower sp:field-texture-ZMHC-I ;
  skos:notation "MHCI" ;
  skos:note "Approximate clay content (%): 50% or more"@en ;
  skos:prefLabel "Fibric medium heavy clay"@en ;
.
sp:field-texture-S
  a sp:Field-texture-mineral ;
  a skos:Concept ;
  skos:definition "Behaviour of moist bolus: coherence nil to very slight, cannot be moulded; sand grains of medium size; single sand grains adhere to fingers."@en ;
  skos:narrower sp:field-texture-FS ;
  skos:narrower sp:field-texture-KS ;
  skos:narrower sp:field-texture-S-A ;
  skos:narrower sp:field-texture-S-I ;
  skos:notation "S" ;
  skos:note "Approximate clay content (%): commonly less than 5%"@en ;
  skos:prefLabel "Sand (field texture)"@en ;
.
sp:field-texture-S-A
  a skos:Concept ;
  skos:broader sp:field-texture-S ;
  skos:definition "Behaviour of moist bolus: coherence nil to very slight, cannot be moulded; sand grains of medium size; single sand grains adhere to fingers."@en ;
  skos:narrower sp:field-texture-FS-A ;
  skos:narrower sp:field-texture-KS-A ;
  skos:notation "SA" ;
  skos:note """Approximate clay content (%): commonly less than 5%
Organic and non-fibrous; dark organic stain discolours fingers; greasy feel in clayey textures and coherence in sandy textures. Fibres (excluding living roots) or plant tissue remains are not visible to naked eye and little or none visible with ×10 hand lens."""@en ;
  skos:prefLabel "Sapric sand"@en ;
.
sp:field-texture-S-I
  a skos:Concept ;
  skos:broader sp:field-texture-S ;
  skos:definition "Behaviour of moist bolus: coherence nil to very slight, cannot be moulded; sand grains of medium size; single sand grains adhere to fingers."@en ;
  skos:narrower sp:field-texture-FS-I ;
  skos:narrower sp:field-texture-KS-I ;
  skos:notation "SI" ;
  skos:note """Approximate clay content (%): commonly less than 5%
Organic and fibrous; dark organic stain discolours fingers; greasy feel in clayey textures and coherence in sandy textures. Fibres (excluding living roots) or plant tissue remain visible to naked eye or easily visible with ×10 hand lens."""@en ;
  skos:prefLabel "Fibric sand"@en ;
.
sp:field-texture-SCL
  a sp:Field-texture-mineral ;
  a skos:Concept ;
  skos:definition "Behaviour of moist bolus: strongly coherent bolus, sandy to touch; medium-size sand grains visible in finer matrix; will form ribbon of 25–40 mm."@en ;
  skos:narrower sp:field-texture-FSCL ;
  skos:narrower sp:field-texture-KSCL ;
  skos:narrower sp:field-texture-SCL-A ;
  skos:narrower sp:field-texture-SCL-I ;
  skos:narrower sp:field-texture-SCL-heavy ;
  skos:narrower sp:field-texture-SCL-light ;
  skos:notation "SCL" ;
  skos:note "Approximate clay content (%): 20 - 30%"@en ;
  skos:prefLabel "Sandy clay loam"@en ;
.
sp:field-texture-SCL-A
  a skos:Concept ;
  skos:broader sp:field-texture-SCL ;
  skos:definition "Behaviour of moist bolus: strongly coherent bolus, sandy to touch; medium-size sand grains visible in finer matrix; will form ribbon of 25–40 mm."@en ;
  skos:narrower sp:field-texture-FSCL-A ;
  skos:narrower sp:field-texture-KSCL-A ;
  skos:notation "SCLA" ;
  skos:note "Approximate clay content (%): 20 - 30%"@en ;
  skos:prefLabel "Sapric sandy clay loam"@en ;
.
sp:field-texture-SCL-I
  a skos:Concept ;
  skos:broader sp:field-texture-SCL ;
  skos:definition "Behaviour of moist bolus: strongly coherent bolus, sandy to touch; medium-size sand grains visible in finer matrix; will form ribbon of 25–40 mm."@en ;
  skos:narrower sp:field-texture-FSCL-I ;
  skos:narrower sp:field-texture-KSCL-I ;
  skos:notation "SCLI" ;
  skos:note "Approximate clay content (%): 20 - 30%"@en ;
  skos:prefLabel "Fibric sandy clay loam"@en ;
.
sp:field-texture-SCL-heavy
  a skos:Concept ;
  skos:broader sp:field-texture-SCL ;
  skos:definition "Behaviour of moist bolus: strongly coherent bolus, sandy to touch; medium-size sand grains visible in finer matrix; will form ribbon of 25–40 mm."@en ;
  skos:narrower sp:field-texture-FSCL-heavy ;
  skos:narrower sp:field-texture-KSCL-heavy ;
  skos:notation "SCL+"@en ;
  skos:note "Approximate clay content (%): 20 - 30%"@en ;
  skos:prefLabel "Heavy sandy clay loam"@en ;
.
sp:field-texture-SCL-light
  a skos:Concept ;
  skos:broader sp:field-texture-SCL ;
  skos:definition "Behaviour of moist bolus: strongly coherent bolus, sandy to touch; medium-size sand grains visible in finer matrix; will form ribbon of 25–40 mm."@en ;
  skos:narrower sp:field-texture-FSCL-light ;
  skos:narrower sp:field-texture-KSCL-light ;
  skos:notation "SCL-"@en ;
  skos:note "Approximate clay content (%): 20 - 30%"@en ;
  skos:prefLabel "Light sandy clay loam"@en ;
.
sp:field-texture-SHC
  a skos:Concept ;
  skos:broader sp:field-texture-HC ;
  skos:definition "Behaviour of moist bolus: smooth plastic bolus; handles like stiff plasticine; can be moulded into rods without fracture; has firm resistance to ribboning shear; will form ribbon of 75 mm or more."@en ;
  skos:narrower sp:field-texture-SHC-A ;
  skos:narrower sp:field-texture-SHC-I ;
  skos:notation "SHC" ;
  skos:note "Approximate clay content (%): 50% or more"@en ;
  skos:prefLabel "Sandy heavy clay"@en ;
.
sp:field-texture-SHC-A
  a skos:Concept ;
  skos:broader sp:field-texture-HC-A ;
  skos:broader sp:field-texture-SHC ;
  skos:definition "Behaviour of moist bolus: smooth plastic bolus; handles like stiff plasticine; can be moulded into rods without fracture; has firm resistance to ribboning shear; will form ribbon of 75 mm or more."@en ;
  skos:notation "SHCA" ;
  skos:note "Approximate clay content (%): 50% or more"@en ;
  skos:prefLabel "Sapric sandy heavy clay"@en ;
.
sp:field-texture-SHC-I
  a skos:Concept ;
  skos:broader sp:field-texture-HC-I ;
  skos:broader sp:field-texture-SHC ;
  skos:definition "Behaviour of moist bolus: smooth plastic bolus; handles like stiff plasticine; can be moulded into rods without fracture; has firm resistance to ribboning shear; will form ribbon of 75 mm or more."@en ;
  skos:notation "SHCI" ;
  skos:note "Approximate clay content (%): 50% or more"@en ;
  skos:prefLabel "Fibric sandy heavy clay"@en ;
.
sp:field-texture-SL
  a sp:Field-texture-mineral ;
  a skos:Concept ;
  skos:definition "Behaviour of moist bolus: bolus coherent but very sandy to touch; will form ribbon of 15–25 mm; dominant sand grains are of medium size and are readily visible."@en ;
  skos:narrower sp:field-texture-FSL ;
  skos:narrower sp:field-texture-KSL ;
  skos:narrower sp:field-texture-SL-A ;
  skos:narrower sp:field-texture-SL-I ;
  skos:notation "SL" ;
  skos:note "Approximate clay content (%): 10 - 20%"@en ;
  skos:prefLabel "Sandy loam"@en ;
.
sp:field-texture-SL-A
  a skos:Concept ;
  skos:broader sp:field-texture-SL ;
  skos:definition "Behaviour of moist bolus: bolus coherent but very sandy to touch; will form ribbon of 15–25 mm; dominant sand grains are of medium size and are readily visible."@en ;
  skos:narrower sp:field-texture-FSL-A ;
  skos:narrower sp:field-texture-KSL-A ;
  skos:notation "SLA" ;
  skos:note "Approximate clay content (%): 10 - 20%"@en ;
  skos:prefLabel "Sapric sandy loam"@en ;
.
sp:field-texture-SL-I
  a skos:Concept ;
  skos:broader sp:field-texture-SL ;
  skos:definition "Behaviour of moist bolus: bolus coherent but very sandy to touch; will form ribbon of 15–25 mm; dominant sand grains are of medium size and are readily visible."@en ;
  skos:narrower sp:field-texture-FSL-I ;
  skos:narrower sp:field-texture-KSL-I ;
  skos:notation "SLI" ;
  skos:note "Approximate clay content (%): 10 - 20%"@en ;
  skos:prefLabel "Fibric sandy loam"@en ;
.
sp:field-texture-SLC
  a skos:Concept ;
  skos:broader sp:field-texture-LC ;
  skos:definition "Behaviour of moist bolus: plastic bolus; smooth to touch; slight resistance to shearing between thumb and forefinger; will form ribbon of 50–75 mm."@en ;
  skos:narrower sp:field-texture-SLC-A ;
  skos:narrower sp:field-texture-SLC-I ;
  skos:notation "SLC" ;
  skos:note "Approximate clay content (%): 35 - 40%"@en ;
  skos:prefLabel "Sandy light clay"@en ;
.
sp:field-texture-SLC-A
  a skos:Concept ;
  skos:broader sp:field-texture-LC-A ;
  skos:broader sp:field-texture-SLC ;
  skos:definition "Behaviour of moist bolus: plastic bolus; smooth to touch; slight resistance to shearing between thumb and forefinger; will form ribbon of 50–75 mm."@en ;
  skos:notation "SLCA" ;
  skos:note "Approximate clay content (%): 35 - 40%"@en ;
  skos:prefLabel "Sapric sandy light clay"@en ;
.
sp:field-texture-SLC-I
  a skos:Concept ;
  skos:broader sp:field-texture-LC-I ;
  skos:broader sp:field-texture-SLC ;
  skos:definition "Behaviour of moist bolus: plastic bolus; smooth to touch; slight resistance to shearing between thumb and forefinger; will form ribbon of 50–75 mm."@en ;
  skos:notation "SLCI" ;
  skos:note "Approximate clay content (%): 35 - 40%"@en ;
  skos:prefLabel "Fibric sandy light clay"@en ;
.
sp:field-texture-SLMC
  a skos:Concept ;
  skos:broader sp:field-texture-LMC ;
  skos:definition "Behaviour of moist bolus: plastic bolus; smooth to touch; slight to moderate resistance to ribboning shear; will form ribbon of about 75 mm."@en ;
  skos:narrower sp:field-texture-SLMC-A ;
  skos:narrower sp:field-texture-SLMC-I ;
  skos:notation "SLMC" ;
  skos:note "Approximate clay content (%): 40 - 45%"@en ;
  skos:prefLabel "Sandy light medium clay"@en ;
.
sp:field-texture-SLMC-A
  a skos:Concept ;
  skos:broader sp:field-texture-LMC-A ;
  skos:broader sp:field-texture-SLMC ;
  skos:definition "Behaviour of moist bolus: plastic bolus; smooth to touch; slight to moderate resistance to ribboning shear; will form ribbon of about 75 mm."@en ;
  skos:notation "SLMCA" ;
  skos:note "Approximate clay content (%): 40 - 45%"@en ;
  skos:prefLabel "Sapric sandy light medium clay"@en ;
.
sp:field-texture-SLMC-I
  a skos:Concept ;
  skos:broader sp:field-texture-LMC-I ;
  skos:broader sp:field-texture-SLMC ;
  skos:definition "Behaviour of moist bolus: plastic bolus; smooth to touch; slight to moderate resistance to ribboning shear; will form ribbon of about 75 mm."@en ;
  skos:notation "SLMCI" ;
  skos:note "Approximate clay content (%): 40 - 45%"@en ;
  skos:prefLabel "Fibric sandy light medium clay"@en ;
.
sp:field-texture-SMC
  a skos:Concept ;
  skos:broader sp:field-texture-MC ;
  skos:definition "Behaviour of moist bolus: smooth plastic bolus; handles like plasticine and can be moulded into rods without fracture; has moderate resistance to ribboning shear; will form ribbon of 75 mm or more."@en ;
  skos:narrower sp:field-texture-SMC-A ;
  skos:narrower sp:field-texture-SMC-I ;
  skos:notation "SMC" ;
  skos:note "Approximate clay content (%): 45 - 55%"@en ;
  skos:prefLabel "Sandy medium clay"@en ;
.
sp:field-texture-SMC-A
  a skos:Concept ;
  skos:broader sp:field-texture-MC-A ;
  skos:broader sp:field-texture-SMC ;
  skos:definition "Behaviour of moist bolus: smooth plastic bolus; handles like plasticine and can be moulded into rods without fracture; has moderate resistance to ribboning shear; will form ribbon of 75 mm or more."@en ;
  skos:notation "SMCA" ;
  skos:note "Approximate clay content (%): 45 - 55%"@en ;
  skos:prefLabel "Sapric sandy medium clay"@en ;
.
sp:field-texture-SMC-I
  a skos:Concept ;
  skos:broader sp:field-texture-MC-I ;
  skos:broader sp:field-texture-SMC ;
  skos:definition "Behaviour of moist bolus: smooth plastic bolus; handles like plasticine and can be moulded into rods without fracture; has moderate resistance to ribboning shear; will form ribbon of 75 mm or more."@en ;
  skos:notation "SMCI" ;
  skos:note "Approximate clay content (%): 45 - 55%"@en ;
  skos:prefLabel "Fibric sandy medium clay"@en ;
.
sp:field-texture-SMHC
  a skos:Concept ;
  skos:broader sp:field-texture-MHC ;
  skos:definition "Behaviour of moist bolus: smooth plastic bolus; handles like plasticine; can be moulded into rods without fracture; has moderate to firm resistance to ribboning shear; will form ribbon of 75 mm or more."@en ;
  skos:narrower sp:field-texture-SMHC-A ;
  skos:narrower sp:field-texture-SMHC-I ;
  skos:notation "SMHC" ;
  skos:note "Approximate clay content (%): 50% or more"@en ;
  skos:prefLabel "Sandy medium heavy clay"@en ;
.
sp:field-texture-SMHC-A
  a skos:Concept ;
  skos:broader sp:field-texture-MHC-A ;
  skos:broader sp:field-texture-SMHC ;
  skos:definition "Behaviour of moist bolus: smooth plastic bolus; handles like plasticine; can be moulded into rods without fracture; has moderate to firm resistance to ribboning shear; will form ribbon of 75 mm or more."@en ;
  skos:notation "SMHCA" ;
  skos:note "Approximate clay content (%): 50% or more"@en ;
  skos:prefLabel "Sapric sandy medium heavy clay"@en ;
.
sp:field-texture-SMHC-I
  a skos:Concept ;
  skos:broader sp:field-texture-MHC-I ;
  skos:broader sp:field-texture-SMHC ;
  skos:definition "Behaviour of moist bolus: smooth plastic bolus; handles like plasticine; can be moulded into rods without fracture; has moderate to firm resistance to ribboning shear; will form ribbon of 75 mm or more."@en ;
  skos:notation "SMHCI" ;
  skos:note "Approximate clay content (%): 50% or more"@en ;
  skos:prefLabel "Fibric sandy medium heavy clay"@en ;
.
sp:field-texture-SP
  a sp:Field-texture-organic ;
  a skos:Concept ;
  skos:definition "bolus is sandy to touch."@en ;
  skos:notation "SP" ;
  skos:note "Organic soil"@en ;
  skos:prefLabel "Sandy peat"@en ;
.
sp:field-texture-ZCL
  a sp:Field-texture-mineral ;
  a skos:Concept ;
  skos:definition "Behaviour of moist bolus: coherent smooth bolus, plastic and often silky to the touch; will form ribbon of 40–50 mm."@en ;
  skos:narrower sp:field-texture-ZCL-A ;
  skos:narrower sp:field-texture-ZCL-I ;
  skos:narrower sp:field-texture-ZCL-heavy ;
  skos:narrower sp:field-texture-ZCL-light ;
  skos:notation "ZCL" ;
  skos:note "Approximate clay content (%): 30 - 35% and with silt 25% or more"@en ;
  skos:prefLabel "Silty clay loam"@en ;
.
sp:field-texture-ZCL-A
  a skos:Concept ;
  skos:broader sp:field-texture-ZCL ;
  skos:definition "Behaviour of moist bolus: coherent smooth bolus, plastic and often silky to the touch; will form ribbon of 40–50 mm."@en ;
  skos:notation "ZCLA" ;
  skos:note "Approximate clay content (%): 30 - 35% and with silt 25% or more"@en ;
  skos:prefLabel "Sapric silty clay loam"@en ;
.
sp:field-texture-ZCL-I
  a skos:Concept ;
  skos:broader sp:field-texture-ZCL ;
  skos:definition "Behaviour of moist bolus: coherent smooth bolus, plastic and often silky to the touch; will form ribbon of 40–50 mm."@en ;
  skos:notation "ZCLI" ;
  skos:note "Approximate clay content (%): 30 - 35% and with silt 25% or more"@en ;
  skos:prefLabel "Fibric silty clay loam"@en ;
.
sp:field-texture-ZCL-heavy
  a skos:Concept ;
  skos:broader sp:field-texture-ZCL ;
  skos:definition "Behaviour of moist bolus: coherent smooth bolus, plastic and often silky to the touch; will form ribbon of 40–50 mm."@en ;
  skos:notation "ZCL+"@en ;
  skos:note "Approximate clay content (%): 30 - 35% and with silt 25% or more"@en ;
  skos:prefLabel "Heavy silty clay loam"@en ;
.
sp:field-texture-ZCL-light
  a skos:Concept ;
  skos:broader sp:field-texture-ZCL ;
  skos:definition "Behaviour of moist bolus: coherent smooth bolus, plastic and often silky to the touch; will form ribbon of 40–50 mm."@en ;
  skos:notation "ZCL-"@en ;
  skos:note "Approximate clay content (%): 30 - 35% and with silt 25% or more"@en ;
  skos:prefLabel "Light silty clay loam"@en ;
.
sp:field-texture-ZHC
  a skos:Concept ;
  skos:broader sp:field-texture-HC ;
  skos:definition "Behaviour of moist bolus: smooth plastic bolus; handles like stiff plasticine; can be moulded into rods without fracture; has firm resistance to ribboning shear; will form ribbon of 75 mm or more."@en ;
  skos:narrower sp:field-texture-ZHC-A ;
  skos:narrower sp:field-texture-ZHC-I ;
  skos:notation "ZHC" ;
  skos:note "Approximate clay content (%): 50% or more"@en ;
  skos:prefLabel "Silty heavy clay"@en ;
.
sp:field-texture-ZHC-A
  a skos:Concept ;
  skos:broader sp:field-texture-HC-A ;
  skos:broader sp:field-texture-ZHC ;
  skos:definition "Behaviour of moist bolus: smooth plastic bolus; handles like stiff plasticine; can be moulded into rods without fracture; has firm resistance to ribboning shear; will form ribbon of 75 mm or more."@en ;
  skos:notation "ZHCA" ;
  skos:note "Approximate clay content (%): 50% or more"@en ;
  skos:prefLabel "Sapric silty heavy clay"@en ;
.
sp:field-texture-ZHC-I
  a skos:Concept ;
  skos:broader sp:field-texture-HC-I ;
  skos:broader sp:field-texture-ZHC ;
  skos:definition "Behaviour of moist bolus: smooth plastic bolus; handles like stiff plasticine; can be moulded into rods without fracture; has firm resistance to ribboning shear; will form ribbon of 75 mm or more."@en ;
  skos:notation "ZHCI" ;
  skos:note "Approximate clay content (%): 50% or more"@en ;
  skos:prefLabel "Fibric silty heavy clay"@en ;
.
sp:field-texture-ZL
  a sp:Field-texture-mineral ;
  a skos:Concept ;
  skos:definition "Behaviour of moist bolus: coherent bolus; very smooth to often silky when manipulated; will form ribbon of about 25 mm."@en ;
  skos:narrower sp:field-texture-ZL-A ;
  skos:narrower sp:field-texture-ZL-I ;
  skos:notation "ZL" ;
  skos:note "Approximate clay content (%): about 25% and with silt 25% or more."@en ;
  skos:prefLabel "Silty loam"@en ;
.
sp:field-texture-ZL-A
  a skos:Concept ;
  skos:broader sp:field-texture-ZL ;
  skos:definition "Behaviour of moist bolus: coherent bolus; very smooth to often silky when manipulated; will form ribbon of about 25 mm."@en ;
  skos:notation "ZLA" ;
  skos:note "Approximate clay content (%): about 25% and with silt 25% or more."@en ;
  skos:prefLabel "Sapric silty loam"@en ;
.
sp:field-texture-ZL-I
  a skos:Concept ;
  skos:broader sp:field-texture-ZL ;
  skos:definition "Behaviour of moist bolus: coherent bolus; very smooth to often silky when manipulated; will form ribbon of about 25 mm."@en ;
  skos:notation "ZLI" ;
  skos:note "Approximate clay content (%): about 25% and with silt 25% or more."@en ;
  skos:prefLabel "Fibric silty loam"@en ;
.
sp:field-texture-ZLC
  a skos:Concept ;
  skos:broader sp:field-texture-LC ;
  skos:definition "Behaviour of moist bolus: plastic bolus; smooth to touch; slight resistance to shearing between thumb and forefinger; will form ribbon of 50–75 mm."@en ;
  skos:narrower sp:field-texture-ZLC-A ;
  skos:narrower sp:field-texture-ZLC-I ;
  skos:notation "ZLC" ;
  skos:note "Approximate clay content (%): 35 - 40%"@en ;
  skos:prefLabel "Silty light clay"@en ;
.
sp:field-texture-ZLC-A
  a skos:Concept ;
  skos:broader sp:field-texture-LC-A ;
  skos:broader sp:field-texture-ZLC ;
  skos:definition "Behaviour of moist bolus: plastic bolus; smooth to touch; slight resistance to shearing between thumb and forefinger; will form ribbon of 50–75 mm."@en ;
  skos:notation "ZLCA" ;
  skos:note "Approximate clay content (%): 35 - 40%"@en ;
  skos:prefLabel "Sapric silty light clay"@en ;
.
sp:field-texture-ZLC-I
  a skos:Concept ;
  skos:broader sp:field-texture-LC-I ;
  skos:broader sp:field-texture-ZLC ;
  skos:definition "Behaviour of moist bolus: plastic bolus; smooth to touch; slight resistance to shearing between thumb and forefinger; will form ribbon of 50–75 mm."@en ;
  skos:notation "ZLCI" ;
  skos:note "Approximate clay content (%): 35 - 40%"@en ;
  skos:prefLabel "Fibric silty light clay"@en ;
.
sp:field-texture-ZLMC
  a skos:Concept ;
  skos:broader sp:field-texture-LMC ;
  skos:definition "Behaviour of moist bolus: plastic bolus; smooth to touch; slight to moderate resistance to ribboning shear; will form ribbon of about 75 mm."@en ;
  skos:narrower sp:field-texture-ZLMC-A ;
  skos:narrower sp:field-texture-ZLMC-I ;
  skos:notation "ZLMC" ;
  skos:note "Approximate clay content (%): 40 - 45%"@en ;
  skos:prefLabel "Silty light medium clay"@en ;
.
sp:field-texture-ZLMC-A
  a skos:Concept ;
  skos:broader sp:field-texture-LMC-A ;
  skos:broader sp:field-texture-ZLMC ;
  skos:definition "Behaviour of moist bolus: plastic bolus; smooth to touch; slight to moderate resistance to ribboning shear; will form ribbon of about 75 mm."@en ;
  skos:notation "ZLMCA" ;
  skos:note "Approximate clay content (%): 40 - 45%"@en ;
  skos:prefLabel "Sapric silty light medium clay"@en ;
.
sp:field-texture-ZLMC-I
  a skos:Concept ;
  skos:broader sp:field-texture-LMC-I ;
  skos:broader sp:field-texture-ZLMC ;
  skos:definition "Behaviour of moist bolus: plastic bolus; smooth to touch; slight to moderate resistance to ribboning shear; will form ribbon of about 75 mm."@en ;
  skos:notation "ZLMCI" ;
  skos:note "Approximate clay content (%): 40 - 45%"@en ;
  skos:prefLabel "Fibric silty light medium clay"@en ;
.
sp:field-texture-ZMC
  a skos:Concept ;
  skos:broader sp:field-texture-MC ;
  skos:definition "Behaviour of moist bolus: smooth plastic bolus; handles like plasticine and can be moulded into rods without fracture; has moderate resistance to ribboning shear; will form ribbon of 75 mm or more."@en ;
  skos:narrower sp:field-texture-ZMC-A ;
  skos:narrower sp:field-texture-ZMC-I ;
  skos:notation "ZMC" ;
  skos:note "Approximate clay content (%): 45 - 55%"@en ;
  skos:prefLabel "Silty medium clay"@en ;
.
sp:field-texture-ZMC-A
  a skos:Concept ;
  skos:broader sp:field-texture-MC-A ;
  skos:broader sp:field-texture-ZMC ;
  skos:definition "Behaviour of moist bolus: smooth plastic bolus; handles like plasticine and can be moulded into rods without fracture; has moderate resistance to ribboning shear; will form ribbon of 75 mm or more."@en ;
  skos:notation "ZMCA" ;
  skos:note "Approximate clay content (%): 45 - 55%"@en ;
  skos:prefLabel "Sapric silty medium clay"@en ;
.
sp:field-texture-ZMC-I
  a skos:Concept ;
  skos:broader sp:field-texture-MC-I ;
  skos:broader sp:field-texture-ZMC ;
  skos:definition "Behaviour of moist bolus: smooth plastic bolus; handles like plasticine and can be moulded into rods without fracture; has moderate resistance to ribboning shear; will form ribbon of 75 mm or more."@en ;
  skos:notation "ZMCI" ;
  skos:note "Approximate clay content (%): 45 - 55%"@en ;
  skos:prefLabel "Fibric silty medium clay"@en ;
.
sp:field-texture-ZMHC
  a skos:Concept ;
  skos:broader sp:field-texture-MHC ;
  skos:definition "Behaviour of moist bolus: smooth plastic bolus; handles like plasticine; can be moulded into rods without fracture; has moderate to firm resistance to ribboning shear; will form ribbon of 75 mm or more."@en ;
  skos:narrower sp:field-texture-ZMHC-A ;
  skos:narrower sp:field-texture-ZMHC-I ;
  skos:notation "ZMHC" ;
  skos:note "Approximate clay content (%): 50% or more"@en ;
  skos:prefLabel "Silty medium heavy clay"@en ;
.
sp:field-texture-ZMHC-A
  a skos:Concept ;
  skos:broader sp:field-texture-MHC-A ;
  skos:broader sp:field-texture-ZMHC ;
  skos:definition "Behaviour of moist bolus: smooth plastic bolus; handles like plasticine; can be moulded into rods without fracture; has moderate to firm resistance to ribboning shear; will form ribbon of 75 mm or more."@en ;
  skos:notation "ZMHCA" ;
  skos:note "Approximate clay content (%): 50% or more"@en ;
  skos:prefLabel "Sapric silty medium heavy clay"@en ;
.
sp:field-texture-ZMHC-I
  a skos:Concept ;
  skos:broader sp:field-texture-MHC-I ;
  skos:broader sp:field-texture-ZMHC ;
  skos:definition "Behaviour of moist bolus: smooth plastic bolus; handles like plasticine; can be moulded into rods without fracture; has moderate to firm resistance to ribboning shear; will form ribbon of 75 mm or more."@en ;
  skos:notation "ZMHCI" ;
  skos:note "Approximate clay content (%): 50% or more"@en ;
  skos:prefLabel "Fibric silty medium heavy clay"@en ;
.
sp:field-texture-qualifier-fibric
  a sp:Field-texture-qualifier ;
  a skos:Concept ;
  skos:definition "Organic and non-fibrous; dark organic stain discolours fingers; greasy feel in clayey textures and coherence in sandy textures. Fibres (excluding living roots) or plant tissue remains are not visible to naked eye and little or none visible with ×10 hand lens."@en ;
  skos:notation "I" ;
  skos:note "The qualifier code is added after the field texture." ;
  skos:prefLabel "Fibric"@en ;
.
sp:field-texture-qualifier-heavy
  a sp:Field-texture-qualifier ;
  a skos:Concept ;
  skos:definition "Higher clay content end of the range"@en ;
  skos:notation "+" ;
  skos:note "The qualifier code is added after the field texture." ;
  skos:prefLabel "Heavy"@en ;
.
sp:field-texture-qualifier-light
  a sp:Field-texture-qualifier ;
  a skos:Concept ;
  skos:definition "Lighter clay content end of the range"@en ;
  skos:notation "-" ;
  skos:note "The qualifier code is added after the field texture." ;
  skos:prefLabel "Light"@en ;
.
sp:field-texture-qualifier-sapric
  a sp:Field-texture-qualifier ;
  a skos:Concept ;
  skos:definition "Organic and non-fibrous; dark organic stain discolours fingers; greasy feel in clayey textures and coherence in sandy textures. Fibres (excluding living roots) or plant tissue remains are not visible to naked eye and little or none visible with ×10 hand lens."@en ;
  skos:notation "A" ;
  skos:note "The qualifier code is added after the field texture." ;
  skos:prefLabel "Sapric"@en ;
.
sp:field-textures
  a skos:Collection ;
  rdfs:isDefinedBy asls:soil-profile ;
  skos:inScheme asls:soil-profile ;
  dcterms:description """<p><img src=\"http://anzsoil.org/resources/yellowbook/Figure15.png\" /></p>
<p> Figure 15 Size Fractions in several major classification systems. </p>"""^^rdf:HTML ;
  rdfs:comment "C_H_TEXTURE" ;
  skos:definition """Soil texture is determined by the size distribution of mineral particles finer than 2 mm, that is, only material that will pass a 2 mm sieve should be used in determination of field texture. Organic soils are also included.
In Australia, field texture classes or field texture grades (Northcote 1979) are based on field determination of texture and not on laboratory determinations of particle size, as is done in USA for example (Soil Survey Staff 1975). There is only an approximate relationship between field texture and particle size distribution (see Marshall 1947), as factors other than clay, silt and sand content influence field texture.
Figure 15 gives a comparison between International particle size fractions, used in Australia, and those of other major classifications."""@en ;
  skos:member sp:Field-texture-mineral ;
  skos:member sp:Field-texture-organic ;
  skos:note "Adapted from Northcote (1979). The clay percentages must not be used to determine a field texture, that is, do not use them to convert a laboratory particle size value to a field texture grade. Similarly, do not adjust a field texture grade when laboratory particle size data become available."@en ;
  skos:prefLabel "Field texture"@en ;
.
sp:horizon-A1
  a skos:Concept ;
  skos:broader sp:horizons-A ;
  skos:definition "mineral horizon at or near the soil surface with some accumulation of humified organic matter, usually darker in colour than underlying horizons and with maximum biologic activity for any given soil profile. It may be divided into subhorizons and of these the A11 horizon is usually the more organic, or darker coloured uppermost portion. The A12 differs in either hue, value or chroma from the A11, usually being lighter in colour. It is not pale enough to qualify as an A2 horizon. The A1 may be further divided into subhorizons if necessary (e.g. A13, A14)."@en ;
  skos:notation "A1" ;
  skos:prefLabel "A1 horizon"@en ;
.
sp:horizon-A2
  a skos:Concept ;
  skos:broader sp:horizons-A ;
  skos:definition "mineral horizon having, either alone or in combination, less organic matter, sesquioxides, or silicate clay than immediately adjacent horizons. It is usually differentiated from the A1 horizon by its paler colour, that is, by having colour value at least one unit higher and usually less organic matter. It is usually differentiated from the B horizon by having colour value at least one unit higher and chroma at least two units lower, by coarser texture or by a combination of these attributes."@en ;
  skos:notation "A2" ;
  skos:prefLabel "A2 horizon"@en ;
.
sp:horizon-A3
  a skos:Concept ;
  skos:broader sp:horizons-A ;
  skos:definition "transitional horizon between A and B, which is dominated by properties characteristic of an overlying A1 or A2."@en ;
  skos:notation "A3" ;
  skos:prefLabel "A3 horizon"@en ;
.
sp:horizon-B1
  a skos:Concept ;
  skos:broader sp:horizons-B ;
  skos:definition "transitional horizon between A and B, which is dominated by properties characteristic of an underlying B2."@en ;
  skos:notation "B1" ;
  skos:prefLabel "B1 horizon"@en ;
.
sp:horizon-B2
  a skos:Concept ;
  dcterms:description """horizon in which the dominant feature is one or more of the following:
•	an illuvial, residual or other concentration of silicate clay, or iron, aluminium or humus, either alone or in combination
•	maximum development of pedologic organisation* as evidenced by a different structure and/or consistence, and/or stronger colours than the A horizons above or any horizon immediately below.
It may be divided into subhorizons, for example B21, B22, B23."""@en ;
  skos:broader sp:horizons-B ;
  skos:definition """horizon in which the dominant feature is one or more of the following:
•	an illuvial, residual or other concentration of silicate clay, or iron, aluminium or humus, either alone or in combination
•	maximum development of pedologic organisation* as evidenced by a different structure and/or consistence, and/or stronger colours than the A horizons above or any horizon immediately below.
It may be divided into subhorizons, for example B21, B22, B23.
"""@en ;
  skos:notation "B2" ;
  skos:note "Pedologic organisation is a broad term used to include all changes in soil material resulting from the effect of physical, chemical and biologic processes, that is, soil formation. Results of these processes include horizonation, colour differences, presence of pedality, and texture and/or consistence changes"@en ;
  skos:prefLabel "B2 horizon"@en ;
.
sp:horizon-B3
  a skos:Concept ;
  skos:broader sp:horizons-B ;
  skos:definition "transitional horizon between B and C or other subsolum material in which properties characteristic of an overlying B2 dominate, but intergrade to those of the underlying material."@en ;
  skos:notation "B3" ;
  skos:prefLabel "B3 horizon"@en ;
.
sp:horizon-O1
  a skos:Concept ;
  skos:broader sp:horizons-O ;
  skos:definition "consists of undecomposed organic debris, usually dominated by leaves and twigs. The original form of the debris can be recognised with the naked eye."@en ;
  skos:notation "O1" ;
  skos:prefLabel "O1 horizon"@en ;
.
sp:horizon-O2
  a skos:Concept ;
  skos:broader sp:horizons-O ;
  skos:definition "consists of organic debris in various stages of decomposition. The original form of most of the debris cannot be recognised with the naked eye."@en ;
  skos:notation "O2" ;
  skos:prefLabel "O2 horizon"@en ;
.
sp:horizon-P1
  a skos:Concept ;
  skos:broader sp:horizons-P ;
  skos:definition "consists primarily of undecomposed or weakly decomposed organic material (fibric peat). Plant remains are distinct and readily identifiable."@en ;
  skos:notation "P1" ;
  skos:prefLabel "P1 horizon"@en ;
.
sp:horizon-P2
  a skos:Concept ;
  skos:broader sp:horizons-P ;
  skos:definition "consists primarily of moderately to completely decomposed organic material (hemic to sapric peat). Plant remains vary from being difficult to identify to completely amorphous."@en ;
  skos:notation "P2" ;
  skos:prefLabel "P2 horizon"@en ;
.
sp:horizon-boundaries
  a skos:Collection ;
  rdfs:isDefinedBy asls:soil-profile ;
  skos:inScheme asls:soil-profile ;
  skos:definition "Description of the boundary conditions between horizons"@en ;
  skos:member sp:Boundary-distinctness ;
  skos:member sp:Boundary-shape ;
  skos:prefLabel "Boundaries between horizons"@en ;
.
sp:horizon-boundary-distinctness-A
  a sp:Boundary-distinctness ;
  a skos:Concept ;
  skos:definition "width of boundary is 5-20 mm."@en ;
  skos:notation "A" ;
  skos:prefLabel "Abrupt"@en ;
.
sp:horizon-boundary-distinctness-C
  a sp:Boundary-distinctness ;
  a skos:Concept ;
  skos:definition "width of boundary is 20-50 mm."@en ;
  skos:notation "C" ;
  skos:prefLabel "Clear (horizon boundary distinctness)"@en ;
.
sp:horizon-boundary-distinctness-D
  a sp:Boundary-distinctness ;
  a skos:Concept ;
  skos:definition "width of boundary is >100 mm."@en ;
  skos:notation "D" ;
  skos:prefLabel "Diffuse (horizon boundary distinctness)"@en ;
.
sp:horizon-boundary-distinctness-G
  a sp:Boundary-distinctness ;
  a skos:Concept ;
  skos:definition "width of boundary is 50-100 mm."@en ;
  skos:notation "G" ;
  skos:prefLabel "Gradual (horizon boundary distinctness)"@en ;
.
sp:horizon-boundary-distinctness-S
  a sp:Boundary-distinctness ;
  a skos:Concept ;
  skos:definition "width of boundary is <5 mm."@en ;
  skos:notation "S" ;
  skos:prefLabel "Sharp (horizon boundary distinctness)"@en ;
.
sp:horizon-boundary-shape-B
  a sp:Boundary-shape ;
  a skos:Concept ;
  skos:definition "discontinuous."@en ;
  skos:notation "B" ;
  skos:prefLabel "Broken (horizon boundary shape)"@en ;
.
sp:horizon-boundary-shape-I
  a sp:Boundary-shape ;
  a skos:Concept ;
  skos:definition "undulations with depressions deeper than they are wide."@en ;
  skos:notation "I" ;
  skos:prefLabel "Irregular"@en ;
.
sp:horizon-boundary-shape-S
  a sp:Boundary-shape ;
  a skos:Concept ;
  skos:definition "almost a plane surface."@en ;
  skos:notation "S" ;
  skos:prefLabel "Smooth"@en ;
.
sp:horizon-boundary-shape-T
  a sp:Boundary-shape ;
  a skos:Concept ;
  skos:definition "depressions considerably deeper than they are wide."@en ;
  skos:notation "T" ;
  skos:prefLabel "Tongued"@en ;
.
sp:horizon-boundary-shape-W
  a sp:Boundary-shape ;
  a skos:Concept ;
  skos:definition "undulations with depressions wider than they are deep."@en ;
  skos:notation "W" ;
  skos:prefLabel "Wavy"@en ;
.
sp:horizon-prefix
  a sp:horizons ;
  a skos:Concept ;
  skos:definition """Where obvious contrasts in lithology exist between different horizons in the soil profile, or between the soil profile and the underlying lithology, the different lithologic layers are given a numeric prefix (Figure 13).

Each layer may consist of one or more horizons. The different layers are numbered from the top downward. The upper layer is not numbered 1, this being understood. Numbering starts with the second layer, which is designated 2. Even though a layer below material 3, for example, is similar to material 2, it is designated 4 in the sequence (see Profiles C and D in Figure 13). Discrimination of lithological discontinuities from soil horizon boundaries will depend in each case upon the degree of pedological organisation and the contrast between lithological units (see, for example, Profiles C and D in Figure 13).

Where lithologic discontinuities are suspected in the profile but there is no clear evidence, either the numeric prefix should not be used or a query should be added to indicate doubt. It is better used only where there is clear evidence. Whether the numeric prefix is used or not, the horizon naming, with appropriate suffixes, remains the same, as illustrated in the examples in Figure 13."""@en ;
  skos:note """<p>Figure 13	Lithologic discontinuities and soil horizon nomenclature.</p><p>
	In Profile C, the degree of development of the B22 horizon overrides any lithologic discontinuity between the B22 and 2B22 horizon; hence, no soil horizon boundary is shown between them.</p><p>
	In Profile D, lithologic characteristics allow recognition of separate sedimentary layers in the upper solum. The horizon boundary between the A11 and 2A12 is also recognised by the pedological differences within the A1 horizon. On the other hand, the gross characteristics of the A2 horizon (for example, a conspicuous bleach) have developed in two different lithologies in layers 2A2 and 3A2.</p><p>
	In Profile E, layer 3D is equivalent to layer 5D in Profiles C and D.</p><p>
<img src=\"http://anzsoil.org/resources/yellowbook/Figure13.png\" /></p>"""^^rdf:HTML ;
  skos:prefLabel "Lithologic discontinuity"@en ;
.
sp:horizon-suffix-b
  a sp:Horizon-suffix ;
  a skos:Concept ;
  skos:altLabel "Buried soils"@en ;
  skos:definition "used for buried soil horizons. Used in mineral soils only. The suffix is written last, for example 2B2b."@en ;
  skos:notation "b" ;
  skos:note """<p>Figure 14	Buried soils and soil horizon nomenclature.</p><p>
	In Profile A, the buried soils have reliably identified horizons; in Profile B, they do not. Buried soils will always be overlain by a sedimentary layer that is different from the material in which they occur. Lithologic discontinuities in the profile must therefore be designated. 
<img src=\"http://anzsoil.org/resources/yellowbook/Figure14.png\" /></p>"""^^rdf:HTML ;
  skos:note "Where there are buried soils, and it is possible to designate reliably the horizon nomenclature in the buried profiles, the buried horizons are given the suffix ‘b’ which is written last. Number the different soils from the top downward. The upper soil, or modern soil, is not numbered 1, this being understood. Two examples are given in Figure 14"@en ;
  skos:prefLabel "Horizon suffix b"@en ;
.
sp:horizon-suffix-c
  a sp:Horizon-suffix ;
  a skos:Concept ;
  skos:definition "used for horizons with accumulation of concretions or nodules of iron and/or aluminium and/or manganese, as in B2c."@en ;
  skos:notation "c" ;
  skos:prefLabel "Horizon suffix c"@en ;
.
sp:horizon-suffix-d
  a sp:Horizon-suffix ;
  a skos:Concept ;
  skos:definition "used for densipans. Very fine, sandy, earthy pan."@en ;
  skos:notation "d" ;
  skos:prefLabel "Horizon suffix d"@en ;
.
sp:horizon-suffix-e
  a sp:Horizon-suffix ;
  a skos:Concept ;
  skos:definition "used for conspicuously bleached horizons, for example A2e."@en ;
  skos:notation "e" ;
  skos:prefLabel "Horizon suffix e"@en ;
.
sp:horizon-suffix-f
  a sp:Horizon-suffix ;
  a skos:Concept ;
  skos:definition "used when faunal accumulation, such as worm casts, dominates certain A1 horizons, for example A1f in some soils under rainforest."@en ;
  skos:notation "f" ;
  skos:prefLabel "Horizon suffix f"@en ;
.
sp:horizon-suffix-g
  a sp:Horizon-suffix ;
  a skos:Concept ;
  skos:definition "indicates strong gleying, as in B2g. Gleying is indicative of permanent or periodic intense reduction due to wetness; it is characterised by greyish, bluish or greenish colours, generally of low chroma. Mottling may be prominent; mottles may have reddish hues and higher chromas if oxidising conditions occur periodically. Roots may have rusty or yellowish outlines; hence horizons such as A1g can occur."@en ;
  skos:notation "g" ;
  skos:prefLabel "Horizon suffix g"@en ;
.
sp:horizon-suffix-h
  a sp:Horizon-suffix ;
  a skos:Concept ;
  skos:definition "used where horizons contain accumulation of amorphous, organic matter – aluminium complexes in which iron contents are very low. The dominantly organic matter – aluminium  complexes occur as discrete pellets between clean sand grains or completely fill the voids; occasionally they may coat sand grains. Such horizons may be soft or cemented and form the characteristic B horizon of poorly drained soils known as podzols or Podosols."@en ;
  skos:notation "h" ;
  skos:prefLabel "Horizon suffix h"@en ;
.
sp:horizon-suffix-j
  a sp:Horizon-suffix ;
  a skos:Concept ;
  skos:definition "used for sporadically bleached horizons, for example A2j."@en ;
  skos:notation "j" ;
  skos:prefLabel "Horizon suffix j"@en ;
.
sp:horizon-suffix-k
  a sp:Horizon-suffix ;
  a skos:Concept ;
  skos:definition "used for horizons with accumulation of carbonates, commonly calcium carbonate, as in B2k."@en ;
  skos:notation "k" ;
  skos:note "This suffix is usually recorded only if there is a common or larger abundance of these segregations. Horizons with few (2–10%) or very few (<2%) segregations are not usually given these horizon notations. This suffix indicates relative accumulations compared with other horizons. Thus in a soil with no carbonate except for one horizon with few segregations, this horizon could be designated with a suffix ‘k’, for example B22tk. However, in a soil with few segregations of carbonate throughout, no horizon would be given the suffix ‘k’ unless it had common or more segregations, that is, a relatively larger amount than adjacent horizons."@en ;
  skos:prefLabel "Horizon suffix k"@en ;
.
sp:horizon-suffix-m
  a sp:Horizon-suffix ;
  a skos:Concept ;
  skos:definition "used for horizons with strong cementation or induration. It is confined to irreversibly cemented horizons that are essentially continuous (more than 90%) though they may be fractured."@en ;
  skos:notation "m" ;
  skos:prefLabel "Horizon suffix m"@en ;
.
sp:horizon-suffix-p
  a sp:Horizon-suffix ;
  a skos:Concept ;
  skos:definition """used for horizons where ploughing, tillage practices or other disturbance by humans has occurred, for example deep ripping. This suffix is used only with A, as in Ap2. Where the plough layer clearly includes what was once B horizon and it is no longer possible to infer with any reliability what the texture and depth of the A horizon was, the plough layer is designated Ap.
An Ap horizon may be subdivided into subhorizons (e.g. Ap1, Ap2)."""@en ;
  skos:notation "p" ;
  skos:note "An Ap2 horizon is not the same as an A2 horizon but a subdivision equivalent to A12."@en ;
  skos:prefLabel "Horizon suffix p"@en ;
.
sp:horizon-suffix-q
  a sp:Horizon-suffix ;
  a skos:Concept ;
  skos:definition "used for horizons with accumulation of secondary silica. If silica cementation is continuous or nearly continuous, ‘qm’ is used."@en ;
  skos:notation "q" ;
  skos:prefLabel "Horizon suffix q"@en ;
.
sp:horizon-suffix-r
  a sp:Horizon-suffix ;
  a skos:Concept ;
  skos:definition "used for horizons with layers of weathered rock (including saprolite) that, although consolidated, can be dug with hand tools."@en ;
  skos:notation "r" ;
  skos:prefLabel "Horizon suffix r"@en ;
.
sp:horizon-suffix-s
  a sp:Horizon-suffix ;
  a skos:Concept ;
  skos:definition "used for horizons with an accumulation of sesquioxide – organic matter complexes in which iron is dominant relative to aluminium. These complexes coat sand grains, occur as discrete pellets, or, with moderate amounts of iron, may fill voids forming cemented patches. The content of organic matter is variable and its distribution is often irregular. The suffix ‘s’ is often used in combination with ‘h’ (as in Bhs) where both organic and iron components are significant; s or Bhs horizons may be soft or hard and form the characteristic B horizon of free-draining podzols or Podosols."@en ;
  skos:notation "s" ;
  skos:prefLabel "Horizon suffix s"@en ;
.
sp:horizon-suffix-t
  a sp:Horizon-suffix ;
  a skos:Concept ;
  skos:definition "used for horizons with accumulation of silicate clay (from German ton, clay). Different mechanisms (such as illuviation, formation in situ) may be responsible for the clay accumulation, but these may be difficult to confirm. This suffix is used only with the B, for example B2t, to indicate the nature of the B."@en ;
  skos:notation "t" ;
  skos:prefLabel "Horizon suffix t"@en ;
.
sp:horizon-suffix-w
  a sp:Horizon-suffix ;
  a skos:Concept ;
  skos:definition "used where development of colour and/or structure, or both, in the B horizon is observed, with little or no accumulation of sesquioxide – organic matter complexes."@en ;
  skos:notation "w" ;
  skos:prefLabel "Horizon suffix w"@en ;
.
sp:horizon-suffix-x
  a sp:Horizon-suffix ;
  a skos:Concept ;
  skos:definition "used for fragipans or earthy pans. A horizon with high bulk density relative to the horizon above, seemingly cemented when dry, but showing a moderate to weak cementation when moist."@en ;
  skos:notation "x" ;
  skos:prefLabel "Horizon suffix x"@en ;
.
sp:horizon-suffix-y
  a sp:Horizon-suffix ;
  a skos:Concept ;
  skos:definition "used for horizons with accumulation of calcium sulphate (gypsum), as in B21, B22."@en ;
  skos:notation "y" ;
  skos:note "This suffix is usually recorded only if there is a common or larger abundance of these segregations. Horizons with few (2–10%) or very few (<2%) segregations are not usually given these horizon notations. This suffix indicates relative accumulations compared with other horizons. Thus in a soil with no carbonate except for one horizon with few segregations, this horizon could be designated with a suffix ‘k’, for example B22tk. However, in a soil with few segregations of carbonate throughout, no horizon would be given the suffix ‘k’ unless it had common or more segregations, that is, a relatively larger amount than adjacent horizons."@en ;
  skos:prefLabel "Horizon suffix y"@en ;
.
sp:horizon-suffix-z
  a sp:Horizon-suffix ;
  a skos:Concept ;
  skos:definition "used for horizons with accumulation of salts more soluble than calcium sulphate and calcium carbonate."@en ;
  skos:notation "z" ;
  skos:prefLabel "Horizon suffix z"@en ;
.
sp:horizons
  a owl:Class ;
  a skos:Collection ;
  rdfs:isDefinedBy asls:soil-profile ;
  skos:inScheme asls:soil-profile ;
  rdfs:subClassOf skos:Concept ;
  skos:definition "A soil horizon is a layer of soil, approximately parallel to the land surface, with morphological properties different from layers below and/or above it. Tongues of material from one horizon may penetrate into adjacent horizons."@en ;
  skos:member sp:Horizon-code ;
  skos:member sp:Horizon-suffix ;
  skos:member sp:depth-of-horizon ;
  skos:member sp:depth-of-horizon-lower ;
  skos:member sp:depth-of-horizon-upper ;
  skos:member sp:depth-to-r-horizon ;
  skos:member sp:horizon-prefix ;
  skos:member sp:horizons-bleached ;
  skos:member sp:horizons-subdivision ;
  skos:member sp:horizons-transitional ;
  skos:note """As horizon notation is deduced from the profile description data (Northcote 1979) and in some instances laboratory data, record it after the profile is described. Horizons may be difficult to name, but should be named in the field. Opinions formed at the time of description are useful for later reference.
Cracking clays
The A and B horizons in cracking clays are defined and recognised on the basis of structure rather than colour (McDonald 1977).
The A horizon in cracking clays may be structured or massive. The structural A horizon is the granular, subangular blocky, angular blocky or polyhedral surface horizon where ped faces are not accommodated and have irregular coarse voids between them. This is exemplified in soils with a self-mulching surface. The A horizon structure is unstable only in the sense that relatively rapid wetting and drying continually creates new peds and voids.
The B horizon is the coarse angular blocky and/or lenticular horizon where ped faces are all accommodated and usually have only narrow planar voids between them. The B horizon structure is stable because of relatively slow wetting and drying. The B horizon will usually occur within 200 mm of the surface, but the structural change must be confirmed using a spade or exposure to examine the soil. The boundary may often be gradual or diffuse, but can be clear or abrupt."""@en ;
  skos:prefLabel "Horizon classification"@en ;
.
sp:horizons-A
  a sp:Horizon-code ;
  a skos:Concept ;
  skos:definition "These are horizons either consisting of one or more surface mineral horizons with some organic accumulation and usually darker in colour than the underlying horizons, or consisting of surface and subsurface horizons that are lighter in colour but have a lower content of silicate clay and/or sesquioxides than the underlying horizons."@en ;
  skos:narrower sp:horizon-A1 ;
  skos:narrower sp:horizon-A2 ;
  skos:narrower sp:horizon-A3 ;
  skos:notation "A" ;
  skos:prefLabel "A horizons"@en ;
.
sp:horizons-B
  a sp:Horizon-code ;
  a skos:Concept ;
  skos:definition "These are horizons consisting of one or more mineral soil layers characterised by one or more of the following: a concentration of silicate clay, iron, aluminium, organic material or several of these; a structure and/or consistence unlike that of the A horizons above or of any horizons immediately below; stronger colours, usually expressed as higher chroma and/or redder hue, than those of the A horizons above or those of the horizons below."@en ;
  skos:narrower sp:horizon-B1 ;
  skos:narrower sp:horizon-B2 ;
  skos:narrower sp:horizon-B3 ;
  skos:notation "B" ;
  skos:prefLabel "B horizons"@en ;
.
sp:horizons-C
  a sp:Horizon-code ;
  a skos:Concept ;
  skos:definition "These are layers below the solum (AB profile) of consolidated or unconsolidated material, usually partially weathered, little affected by pedogenic processes, and either like or unlike the material from which the solum presumably formed. The C horizon lacks properties characteristic of O, P, A, B or D horizons. It is recognised by its lack of pedological development and/or the presence of geologic organisation frequently expressed as sedimentary laminae or as ghost rock structure as in saprolite. C horizons include consolidated rock and sediments that, when moist, can be dug with hand tools. Rock strength is generally weak or weaker. Because of their nature, C horizons may alternatively be described as substrate."@en ;
  skos:notation "C" ;
  skos:prefLabel "C horizons"@en ;
.
sp:horizons-D
  a sp:Horizon-code ;
  a skos:Concept ;
  skos:definition "These are considered to be any soil material below the solum that is unlike the solum in its general character, is not C horizon, and cannot be given reliable horizon designation as with ‘Buried soils’ or ‘Lithologic discontinuities’. Thus a D horizon may be recognised by the contrast in pedologic organisation between it and the overlying horizons."@en ;
  skos:notation "D" ;
  skos:prefLabel "D horizons"@en ;
.
sp:horizons-O
  a sp:Horizon-code ;
  a skos:Concept ;
  skos:definition "These are horizons dominated by organic materials in varying stages of decomposition that have accumulated on the mineral soil surface. They are usually divided into O1 and O2 horizons."@en ;
  skos:narrower sp:horizon-O1 ;
  skos:narrower sp:horizon-O2 ;
  skos:notation "O" ;
  skos:prefLabel "O horizons"@en ;
.
sp:horizons-P
  a sp:Horizon-code ;
  a skos:Concept ;
  dcterms:description "These are horizons dominated by organic materials in various stages of decomposition that have accumulated either under water or in conditions of excessive wetness. They have long been known as peat. The organic material consists of the remains of plants that have been growing in place. "@en ;
  skos:definition "These are horizons dominated by organic materials in various stages of decomposition that have accumulated either under water or in conditions of excessive wetness. They have long been known as peat. The organic material consists of the remains of plants that have been growing in place."@en ;
  skos:narrower sp:horizon-P1 ;
  skos:narrower sp:horizon-P2 ;
  skos:notation "P" ;
  skos:note "When such horizons are buried, they may be designated in a manner similar to designations for buried mineral soils, for example 2P1, 3P2, etc."@en ;
  skos:prefLabel "P horizons"@en ;
.
sp:horizons-R
  a sp:Horizon-code ;
  a skos:Concept ;
  skos:definition "These horizons consist of continuous masses (not boulders) of moderately strong to very strong rock (excluding pans) such as bedrock. R horizons may have cracks but these are few enough and/or fine enough that few roots penetrate and there is no significant displacement of rock. It is usually too strong to dig with hand tools, even when moist."@en ;
  skos:notation "R" ;
  skos:prefLabel "R horizons"@en ;
.
sp:horizons-bleached
  a sp:horizons ;
  a skos:Concept ;
  skos:definition """Some horizons are white, near white or much paler than adjacent horizons. Bleached horizons most commonly occur as A2 horizons but are not restricted to them.

Bleached horizons are defined in terms of Munsell notations for dry soil:
•	for all hues, value 7 or greater with chroma 4 or less
•	where adjacent horizons have hues 5YR or redder, value 6 or greater with chroma 4 or less.

Two kinds of bleached horizons are recognised:
Conspicuously bleached: 80% or more of the horizon is bleached.
Sporadically bleached: bleach occurs:
•	irregularly through the horizon
•	as blotches, often less than 6 mm thick, at the interface of horizons, most commonly A and B horizons
•	as nests of bleached grains of soil material at the interface of horizons, most commonly A and B horizons, when no other evidence of a bleached horizon may occur."""@en ;
  skos:prefLabel "Bleached horizons"@en ;
.
sp:horizons-subdivision
  a sp:horizons ;
  a skos:Concept ;
  skos:definition """All horizon subdivisions are numbered consecutively from the top of each horizon downward, as in A11, A12, A2, B21, B22, B23. The numeric suffix always precedes the alphabetic suffix except with the alphabetic suffix ‘p’ where the number always follows the letter.
The above horizon nomenclature will cover most soils, but there will be instances where there are buried soils (pedologic discontinuities) (Figure 14) and also where a profile has formed on what are obviously different parent materials (lithologic discontinuities) (Figure 13). Where there are buried soils and it is not possible to identify reliably the horizon as A or B, then these are D horizons, for example Profile E, Figure 13.
"""@en ;
  skos:prefLabel "Subdivision of horizons"@en ;
.
sp:horizons-transitional
  a sp:horizons ;
  a skos:Concept ;
  skos:definition """Two main kinds are distinguished:
•	transitional horizons that have subordinate properties of both horizons but are not dominated by properties characteristic of either horizon. For example, AB, AC, BC horizons.
•	transitional horizons in which distinct parts have recognisable properties of two kinds of horizons indicated by capital letters (Soil Survey Staff 1990).

The two capital letters are separated by a virgule (/) as A/B, A/C, B/C. Most of the individual parts of at least one of the components are surrounded by the other. The first symbol is that of the horizon that makes up the greater volume."""@en ;
  skos:prefLabel "Transitional horizons"@en ;
.
sp:mottle-abundance-0
  a sp:Mottle-abundance ;
  a skos:Concept ;
  rdfs:comment "N_MOTT_ABUN" ;
  skos:definition "0%"@en ;
  skos:notation "0" ;
  skos:prefLabel "No mottles or other colour patterns"@en ;
.
sp:mottle-abundance-1
  a sp:Mottle-abundance ;
  a skos:Concept ;
  rdfs:comment "N_MOTT_ABUN" ;
  skos:definition "<2%"@en ;
  skos:notation "1" ;
  skos:prefLabel "Very few (mottle abundance)"@en ;
.
sp:mottle-abundance-2
  a sp:Mottle-abundance ;
  a skos:Concept ;
  rdfs:comment "N_MOTT_ABUN" ;
  skos:definition "2-10%"@en ;
  skos:notation "2" ;
  skos:prefLabel "Few (mottle abundance)"@en ;
.
sp:mottle-abundance-3
  a sp:Mottle-abundance ;
  a skos:Concept ;
  rdfs:comment "N_MOTT_ABUN" ;
  skos:definition "10-20%"@en ;
  skos:notation "3" ;
  skos:prefLabel "Common (mottle abundance)"@en ;
.
sp:mottle-abundance-4
  a sp:Mottle-abundance ;
  a skos:Concept ;
  rdfs:comment "N_MOTT_ABUN" ;
  skos:definition "20-50%"@en ;
  skos:notation "4" ;
  skos:prefLabel "Many (mottle abundance)"@en ;
.
sp:mottle-boundary-C
  a sp:Mottle-distinctness ;
  a skos:Concept ;
  rdfs:comment "C_MOTT_BOUN_DISTINCT" ;
  skos:definition "colour transition over less than 2 mm"@en ;
  skos:notation "C" ;
  skos:prefLabel "Clear (mottle boundary)"@en ;
.
sp:mottle-boundary-D
  a sp:Mottle-distinctness ;
  a skos:Concept ;
  rdfs:comment "C_MOTT_BOUN_DISTINCT" ;
  skos:definition "colour transition over 2 mm or more"@en ;
  skos:notation "D" ;
  skos:prefLabel "Diffuse (mottle boundary)"@en ;
.
sp:mottle-boundary-S
  a sp:Mottle-distinctness ;
  a skos:Concept ;
  rdfs:comment "C_MOTT_BOUN_DISTINCT" ;
  skos:definition "knife-edge boundary between colours"@en ;
  skos:notation "S" ;
  skos:prefLabel "Sharp (mottle boundary)"@en ;
.
sp:mottle-colour-B
  a sp:Mottle-colour ;
  a skos:Concept ;
  rdfs:comment "C_MOTT_COLOUR" ;
  skos:definition "Brown"@en ;
  skos:notation "B" ;
  skos:prefLabel "Brown"@en ;
.
sp:mottle-colour-D
  a sp:Mottle-colour ;
  a skos:Concept ;
  rdfs:comment "C_MOTT_COLOUR" ;
  skos:definition "values 3 or less and chromas 2 or less for all hues."@en ;
  skos:notation "D" ;
  skos:prefLabel "Dark"@en ;
.
sp:mottle-colour-G
  a sp:Mottle-colour ;
  a skos:Concept ;
  rdfs:comment "C_MOTT_COLOUR" ;
  skos:definition "Grey"@en ;
  skos:notation "G" ;
  skos:prefLabel "Grey"@en ;
.
sp:mottle-colour-L
  a sp:Mottle-colour ;
  a skos:Concept ;
  rdfs:comment "C_MOTT_COLOUR" ;
  skos:definition "gley charts only."@en ;
  skos:notation "L" ;
  skos:prefLabel "Gley"@en ;
.
sp:mottle-colour-O
  a sp:Mottle-colour ;
  a skos:Concept ;
  rdfs:comment "C_MOTT_COLOUR" ;
  skos:definition "Orange"@en ;
  skos:notation "O" ;
  skos:prefLabel "Orange"@en ;
.
sp:mottle-colour-P
  a sp:Mottle-colour ;
  a skos:Concept ;
  rdfs:comment "C_MOTT_COLOUR" ;
  skos:definition "values 7 or more and chromas 2 or less for all hues."@en ;
  skos:notation "P" ;
  skos:prefLabel "Pale"@en ;
.
sp:mottle-colour-R
  a sp:Mottle-colour ;
  a skos:Concept ;
  rdfs:comment "C_MOTT_COLOUR" ;
  skos:definition "Red"@en ;
  skos:notation "R" ;
  skos:prefLabel "Red"@en ;
.
sp:mottle-colour-Y
  a sp:Mottle-colour ;
  a skos:Concept ;
  rdfs:comment "C_MOTT_COLOUR" ;
  skos:definition "Yellow"@en ;
  skos:notation "Y" ;
  skos:prefLabel "Yellow"@en ;
.
sp:mottle-contrast-D
  a sp:Mottle-contrast ;
  a skos:Concept ;
  rdfs:comment "C_CONTRAST" ;
  skos:definition "readily evident although not striking."@en ;
  skos:notation "D" ;
  skos:prefLabel "Distinct (mottle contrast)"@en ;
.
sp:mottle-contrast-F
  a sp:Mottle-contrast ;
  a skos:Concept ;
  rdfs:comment "C_CONTRAST" ;
  skos:definition "indistinct; evident only on close examination."@en ;
  skos:notation "F" ;
  skos:prefLabel "Faint (mottle contrast)"@en ;
.
sp:mottle-contrast-P
  a sp:Mottle-contrast ;
  a skos:Concept ;
  rdfs:comment "C_CONTRAST" ;
  skos:definition "striking and conspicuous."@en ;
  skos:notation "P" ;
  skos:prefLabel "Prominent (mottle contrast)"@en ;
.
sp:mottle-size-1
  a sp:Mottle-size ;
  a skos:Concept ;
  rdfs:comment "N_MOTT_SIZE" ;
  skos:definition "<5 mm"@en ;
  skos:notation "1" ;
  skos:prefLabel "Fine (mottle size)"@en ;
.
sp:mottle-size-2
  a sp:Mottle-size ;
  a skos:Concept ;
  rdfs:comment "N_MOTT_SIZE" ;
  skos:definition "5-15 mm"@en ;
  skos:notation "2" ;
  skos:prefLabel "Medium (mottle size)"@en ;
.
sp:mottle-size-3
  a sp:Mottle-size ;
  a skos:Concept ;
  rdfs:comment "N_MOTT_SIZE" ;
  skos:definition "15-30 mm"@en ;
  skos:notation "3" ;
  skos:prefLabel "Coarse (mottle size)"@en ;
.
sp:mottle-size-4
  a sp:Mottle-size ;
  a skos:Concept ;
  rdfs:comment "N_MOTT_SIZE" ;
  skos:definition ">30 mm"@en ;
  skos:notation "4" ;
  skos:prefLabel "Very coarse (mottle size)"@en ;
.
sp:mottle-type-M
  a sp:Mottle-type ;
  a skos:Concept ;
  rdfs:comment "C_MOTT_TYPE" ;
  skos:definition "Mottles"@en ;
  skos:notation "M" ;
  skos:prefLabel "Mottles"@en ;
.
sp:mottle-type-X
  a sp:Mottle-type ;
  a skos:Concept ;
  rdfs:comment "C_MOTT_TYPE" ;
  skos:definition "Colour patterns due to biological mixing of soil material from other horizons (e.g. worm casts)."@en ;
  skos:notation "X" ;
  skos:prefLabel "Mottle type X"@en ;
.
sp:mottle-type-Y
  a sp:Mottle-type ;
  a skos:Concept ;
  rdfs:comment "C_MOTT_TYPE" ;
  skos:definition "Colour patterns due to mechanical mixing of soil material from other horizons (e.g.  inclusions of B horizon material in Ap horizons)."@en ;
  skos:notation "Y" ;
  skos:prefLabel "Mottle type Y"@en ;
.
sp:mottle-type-Z
  a sp:Mottle-type ;
  a skos:Concept ;
  rdfs:comment "C_MOTT_TYPE" ;
  skos:definition "Colour patterns due to inclusions of weathered substrate material."@en ;
  skos:notation "Z" ;
  skos:prefLabel "Mottle type Z"@en ;
.
sp:mottles
  a skos:Collection ;
  rdfs:isDefinedBy asls:soil-profile ;
  skos:inScheme asls:soil-profile ;
  skos:definition "Mottles are spots, blotches or streaks of subdominant colours different from the matrix colour and also different from the colour of the ped surface. Segregations of pedogenic origin are not considered to be mottles and are recorded elsewhere. Colour patterns due to biological or mechanical mixing and inclusions of weathered substrate material are described separately."@en ;
  skos:member sp:Mottle-abundance ;
  skos:member sp:Mottle-colour ;
  skos:member sp:Mottle-contrast ;
  skos:member sp:Mottle-distinctness ;
  skos:member sp:Mottle-size ;
  skos:member sp:Mottle-type ;
  skos:prefLabel "Mottles and other colour patterns"@en ;
.
sp:observation-type-A
  a sp:Profile-construction ;
  a skos:Concept ;
  rdfs:comment "C_O_TYPE" ;
  skos:definition "Auger boring is used to describe the soil profile."@en ;
  skos:notation "A" ;
  skos:prefLabel "Auger boring"@en ;
.
sp:observation-type-C
  a sp:Profile-construction ;
  a skos:Concept ;
  rdfs:comment "C_O_TYPE" ;
  skos:definition "The profile is described from a soil core that it relatively undisturbed."@en ;
  skos:notation "C" ;
  skos:prefLabel "Relatively undisturbed soil core"@en ;
.
sp:observation-type-E
  a sp:Profile-construction ;
  a skos:Concept ;
  rdfs:comment "C_O_TYPE" ;
  skos:definition "An existing vertical exposure (e.g. road cutting) can be used to describe the soil profile."@en ;
  skos:notation "E" ;
  skos:prefLabel "Existing vertical exposure"@en ;
.
sp:observation-type-P
  a sp:Profile-construction ;
  a skos:Concept ;
  rdfs:comment "C_O_TYPE" ;
  skos:definition "The soil pit is one of several types of observation used to describe the soil profile."@en ;
  skos:notation "P" ;
  skos:prefLabel "Soil pit"@en ;
.
sp:pans
  a skos:Collection ;
  rdfs:isDefinedBy asls:soil-profile ;
  skos:inScheme asls:soil-profile ;
  skos:definition "A pan is an indurated and/or cemented soil horizon."@en ;
  skos:member sp:Pans-cementation ;
  skos:member sp:Pans-continuity ;
  skos:member sp:Pans-structure ;
  skos:member sp:Pans-type ;
  skos:prefLabel "Pans"@en ;
.
sp:pans-cementation-0
  a sp:Pans-cementation ;
  a skos:Concept ;
  rdfs:comment "C_PAN_CEMENTATION" ;
  skos:definition "slakes."@en ;
  skos:notation "0" ;
  skos:prefLabel "Uncemented"@en ;
.
sp:pans-cementation-1
  a sp:Pans-cementation ;
  a skos:Concept ;
  rdfs:comment "C_PAN_CEMENTATION" ;
  skos:definition "can be crushed between thumb and forefinger."@en ;
  skos:notation "1" ;
  skos:prefLabel "Weakly cemented"@en ;
.
sp:pans-cementation-2
  a sp:Pans-cementation ;
  a skos:Concept ;
  rdfs:comment "C_PAN_CEMENTATION" ;
  skos:definition "beyond power of thumb and forefinger. Crushes underfoot on hard, flat surface with weight of average person (80 kg) applied slowly."@en ;
  skos:notation "2" ;
  skos:prefLabel "Moderately cemented"@en ;
.
sp:pans-cementation-3
  a sp:Pans-cementation ;
  a skos:Concept ;
  rdfs:comment "C_PAN_CEMENTATION" ;
  skos:definition "cannot be crushed underfoot by weight of average man applied slowly. Can be broken by hammer."@en ;
  skos:notation "3" ;
  skos:prefLabel "Strongly cemented"@en ;
.
sp:pans-cementation-4
  a sp:Pans-cementation ;
  a skos:Concept ;
  rdfs:comment "C_PAN_CEMENTATION" ;
  skos:definition "cannot be broken by hammer, or only with extreme difficulty."@en ;
  skos:notation "4" ;
  skos:prefLabel "Very strongly cemented"@en ;
.
sp:pans-continuity-B
  a sp:Pans-continuity ;
  a skos:Concept ;
  skos:definition "broken by cracks and fragments are disoriented."@en ;
  skos:notation "B" ;
  skos:prefLabel "Broken (pans continuity)"@en ;
.
sp:pans-continuity-C
  a sp:Pans-continuity ;
  a skos:Concept ;
  skos:definition "extends as a layer with little or no break across 1 m or more."@en ;
  skos:notation "C" ;
  skos:prefLabel "Continuous (pans continuity)"@en ;
.
sp:pans-continuity-D
  a sp:Pans-continuity ;
  a skos:Concept ;
  skos:definition "broken by cracks but original orientation of fragments is preserved."@en ;
  skos:notation "D" ;
  skos:prefLabel "Discontinuous (pans continuity)"@en ;
.
sp:pans-structure-C
  a sp:Pans-structure ;
  a skos:Concept ;
  skos:definition "spheroidal concretions cemented together."@en ;
  skos:notation "C" ;
  skos:prefLabel "Concretionary"@en ;
.
sp:pans-structure-L
  a sp:Pans-structure ;
  a skos:Concept ;
  skos:definition "plate-like units cemented together."@en ;
  skos:notation "L" ;
  skos:prefLabel "Platy (pans structure)"@en ;
.
sp:pans-structure-N
  a sp:Pans-structure ;
  a skos:Concept ;
  skos:definition "nodules of irregular shape cemented together."@en ;
  skos:notation "N" ;
  skos:prefLabel "Nodular (pans)"@en ;
.
sp:pans-structure-R
  a sp:Pans-structure ;
  a skos:Concept ;
  skos:definition "worm-like structure and/or cavities."@en ;
  skos:notation "R" ;
  skos:prefLabel "Vermicular"@en ;
.
sp:pans-structure-S
  a sp:Pans-structure ;
  a skos:Concept ;
  skos:definition "sponge-like structure having large pores, which may or may not be filled with softer material."@en ;
  skos:notation "S" ;
  skos:prefLabel "Vesicular"@en ;
.
sp:pans-structure-V
  a sp:Pans-structure ;
  a skos:Concept ;
  skos:definition "no recognisable structure."@en ;
  skos:notation "V" ;
  skos:prefLabel "Massive (pans structure)"@en ;
.
sp:pans-type-A
  a sp:Pans-type ;
  a skos:Concept ;
  skos:altLabel "Bauxite (pans type)"@en ;
  skos:definition "indurated material rich in aluminium hydroxides. Commonly consists of cemented pisoliths and usually known as bauxite."@en ;
  skos:notation "A" ;
  skos:prefLabel "Alcrete (pans type)"@en ;
.
sp:pans-type-C
  a sp:Pans-type ;
  a skos:Concept ;
  skos:definition "horizon relatively high in organic matter but low in iron. It is relatively thick and weakly to strongly cemented by aluminium and usually becomes progressively more cemented with depth. It is usually relatively uniform in appearance laterally. It is commonly the B horizon of humus podzols, where it is often known as coffee rock or sandrock."@en ;
  skos:notation "C" ;
  skos:prefLabel "Organic pan"@en ;
.
sp:pans-type-D
  a sp:Pans-type ;
  a skos:Concept ;
  skos:definition "earthy pan so cemented by silica that dry fragments do not slake in water and are always brittle, even after prolonged wetting. (Described by Soil Survey Staff 1975.)"@en ;
  skos:notation "D" ;
  skos:prefLabel "Duripan"@en ;
.
sp:pans-type-E
  a sp:Pans-type ;
  a skos:Concept ;
  skos:definition "indurated material rich in hydrated oxides of iron (usually goethite and hematite) occurring as cemented nodules and/or concretions, or as massive sheets. This material has been commonly referred to in local usage around Australia as laterite, duricrust or ironstone."@en ;
  skos:notation "E" ;
  skos:prefLabel "Ferricrete (pans type)"@en ;
.
sp:pans-type-F
  a sp:Pans-type ;
  a skos:Concept ;
  skos:definition "earthy pan, which is usually loamy. A dry fragment slakes in water. A wet fragment does not slake in water but has moderate or weak brittleness. Fragipans are more stable on exposure than overlying or underlying horizons. (Described by Soil Survey Staff 1975.)"@en ;
  skos:notation "F" ;
  skos:prefLabel "Fragipan"@en ;
.
sp:pans-type-I
  a sp:Pans-type ;
  a skos:Concept ;
  skos:definition "commonly thin (2–10 mm), black to dark reddish pan cemented by iron, iron and manganese, or iron – organic matter complexes. Rarely 40 mm thick. Has wavy or convolute form and usually occurs as a single pan. This is a placic horizon (described by Soil Survey Staff 1975.)"@en ;
  skos:notation "I" ;
  skos:prefLabel "Thin ironpan"@en ;
.
sp:pans-type-K
  a sp:Pans-type ;
  a skos:Concept ;
  skos:definition "any cemented, terrestrial carbonate accumulation that may vary significantly in morphology and degree of cementation. Also known as carbonate pan, calcareous pan, caliche, kunkar, secondary limestone, travertine. All show slight to strong effervescence with 1 Molar HCl."@en ;
  skos:notation "K" ;
  skos:prefLabel "Calcrete (pans type)"@en ;
.
sp:pans-type-L
  a sp:Pans-type ;
  a skos:Concept ;
  skos:definition "strongly indurated siliceous material cemented by, and largely composed of, forms of silica, including quartz, chalcedony, opal and chert."@en ;
  skos:notation "L" ;
  skos:prefLabel "Silcrete (pans type)"@en ;
.
sp:pans-type-M
  a sp:Pans-type ;
  a skos:Concept ;
  skos:definition "indurated material dominated by oxides of manganese."@en ;
  skos:notation "M" ;
  skos:prefLabel "Manganiferous pan"@en ;
.
sp:pans-type-N
  a sp:Pans-type ;
  a skos:Concept ;
  skos:definition "earthy pan, which is very fine sandy (0.02–0.05 mm). Fragments, both wet and dry, slake in water. Densipans are less stable on exposure than overlying or underlying horizons. (Described by Smith et al. 1975.)"@en ;
  skos:notation "N" ;
  skos:prefLabel "Densipan"@en ;
.
sp:pans-type-O
  a sp:Pans-type ;
  a skos:Concept ;
  skos:definition "Other pans"@en ;
  skos:notation "O" ;
  skos:prefLabel "Other pans"@en ;
.
sp:pans-type-R
  a sp:Pans-type ;
  a skos:Concept ;
  skos:definition "earthy pan, which is normally reddish brown to red with dense yet porous appearance; it is very hard, has an irregular laminar cleavage and some vertical cracks, and varies from less than 0.3 m to over 30 m thick. Other variable features are bedded and unsorted sand and gravel lenses; wavy black veinings, probably manganiferous; and, less commonly, off-white veins of calcium carbonate. (The presence of calcium carbonate is not common and the red-brown hardpan in which it occurs may be relatively brittle and finely laminar.) The red-brown hardpan is usually present below the soil profile and is not a feature of any particular soil group. (It has some similarity with other silica pans such as duripans of arid climates). In many instances, it is not known if the red-brown hardpan is a paleosol or a cemented sediment (Wright 1983). If thought to be the latter, it may be described as a substrate material. "@en ;
  skos:notation "R" ;
  skos:prefLabel "Red-brown hardpan (pans type)"@en ;
.
sp:pans-type-T
  a sp:Pans-type ;
  a skos:Concept ;
  skos:definition "horizon strongly cemented by iron and organic matter. It has marked local variability in colour, both laterally and vertically. It may occur in the B horizon of podzols."@en ;
  skos:notation "T" ;
  skos:prefLabel "Ortstein"@en ;
.
sp:pans-type-V
  a sp:Pans-type ;
  a skos:Concept ;
  skos:definition "subsurface soil horizon having higher bulk density, lower total porosity, and lower permeability to both air and water than horizons directly above and below as a result of cultivation practices. (After Morse et al. 1987.)"@en ;
  skos:notation "V" ;
  skos:prefLabel "Cultivation pan"@en ;
.
sp:pans-type-Z
  a sp:Pans-type ;
  a skos:Concept ;
  skos:definition "Zero or no pan"@en ;
  skos:notation "Z" ;
  skos:prefLabel "Zero or no pan"@en ;
.
sp:particle-size-fraction-boulders
  a sp:Particle-size-fractions ;
  a skos:Concept ;
  skos:definition "600 - 2000 mm"@en ;
  skos:prefLabel "Boulders"@en ;
.
sp:particle-size-fraction-clay
  a sp:Particle-size-fractions ;
  a skos:Concept ;
  skos:definition "0.0002 - 0.002 mm"@en ;
  skos:prefLabel "Clay"@en ;
.
sp:particle-size-fraction-coarse-gravel
  a sp:Particle-size-fractions ;
  a skos:Concept ;
  skos:definition "20 - 60 mm"@en ;
  skos:prefLabel "Coarse gravel"@en ;
.
sp:particle-size-fraction-coarse-sand
  a sp:Particle-size-fractions ;
  a skos:Concept ;
  skos:broader sp:particle-size-fraction-sand ;
  skos:definition "0.2 - 2.0 mm"@en ;
  skos:prefLabel "Coarse sand (particle size fraction)"@en ;
.
sp:particle-size-fraction-cobbles
  a sp:Particle-size-fractions ;
  a skos:Concept ;
  skos:definition "60 - 200 mm"@en ;
  skos:prefLabel "Cobbles"@en ;
.
sp:particle-size-fraction-fine-clay
  a sp:Particle-size-fractions ;
  a skos:Concept ;
  skos:definition "< 0.0002 mm"@en ;
  skos:prefLabel "Fine clay"@en ;
.
sp:particle-size-fraction-fine-gravel
  a sp:Particle-size-fractions ;
  a skos:Concept ;
  skos:definition "2.0 - 6.0 mm"@en ;
  skos:prefLabel "Fine gravel"@en ;
.
sp:particle-size-fraction-fine-sand
  a sp:Particle-size-fractions ;
  a skos:Concept ;
  skos:broader sp:particle-size-fraction-sand ;
  skos:definition "0.02 - 0.2 mm"@en ;
  skos:prefLabel "Fine sand (particle size fraction)"@en ;
.
sp:particle-size-fraction-medium-gravel
  a sp:Particle-size-fractions ;
  a skos:Concept ;
  skos:definition "6.0 - 20 mm"@en ;
  skos:prefLabel "Medium gravel"@en ;
.
sp:particle-size-fraction-sand
  a sp:Particle-size-fractions ;
  a skos:Concept ;
  dcterms:description "0.2 - 2.0 mm"@en ;
  skos:definition "0.02 - 2.0 mm"@en ;
  skos:narrower sp:particle-size-fraction-coarse-sand ;
  skos:narrower sp:particle-size-fraction-fine-sand ;
  skos:prefLabel "Sand (particle size fraction)"@en ;
.
sp:particle-size-fraction-silt
  a sp:Particle-size-fractions ;
  a skos:Concept ;
  skos:definition "0.002 - 0.02 mm"@en ;
  skos:prefLabel "Silt"@en ;
.
sp:particle-size-fraction-stones
  a sp:Particle-size-fractions ;
  a skos:Concept ;
  skos:definition "200 - 600 mm"@en ;
  skos:prefLabel "Stones"@en ;
.
sp:roots
  a skos:Collection ;
  rdfs:isDefinedBy asls:soil-profile ;
  skos:inScheme asls:soil-profile ;
  skos:definition "Record the presence of roots observed in each horizon in areas 100 mm square on a cleaned exposure face."@en ;
  skos:member sp:Root-abundance ;
  skos:member sp:Root-size ;
  skos:prefLabel "Roots"@en ;
.
sp:roots-abundance-0
  a sp:Root-abundance ;
  a skos:Concept ;
  skos:definition "0"@en ;
  skos:notation "0" ;
  skos:prefLabel "No roots"@en ;
.
sp:roots-abundance-1
  a sp:Root-abundance ;
  a skos:Concept ;
  skos:definition """1 - 10 very fine and fine roots
Or
1 - 2 medium and coarse roots"""@en ;
  skos:notation "1" ;
  skos:prefLabel "Few (roots abundance)"@en ;
.
sp:roots-abundance-2
  a sp:Root-abundance ;
  a skos:Concept ;
  skos:definition """10 - 25 very fine and fine roots
Or
2 - 5 medium and coarse roots"""@en ;
  skos:notation "2" ;
  skos:prefLabel "Common (roots abundance)"@en ;
.
sp:roots-abundance-3
  a sp:Root-abundance ;
  a skos:Concept ;
  skos:definition """25 - 200 very fine and fine roots
Or
> 5 medium and coarse roots"""@en ;
  skos:notation "3" ;
  skos:prefLabel "Many (roots abundance)"@en ;
.
sp:roots-abundance-4
  a sp:Root-abundance ;
  a skos:Concept ;
  skos:definition """> 200 very fine and fine roots
Or
> 5 medium and coarse roots"""@en ;
  skos:notation "4" ;
  skos:prefLabel "Abundant (roots abundance)"@en ;
.
sp:roots-size-1
  a sp:Root-size ;
  a skos:Concept ;
  skos:definition "less than 1 mm"@en ;
  skos:notation "1" ;
  skos:prefLabel "Very fine (roots size)"@en ;
.
sp:roots-size-2
  a sp:Root-size ;
  a skos:Concept ;
  skos:definition "1 - 2 mm"@en ;
  skos:notation "2" ;
  skos:prefLabel "Fine (roots size)"@en ;
.
sp:roots-size-3
  a sp:Root-size ;
  a skos:Concept ;
  skos:definition "2 - 5 mm"@en ;
  skos:notation "3" ;
  skos:prefLabel "Medium (roots size)"@en ;
.
sp:roots-size-4
  a sp:Root-size ;
  a skos:Concept ;
  skos:definition ">5 mm"@en ;
  skos:notation "4" ;
  skos:prefLabel "Coarse (roots size)"@en ;
.
sp:segregations
  a skos:Collection ;
  rdfs:isDefinedBy asls:soil-profile ;
  skos:inScheme asls:soil-profile ;
  skos:definition """This refers to discrete segregations that have accumulated in the soil because of the concentration of some constituent, usually by chemical or biological action.
Segregations may be relict or formed in situ by current pedogenic processes."""@en ;
  skos:member sp:Segregations-abundance ;
  skos:member sp:Segregations-form ;
  skos:member sp:Segregations-magnetic-attributes ;
  skos:member sp:Segregations-nature ;
  skos:member sp:Segregations-size ;
  skos:member sp:Segregations-strength ;
  skos:prefLabel "Segregations of pedogenic origin"@en ;
.
sp:segregations-abundance-0
  a sp:Segregations-abundance ;
  a skos:Concept ;
  rdfs:comment "N_SEG_ABUN" ;
  skos:definition "0"@en ;
  skos:notation "0" ;
  skos:prefLabel "No segregations"@en ;
.
sp:segregations-abundance-1
  a sp:Segregations-abundance ;
  a skos:Concept ;
  rdfs:comment "N_SEG_ABUN" ;
  skos:definition "< 2%"@en ;
  skos:notation "1" ;
  skos:prefLabel "Very few (segregations abundance)"@en ;
.
sp:segregations-abundance-2
  a sp:Segregations-abundance ;
  a skos:Concept ;
  rdfs:comment "N_SEG_ABUN" ;
  skos:definition "2 - 10%"@en ;
  skos:notation "2" ;
  skos:prefLabel "Few (segregations abundance)"@en ;
.
sp:segregations-abundance-3
  a sp:Segregations-abundance ;
  a skos:Concept ;
  rdfs:comment "N_SEG_ABUN" ;
  skos:definition "10 - 20%"@en ;
  skos:notation "3" ;
  skos:prefLabel "Common (segregations abundance)"@en ;
.
sp:segregations-abundance-4
  a sp:Segregations-abundance ;
  a skos:Concept ;
  rdfs:comment "N_SEG_ABUN" ;
  skos:definition "20 - 50%"@en ;
  skos:notation "4" ;
  skos:prefLabel "Many (segregations abundance)"@en ;
.
sp:segregations-abundance-5
  a sp:Segregations-abundance ;
  a skos:Concept ;
  rdfs:comment "N_SEG_ABUN" ;
  skos:definition "> 50%"@en ;
  skos:notation "5" ;
  skos:prefLabel "Very many (segregations abundance)"@en ;
.
sp:segregations-form-C
  a sp:Segregations-form ;
  a skos:Concept ;
  rdfs:comment "C_SEG_FORM" ;
  skos:definition "spheroidal mineral aggregates. Crudely concentric internal fabric can be seen with naked eye. Includes pisoliths and ooliths."@en ;
  skos:notation "C" ;
  skos:prefLabel "Concretions"@en ;
.
sp:segregations-form-F
  a sp:Segregations-form ;
  a skos:Concept ;
  rdfs:comment "C_SEG_FORM" ;
  skos:definition "broken pieces of segregations."@en ;
  skos:notation "F" ;
  skos:prefLabel "Fragments"@en ;
.
sp:segregations-form-L
  a sp:Segregations-form ;
  a skos:Concept ;
  rdfs:comment "C_SEG_FORM" ;
  skos:definition "planar, plate-like or sheet-like segregations."@en ;
  skos:notation "L" ;
  skos:prefLabel "Laminae"@en ;
.
sp:segregations-form-N
  a sp:Segregations-form ;
  a skos:Concept ;
  rdfs:comment "C_SEG_FORM" ;
  skos:definition "irregular, rounded mineral aggregates. No concentric or symmetric internal fabric. Can have hollow interior."@en ;
  skos:notation "N" ;
  skos:prefLabel "Nodules (segregations)"@en ;
.
sp:segregations-form-R
  a sp:Segregations-form ;
  a skos:Concept ;
  rdfs:comment "C_SEG_FORM" ;
  skos:definition "linings of former or current root channels."@en ;
  skos:notation "R" ;
  skos:prefLabel "Root linings"@en ;
.
sp:segregations-form-S
  a sp:Segregations-form ;
  a skos:Concept ;
  rdfs:comment "C_SEG_FORM" ;
  skos:definition "finely divided soft segregations. They contrast with surrounding soil in colour and composition but are not easily separated as discrete bodies. Boundaries may be clearly defined or diffuse."@en ;
  skos:notation "S" ;
  skos:prefLabel "Soft segregations"@en ;
.
sp:segregations-form-T
  a sp:Segregations-form ;
  a skos:Concept ;
  rdfs:comment "C_SEG_FORM" ;
  skos:definition "medium or coarser (>2 mm wide) tube-like segregations, which may or may not be hollow."@en ;
  skos:notation "T" ;
  skos:prefLabel "Tubules"@en ;
.
sp:segregations-form-V
  a sp:Segregations-form ;
  a skos:Concept ;
  rdfs:comment "C_SEG_FORM" ;
  skos:definition "fine (<2 mm wide) linear segregations."@en ;
  skos:notation "V" ;
  skos:prefLabel "Veins"@en ;
.
sp:segregations-form-X
  a sp:Segregations-form ;
  a skos:Concept ;
  rdfs:comment "C_SEG_FORM" ;
  skos:definition "single or complex clusters of crystals visible with naked eye or ×10 hand lens."@en ;
  skos:notation "X" ;
  skos:prefLabel "Crystals"@en ;
.
sp:segregations-magnetic-M
  a sp:Segregations-magnetic-attributes ;
  a skos:Concept ;
  rdfs:comment "C_SEG_MAGNETIC_ATTR" ;
  skos:definition "attracted onto surface of hand-held magnet."@en ;
  skos:notation "M" ;
  skos:prefLabel "Magnetic"@en ;
.
sp:segregations-magnetic-N
  a sp:Segregations-magnetic-attributes ;
  a skos:Concept ;
  rdfs:comment "C_SEG_MAGNETIC_ATTR" ;
  skos:definition "not attracted onto surface of hand-held magnet."@en ;
  skos:notation "N" ;
  skos:prefLabel "Non-magnetic"@en ;
.
sp:segregations-nature-A
  a sp:Segregations-nature ;
  a skos:Concept ;
  rdfs:comment "C_SEG_NATURE" ;
  skos:definition "Aluminous (aluminium)"@en ;
  skos:notation "A" ;
  skos:prefLabel "Aluminous"@en ;
.
sp:segregations-nature-E
  a sp:Segregations-nature ;
  a skos:Concept ;
  rdfs:comment "C_SEG_NATURE" ;
  skos:definition "Earthy (dominantly non-clayey)"@en ;
  skos:notation "E" ;
  skos:prefLabel "Earthy"@en ;
.
sp:segregations-nature-F
  a sp:Segregations-nature ;
  a skos:Concept ;
  rdfs:comment "C_SEG_NATURE" ;
  skos:definition "Ferruginous (iron)"@en ;
  skos:notation "F" ;
  skos:prefLabel "Ferruginous"@en ;
.
sp:segregations-nature-G
  a sp:Segregations-nature ;
  a skos:Concept ;
  rdfs:comment "C_SEG_NATURE" ;
  skos:definition "Ferruginous–organic (iron – organic matter)"@en ;
  skos:notation "G" ;
  skos:prefLabel "Ferruginous–organic"@en ;
.
sp:segregations-nature-H
  a sp:Segregations-nature ;
  a skos:Concept ;
  rdfs:comment "C_SEG_NATURE" ;
  skos:definition "Organic (humified, well-decomposed organic matter)"@en ;
  skos:notation "H" ;
  skos:prefLabel "Organic"@en ;
.
sp:segregations-nature-K
  a sp:Segregations-nature ;
  a skos:Concept ;
  rdfs:comment "C_SEG_NATURE" ;
  skos:definition "Calcareous (carbonate)"@en ;
  skos:notation "K" ;
  skos:prefLabel "Calcareous"@en ;
.
sp:segregations-nature-L
  a sp:Segregations-nature ;
  a skos:Concept ;
  rdfs:comment "C_SEG_NATURE" ;
  skos:definition "Argillaceous (clayey)"@en ;
  skos:notation "L" ;
  skos:prefLabel "Argillaceous"@en ;
.
sp:segregations-nature-M
  a sp:Segregations-nature ;
  a skos:Concept ;
  rdfs:comment "C_SEG_NATURE" ;
  skos:definition "Manganiferous (manganese)"@en ;
  skos:notation "M" ;
  skos:prefLabel "Manganiferous"@en ;
.
sp:segregations-nature-N
  a sp:Segregations-nature ;
  a skos:Concept ;
  rdfs:comment "C_SEG_NATURE" ;
  skos:definition "Ferromanganiferous (iron–manganese)"@en ;
  skos:notation "N" ;
  skos:prefLabel "Ferromanganiferous"@en ;
.
sp:segregations-nature-O
  a sp:Segregations-nature ;
  a skos:Concept ;
  rdfs:comment "C_SEG_NATURE" ;
  skos:definition "Other"@en ;
  skos:notation "O" ;
  skos:prefLabel "Other (segregations nature)"@en ;
.
sp:segregations-nature-S
  a sp:Segregations-nature ;
  a skos:Concept ;
  rdfs:comment "C_SEG_NATURE" ;
  skos:definition "Sulphurous (sulphur), for example in acid sulphate soils"@en ;
  skos:notation "S" ;
  skos:prefLabel "Sulphurous"@en ;
.
sp:segregations-nature-U
  a sp:Segregations-nature ;
  a skos:Concept ;
  rdfs:comment "C_SEG_NATURE" ;
  skos:definition "Unidentified"@en ;
  skos:notation "U" ;
  skos:prefLabel "Unidentified"@en ;
.
sp:segregations-nature-Y
  a sp:Segregations-nature ;
  a skos:Concept ;
  rdfs:comment "C_SEG_NATURE" ;
  skos:definition "Gypseous (gypsum)"@en ;
  skos:notation "Y" ;
  skos:prefLabel "Gypseous"@en ;
.
sp:segregations-nature-Z
  a sp:Segregations-nature ;
  a skos:Concept ;
  rdfs:comment "C_SEG_NATURE" ;
  skos:definition "Saline (visible salt)"@en ;
  skos:notation "Z" ;
  skos:prefLabel "Saline (segregations nature)"@en ;
.
sp:segregations-size-1
  a sp:Segregations-size ;
  a skos:Concept ;
  rdfs:comment "N_SEG_SIZE" ;
  skos:definition "< 2mm"@en ;
  skos:notation "1" ;
  skos:prefLabel "Fine (segregations size)"@en ;
.
sp:segregations-size-2
  a sp:Segregations-size ;
  a skos:Concept ;
  rdfs:comment "N_SEG_SIZE" ;
  skos:definition "2 - 6mm"@en ;
  skos:notation "2" ;
  skos:prefLabel "Medium (segregations size)"@en ;
.
sp:segregations-size-3
  a sp:Segregations-size ;
  a skos:Concept ;
  rdfs:comment "N_SEG_SIZE" ;
  skos:definition "6 - 20mm"@en ;
  skos:notation "3" ;
  skos:prefLabel "Coarse (segregations size)"@en ;
.
sp:segregations-size-4
  a sp:Segregations-size ;
  a skos:Concept ;
  rdfs:comment "N_SEG_SIZE" ;
  skos:definition "20 - 60mm"@en ;
  skos:notation "4" ;
  skos:prefLabel "Very coarse (segregations size)"@en ;
.
sp:segregations-size-5
  a sp:Segregations-size ;
  a skos:Concept ;
  rdfs:comment "N_SEG_SIZE" ;
  skos:definition "> 60mm"@en ;
  skos:notation "5" ;
  skos:prefLabel "Extremely coarse (segregations size)"@en ;
.
sp:segregations-strength-1
  a sp:Segregations-strength ;
  a skos:Concept ;
  rdfs:comment "C_SEG_STRENGTH" ;
  skos:definition "can be broken between thumb and forefinger."@en ;
  skos:notation "1" ;
  skos:prefLabel "Weak (segregations strength)"@en ;
.
sp:segregations-strength-2
  a sp:Segregations-strength ;
  a skos:Concept ;
  rdfs:comment "C_SEG_STRENGTH" ;
  skos:definition "cannot be broken between thumb and forefinger."@en ;
  skos:notation "2" ;
  skos:prefLabel "Strong (segregations strength)"@en ;
.
sp:soil-water-drainage-1
  a sp:Site-drainage ;
  a skos:Concept ;
  rdfs:comment "C_O_DRAINAGE" ;
  skos:definition "water is removed from the soil so slowly that the water table remains at or near the surface for most of the year. Surface flow, groundwater and subsurface flow are major sources of water, although precipitation may be important where there is a perched water table and precipitation exceeds evapotranspiration. Soils have a wide range in texture and depth, and often occur in depressed sites. Strong gleying and accumulation of surface organic matter are usually features of most soils."@en ;
  skos:notation "1" ;
  skos:prefLabel "Very poorly drained"@en ;
.
sp:soil-water-drainage-2
  a sp:Site-drainage ;
  a skos:Concept ;
  rdfs:comment "C_O_DRAINAGE" ;
  skos:definition "water is removed very slowly in relation to supply. Subsurface and/or groundwater flow, as well as precipitation, may be a significant water source. Seasonal ponding, resulting from runon and insufficient outfall, also occurs. A perched water table may be present. Soils have a wide range in texture and depth; many have horizons that are gleyed, mottled, or possess orange or rusty linings of root channels. All horizons remain wet for periods of several months."@en ;
  skos:notation "2" ;
  skos:prefLabel "Poorly drained"@en ;
.
sp:soil-water-drainage-3
  a sp:Site-drainage ;
  a skos:Concept ;
  rdfs:comment "C_O_DRAINAGE" ;
  skos:definition "water is removed only slowly in relation to supply. Precipitation is the main source if available water storage capacity is high, but subsurface flow and/or groundwater contribute as available water storage capacity decreases. Soils have a wide range in texture and depth. Some horizons may be mottled and/or have orange or rusty linings of root channels, and are wet for several weeks."@en ;
  skos:notation "3" ;
  skos:prefLabel "Imperfectly drained"@en ;
.
sp:soil-water-drainage-4
  a sp:Site-drainage ;
  a skos:Concept ;
  rdfs:comment "C_O_DRAINAGE" ;
  skos:definition "water is removed from the soil somewhat slowly in relation to supply, due to low permeability, shallow water table, lack of gradient, or some combination of these. Soils are usually medium to fine in texture. Significant additions of water by subsurface flow are necessary in coarse-textured soils. Some horizons may remain wet for as long as one week after water addition."@en ;
  skos:notation "4" ;
  skos:prefLabel "Moderately well drained"@en ;
.
sp:soil-water-drainage-5
  a sp:Site-drainage ;
  a skos:Concept ;
  rdfs:comment "C_O_DRAINAGE" ;
  skos:definition "water is removed from the soil readily but not rapidly. Excess water flows downward readily into underlying, moderately permeable material or laterally as subsurface flow. The soils are often medium in texture. Some horizons may remain wet for several days after water addition."@en ;
  skos:notation "5" ;
  skos:prefLabel "Well drained"@en ;
.
sp:soil-water-drainage-6
  a sp:Site-drainage ;
  a skos:Concept ;
  rdfs:comment "C_O_DRAINAGE" ;
  skos:definition "water is removed from the soil rapidly in relation to supply. Excess water flows downward rapidly if underlying material is highly permeable. There may be rapid subsurface lateral flow during heavy rainfall provided there is a steep gradient. Soils are usually coarse-textured, or shallow, or both. No horizon is normally wet for more than several hours after water addition."@en ;
  skos:notation "6" ;
  skos:prefLabel "Rapidly drained"@en ;
.
sp:soil-water-permeability-1
  a sp:Soil-permeability ;
  a skos:Concept ;
  rdfs:comment "C_PERMEABILITY" ;
  skos:definition """vertical transmission of water in the least permeable horizon is very slow; the profile would take periods of a month or more after thorough wetting to reach field capacity if there were no obstructions to movement from the profile. Structure may vary, but cracks or spaces between peds when dry close on wetting. Texture is usually clay or silty clay, and there are no pores visible (with a hand lens) that could conduct water when wet.
Ks range: <5 mm/day
Drainage time: months"""@en ;
  skos:notation "1" ;
  skos:prefLabel "Very slowly permeable"@en ;
.
sp:soil-water-permeability-2
  a sp:Soil-permeability ;
  a skos:Concept ;
  rdfs:comment "C_PERMEABILITY" ;
  skos:definition """vertical transmission of water in the least permeable horizon is slow; the profile would take periods of a week or more after thorough wetting to reach field capacity if there were no obstructions to movement from the profile. Structure may vary, usually from massive to moderate grade. Texture is usually clay or silty clay, and there will be few pores visible (with a hand lens) that conduct water when wet. If texture is coarser, the interparticle voids are filled with fine mineral.
Ks range: 5-50 mm/day
Drainage time: weeks"""@en ;
  skos:notation "2" ;
  skos:prefLabel "Slowly permeable"@en ;
.
sp:soil-water-permeability-3
  a sp:Soil-permeability ;
  a skos:Concept ;
  rdfs:comment "C_PERMEABILITY" ;
  skos:definition """vertical transmission of water in the least permeable horizon is such that the profile would take no more than a number (1–5) of days after a thorough wetting to reach field capacity if there were no obstructions to water movement from the profile. The soil may vary in structure but grade is usually at least moderate, and blocky or polyhedral peds are common. If massive, the soil material is always porous. The pores and channels that remain open when wet are clearly visible with a hand lens.
Ks range: 50-500 mm/day
Drainage time: days"""@en ;
  skos:notation "3" ;
  skos:prefLabel "Moderately permeable"@en ;
.
sp:soil-water-permeability-4
  a sp:Soil-permeability ;
  a skos:Concept ;
  rdfs:comment "C_PERMEABILITY" ;
  skos:definition """vertical transmission of water in the least permeable horizon is such that the profile would take no more than a number (1–12) of hours after a thorough wetting to reach field capacity if there were no obstructions to water movement from the profile. Horizons have large, continuous and clearly visible connecting pores and cracks that do not close with wetting. Texture is usually sandy and nodules or gravel are commonly present. Soil horizons are usually apedal, but some medium- to fine-textured soils with strong granular structure or cementation of aggregates can be highly permeable.
Ks range: >500 mm/day
Drainage time: hours"""@en ;
  skos:notation "4" ;
  skos:prefLabel "Highly permeable"@en ;
.
sp:soil-water-regime
  a skos:Collection ;
  rdfs:isDefinedBy asls:soil-profile ;
  skos:inScheme asls:soil-profile ;
  skos:definition """Traditional approaches to soil drainage do not adequately differentiate between hydrological setting and permeability of the material of the profile. For example, a very permeable, coarse-textured soil occurring in a wet depression would have to be classed as very poorly drained. Hence there is a need to consider permeability, which refers to the potential of a soil to transmit water internally, and drainage, which refers to the rapidity and extent of water removal from the soil profile or site. Both these aspects of internal drainage may be difficult to assess in the field, and cannot be based solely on profile morphology. Mottling may, but not always, reflect drainage status, since mottling may be a relict feature. Vegetation and topography may be useful guides.
These concepts of permeability and drainage are largely based on Canada Soil Survey Committee (1978)."""@en ;
  skos:member sp:Site-drainage ;
  skos:member sp:Soil-permeability ;
  skos:prefLabel "Soil water regime"@en ;
.
sp:soil-water-status-D
  a sp:Soil-water-status ;
  a skos:Concept ;
  skos:definition """Dry is below wilting point. Material becomes darker or has lower colour value when moistened.

Behaviour of soils subjected to field test.
Sands, sandy loams: will flow through fingers or fragments will powder.
Loams: will not ball when squeezed in hand. Fragments will powder.
Clay loams, clays: will not ball when squeezed in hand. Fragments will break to smaller fragments or peds."""@en ;
  skos:notation "D" ;
  skos:note "These guidelines may not apply with sodic 2:1 clays, as, for example, they may be moderately moist but below wilting point."@en ;
  skos:prefLabel "Dry (soil water status)"@en ;
.
sp:soil-water-status-M
  a sp:Soil-water-status ;
  a skos:Concept ;
  skos:definition """Moist is the wetter half of the available moisture range.

Behaviour of soils subjected to field test.
Sands, sandy loams: forms weak ball but breaks easily.
Loams: will ball. Will not ribbon.
Clay loams, clays: will ball. Will ribbon easily."""@en ;
  skos:notation "M" ;
  skos:note "These guidelines may not apply with sodic 2:1 clays, as, for example, they may be moderately moist but below wilting point."@en ;
  skos:prefLabel "Moist (soil water status)"@en ;
.
sp:soil-water-status-T
  a sp:Soil-water-status ;
  a skos:Concept ;
  skos:definition """Moderately moist is the drier half of the available moisture range.

Behaviour of soils subjected to field test.
Sands, sandy loams: appears dry. Ball will not hold together.
Loams: forms crumbly ball on squeezing in hand.
Clay loams, clays: will ball. Will not ribbon."""@en ;
  skos:notation "T" ;
  skos:note "These guidelines may not apply with sodic 2:1 clays, as, for example, they may be moderately moist but below wilting point."@en ;
  skos:prefLabel "Moderately moist (soil water status)"@en ;
.
sp:soil-water-status-W
  a sp:Soil-water-status ;
  a skos:Concept ;
  skos:definition """Wet is at, or exceeding, field capacity. Will wet and/or stick to fingers when moulded.

Behaviour of soils subjected to field test.
Sands, sandy loams: ball leaves wet outline on hand when squeezed, or is wetter.
Loams: ball leaves wet outline on hand when squeezed, or is wetter. Sticky.
Clay loams, clays: ball leaves wet outline on hand when squeezed, or is wetter. Sticky."""@en ;
  skos:notation "W" ;
  skos:note "These guidelines may not apply with sodic 2:1 clays, as, for example, they may be moderately moist but below wilting point."@en ;
  skos:prefLabel "Wet (soil water status)"@en ;
.
sp:structure
  a skos:Collection ;
  rdfs:isDefinedBy asls:soil-profile ;
  skos:inScheme asls:soil-profile ;
  skos:definition """Soil structure refers to the distinctness, size and shape of peds. A ped is an individual natural soil aggregate consisting of a cluster of primary particles. Peds are separated from adjoining peds by surfaces of weakness that are recognisable as natural voids or by the occurrence of cutans (Brewer 1960).
Soil structure can only be described reliably in a relatively fresh vertical exposure or relatively undisturbed soil core, not from an auger boring. Vertical exposures that have been exposed for a long time (road cuttings, gullies) are unsuitable for the determination of structure that may alter due to daily or seasonal changes in moisture and temperature."""@en ;
  skos:member sp:Artificial-aggregates-structure ;
  skos:member sp:Pedality-size ;
  skos:member sp:Pedality-type ;
  skos:member sp:structure-pedality-compound ;
  skos:member sp:structure-pedality-grade ;
  skos:prefLabel "Structure"@en ;
.
sp:structure-artificial-CL
  a sp:Artificial-aggregates-structure ;
  a skos:Concept ;
  skos:definition "artificial aggregate with diameter 100 mm or more."@en ;
  skos:notation "CL" ;
  skos:prefLabel "Clod"@en ;
.
sp:structure-artificial-FR
  a sp:Artificial-aggregates-structure ;
  a skos:Concept ;
  skos:definition "artificial aggregate with diameter less than 100 mm."@en ;
  skos:notation "FR" ;
  skos:prefLabel "Fragment"@en ;
.
sp:structure-pedality-compound
  a skos:Collection ;
  rdfs:isDefinedBy asls:soil-profile ;
  skos:inScheme asls:soil-profile ;
  skos:definition """Compound pedality occurs where large peds part along natural planes of weakness to form smaller peds, which may again part to smaller peds, and so on to the smallest or primary peds.
Primary peds are the simplest peds occurring in soil material; they cannot be divided into smaller peds, but may be packed together to form compound peds of a higher level of organisation (Brewer 1964).
The order of peds and relationship of one to the other is important and may be described as the larger peds parting to the smaller and further where necessary. For example, 'strong 50-100 mm columnar, parting to moderate 20-50 mm prismatic, parting to moderate
10-20 mm angular blocky'. The word 'parting' and not 'breaking' is used. The term 'breaking' is used when soil is fractured along planes other than natural planes of weakness.
1	Largest peds (in the type of soil observation described), parting to
2	Next size peds, parting to
3	Next size peds, ... and further, if required, to the primary ped."""@en ;
  skos:prefLabel "Compound pedality"@en ;
.
sp:structure-pedality-grade
  a skos:Collection ;
  rdfs:isDefinedBy asls:soil-profile ;
  skos:inScheme asls:soil-profile ;
  rdfs:comment "C_STR_PED_GRADE" ;
  skos:definition "Grade of pedality is the degree of development and distinctness of peds. In virtually all material that has structure, the surface of individual peds will differ in some way from the interior of peds. The degree of development expresses the relative difference between the strength of cohesion within peds and the strength of adhesion between adjacent peds. Determination of grade of structure in the field depends on the proportion of peds that hold together as entire peds when displaced and also on the ease with which the soil separates into discrete peds. Grade of pedality varies with the soil water status. It is important to record the soil water status of the described profile, and it is desirable that the grade of pedality be described at the soil water status most common for the horizon."@en ;
  skos:member sp:Pedality-grade-apedal ;
  skos:member sp:Pedality-grade-pedal ;
  skos:prefLabel "Grade of pedality"@en ;
.
sp:structure-pedality-grade-G
  a sp:Pedality-grade-apedal ;
  a skos:Concept ;
  skos:definition "loose, incoherent* mass of individual particles. When displaced, soil separates into ultimate particles."@en ;
  skos:notation "G" ;
  skos:note """Apedal soil (no observable peds).
*Incoherent means that less than two-thirds of the soil material will remain united at the given moisture state without very small force (force 1, see ‘Consistence’) having been applied."""@en ;
  skos:prefLabel "Single grain"@en ;
.
sp:structure-pedality-grade-M
  a sp:Pedality-grade-pedal ;
  a skos:Concept ;
  skos:definition "peds well-formed and evident but not distinct in undisplaced soil. Adhesion between peds is usually firm or stronger. When displaced, more than one-third of the soil material consists of entire peds, the remainder consisting of broken peds, fragments and ultimate particles."@en ;
  skos:notation "M" ;
  skos:note "Pedal soil (observable peds)."@en ;
  skos:prefLabel "Moderate (structure pedality grade)"@en ;
.
sp:structure-pedality-grade-S
  a sp:Pedality-grade-pedal ;
  a skos:Concept ;
  skos:definition "peds quite distinct in undisplaced soil. Adhesion between peds is usually firm or weaker. When displaced, more than two-thirds of the soil material consists of entire peds."@en ;
  skos:notation "S" ;
  skos:note "Pedal soil (observable peds)."@en ;
  skos:prefLabel "Strong (structure pedality grade)"@en ;
.
sp:structure-pedality-grade-V
  a sp:Pedality-grade-apedal ;
  a skos:Concept ;
  dcterms:description "coherent. When displaced, soil separates into fragments, which may be crushed to ultimate particles."@en ;
  skos:definition "coherent*. When displaced, soil separates into fragments, which may be crushed to ultimate particles."@en ;
  skos:notation "V" ;
  skos:note """Apedal soil (no observable peds)
*Coherent means that two-thirds or more of the soil material will remain united at the given moisture state unless force is applied."""@en ;
  skos:prefLabel "Massive (structure pedality grade)"@en ;
.
sp:structure-pedality-grade-W
  a sp:Pedality-grade-pedal ;
  a skos:Concept ;
  skos:definition "peds indistinct and barely observable in undisplaced soil. When displaced, up to one-third of the soil material consists of peds, the remainder consisting of variable amounts of fragments and ultimate particles."@en ;
  skos:notation "W" ;
  skos:note "Pedal soil (observable peds)."@en ;
  skos:prefLabel "Weak (structure pedality grade)"@en ;
.
sp:structure-pedality-size-1
  a sp:Pedality-size ;
  a skos:Concept ;
  dcterms:description "<2 mm"@en ;
  skos:definition "< 2 mm"@en ;
  skos:notation "1" ;
  skos:prefLabel "< 2 mm"@en ;
.
sp:structure-pedality-size-2
  a sp:Pedality-size ;
  a skos:Concept ;
  skos:definition "2-5 mm"@en ;
  skos:notation "2" ;
  skos:prefLabel "2-5 mm"@en ;
.
sp:structure-pedality-size-3
  a sp:Pedality-size ;
  a skos:Concept ;
  skos:definition "5-10 mm"@en ;
  skos:notation "3" ;
  skos:prefLabel "5-10 mm"@en ;
.
sp:structure-pedality-size-4
  a sp:Pedality-size ;
  a skos:Concept ;
  skos:definition "10-20 mm"@en ;
  skos:notation "4" ;
  skos:prefLabel "10-20 mm"@en ;
.
sp:structure-pedality-size-5
  a sp:Pedality-size ;
  a skos:Concept ;
  skos:definition "20-50 mm"@en ;
  skos:notation "5" ;
  skos:prefLabel "20-50 mm"@en ;
.
sp:structure-pedality-size-6
  a sp:Pedality-size ;
  a skos:Concept ;
  skos:definition "50-100 mm"@en ;
  skos:notation "6" ;
  skos:prefLabel "50-100 mm"@en ;
.
sp:structure-pedality-size-7
  a sp:Pedality-size ;
  a skos:Concept ;
  skos:definition "100-200 mm"@en ;
  skos:notation "7" ;
  skos:prefLabel "100-200 mm"@en ;
.
sp:structure-pedality-size-8
  a sp:Pedality-size ;
  a skos:Concept ;
  skos:definition "200-500 mm"@en ;
  skos:notation "8" ;
  skos:prefLabel "200-500 mm"@en ;
.
sp:structure-pedality-size-9
  a sp:Pedality-size ;
  a skos:Concept ;
  skos:definition "> 500 mm"@en ;
  skos:notation "9" ;
  skos:prefLabel "> 500 mm"@en ;
.
sp:structure-pedality-type-AB
  a sp:Pedality-type ;
  a skos:Concept ;
  skos:definition "soil particles arranged around a point and bounded by six relatively flat, roughly equal faces. Re-entrant angles between adjoining faces are few or absent. There is usually much accommodation of ped faces to the faces of surrounding peds. Most vertices between adjoining faces are angular.	Angular blocky	Soil particles arranged around a point and bounded by six relatively flat, roughly equal faces. Re-entrant angles between adjoining faces are few or absent. There is usually much accommodation of ped faces to the faces of surrounding peds. Most vertices between adjoining faces are angular."@en ;
  skos:notation "AB" ;
  skos:prefLabel "Angular blocky"@en ;
.
sp:structure-pedality-type-CA
  a sp:Pedality-type ;
  a skos:Concept ;
  skos:definition "faunal casts are strictly not peds, but they are described in a similar manner. They are formed from, or are deposited in, the O horizons or the soil solum and include: excreta of soil fauna which may be discrete particles, for example insect faeces or the dense, coherent, globular forms of earthworm excreta. They are generally spherical or ovate in shape and have a strong conchoidal fracture; soil masticated with salivary secretions into globular forms, for example, by ants, crickets, wasps.	Cast	Faunal casts are strictly not peds, but they are described in a similar manner. They are formed from, or are deposited in, the O horizons or the soil solum and include: excreta of soil fauna which may be discrete particles, for example insect faeces or the dense, coherent, globular forms of earthworm excreta. They are generally spherical or ovate in shape and have a strong conchoidal fracture; soil masticated with salivary secretions into globular forms, for example, by ants, crickets, wasps."@en ;
  skos:notation "CA" ;
  skos:prefLabel "Cast"@en ;
.
sp:structure-pedality-type-CO
  a sp:Pedality-type ;
  a skos:Concept ;
  skos:definition "soil particles arranged around a vertical axis and bounded by well-defined, relatively flat faces with much accommodation to the faces of surrounding peds. Vertices between adjoining faces are usually angular with domed tops.	Columnar	Soil particles arranged around a vertical axis and bounded by well-defined, relatively flat faces with much accommodation to the faces of surrounding peds. Vertices between adjoining faces are usually angular with domed tops."@en ;
  skos:notation "CO" ;
  skos:prefLabel "Columnar"@en ;
.
sp:structure-pedality-type-GR
  a sp:Pedality-type ;
  a skos:Concept ;
  skos:definition "spheroidal with limited accommodation to the faces of surrounding peds.	Granular	Spheroidal with limited accommodation to the faces of surrounding peds."@en ;
  skos:notation "GR" ;
  skos:prefLabel "Granular"@en ;
.
sp:structure-pedality-type-LE
  a sp:Pedality-type ;
  a skos:Concept ;
  skos:definition "soil particles arranged around an elliptical or circular plane and bounded by curved faces with much accommodation to the faces of surrounding peds. Most vertices are angular and acute.	Lenticular	Soil particles arranged around an elliptical or circular plane and bounded by curved faces with much accommodation to the faces of surrounding peds. Most vertices are angular and acute."@en ;
  skos:notation "LE" ;
  skos:prefLabel "Lenticular"@en ;
.
sp:structure-pedality-type-PL
  a sp:Pedality-type ;
  a skos:Concept ;
  skos:definition "soil particles arranged around a horizontal plane and bounded by relatively flat horizontal faces with much accommodation to the faces of surrounding peds.	Platy	Soil particles arranged around a horizontal plane and bounded by relatively flat horizontal faces with much accommodation to the faces of surrounding peds."@en ;
  skos:notation "PL" ;
  skos:prefLabel "Platy (structure pedality)"@en ;
.
sp:structure-pedality-type-PO
  a sp:Pedality-type ;
  a skos:Concept ;
  skos:definition "soil particles arranged around a point and bounded by more than six relatively flat, unequal, dissimilar faces. Re-entrant angles between adjoining faces are a feature. There is usually much accommodation of ped faces to the faces of surrounding peds. Most vertices are angular.	Polyhedral	Soil particles arranged around a point and bounded by more than six relatively flat, unequal, dissimilar faces. Re-entrant angles between adjoining faces are a feature. There is usually much accommodation of ped faces to the faces of surrounding peds. Most vertices are angular."@en ;
  skos:notation "PO" ;
  skos:prefLabel "Polyhedral"@en ;
.
sp:structure-pedality-type-PR
  a sp:Pedality-type ;
  a skos:Concept ;
  skos:definition "soil particles arranged around a vertical axis and bounded by well-defined, relatively flat faces with much accommodation to the faces of surrounding peds. Vertices between adjoining faces are usually angular.	Prismatic	Soil particles arranged around a vertical axis and bounded by well-defined, relatively flat faces with much accommodation to the faces of surrounding peds. Vertices between adjoining faces are usually angular."@en ;
  skos:notation "PR" ;
  skos:prefLabel "Prismatic"@en ;
.
sp:structure-pedality-type-SB
  a sp:Pedality-type ;
  a skos:Concept ;
  skos:definition "soil particles arranged around a point and bounded by flat and rounded faces with limited accommodation to the faces of surrounding peds. Many vertices are rounded.	Subangular blocky	Soil particles arranged around a point and bounded by flat and rounded faces with limited accommodation to the faces of surrounding peds. Many vertices are rounded."@en ;
  skos:notation "SB" ;
  skos:prefLabel "Subangular blocky"@en ;
.
sp:surfacecondition-C
  a sp:Surface-condition ;
  a skos:Concept ;
  skos:definition "distinct surface layer, often laminated, ranging in thickness from a few millimetres to a few tens of millimetres, which is hard and brittle when dry and cannot be readily separated from, and lifted off, the underlying soil material."@en ;
  skos:notation "C" ;
  skos:prefLabel "Surface crust"@en ;
.
sp:surfacecondition-F
  a sp:Surface-condition ;
  a skos:Concept ;
  skos:definition "coherent mass of individual particles or aggregates. Surface disturbed or indented by moderate pressure of forefinger."@en ;
  skos:notation "F" ;
  skos:note "Coherent means that two-thirds of the soil material, whether composed of peds or not, will remain united at the given moisture state unless force is applied."@en ;
  skos:prefLabel "Firm (surface condition)"@en ;
.
sp:surfacecondition-G
  a sp:Surface-condition ;
  a skos:Concept ;
  skos:definition "cracks at least 5 mm wide and extending upwards to the surface or to the base of any plough layer or thin (<0.03 m) surface horizon."@en ;
  skos:notation "G" ;
  skos:prefLabel "Cracking"@en ;
.
sp:surfacecondition-H
  a sp:Surface-condition ;
  a skos:Concept ;
  skos:definition "compact, hard, apparently apedal condition forms on drying but softens on wetting. When dry, the material is hard below any surface crust or flake that may occur, and is not disturbed or indented by pressure of forefinger."@en ;
  skos:notation "H" ;
  skos:prefLabel "Hard setting"@en ;
.
sp:surfacecondition-L
  a sp:Surface-condition ;
  a skos:Concept ;
  skos:definition "incoherent mass of individual particles or aggregates. Surface easily disturbed by pressure of forefinger."@en ;
  skos:notation "L" ;
  skos:note "Incoherent means that less than two-thirds of the soil material, whether composed of peds or not, will remain united at the given moisture state without very small force (force 1, see ‘Consistence’) having been applied."@en ;
  skos:prefLabel "Loose (surface condition)"@en ;
.
sp:surfacecondition-M
  a sp:Surface-condition ;
  a skos:Concept ;
  skos:definition "strongly pedal loose surface mulch forms on wetting and drying. Peds commonly less than 5 mm in least dimension."@en ;
  skos:notation "M" ;
  skos:prefLabel "Self-mulching"@en ;
.
sp:surfacecondition-O
  a sp:Surface-condition ;
  a skos:Concept ;
  skos:definition "Other"@en ;
  skos:notation "O" ;
  skos:prefLabel "Other (surface condition)"@en ;
.
sp:surfacecondition-P
  a sp:Surface-condition ;
  a skos:Concept ;
  skos:definition "soil that has been extensively trampled under wet conditions by hoofed animals."@en ;
  skos:notation "P" ;
  skos:prefLabel "Poached"@en ;
.
sp:surfacecondition-R
  a sp:Surface-condition ;
  a skos:Concept ;
  skos:definition "effect of cultivation is obvious."@en ;
  skos:notation "R" ;
  skos:prefLabel "Recently cultivated"@en ;
.
sp:surfacecondition-S
  a sp:Surface-condition ;
  a skos:Concept ;
  skos:definition "coherent mass of individual particles or aggregates. Surface easily disturbed by pressure of forefinger."@en ;
  skos:notation "S" ;
  skos:note "Coherent means that two-thirds of the soil material, whether composed of peds or not, will remain united at the given moisture state unless force is applied."@en ;
  skos:prefLabel "Soft"@en ;
.
sp:surfacecondition-T
  a sp:Surface-condition ;
  a skos:Concept ;
  skos:definition "soil that has been extensively trampled under dry conditions by hoofed animals."@en ;
  skos:notation "T" ;
  skos:prefLabel "Trampled"@en ;
.
sp:surfacecondition-X
  a sp:Surface-condition ;
  a skos:Concept ;
  skos:definition "thin, massive surface layer, usually less than 10 mm thick, which on drying separates from, and can be readily lifted off, the soil below. It usually consists mainly of dispersed clay, and may become increasingly fragile as the soil dries."@en ;
  skos:notation "X" ;
  skos:prefLabel "Surface flake"@en ;
.
sp:surfacecondition-Y
  a sp:Surface-condition ;
  a skos:Concept ;
  skos:definition "thin, more or less continuous crust of biologically stabilised soil material usually due to algae, liverworts and mosses."@en ;
  skos:notation "Y" ;
  skos:prefLabel "Cryptogam surface"@en ;
.
sp:surfacecondition-Z
  a sp:Surface-condition ;
  a skos:Concept ;
  skos:definition "surface has visible salt, or salinity is evident from the absence or nature of the vegetation or from soil consistence. These conditions are characterised by their notable difference from adjacent non-saline areas."@en ;
  skos:notation "Z" ;
  skos:prefLabel "Saline (surface condition)"@en ;
.
sp:voids
  a owl:Class ;
  a skos:Collection ;
  rdfs:isDefinedBy asls:soil-profile ;
  skos:inScheme asls:soil-profile ;
  rdfs:subClassOf skos:Concept ;
  skos:definition "This is a general term for pore space and other openings in soils not occupied by solid mineral matter. The most important are cracks (planar voids) and pores, which are approximately circular in cross-section."@en ;
  skos:member sp:Cracks-width ;
  skos:member sp:voids-micropores ;
  skos:member sp:voids-pores ;
  skos:prefLabel "Voids"@en ;
.
sp:voids-cracks-1
  a sp:Cracks-width ;
  a skos:Concept ;
  skos:definition "<5 mm width"@en ;
  skos:notation "1" ;
  skos:prefLabel "Fine (voids cracks)"@en ;
.
sp:voids-cracks-2
  a sp:Cracks-width ;
  a skos:Concept ;
  skos:definition "5 - 10 mm width"@en ;
  skos:notation "2" ;
  skos:prefLabel "Medium (voids cracks)"@en ;
.
sp:voids-cracks-3
  a sp:Cracks-width ;
  a skos:Concept ;
  skos:definition "10–20 mm width"@en ;
  skos:notation "3" ;
  skos:prefLabel "Coarse (voids cracks)"@en ;
.
sp:voids-cracks-4
  a sp:Cracks-width ;
  a skos:Concept ;
  skos:definition "20–50 mm width"@en ;
  skos:notation "4" ;
  skos:prefLabel "Very coarse (voids cracks)"@en ;
.
sp:voids-cracks-5
  a sp:Cracks-width ;
  a skos:Concept ;
  skos:definition "20–50 mm width"@en ;
  skos:notation "5" ;
  skos:prefLabel "Extremely coarse (voids cracks)"@en ;
.
sp:voids-macropores-abundance
  a skos:Collection ;
  rdfs:isDefinedBy asls:soil-profile ;
  skos:inScheme asls:soil-profile ;
  rdfs:comment "N_PORE_ABUN" ;
  skos:definition "abundance of macropores based relevant to the diameter of the macropores"@en ;
  skos:member sp:Pore-abundance-coarse ;
  skos:member sp:Pore-abundance-fine ;
  skos:prefLabel "Abundance of macropores"@en ;
.
sp:voids-macropores-abundance-0
  a sp:Pore-abundance-coarse ;
  a sp:Pore-abundance-fine ;
  a skos:Concept ;
  skos:definition "No fine, very fine, medium or coarse macropores"@en ;
  skos:notation "0" ;
  skos:prefLabel "No macropores"@en ;
.
sp:voids-macropores-abundance-1
  a sp:Pore-abundance-fine ;
  a skos:Concept ;
  skos:definition "<1 per 100 mm2 of diameter less than 2mm"@en ;
  skos:notation "1" ;
  skos:prefLabel "Few fine or very fine macropores"@en ;
.
sp:voids-macropores-abundance-2
  a sp:Pore-abundance-fine ;
  a skos:Concept ;
  skos:definition "1–5 per 100 mm2 of diameter less than 2mm"@en ;
  skos:notation "2" ;
  skos:prefLabel "Common fine or very fine macropores"@en ;
.
sp:voids-macropores-abundance-3
  a sp:Pore-abundance-fine ;
  a skos:Concept ;
  skos:definition ">5 per 100 mm2 of diameter less than 2mm"@en ;
  skos:notation "3" ;
  skos:prefLabel "Many fine or very fine macropores"@en ;
.
sp:voids-macropores-abundance-4
  a sp:Pore-abundance-coarse ;
  a skos:Concept ;
  skos:definition "<1 per 0.01 m2 of diameter greater than 2mm"@en ;
  skos:notation "4" ;
  skos:prefLabel "Few medium or coarse macropores"@en ;
.
sp:voids-macropores-abundance-5
  a sp:Pore-abundance-coarse ;
  a skos:Concept ;
  skos:definition "1–5 per 0.01 m2 of diameter greater than 2mm"@en ;
  skos:notation "5" ;
  skos:prefLabel "Common medium or coarse macropores"@en ;
.
sp:voids-macropores-abundance-6
  a sp:Pore-abundance-coarse ;
  a skos:Concept ;
  skos:definition ">5 per 0.01 m2 of diameter greater than 2mm"@en ;
  skos:notation "6" ;
  skos:prefLabel "Many medium or coarse macropores"@en ;
.
sp:voids-macropores-diameter-1
  a sp:Pore-diameter ;
  a skos:Concept ;
  dcterms:description "0.075–1 mm"@en ;
  skos:definition "0.075–1 m"@en ;
  skos:notation "1" ;
  skos:note "Use Figure 18 as a guide to average diameter"@en ;
  skos:prefLabel "Very fine (voids macropores)"@en ;
.
sp:voids-macropores-diameter-2
  a sp:Pore-diameter ;
  a skos:Concept ;
  skos:definition "1–2 mm"@en ;
  skos:notation "2" ;
  skos:note "Use Figure 18 as a guide to average diameter"@en ;
  skos:prefLabel "Fine (voids macropores)"@en ;
.
sp:voids-macropores-diameter-3
  a sp:Pore-diameter ;
  a skos:Concept ;
  skos:definition "2–5 mm"@en ;
  skos:notation "3" ;
  skos:note "Use Figure 18 as a guide to average diameter"@en ;
  skos:prefLabel "Medium (voids macropores)"@en ;
.
sp:voids-macropores-diameter-4
  a sp:Pore-diameter ;
  a skos:Concept ;
  skos:definition ">5 mm"@en ;
  skos:notation "4" ;
  skos:note "Use Figure 18 as a guide to average diameter"@en ;
  skos:prefLabel "Coarse (voids macropores)"@en ;
.
sp:voids-micropores
  a sp:voids ;
  a skos:Concept ;
  dcterms:identifier "http://anzsoil.org/def/au/asls/soil-profile/voids-micropores" ;
  skos:definition "voids that are approximately circular in cross-section and less than 0.075 mm diameter"@en ;
  skos:note "Only macropores can be seen with the naked eye"@en ;
  skos:prefLabel "Micropores (presence)"@en ;
.
sp:voids-pores
  a skos:Collection ;
  rdfs:isDefinedBy asls:soil-profile ;
  skos:inScheme asls:soil-profile ;
  skos:definition """Pores are divided into:

Micropores	less than 0.075 mm diameter
Macropores	greater than 0.075 mm diameter

Only macropores can be seen with the naked eye. All visible pores, holes and tubes within peds, clods, fragments or apedal soil are recorded in the classes below."""@en ;
  skos:member sp:Pore-diameter ;
  skos:member sp:voids-macropores-abundance ;
  skos:note "Only macropores can be seen with the naked eye"@en ;
  skos:prefLabel "Pores"@en ;
.
sp:water-repellence-N
  a sp:Water-repellence ;
  a skos:Concept ;
  skos:definition "water is absorbed into soil in 10 seconds or less."@en ;
  skos:notation "N" ;
  skos:prefLabel "Non water repellent"@en ;
.
sp:water-repellence-R
  a sp:Water-repellence ;
  a skos:Concept ;
  skos:definition "water takes greater than 10 seconds and 2-molar ethanol takes 10 seconds or less to be absorbed into soil."@en ;
  skos:notation "R" ;
  skos:prefLabel "Water repellent"@en ;
.
sp:water-repellence-S
  a sp:Water-repellence ;
  a skos:Concept ;
  skos:definition "2 Molar ethanol takes greater than 10 seconds to be absorbed into soil."@en ;
  skos:notation "S" ;
  skos:prefLabel "Strongly water repellent"@en ;
.
subst:lithology-AC
  a skos:Concept ;
  skos:prefLabel "Alcrete"@en ;
.
subst:lithology-AD
  a skos:Concept ;
  skos:prefLabel "Adamellite"@en ;
.
subst:lithology-AF
  a skos:Concept ;
  skos:prefLabel "Volcanic ash (fine)"@en ;
.
subst:lithology-AG
  a skos:Concept ;
  skos:prefLabel "Agglomerate"@en ;
.
subst:lithology-AH
  a skos:Concept ;
  skos:prefLabel "Anhydrite"@en ;
.
subst:lithology-AM
  a skos:Concept ;
  skos:prefLabel "Amphibolite"@en ;
.
subst:lithology-AN
  a skos:Concept ;
  skos:prefLabel "Andesite"@en ;
.
subst:lithology-AP
  a skos:Concept ;
  skos:prefLabel "Aplite"@en ;
.
subst:lithology-AR
  a skos:Concept ;
  skos:prefLabel "Arkose"@en ;
.
subst:lithology-AS
  a skos:Concept ;
  skos:prefLabel "Volcanic ash (sandy)"@en ;
.
subst:lithology-BA
  a skos:Concept ;
  skos:prefLabel "Basalt"@en ;
.
subst:lithology-BB
  a skos:Concept ;
  skos:prefLabel "Bombs (or blocks)"@en ;
.
subst:lithology-BO
  a skos:Concept ;
  skos:prefLabel "Boulders" ;
.
subst:lithology-BR
  a skos:Concept ;
  skos:prefLabel "Breccia"@en ;
.
subst:lithology-C
  a skos:Concept ;
  skos:prefLabel "Clay"@en ;
.
subst:lithology-CB
  a skos:Concept ;
  skos:prefLabel "Cobbles" ;
.
subst:lithology-CG
  a skos:Concept ;
  skos:prefLabel "Conglomerate"@en ;
.
subst:lithology-CH
  a skos:Concept ;
  skos:prefLabel "Chert"@en ;
.
subst:lithology-CO
  a skos:Concept ;
  skos:prefLabel "Coal"@en ;
.
subst:lithology-CU
  a skos:Concept ;
  skos:prefLabel "Consolidated rock"@en ;
.
subst:lithology-DI
  a skos:Concept ;
  skos:prefLabel "Diorite"@en ;
.
subst:lithology-DM
  a skos:Concept ;
  skos:prefLabel "Dolomite"@en ;
.
subst:lithology-DR
  a skos:Concept ;
  skos:prefLabel "Dolerite"@en ;
.
subst:lithology-FC
  a skos:Concept ;
  skos:prefLabel "Ferricrete"@en ;
.
subst:lithology-GA
  a skos:Concept ;
  skos:prefLabel "Gabbro"@en ;
.
subst:lithology-GD
  a skos:Concept ;
  skos:prefLabel "Granodiorite"@en ;
.
subst:lithology-GE
  a skos:Concept ;
  skos:prefLabel "Greenstone"@en ;
.
subst:lithology-GN
  a skos:Concept ;
  skos:prefLabel "Granite"@en ;
.
subst:lithology-GR
  a skos:Concept ;
  skos:prefLabel "Granulite"@en ;
.
subst:lithology-GS
  a skos:Concept ;
  skos:prefLabel "Gneiss"@en ;
.
subst:lithology-GV
  a skos:Concept ;
  skos:prefLabel "Gravel"@en ;
.
subst:lithology-GW
  a skos:Concept ;
  skos:prefLabel "Graywacke"@en ;
.
subst:lithology-GY
  a skos:Concept ;
  skos:prefLabel "Gypsum"@en ;
.
subst:lithology-HA
  a skos:Concept ;
  skos:prefLabel "Halite"@en ;
.
subst:lithology-HO
  a skos:Concept ;
  skos:prefLabel "Hornfels"@en ;
.
subst:lithology-IG
  a skos:Concept ;
  skos:prefLabel "Igneous rock"@en ;
.
subst:lithology-JA
  a skos:Concept ;
  skos:prefLabel "Jasper"@en ;
.
subst:lithology-KA
  a skos:Concept ;
  skos:prefLabel "Calcarenite"@en ;
.
subst:lithology-KC
  a skos:Concept ;
  skos:prefLabel "Calcrete"@en ;
.
subst:lithology-KL
  a skos:Concept ;
  skos:prefLabel "Calcilutite"@en ;
.
subst:lithology-KM
  a skos:Concept ;
  skos:prefLabel "Calcareous mudstone"@en ;
.
subst:lithology-KR
  a skos:Concept ;
  skos:prefLabel "Calcirudite"@en ;
.
subst:lithology-KS
  a skos:Concept ;
  skos:prefLabel "Calcareous sand"@en ;
.
subst:lithology-LC
  a skos:Concept ;
  skos:prefLabel "Silcrete"@en ;
.
subst:lithology-LI
  a skos:Concept ;
  skos:prefLabel "Limestone"@en ;
.
subst:lithology-M
  a skos:Concept ;
  skos:prefLabel "Same as substrate material"@en ;
.
subst:lithology-MB
  a skos:Concept ;
  skos:prefLabel "Marble"@en ;
.
subst:lithology-MD
  a skos:Concept ;
  skos:prefLabel "Microdiorite"@en ;
.
subst:lithology-ME
  a skos:Concept ;
  skos:prefLabel "Metamorphic rock"@en ;
.
subst:lithology-MG
  a skos:Concept ;
  skos:prefLabel "Microgranite"@en ;
.
subst:lithology-MI
  a skos:Concept ;
  skos:prefLabel "Migmatite"@en ;
.
subst:lithology-ML
  a skos:Concept ;
  skos:prefLabel "Marl"@en ;
.
subst:lithology-MS
  a skos:Concept ;
  skos:prefLabel "Microsyenite"@en ;
.
subst:lithology-MU
  a skos:Concept ;
  skos:prefLabel "Mudstone"@en ;
.
subst:lithology-MY
  a skos:Concept ;
  skos:prefLabel "Mylonite"@en ;
.
subst:lithology-PC
  a skos:Concept ;
  skos:prefLabel "Porcellanite"@en ;
.
subst:lithology-PE
  a skos:Concept ;
  skos:prefLabel "Peridotite"@en ;
.
subst:lithology-PG
  a skos:Concept ;
  skos:prefLabel "Pegmatite"@en ;
.
subst:lithology-PH
  a skos:Concept ;
  skos:prefLabel "Phyllite"@en ;
.
subst:lithology-PL
  a skos:Concept ;
  skos:prefLabel "Phonolite"@en ;
.
subst:lithology-PO
  a skos:Concept ;
  skos:prefLabel "Porphyry"@en ;
.
subst:lithology-PY
  a skos:Concept ;
  skos:prefLabel "Pyroxenite"@en ;
.
subst:lithology-QP
  a skos:Concept ;
  skos:prefLabel "Quartz porphyry"@en ;
.
subst:lithology-QS
  a skos:Concept ;
  skos:prefLabel "Quartz sandstone"@en ;
.
subst:lithology-QU
  a skos:Concept ;
  skos:prefLabel "Quartzite"@en ;
.
subst:lithology-QZ
  a skos:Concept ;
  skos:prefLabel "Quartz"@en ;
.
subst:lithology-R
  a skos:Concept ;
  skos:prefLabel "Same as rock outcrop"@en ;
.
subst:lithology-RB
  a skos:Concept ;
  skos:prefLabel "Red-brown hardpan"@en ;
.
subst:lithology-RH
  a skos:Concept ;
  skos:prefLabel "Rhyolite"@en ;
.
subst:lithology-S
  a skos:Concept ;
  skos:prefLabel "Sand"@en ;
.
subst:lithology-SA
  a skos:Concept ;
  skos:prefLabel "Sandstone"@en ;
.
subst:lithology-SD
  a skos:Concept ;
  skos:prefLabel "Detrital sedimentary rock"@en ;
.
subst:lithology-SH
  a skos:Concept ;
  skos:prefLabel "Shale"@en ;
.
subst:lithology-SK
  a skos:Concept ;
  skos:prefLabel "Scoria"@en ;
.
subst:lithology-SL
  a skos:Concept ;
  skos:prefLabel "Slate"@en ;
.
subst:lithology-SN
  a skos:Concept ;
  skos:prefLabel "Stones" ;
.
subst:lithology-SR
  a skos:Concept ;
  skos:prefLabel "Serpentinite"@en ;
.
subst:lithology-ST
  a skos:Concept ;
  skos:prefLabel "Schist"@en ;
.
subst:lithology-SY
  a skos:Concept ;
  skos:prefLabel "Syenite"@en ;
.
subst:lithology-TR
  a skos:Concept ;
  skos:prefLabel "Trachyte"@en ;
.
subst:lithology-TU
  a skos:Concept ;
  skos:prefLabel "Tuff"@en ;
.
subst:lithology-UC
  a skos:Concept ;
  skos:prefLabel "Unconsolidated material"@en ;
.
subst:lithology-VB
  a skos:Concept ;
  skos:prefLabel "Volcanic breccia"@en ;
.
subst:lithology-VG
  a skos:Concept ;
  skos:prefLabel "Volcanic glass"@en ;
.
subst:lithology-Z
  a skos:Concept ;
  skos:prefLabel "Silt"@en ;
.
subst:lithology-ZS
  a skos:Concept ;
  skos:prefLabel "Siltstone"@en ;
.
subst:material-strength
  a skos:Collection ;
  rdfs:isDefinedBy asls:soil-profile ;
  skos:inScheme asls:soil-profile ;
  skos:prefLabel "Strength of material - enumeration"@en ;
  skos:definition "Strength of material - enumeration"@en ;
  skos:member
    subst:material-strength-M ,
    subst:material-strength-S ,
    subst:material-strength-VS ,
    subst:material-strength-VW ,
    subst:material-strength-W ;
.
subst:material-strength-M
  a skos:Concept ;
  skos:prefLabel "Moderately strong rock"@en ;
.
subst:material-strength-S
  a skos:Concept ;
  skos:prefLabel "Strong rock"@en ;
.
subst:material-strength-VS
  a skos:Concept ;
  skos:prefLabel "Very strong rock"@en ;
.
subst:material-strength-VW
  a skos:Concept ;
  skos:prefLabel "Very weak rock"@en ;
.
subst:material-strength-W
  a skos:Concept ;
  skos:prefLabel "Weak rock"@en ;
.

ls:coarse-fragments-abundance-0 skos:definition "No coarse fragments"@en .
ls:coarse-fragments-abundance-1 skos:definition "Very slightly or very few"@en .
ls:coarse-fragments-abundance-2 skos:definition "Slightly or few"@en .
ls:coarse-fragments-abundance-3 skos:definition "No qualifier or common"@en .
ls:coarse-fragments-abundance-4 skos:definition "Moderately or many"@en .
ls:coarse-fragments-abundance-5 skos:definition "Very or abundant"@en .
ls:coarse-fragments-abundance-6 skos:definition "Extremely or very abundant"@en .
ls:coarse-fragments-shape-A skos:definition "Angular"@en .
ls:coarse-fragments-shape-AP skos:definition "Angular platy"@en .
ls:coarse-fragments-shape-AT skos:definition "Angular tabular"@en .
ls:coarse-fragments-shape-R skos:definition "Rounded"@en .
ls:coarse-fragments-shape-RP skos:definition "Rounded platy"@en .
ls:coarse-fragments-shape-RT skos:definition "Rounded tabular"@en .
ls:coarse-fragments-shape-S skos:definition "Subangular"@en .
ls:coarse-fragments-shape-SP skos:definition "Subangular platy"@en .
ls:coarse-fragments-shape-ST skos:definition "Subangular tabular"@en .
ls:coarse-fragments-shape-U skos:definition "Subrounded"@en .
ls:coarse-fragments-shape-UP skos:definition "Subrounded platy"@en .
ls:coarse-fragments-shape-UT skos:definition "Subrounded tabular"@en .
ls:coarse-fragments-size-1 skos:definition "Fine gravelly or small pebbles"@en .
ls:coarse-fragments-size-2 skos:definition "Medium gravelly or medium pebbles"@en .
ls:coarse-fragments-size-3 skos:definition "Coarse gravelly or large pebbles"@en .
ls:coarse-fragments-size-4 skos:definition "Cobbly or cobbles"@en .
ls:coarse-fragments-size-5 skos:definition "Stony or stones"@en .
ls:coarse-fragments-size-6 skos:definition "Bouldery or boulders"@en .
ls:coarse-fragments-size-7 skos:definition "Large boulders"@en .
ls:lithology-CC skos:definition "Charcoal"@en .
ls:lithology-IS skos:definition "Ironstone"@en .
ls:lithology-M skos:definition "Same as substrate material"@en .
ls:lithology-OT skos:definition "Other"@en .
ls:lithology-OW skos:definition "Opalised wood"@en .
ls:lithology-PU skos:definition "Pumice"@en .
ls:lithology-R skos:definition "Same as rock outcrop"@en .
ls:lithology-SS skos:definition "Shells"@en .
sp:depth-of-horizon-lower skos:definition "Lower depth of soil horizon in metres"@en .
sp:depth-of-horizon-upper skos:definition "Upper depth of soil horizon in metres"@en .
subst:lithology-AC skos:definition "Alcrete"@en .
subst:lithology-AD skos:definition "Adamellite"@en .
subst:lithology-AF skos:definition "Ash (fine)"@en .
subst:lithology-AG skos:definition "Agglomerate"@en .
subst:lithology-AH skos:definition "Anhydrite"@en .
subst:lithology-AM skos:definition "Amphibolite"@en .
subst:lithology-AN skos:definition "Andesite"@en .
subst:lithology-AP skos:definition "Aplite"@en .
subst:lithology-AR skos:definition "Arkose"@en .
subst:lithology-AS skos:definition "Ash (sandy)"@en .
subst:lithology-BA skos:definition "Basalt"@en .
subst:lithology-BB skos:definition "Bombs (or blocks)"@en .
subst:lithology-BO skos:definition "Boulders"@en .
subst:lithology-BR skos:definition "Breccia"@en .
subst:lithology-C skos:definition "Clay"@en .
subst:lithology-CB skos:definition "Cobbles"@en .
subst:lithology-CG skos:definition "Conglomerate"@en .
subst:lithology-CH skos:definition "Chert"@en .
subst:lithology-CO skos:definition "Coal"@en .
subst:lithology-CU skos:definition "Consolidated rock"@en .
subst:lithology-DI skos:definition "Diorite"@en .
subst:lithology-DM skos:definition "Dolomite"@en .
subst:lithology-DR skos:definition "Dolerite"@en .
subst:lithology-FC skos:definition "Ferricrete"@en .
subst:lithology-GA skos:definition "Gabbro"@en .
subst:lithology-GD skos:definition "Granodiorite"@en .
subst:lithology-GE skos:definition "Greenstone"@en .
subst:lithology-GN skos:definition "Granite"@en .
subst:lithology-GR skos:definition "Granulite"@en .
subst:lithology-GS skos:definition "Gneiss"@en .
subst:lithology-GV skos:definition "Gravel"@en .
subst:lithology-GW skos:definition "Graywacke"@en .
subst:lithology-GY skos:definition "Gypsum"@en .
subst:lithology-HA skos:definition "Halite"@en .
subst:lithology-HO skos:definition "Hornfels"@en .
subst:lithology-IG skos:definition "Igneous rock"@en .
subst:lithology-JA skos:definition "Jasper"@en .
subst:lithology-KA skos:definition "Calcarenite"@en .
subst:lithology-KC skos:definition "Calcrete"@en .
subst:lithology-KL skos:definition "Calcilutite"@en .
subst:lithology-KM skos:definition "Calcareous mudstone"@en .
subst:lithology-KR skos:definition "Calcirudite"@en .
subst:lithology-KS skos:definition "Calcareous sand"@en .
subst:lithology-LC skos:definition "Silcrete"@en .
subst:lithology-LI skos:definition "Limestone"@en .
subst:lithology-M skos:definition "Same as substrate material"@en .
subst:lithology-MB skos:definition "Marble"@en .
subst:lithology-MD skos:definition "Microdiorite"@en .
subst:lithology-ME skos:definition "Metamorphic rock"@en .
subst:lithology-MG skos:definition "Microgranite"@en .
subst:lithology-MI skos:definition "Migmatite"@en .
subst:lithology-ML skos:definition "Marl"@en .
subst:lithology-MS skos:definition "Microsyenite"@en .
subst:lithology-MU skos:definition "Mudstone"@en .
subst:lithology-MY skos:definition "Mylonite"@en .
subst:lithology-PC skos:definition "Porcellanite"@en .
subst:lithology-PE skos:definition "Peridotite"@en .
subst:lithology-PG skos:definition "Pegmatite"@en .
subst:lithology-PH skos:definition "Phyllite"@en .
subst:lithology-PL skos:definition "Phonolite"@en .
subst:lithology-PO skos:definition "Porphyry"@en .
subst:lithology-PY skos:definition "Pyroxenite"@en .
subst:lithology-QP skos:definition "Quartz porphyry"@en .
subst:lithology-QS skos:definition "Quartz sandstone"@en .
subst:lithology-QU skos:definition "Quartzite"@en .
subst:lithology-QZ skos:definition "Quartz"@en .
subst:lithology-R skos:definition "Same as rock outcrop"@en .
subst:lithology-RB skos:definition "Red-brown hardpan"@en .
subst:lithology-RH skos:definition "Rhyolite"@en .
subst:lithology-S skos:definition "Sand"@en .
subst:lithology-SA skos:definition "Sandstone"@en .
subst:lithology-SD skos:definition "Detrital sedimentary rock"@en .
subst:lithology-SH skos:definition "Shale"@en .
subst:lithology-SK skos:definition "Scoria"@en .
subst:lithology-SL skos:definition "Slate"@en .
subst:lithology-SN skos:definition "Stones"@en .
subst:lithology-SR skos:definition "Serpentinite"@en .
subst:lithology-ST skos:definition "Schist"@en .
subst:lithology-SY skos:definition "Syenite"@en .
subst:lithology-TR skos:definition "Trachyte"@en .
subst:lithology-TU skos:definition "Tuff"@en .
subst:lithology-UC skos:definition "Unconsolidated material"@en .
subst:lithology-VB skos:definition "Volcanic breccia"@en .
subst:lithology-VG skos:definition "Volcanic glass"@en .
subst:lithology-Z skos:definition "Silt"@en .
subst:lithology-ZS skos:definition "Siltstone"@en .
subst:material-strength-M skos:definition "Moderately strong rock"@en .
subst:material-strength-S skos:definition "Strong rock"@en .
subst:material-strength-VS skos:definition "Very strong rock"@en .
subst:material-strength-VW skos:definition "Very weak rock"@en .
subst:material-strength-W skos:definition "Weak rock"@en .

ls:coarse-fragments-abundance-0 rdfs:isDefinedBy asls:soil-profile .
ls:coarse-fragments-abundance-0 skos:inScheme asls:soil-profile .
ls:coarse-fragments-abundance-1 rdfs:isDefinedBy asls:soil-profile .
ls:coarse-fragments-abundance-1 skos:inScheme asls:soil-profile .
ls:coarse-fragments-abundance-2 rdfs:isDefinedBy asls:soil-profile .
ls:coarse-fragments-abundance-2 skos:inScheme asls:soil-profile .
ls:coarse-fragments-abundance-3 rdfs:isDefinedBy asls:soil-profile .
ls:coarse-fragments-abundance-3 skos:inScheme asls:soil-profile .
ls:coarse-fragments-abundance-4 rdfs:isDefinedBy asls:soil-profile .
ls:coarse-fragments-abundance-4 skos:inScheme asls:soil-profile .
ls:coarse-fragments-abundance-5 rdfs:isDefinedBy asls:soil-profile .
ls:coarse-fragments-abundance-5 skos:inScheme asls:soil-profile .
ls:coarse-fragments-abundance-6 rdfs:isDefinedBy asls:soil-profile .
ls:coarse-fragments-abundance-6 skos:inScheme asls:soil-profile .
ls:coarse-fragments-shape-A rdfs:isDefinedBy asls:soil-profile .
ls:coarse-fragments-shape-A skos:inScheme asls:soil-profile .
ls:coarse-fragments-shape-AP rdfs:isDefinedBy asls:soil-profile .
ls:coarse-fragments-shape-AP skos:inScheme asls:soil-profile .
ls:coarse-fragments-shape-AT rdfs:isDefinedBy asls:soil-profile .
ls:coarse-fragments-shape-AT skos:inScheme asls:soil-profile .
ls:coarse-fragments-shape-R rdfs:isDefinedBy asls:soil-profile .
ls:coarse-fragments-shape-R skos:inScheme asls:soil-profile .
ls:coarse-fragments-shape-RP rdfs:isDefinedBy asls:soil-profile .
ls:coarse-fragments-shape-RP skos:inScheme asls:soil-profile .
ls:coarse-fragments-shape-RT rdfs:isDefinedBy asls:soil-profile .
ls:coarse-fragments-shape-RT skos:inScheme asls:soil-profile .
ls:coarse-fragments-shape-S rdfs:isDefinedBy asls:soil-profile .
ls:coarse-fragments-shape-S skos:inScheme asls:soil-profile .
ls:coarse-fragments-shape-SP rdfs:isDefinedBy asls:soil-profile .
ls:coarse-fragments-shape-SP skos:inScheme asls:soil-profile .
ls:coarse-fragments-shape-ST rdfs:isDefinedBy asls:soil-profile .
ls:coarse-fragments-shape-ST skos:inScheme asls:soil-profile .
ls:coarse-fragments-shape-U rdfs:isDefinedBy asls:soil-profile .
ls:coarse-fragments-shape-U skos:inScheme asls:soil-profile .
ls:coarse-fragments-shape-UP rdfs:isDefinedBy asls:soil-profile .
ls:coarse-fragments-shape-UP skos:inScheme asls:soil-profile .
ls:coarse-fragments-shape-UT rdfs:isDefinedBy asls:soil-profile .
ls:coarse-fragments-shape-UT skos:inScheme asls:soil-profile .
ls:coarse-fragments-size-1 rdfs:isDefinedBy asls:soil-profile .
ls:coarse-fragments-size-1 skos:inScheme asls:soil-profile .
ls:coarse-fragments-size-2 rdfs:isDefinedBy asls:soil-profile .
ls:coarse-fragments-size-2 skos:inScheme asls:soil-profile .
ls:coarse-fragments-size-3 rdfs:isDefinedBy asls:soil-profile .
ls:coarse-fragments-size-3 skos:inScheme asls:soil-profile .
ls:coarse-fragments-size-4 rdfs:isDefinedBy asls:soil-profile .
ls:coarse-fragments-size-4 skos:inScheme asls:soil-profile .
ls:coarse-fragments-size-5 rdfs:isDefinedBy asls:soil-profile .
ls:coarse-fragments-size-5 skos:inScheme asls:soil-profile .
ls:coarse-fragments-size-6 rdfs:isDefinedBy asls:soil-profile .
ls:coarse-fragments-size-6 skos:inScheme asls:soil-profile .
ls:coarse-fragments-size-7 rdfs:isDefinedBy asls:soil-profile .
ls:coarse-fragments-size-7 skos:inScheme asls:soil-profile .
ls:lithology-CC rdfs:isDefinedBy asls:soil-profile .
ls:lithology-CC skos:inScheme asls:soil-profile .
ls:lithology-IS rdfs:isDefinedBy asls:soil-profile .
ls:lithology-IS skos:inScheme asls:soil-profile .
ls:lithology-M rdfs:isDefinedBy asls:soil-profile .
ls:lithology-M skos:inScheme asls:soil-profile .
ls:lithology-OT rdfs:isDefinedBy asls:soil-profile .
ls:lithology-OT skos:inScheme asls:soil-profile .
ls:lithology-OW rdfs:isDefinedBy asls:soil-profile .
ls:lithology-OW skos:inScheme asls:soil-profile .
ls:lithology-PU rdfs:isDefinedBy asls:soil-profile .
ls:lithology-PU skos:inScheme asls:soil-profile .
ls:lithology-R rdfs:isDefinedBy asls:soil-profile .
ls:lithology-R skos:inScheme asls:soil-profile .
ls:lithology-SS rdfs:isDefinedBy asls:soil-profile .
ls:lithology-SS skos:inScheme asls:soil-profile .
sp:coarse-fragments-distribution-D rdfs:isDefinedBy asls:soil-profile .
sp:coarse-fragments-distribution-D skos:inScheme asls:soil-profile .
sp:coarse-fragments-distribution-R rdfs:isDefinedBy asls:soil-profile .
sp:coarse-fragments-distribution-R skos:inScheme asls:soil-profile .
sp:coarse-fragments-distribution-S rdfs:isDefinedBy asls:soil-profile .
sp:coarse-fragments-distribution-S skos:inScheme asls:soil-profile .
sp:coarse-fragments-distribution-U rdfs:isDefinedBy asls:soil-profile .
sp:coarse-fragments-distribution-U skos:inScheme asls:soil-profile .
sp:colour-stat-D rdfs:isDefinedBy asls:soil-profile .
sp:colour-stat-D skos:inScheme asls:soil-profile .
sp:colour-stat-M rdfs:isDefinedBy asls:soil-profile .
sp:colour-stat-M skos:inScheme asls:soil-profile .
sp:colour-value rdfs:isDefinedBy asls:soil-profile .
sp:colour-value skos:inScheme asls:soil-profile .
sp:consistence-plasticity-degree-0 rdfs:isDefinedBy asls:soil-profile .
sp:consistence-plasticity-degree-0 skos:inScheme asls:soil-profile .
sp:consistence-plasticity-degree-1 rdfs:isDefinedBy asls:soil-profile .
sp:consistence-plasticity-degree-1 skos:inScheme asls:soil-profile .
sp:consistence-plasticity-degree-2 rdfs:isDefinedBy asls:soil-profile .
sp:consistence-plasticity-degree-2 skos:inScheme asls:soil-profile .
sp:consistence-plasticity-degree-3 rdfs:isDefinedBy asls:soil-profile .
sp:consistence-plasticity-degree-3 skos:inScheme asls:soil-profile .
sp:consistence-plasticity-type-N rdfs:isDefinedBy asls:soil-profile .
sp:consistence-plasticity-type-N skos:inScheme asls:soil-profile .
sp:consistence-plasticity-type-S rdfs:isDefinedBy asls:soil-profile .
sp:consistence-plasticity-type-S skos:inScheme asls:soil-profile .
sp:consistence-plasticity-type-T rdfs:isDefinedBy asls:soil-profile .
sp:consistence-plasticity-type-T skos:inScheme asls:soil-profile .
sp:consistence-plasticity-type-U rdfs:isDefinedBy asls:soil-profile .
sp:consistence-plasticity-type-U skos:inScheme asls:soil-profile .
sp:consistence-stickiness-0 rdfs:isDefinedBy asls:soil-profile .
sp:consistence-stickiness-0 skos:inScheme asls:soil-profile .
sp:consistence-stickiness-1 rdfs:isDefinedBy asls:soil-profile .
sp:consistence-stickiness-1 skos:inScheme asls:soil-profile .
sp:consistence-stickiness-2 rdfs:isDefinedBy asls:soil-profile .
sp:consistence-stickiness-2 skos:inScheme asls:soil-profile .
sp:consistence-stickiness-3 rdfs:isDefinedBy asls:soil-profile .
sp:consistence-stickiness-3 skos:inScheme asls:soil-profile .
sp:consistence-strength-0 rdfs:isDefinedBy asls:soil-profile .
sp:consistence-strength-0 skos:inScheme asls:soil-profile .
sp:consistence-strength-1 rdfs:isDefinedBy asls:soil-profile .
sp:consistence-strength-1 skos:inScheme asls:soil-profile .
sp:consistence-strength-2 rdfs:isDefinedBy asls:soil-profile .
sp:consistence-strength-2 skos:inScheme asls:soil-profile .
sp:consistence-strength-3 rdfs:isDefinedBy asls:soil-profile .
sp:consistence-strength-3 skos:inScheme asls:soil-profile .
sp:consistence-strength-4 rdfs:isDefinedBy asls:soil-profile .
sp:consistence-strength-4 skos:inScheme asls:soil-profile .
sp:consistence-strength-5 rdfs:isDefinedBy asls:soil-profile .
sp:consistence-strength-5 skos:inScheme asls:soil-profile .
sp:consistence-strength-6 rdfs:isDefinedBy asls:soil-profile .
sp:consistence-strength-6 skos:inScheme asls:soil-profile .
sp:consistence-strength-7 rdfs:isDefinedBy asls:soil-profile .
sp:consistence-strength-7 skos:inScheme asls:soil-profile .
sp:cutans-abundance-0 rdfs:isDefinedBy asls:soil-profile .
sp:cutans-abundance-0 skos:inScheme asls:soil-profile .
sp:cutans-abundance-1 rdfs:isDefinedBy asls:soil-profile .
sp:cutans-abundance-1 skos:inScheme asls:soil-profile .
sp:cutans-abundance-2 rdfs:isDefinedBy asls:soil-profile .
sp:cutans-abundance-2 skos:inScheme asls:soil-profile .
sp:cutans-abundance-3 rdfs:isDefinedBy asls:soil-profile .
sp:cutans-abundance-3 skos:inScheme asls:soil-profile .
sp:cutans-distinctness-D rdfs:isDefinedBy asls:soil-profile .
sp:cutans-distinctness-D skos:inScheme asls:soil-profile .
sp:cutans-distinctness-F rdfs:isDefinedBy asls:soil-profile .
sp:cutans-distinctness-F skos:inScheme asls:soil-profile .
sp:cutans-distinctness-P rdfs:isDefinedBy asls:soil-profile .
sp:cutans-distinctness-P skos:inScheme asls:soil-profile .
sp:cutans-type-C rdfs:isDefinedBy asls:soil-profile .
sp:cutans-type-C skos:inScheme asls:soil-profile .
sp:cutans-type-K rdfs:isDefinedBy asls:soil-profile .
sp:cutans-type-K skos:inScheme asls:soil-profile .
sp:cutans-type-M rdfs:isDefinedBy asls:soil-profile .
sp:cutans-type-M skos:inScheme asls:soil-profile .
sp:cutans-type-O rdfs:isDefinedBy asls:soil-profile .
sp:cutans-type-O skos:inScheme asls:soil-profile .
sp:cutans-type-S rdfs:isDefinedBy asls:soil-profile .
sp:cutans-type-S skos:inScheme asls:soil-profile .
sp:cutans-type-U rdfs:isDefinedBy asls:soil-profile .
sp:cutans-type-U skos:inScheme asls:soil-profile .
sp:cutans-type-Z rdfs:isDefinedBy asls:soil-profile .
sp:cutans-type-Z skos:inScheme asls:soil-profile .
sp:depth-of-horizon rdfs:isDefinedBy asls:soil-profile .
sp:depth-of-horizon skos:inScheme asls:soil-profile .
sp:depth-of-horizon-lower rdfs:isDefinedBy asls:soil-profile .
sp:depth-of-horizon-lower skos:inScheme asls:soil-profile .
sp:depth-of-horizon-upper rdfs:isDefinedBy asls:soil-profile .
sp:depth-of-horizon-upper skos:inScheme asls:soil-profile .
sp:depth-to-r-horizon rdfs:isDefinedBy asls:soil-profile .
sp:depth-to-r-horizon skos:inScheme asls:soil-profile .
sp:effervescence-H rdfs:isDefinedBy asls:soil-profile .
sp:effervescence-H skos:inScheme asls:soil-profile .
sp:effervescence-M rdfs:isDefinedBy asls:soil-profile .
sp:effervescence-M skos:inScheme asls:soil-profile .
sp:effervescence-N rdfs:isDefinedBy asls:soil-profile .
sp:effervescence-N skos:inScheme asls:soil-profile .
sp:effervescence-S rdfs:isDefinedBy asls:soil-profile .
sp:effervescence-S skos:inScheme asls:soil-profile .
sp:effervescence-V rdfs:isDefinedBy asls:soil-profile .
sp:effervescence-V skos:inScheme asls:soil-profile .
sp:fabric-E rdfs:isDefinedBy asls:soil-profile .
sp:fabric-E skos:inScheme asls:soil-profile .
sp:fabric-G rdfs:isDefinedBy asls:soil-profile .
sp:fabric-G skos:inScheme asls:soil-profile .
sp:fabric-R rdfs:isDefinedBy asls:soil-profile .
sp:fabric-R skos:inScheme asls:soil-profile .
sp:fabric-S rdfs:isDefinedBy asls:soil-profile .
sp:fabric-S skos:inScheme asls:soil-profile .
sp:field-ph rdfs:isDefinedBy asls:soil-profile .
sp:field-ph skos:inScheme asls:soil-profile .
sp:field-texture-AP rdfs:isDefinedBy asls:soil-profile .
sp:field-texture-AP skos:inScheme asls:soil-profile .
sp:field-texture-C rdfs:isDefinedBy asls:soil-profile .
sp:field-texture-C skos:inScheme asls:soil-profile .
sp:field-texture-CFS rdfs:isDefinedBy asls:soil-profile .
sp:field-texture-CFS skos:inScheme asls:soil-profile .
sp:field-texture-CFS-heavy rdfs:isDefinedBy asls:soil-profile .
sp:field-texture-CFS-heavy skos:inScheme asls:soil-profile .
sp:field-texture-CFS-light rdfs:isDefinedBy asls:soil-profile .
sp:field-texture-CFS-light skos:inScheme asls:soil-profile .
sp:field-texture-CKS rdfs:isDefinedBy asls:soil-profile .
sp:field-texture-CKS skos:inScheme asls:soil-profile .
sp:field-texture-CKS-heavy rdfs:isDefinedBy asls:soil-profile .
sp:field-texture-CKS-heavy skos:inScheme asls:soil-profile .
sp:field-texture-CKS-light rdfs:isDefinedBy asls:soil-profile .
sp:field-texture-CKS-light skos:inScheme asls:soil-profile .
sp:field-texture-CL rdfs:isDefinedBy asls:soil-profile .
sp:field-texture-CL skos:inScheme asls:soil-profile .
sp:field-texture-CL-A rdfs:isDefinedBy asls:soil-profile .
sp:field-texture-CL-A skos:inScheme asls:soil-profile .
sp:field-texture-CL-I rdfs:isDefinedBy asls:soil-profile .
sp:field-texture-CL-I skos:inScheme asls:soil-profile .
sp:field-texture-CL-heavy rdfs:isDefinedBy asls:soil-profile .
sp:field-texture-CL-heavy skos:inScheme asls:soil-profile .
sp:field-texture-CL-light rdfs:isDefinedBy asls:soil-profile .
sp:field-texture-CL-light skos:inScheme asls:soil-profile .
sp:field-texture-CLFS rdfs:isDefinedBy asls:soil-profile .
sp:field-texture-CLFS skos:inScheme asls:soil-profile .
sp:field-texture-CLFS-A rdfs:isDefinedBy asls:soil-profile .
sp:field-texture-CLFS-A skos:inScheme asls:soil-profile .
sp:field-texture-CLFS-I rdfs:isDefinedBy asls:soil-profile .
sp:field-texture-CLFS-I skos:inScheme asls:soil-profile .
sp:field-texture-CLFS-heavy rdfs:isDefinedBy asls:soil-profile .
sp:field-texture-CLFS-heavy skos:inScheme asls:soil-profile .
sp:field-texture-CLFS-light rdfs:isDefinedBy asls:soil-profile .
sp:field-texture-CLFS-light skos:inScheme asls:soil-profile .
sp:field-texture-CLKS rdfs:isDefinedBy asls:soil-profile .
sp:field-texture-CLKS skos:inScheme asls:soil-profile .
sp:field-texture-CLKS-A rdfs:isDefinedBy asls:soil-profile .
sp:field-texture-CLKS-A skos:inScheme asls:soil-profile .
sp:field-texture-CLKS-I rdfs:isDefinedBy asls:soil-profile .
sp:field-texture-CLKS-I skos:inScheme asls:soil-profile .
sp:field-texture-CLKS-heavy rdfs:isDefinedBy asls:soil-profile .
sp:field-texture-CLKS-heavy skos:inScheme asls:soil-profile .
sp:field-texture-CLKS-light rdfs:isDefinedBy asls:soil-profile .
sp:field-texture-CLKS-light skos:inScheme asls:soil-profile .
sp:field-texture-CLS rdfs:isDefinedBy asls:soil-profile .
sp:field-texture-CLS skos:inScheme asls:soil-profile .
sp:field-texture-CLS-A rdfs:isDefinedBy asls:soil-profile .
sp:field-texture-CLS-A skos:inScheme asls:soil-profile .
sp:field-texture-CLS-I rdfs:isDefinedBy asls:soil-profile .
sp:field-texture-CLS-I skos:inScheme asls:soil-profile .
sp:field-texture-CLS-heavy rdfs:isDefinedBy asls:soil-profile .
sp:field-texture-CLS-heavy skos:inScheme asls:soil-profile .
sp:field-texture-CLS-light rdfs:isDefinedBy asls:soil-profile .
sp:field-texture-CLS-light skos:inScheme asls:soil-profile .
sp:field-texture-CP rdfs:isDefinedBy asls:soil-profile .
sp:field-texture-CP skos:inScheme asls:soil-profile .
sp:field-texture-CS rdfs:isDefinedBy asls:soil-profile .
sp:field-texture-CS skos:inScheme asls:soil-profile .
sp:field-texture-CS-heavy rdfs:isDefinedBy asls:soil-profile .
sp:field-texture-CS-heavy skos:inScheme asls:soil-profile .
sp:field-texture-CS-light rdfs:isDefinedBy asls:soil-profile .
sp:field-texture-CS-light skos:inScheme asls:soil-profile .
sp:field-texture-FS rdfs:isDefinedBy asls:soil-profile .
sp:field-texture-FS skos:inScheme asls:soil-profile .
sp:field-texture-FS-A rdfs:isDefinedBy asls:soil-profile .
sp:field-texture-FS-A skos:inScheme asls:soil-profile .
sp:field-texture-FS-I rdfs:isDefinedBy asls:soil-profile .
sp:field-texture-FS-I skos:inScheme asls:soil-profile .
sp:field-texture-FSCL rdfs:isDefinedBy asls:soil-profile .
sp:field-texture-FSCL skos:inScheme asls:soil-profile .
sp:field-texture-FSCL-A rdfs:isDefinedBy asls:soil-profile .
sp:field-texture-FSCL-A skos:inScheme asls:soil-profile .
sp:field-texture-FSCL-I rdfs:isDefinedBy asls:soil-profile .
sp:field-texture-FSCL-I skos:inScheme asls:soil-profile .
sp:field-texture-FSCL-heavy rdfs:isDefinedBy asls:soil-profile .
sp:field-texture-FSCL-heavy skos:inScheme asls:soil-profile .
sp:field-texture-FSCL-light rdfs:isDefinedBy asls:soil-profile .
sp:field-texture-FSCL-light skos:inScheme asls:soil-profile .
sp:field-texture-FSHC rdfs:isDefinedBy asls:soil-profile .
sp:field-texture-FSHC skos:inScheme asls:soil-profile .
sp:field-texture-FSHC-A rdfs:isDefinedBy asls:soil-profile .
sp:field-texture-FSHC-A skos:inScheme asls:soil-profile .
sp:field-texture-FSHC-I rdfs:isDefinedBy asls:soil-profile .
sp:field-texture-FSHC-I skos:inScheme asls:soil-profile .
sp:field-texture-FSL rdfs:isDefinedBy asls:soil-profile .
sp:field-texture-FSL skos:inScheme asls:soil-profile .
sp:field-texture-FSL-A rdfs:isDefinedBy asls:soil-profile .
sp:field-texture-FSL-A skos:inScheme asls:soil-profile .
sp:field-texture-FSL-I rdfs:isDefinedBy asls:soil-profile .
sp:field-texture-FSL-I skos:inScheme asls:soil-profile .
sp:field-texture-FSLC rdfs:isDefinedBy asls:soil-profile .
sp:field-texture-FSLC skos:inScheme asls:soil-profile .
sp:field-texture-FSLC-A rdfs:isDefinedBy asls:soil-profile .
sp:field-texture-FSLC-A skos:inScheme asls:soil-profile .
sp:field-texture-FSLC-I rdfs:isDefinedBy asls:soil-profile .
sp:field-texture-FSLC-I skos:inScheme asls:soil-profile .
sp:field-texture-FSLMC rdfs:isDefinedBy asls:soil-profile .
sp:field-texture-FSLMC skos:inScheme asls:soil-profile .
sp:field-texture-FSLMC-A rdfs:isDefinedBy asls:soil-profile .
sp:field-texture-FSLMC-A skos:inScheme asls:soil-profile .
sp:field-texture-FSLMC-I rdfs:isDefinedBy asls:soil-profile .
sp:field-texture-FSLMC-I skos:inScheme asls:soil-profile .
sp:field-texture-FSMC rdfs:isDefinedBy asls:soil-profile .
sp:field-texture-FSMC skos:inScheme asls:soil-profile .
sp:field-texture-FSMC-A rdfs:isDefinedBy asls:soil-profile .
sp:field-texture-FSMC-A skos:inScheme asls:soil-profile .
sp:field-texture-FSMC-I rdfs:isDefinedBy asls:soil-profile .
sp:field-texture-FSMC-I skos:inScheme asls:soil-profile .
sp:field-texture-FSMHC rdfs:isDefinedBy asls:soil-profile .
sp:field-texture-FSMHC skos:inScheme asls:soil-profile .
sp:field-texture-FSMHC-A rdfs:isDefinedBy asls:soil-profile .
sp:field-texture-FSMHC-A skos:inScheme asls:soil-profile .
sp:field-texture-FSMHC-I rdfs:isDefinedBy asls:soil-profile .
sp:field-texture-FSMHC-I skos:inScheme asls:soil-profile .
sp:field-texture-GP rdfs:isDefinedBy asls:soil-profile .
sp:field-texture-GP skos:inScheme asls:soil-profile .
sp:field-texture-HC rdfs:isDefinedBy asls:soil-profile .
sp:field-texture-HC skos:inScheme asls:soil-profile .
sp:field-texture-HC-A rdfs:isDefinedBy asls:soil-profile .
sp:field-texture-HC-A skos:inScheme asls:soil-profile .
sp:field-texture-HC-I rdfs:isDefinedBy asls:soil-profile .
sp:field-texture-HC-I skos:inScheme asls:soil-profile .
sp:field-texture-HP rdfs:isDefinedBy asls:soil-profile .
sp:field-texture-HP skos:inScheme asls:soil-profile .
sp:field-texture-IP rdfs:isDefinedBy asls:soil-profile .
sp:field-texture-IP skos:inScheme asls:soil-profile .
sp:field-texture-KS rdfs:isDefinedBy asls:soil-profile .
sp:field-texture-KS skos:inScheme asls:soil-profile .
sp:field-texture-KS-A rdfs:isDefinedBy asls:soil-profile .
sp:field-texture-KS-A skos:inScheme asls:soil-profile .
sp:field-texture-KS-I rdfs:isDefinedBy asls:soil-profile .
sp:field-texture-KS-I skos:inScheme asls:soil-profile .
sp:field-texture-KSCL rdfs:isDefinedBy asls:soil-profile .
sp:field-texture-KSCL skos:inScheme asls:soil-profile .
sp:field-texture-KSCL-A rdfs:isDefinedBy asls:soil-profile .
sp:field-texture-KSCL-A skos:inScheme asls:soil-profile .
sp:field-texture-KSCL-I rdfs:isDefinedBy asls:soil-profile .
sp:field-texture-KSCL-I skos:inScheme asls:soil-profile .
sp:field-texture-KSCL-heavy rdfs:isDefinedBy asls:soil-profile .
sp:field-texture-KSCL-heavy skos:inScheme asls:soil-profile .
sp:field-texture-KSCL-light rdfs:isDefinedBy asls:soil-profile .
sp:field-texture-KSCL-light skos:inScheme asls:soil-profile .
sp:field-texture-KSHC rdfs:isDefinedBy asls:soil-profile .
sp:field-texture-KSHC skos:inScheme asls:soil-profile .
sp:field-texture-KSHC-A rdfs:isDefinedBy asls:soil-profile .
sp:field-texture-KSHC-A skos:inScheme asls:soil-profile .
sp:field-texture-KSHC-I rdfs:isDefinedBy asls:soil-profile .
sp:field-texture-KSHC-I skos:inScheme asls:soil-profile .
sp:field-texture-KSL rdfs:isDefinedBy asls:soil-profile .
sp:field-texture-KSL skos:inScheme asls:soil-profile .
sp:field-texture-KSL-A rdfs:isDefinedBy asls:soil-profile .
sp:field-texture-KSL-A skos:inScheme asls:soil-profile .
sp:field-texture-KSL-I rdfs:isDefinedBy asls:soil-profile .
sp:field-texture-KSL-I skos:inScheme asls:soil-profile .
sp:field-texture-KSLC rdfs:isDefinedBy asls:soil-profile .
sp:field-texture-KSLC skos:inScheme asls:soil-profile .
sp:field-texture-KSLC-A rdfs:isDefinedBy asls:soil-profile .
sp:field-texture-KSLC-A skos:inScheme asls:soil-profile .
sp:field-texture-KSLC-I rdfs:isDefinedBy asls:soil-profile .
sp:field-texture-KSLC-I skos:inScheme asls:soil-profile .
sp:field-texture-KSLMC rdfs:isDefinedBy asls:soil-profile .
sp:field-texture-KSLMC skos:inScheme asls:soil-profile .
sp:field-texture-KSLMC-A rdfs:isDefinedBy asls:soil-profile .
sp:field-texture-KSLMC-A skos:inScheme asls:soil-profile .
sp:field-texture-KSLMC-I rdfs:isDefinedBy asls:soil-profile .
sp:field-texture-KSLMC-I skos:inScheme asls:soil-profile .
sp:field-texture-KSMC rdfs:isDefinedBy asls:soil-profile .
sp:field-texture-KSMC skos:inScheme asls:soil-profile .
sp:field-texture-KSMC-A rdfs:isDefinedBy asls:soil-profile .
sp:field-texture-KSMC-A skos:inScheme asls:soil-profile .
sp:field-texture-KSMC-I rdfs:isDefinedBy asls:soil-profile .
sp:field-texture-KSMC-I skos:inScheme asls:soil-profile .
sp:field-texture-KSMHC rdfs:isDefinedBy asls:soil-profile .
sp:field-texture-KSMHC skos:inScheme asls:soil-profile .
sp:field-texture-KSMHC-A rdfs:isDefinedBy asls:soil-profile .
sp:field-texture-KSMHC-A skos:inScheme asls:soil-profile .
sp:field-texture-KSMHC-I rdfs:isDefinedBy asls:soil-profile .
sp:field-texture-KSMHC-I skos:inScheme asls:soil-profile .
sp:field-texture-L rdfs:isDefinedBy asls:soil-profile .
sp:field-texture-L skos:inScheme asls:soil-profile .
sp:field-texture-L-A rdfs:isDefinedBy asls:soil-profile .
sp:field-texture-L-A skos:inScheme asls:soil-profile .
sp:field-texture-L-I rdfs:isDefinedBy asls:soil-profile .
sp:field-texture-L-I skos:inScheme asls:soil-profile .
sp:field-texture-LC rdfs:isDefinedBy asls:soil-profile .
sp:field-texture-LC skos:inScheme asls:soil-profile .
sp:field-texture-LC-A rdfs:isDefinedBy asls:soil-profile .
sp:field-texture-LC-A skos:inScheme asls:soil-profile .
sp:field-texture-LC-I rdfs:isDefinedBy asls:soil-profile .
sp:field-texture-LC-I skos:inScheme asls:soil-profile .
sp:field-texture-LFS rdfs:isDefinedBy asls:soil-profile .
sp:field-texture-LFS skos:inScheme asls:soil-profile .
sp:field-texture-LFS-A rdfs:isDefinedBy asls:soil-profile .
sp:field-texture-LFS-A skos:inScheme asls:soil-profile .
sp:field-texture-LFS-I rdfs:isDefinedBy asls:soil-profile .
sp:field-texture-LFS-I skos:inScheme asls:soil-profile .
sp:field-texture-LKS rdfs:isDefinedBy asls:soil-profile .
sp:field-texture-LKS skos:inScheme asls:soil-profile .
sp:field-texture-LKS-A rdfs:isDefinedBy asls:soil-profile .
sp:field-texture-LKS-A skos:inScheme asls:soil-profile .
sp:field-texture-LKS-I rdfs:isDefinedBy asls:soil-profile .
sp:field-texture-LKS-I skos:inScheme asls:soil-profile .
sp:field-texture-LMC rdfs:isDefinedBy asls:soil-profile .
sp:field-texture-LMC skos:inScheme asls:soil-profile .
sp:field-texture-LMC-A rdfs:isDefinedBy asls:soil-profile .
sp:field-texture-LMC-A skos:inScheme asls:soil-profile .
sp:field-texture-LMC-I rdfs:isDefinedBy asls:soil-profile .
sp:field-texture-LMC-I skos:inScheme asls:soil-profile .
sp:field-texture-LP rdfs:isDefinedBy asls:soil-profile .
sp:field-texture-LP skos:inScheme asls:soil-profile .
sp:field-texture-LS rdfs:isDefinedBy asls:soil-profile .
sp:field-texture-LS skos:inScheme asls:soil-profile .
sp:field-texture-LS-A rdfs:isDefinedBy asls:soil-profile .
sp:field-texture-LS-A skos:inScheme asls:soil-profile .
sp:field-texture-LS-I rdfs:isDefinedBy asls:soil-profile .
sp:field-texture-LS-I skos:inScheme asls:soil-profile .
sp:field-texture-MC rdfs:isDefinedBy asls:soil-profile .
sp:field-texture-MC skos:inScheme asls:soil-profile .
sp:field-texture-MC-A rdfs:isDefinedBy asls:soil-profile .
sp:field-texture-MC-A skos:inScheme asls:soil-profile .
sp:field-texture-MC-I rdfs:isDefinedBy asls:soil-profile .
sp:field-texture-MC-I skos:inScheme asls:soil-profile .
sp:field-texture-MHC rdfs:isDefinedBy asls:soil-profile .
sp:field-texture-MHC skos:inScheme asls:soil-profile .
sp:field-texture-MHC-A rdfs:isDefinedBy asls:soil-profile .
sp:field-texture-MHC-A skos:inScheme asls:soil-profile .
sp:field-texture-MHC-I rdfs:isDefinedBy asls:soil-profile .
sp:field-texture-MHC-I skos:inScheme asls:soil-profile .
sp:field-texture-S rdfs:isDefinedBy asls:soil-profile .
sp:field-texture-S skos:inScheme asls:soil-profile .
sp:field-texture-S-A rdfs:isDefinedBy asls:soil-profile .
sp:field-texture-S-A skos:inScheme asls:soil-profile .
sp:field-texture-S-I rdfs:isDefinedBy asls:soil-profile .
sp:field-texture-S-I skos:inScheme asls:soil-profile .
sp:field-texture-SCL rdfs:isDefinedBy asls:soil-profile .
sp:field-texture-SCL skos:inScheme asls:soil-profile .
sp:field-texture-SCL-A rdfs:isDefinedBy asls:soil-profile .
sp:field-texture-SCL-A skos:inScheme asls:soil-profile .
sp:field-texture-SCL-I rdfs:isDefinedBy asls:soil-profile .
sp:field-texture-SCL-I skos:inScheme asls:soil-profile .
sp:field-texture-SCL-heavy rdfs:isDefinedBy asls:soil-profile .
sp:field-texture-SCL-heavy skos:inScheme asls:soil-profile .
sp:field-texture-SCL-light rdfs:isDefinedBy asls:soil-profile .
sp:field-texture-SCL-light skos:inScheme asls:soil-profile .
sp:field-texture-SHC rdfs:isDefinedBy asls:soil-profile .
sp:field-texture-SHC skos:inScheme asls:soil-profile .
sp:field-texture-SHC-A rdfs:isDefinedBy asls:soil-profile .
sp:field-texture-SHC-A skos:inScheme asls:soil-profile .
sp:field-texture-SHC-I rdfs:isDefinedBy asls:soil-profile .
sp:field-texture-SHC-I skos:inScheme asls:soil-profile .
sp:field-texture-SL rdfs:isDefinedBy asls:soil-profile .
sp:field-texture-SL skos:inScheme asls:soil-profile .
sp:field-texture-SL-A rdfs:isDefinedBy asls:soil-profile .
sp:field-texture-SL-A skos:inScheme asls:soil-profile .
sp:field-texture-SL-I rdfs:isDefinedBy asls:soil-profile .
sp:field-texture-SL-I skos:inScheme asls:soil-profile .
sp:field-texture-SLC rdfs:isDefinedBy asls:soil-profile .
sp:field-texture-SLC skos:inScheme asls:soil-profile .
sp:field-texture-SLC-A rdfs:isDefinedBy asls:soil-profile .
sp:field-texture-SLC-A skos:inScheme asls:soil-profile .
sp:field-texture-SLC-I rdfs:isDefinedBy asls:soil-profile .
sp:field-texture-SLC-I skos:inScheme asls:soil-profile .
sp:field-texture-SLMC rdfs:isDefinedBy asls:soil-profile .
sp:field-texture-SLMC skos:inScheme asls:soil-profile .
sp:field-texture-SLMC-A rdfs:isDefinedBy asls:soil-profile .
sp:field-texture-SLMC-A skos:inScheme asls:soil-profile .
sp:field-texture-SLMC-I rdfs:isDefinedBy asls:soil-profile .
sp:field-texture-SLMC-I skos:inScheme asls:soil-profile .
sp:field-texture-SMC rdfs:isDefinedBy asls:soil-profile .
sp:field-texture-SMC skos:inScheme asls:soil-profile .
sp:field-texture-SMC-A rdfs:isDefinedBy asls:soil-profile .
sp:field-texture-SMC-A skos:inScheme asls:soil-profile .
sp:field-texture-SMC-I rdfs:isDefinedBy asls:soil-profile .
sp:field-texture-SMC-I skos:inScheme asls:soil-profile .
sp:field-texture-SMHC rdfs:isDefinedBy asls:soil-profile .
sp:field-texture-SMHC skos:inScheme asls:soil-profile .
sp:field-texture-SMHC-A rdfs:isDefinedBy asls:soil-profile .
sp:field-texture-SMHC-A skos:inScheme asls:soil-profile .
sp:field-texture-SMHC-I rdfs:isDefinedBy asls:soil-profile .
sp:field-texture-SMHC-I skos:inScheme asls:soil-profile .
sp:field-texture-SP rdfs:isDefinedBy asls:soil-profile .
sp:field-texture-SP skos:inScheme asls:soil-profile .
sp:field-texture-ZCL rdfs:isDefinedBy asls:soil-profile .
sp:field-texture-ZCL skos:inScheme asls:soil-profile .
sp:field-texture-ZCL-A rdfs:isDefinedBy asls:soil-profile .
sp:field-texture-ZCL-A skos:inScheme asls:soil-profile .
sp:field-texture-ZCL-I rdfs:isDefinedBy asls:soil-profile .
sp:field-texture-ZCL-I skos:inScheme asls:soil-profile .
sp:field-texture-ZCL-heavy rdfs:isDefinedBy asls:soil-profile .
sp:field-texture-ZCL-heavy skos:inScheme asls:soil-profile .
sp:field-texture-ZCL-light rdfs:isDefinedBy asls:soil-profile .
sp:field-texture-ZCL-light skos:inScheme asls:soil-profile .
sp:field-texture-ZHC rdfs:isDefinedBy asls:soil-profile .
sp:field-texture-ZHC skos:inScheme asls:soil-profile .
sp:field-texture-ZHC-A rdfs:isDefinedBy asls:soil-profile .
sp:field-texture-ZHC-A skos:inScheme asls:soil-profile .
sp:field-texture-ZHC-I rdfs:isDefinedBy asls:soil-profile .
sp:field-texture-ZHC-I skos:inScheme asls:soil-profile .
sp:field-texture-ZL rdfs:isDefinedBy asls:soil-profile .
sp:field-texture-ZL skos:inScheme asls:soil-profile .
sp:field-texture-ZL-A rdfs:isDefinedBy asls:soil-profile .
sp:field-texture-ZL-A skos:inScheme asls:soil-profile .
sp:field-texture-ZL-I rdfs:isDefinedBy asls:soil-profile .
sp:field-texture-ZL-I skos:inScheme asls:soil-profile .
sp:field-texture-ZLC rdfs:isDefinedBy asls:soil-profile .
sp:field-texture-ZLC skos:inScheme asls:soil-profile .
sp:field-texture-ZLC-A rdfs:isDefinedBy asls:soil-profile .
sp:field-texture-ZLC-A skos:inScheme asls:soil-profile .
sp:field-texture-ZLC-I rdfs:isDefinedBy asls:soil-profile .
sp:field-texture-ZLC-I skos:inScheme asls:soil-profile .
sp:field-texture-ZLMC rdfs:isDefinedBy asls:soil-profile .
sp:field-texture-ZLMC skos:inScheme asls:soil-profile .
sp:field-texture-ZLMC-A rdfs:isDefinedBy asls:soil-profile .
sp:field-texture-ZLMC-A skos:inScheme asls:soil-profile .
sp:field-texture-ZLMC-I rdfs:isDefinedBy asls:soil-profile .
sp:field-texture-ZLMC-I skos:inScheme asls:soil-profile .
sp:field-texture-ZMC rdfs:isDefinedBy asls:soil-profile .
sp:field-texture-ZMC skos:inScheme asls:soil-profile .
sp:field-texture-ZMC-A rdfs:isDefinedBy asls:soil-profile .
sp:field-texture-ZMC-A skos:inScheme asls:soil-profile .
sp:field-texture-ZMC-I rdfs:isDefinedBy asls:soil-profile .
sp:field-texture-ZMC-I skos:inScheme asls:soil-profile .
sp:field-texture-ZMHC rdfs:isDefinedBy asls:soil-profile .
sp:field-texture-ZMHC skos:inScheme asls:soil-profile .
sp:field-texture-ZMHC-A rdfs:isDefinedBy asls:soil-profile .
sp:field-texture-ZMHC-A skos:inScheme asls:soil-profile .
sp:field-texture-ZMHC-I rdfs:isDefinedBy asls:soil-profile .
sp:field-texture-ZMHC-I skos:inScheme asls:soil-profile .
sp:field-texture-qualifier-fibric rdfs:isDefinedBy asls:soil-profile .
sp:field-texture-qualifier-fibric skos:inScheme asls:soil-profile .
sp:field-texture-qualifier-heavy rdfs:isDefinedBy asls:soil-profile .
sp:field-texture-qualifier-heavy skos:inScheme asls:soil-profile .
sp:field-texture-qualifier-light rdfs:isDefinedBy asls:soil-profile .
sp:field-texture-qualifier-light skos:inScheme asls:soil-profile .
sp:field-texture-qualifier-sapric rdfs:isDefinedBy asls:soil-profile .
sp:field-texture-qualifier-sapric skos:inScheme asls:soil-profile .
sp:horizon-A1 rdfs:isDefinedBy asls:soil-profile .
sp:horizon-A1 skos:inScheme asls:soil-profile .
sp:horizon-A2 rdfs:isDefinedBy asls:soil-profile .
sp:horizon-A2 skos:inScheme asls:soil-profile .
sp:horizon-A3 rdfs:isDefinedBy asls:soil-profile .
sp:horizon-A3 skos:inScheme asls:soil-profile .
sp:horizon-B1 rdfs:isDefinedBy asls:soil-profile .
sp:horizon-B1 skos:inScheme asls:soil-profile .
sp:horizon-B2 rdfs:isDefinedBy asls:soil-profile .
sp:horizon-B2 skos:inScheme asls:soil-profile .
sp:horizon-B3 rdfs:isDefinedBy asls:soil-profile .
sp:horizon-B3 skos:inScheme asls:soil-profile .
sp:horizon-O1 rdfs:isDefinedBy asls:soil-profile .
sp:horizon-O1 skos:inScheme asls:soil-profile .
sp:horizon-O2 rdfs:isDefinedBy asls:soil-profile .
sp:horizon-O2 skos:inScheme asls:soil-profile .
sp:horizon-P1 rdfs:isDefinedBy asls:soil-profile .
sp:horizon-P1 skos:inScheme asls:soil-profile .
sp:horizon-P2 rdfs:isDefinedBy asls:soil-profile .
sp:horizon-P2 skos:inScheme asls:soil-profile .
sp:horizon-boundary-distinctness-A rdfs:isDefinedBy asls:soil-profile .
sp:horizon-boundary-distinctness-A skos:inScheme asls:soil-profile .
sp:horizon-boundary-distinctness-C rdfs:isDefinedBy asls:soil-profile .
sp:horizon-boundary-distinctness-C skos:inScheme asls:soil-profile .
sp:horizon-boundary-distinctness-D rdfs:isDefinedBy asls:soil-profile .
sp:horizon-boundary-distinctness-D skos:inScheme asls:soil-profile .
sp:horizon-boundary-distinctness-G rdfs:isDefinedBy asls:soil-profile .
sp:horizon-boundary-distinctness-G skos:inScheme asls:soil-profile .
sp:horizon-boundary-distinctness-S rdfs:isDefinedBy asls:soil-profile .
sp:horizon-boundary-distinctness-S skos:inScheme asls:soil-profile .
sp:horizon-boundary-shape-B rdfs:isDefinedBy asls:soil-profile .
sp:horizon-boundary-shape-B skos:inScheme asls:soil-profile .
sp:horizon-boundary-shape-I rdfs:isDefinedBy asls:soil-profile .
sp:horizon-boundary-shape-I skos:inScheme asls:soil-profile .
sp:horizon-boundary-shape-S rdfs:isDefinedBy asls:soil-profile .
sp:horizon-boundary-shape-S skos:inScheme asls:soil-profile .
sp:horizon-boundary-shape-T rdfs:isDefinedBy asls:soil-profile .
sp:horizon-boundary-shape-T skos:inScheme asls:soil-profile .
sp:horizon-boundary-shape-W rdfs:isDefinedBy asls:soil-profile .
sp:horizon-boundary-shape-W skos:inScheme asls:soil-profile .
sp:horizon-prefix rdfs:isDefinedBy asls:soil-profile .
sp:horizon-prefix skos:inScheme asls:soil-profile .
sp:horizon-suffix-b rdfs:isDefinedBy asls:soil-profile .
sp:horizon-suffix-b skos:inScheme asls:soil-profile .
sp:horizon-suffix-c rdfs:isDefinedBy asls:soil-profile .
sp:horizon-suffix-c skos:inScheme asls:soil-profile .
sp:horizon-suffix-d rdfs:isDefinedBy asls:soil-profile .
sp:horizon-suffix-d skos:inScheme asls:soil-profile .
sp:horizon-suffix-e rdfs:isDefinedBy asls:soil-profile .
sp:horizon-suffix-e skos:inScheme asls:soil-profile .
sp:horizon-suffix-f rdfs:isDefinedBy asls:soil-profile .
sp:horizon-suffix-f skos:inScheme asls:soil-profile .
sp:horizon-suffix-g rdfs:isDefinedBy asls:soil-profile .
sp:horizon-suffix-g skos:inScheme asls:soil-profile .
sp:horizon-suffix-h rdfs:isDefinedBy asls:soil-profile .
sp:horizon-suffix-h skos:inScheme asls:soil-profile .
sp:horizon-suffix-j rdfs:isDefinedBy asls:soil-profile .
sp:horizon-suffix-j skos:inScheme asls:soil-profile .
sp:horizon-suffix-k rdfs:isDefinedBy asls:soil-profile .
sp:horizon-suffix-k skos:inScheme asls:soil-profile .
sp:horizon-suffix-m rdfs:isDefinedBy asls:soil-profile .
sp:horizon-suffix-m skos:inScheme asls:soil-profile .
sp:horizon-suffix-p rdfs:isDefinedBy asls:soil-profile .
sp:horizon-suffix-p skos:inScheme asls:soil-profile .
sp:horizon-suffix-q rdfs:isDefinedBy asls:soil-profile .
sp:horizon-suffix-q skos:inScheme asls:soil-profile .
sp:horizon-suffix-r rdfs:isDefinedBy asls:soil-profile .
sp:horizon-suffix-r skos:inScheme asls:soil-profile .
sp:horizon-suffix-s rdfs:isDefinedBy asls:soil-profile .
sp:horizon-suffix-s skos:inScheme asls:soil-profile .
sp:horizon-suffix-t rdfs:isDefinedBy asls:soil-profile .
sp:horizon-suffix-t skos:inScheme asls:soil-profile .
sp:horizon-suffix-w rdfs:isDefinedBy asls:soil-profile .
sp:horizon-suffix-w skos:inScheme asls:soil-profile .
sp:horizon-suffix-x rdfs:isDefinedBy asls:soil-profile .
sp:horizon-suffix-x skos:inScheme asls:soil-profile .
sp:horizon-suffix-y rdfs:isDefinedBy asls:soil-profile .
sp:horizon-suffix-y skos:inScheme asls:soil-profile .
sp:horizon-suffix-z rdfs:isDefinedBy asls:soil-profile .
sp:horizon-suffix-z skos:inScheme asls:soil-profile .
sp:horizons-A rdfs:isDefinedBy asls:soil-profile .
sp:horizons-A skos:inScheme asls:soil-profile .
sp:horizons-B rdfs:isDefinedBy asls:soil-profile .
sp:horizons-B skos:inScheme asls:soil-profile .
sp:horizons-C rdfs:isDefinedBy asls:soil-profile .
sp:horizons-C skos:inScheme asls:soil-profile .
sp:horizons-D rdfs:isDefinedBy asls:soil-profile .
sp:horizons-D skos:inScheme asls:soil-profile .
sp:horizons-O rdfs:isDefinedBy asls:soil-profile .
sp:horizons-O skos:inScheme asls:soil-profile .
sp:horizons-P rdfs:isDefinedBy asls:soil-profile .
sp:horizons-P skos:inScheme asls:soil-profile .
sp:horizons-R rdfs:isDefinedBy asls:soil-profile .
sp:horizons-R skos:inScheme asls:soil-profile .
sp:horizons-bleached rdfs:isDefinedBy asls:soil-profile .
sp:horizons-bleached skos:inScheme asls:soil-profile .
sp:horizons-subdivision rdfs:isDefinedBy asls:soil-profile .
sp:horizons-subdivision skos:inScheme asls:soil-profile .
sp:horizons-transitional rdfs:isDefinedBy asls:soil-profile .
sp:horizons-transitional skos:inScheme asls:soil-profile .
sp:mottle-abundance-0 rdfs:isDefinedBy asls:soil-profile .
sp:mottle-abundance-0 skos:inScheme asls:soil-profile .
sp:mottle-abundance-1 rdfs:isDefinedBy asls:soil-profile .
sp:mottle-abundance-1 skos:inScheme asls:soil-profile .
sp:mottle-abundance-2 rdfs:isDefinedBy asls:soil-profile .
sp:mottle-abundance-2 skos:inScheme asls:soil-profile .
sp:mottle-abundance-3 rdfs:isDefinedBy asls:soil-profile .
sp:mottle-abundance-3 skos:inScheme asls:soil-profile .
sp:mottle-abundance-4 rdfs:isDefinedBy asls:soil-profile .
sp:mottle-abundance-4 skos:inScheme asls:soil-profile .
sp:mottle-boundary-C rdfs:isDefinedBy asls:soil-profile .
sp:mottle-boundary-C skos:inScheme asls:soil-profile .
sp:mottle-boundary-D rdfs:isDefinedBy asls:soil-profile .
sp:mottle-boundary-D skos:inScheme asls:soil-profile .
sp:mottle-boundary-S rdfs:isDefinedBy asls:soil-profile .
sp:mottle-boundary-S skos:inScheme asls:soil-profile .
sp:mottle-colour-B rdfs:isDefinedBy asls:soil-profile .
sp:mottle-colour-B skos:inScheme asls:soil-profile .
sp:mottle-colour-D rdfs:isDefinedBy asls:soil-profile .
sp:mottle-colour-D skos:inScheme asls:soil-profile .
sp:mottle-colour-G rdfs:isDefinedBy asls:soil-profile .
sp:mottle-colour-G skos:inScheme asls:soil-profile .
sp:mottle-colour-L rdfs:isDefinedBy asls:soil-profile .
sp:mottle-colour-L skos:inScheme asls:soil-profile .
sp:mottle-colour-O rdfs:isDefinedBy asls:soil-profile .
sp:mottle-colour-O skos:inScheme asls:soil-profile .
sp:mottle-colour-P rdfs:isDefinedBy asls:soil-profile .
sp:mottle-colour-P skos:inScheme asls:soil-profile .
sp:mottle-colour-R rdfs:isDefinedBy asls:soil-profile .
sp:mottle-colour-R skos:inScheme asls:soil-profile .
sp:mottle-colour-Y rdfs:isDefinedBy asls:soil-profile .
sp:mottle-colour-Y skos:inScheme asls:soil-profile .
sp:mottle-contrast-D rdfs:isDefinedBy asls:soil-profile .
sp:mottle-contrast-D skos:inScheme asls:soil-profile .
sp:mottle-contrast-F rdfs:isDefinedBy asls:soil-profile .
sp:mottle-contrast-F skos:inScheme asls:soil-profile .
sp:mottle-contrast-P rdfs:isDefinedBy asls:soil-profile .
sp:mottle-contrast-P skos:inScheme asls:soil-profile .
sp:mottle-size-1 rdfs:isDefinedBy asls:soil-profile .
sp:mottle-size-1 skos:inScheme asls:soil-profile .
sp:mottle-size-2 rdfs:isDefinedBy asls:soil-profile .
sp:mottle-size-2 skos:inScheme asls:soil-profile .
sp:mottle-size-3 rdfs:isDefinedBy asls:soil-profile .
sp:mottle-size-3 skos:inScheme asls:soil-profile .
sp:mottle-size-4 rdfs:isDefinedBy asls:soil-profile .
sp:mottle-size-4 skos:inScheme asls:soil-profile .
sp:mottle-type-M rdfs:isDefinedBy asls:soil-profile .
sp:mottle-type-M skos:inScheme asls:soil-profile .
sp:mottle-type-X rdfs:isDefinedBy asls:soil-profile .
sp:mottle-type-X skos:inScheme asls:soil-profile .
sp:mottle-type-Y rdfs:isDefinedBy asls:soil-profile .
sp:mottle-type-Y skos:inScheme asls:soil-profile .
sp:mottle-type-Z rdfs:isDefinedBy asls:soil-profile .
sp:mottle-type-Z skos:inScheme asls:soil-profile .
sp:observation-type-A rdfs:isDefinedBy asls:soil-profile .
sp:observation-type-A skos:inScheme asls:soil-profile .
sp:observation-type-C rdfs:isDefinedBy asls:soil-profile .
sp:observation-type-C skos:inScheme asls:soil-profile .
sp:observation-type-E rdfs:isDefinedBy asls:soil-profile .
sp:observation-type-E skos:inScheme asls:soil-profile .
sp:observation-type-P rdfs:isDefinedBy asls:soil-profile .
sp:observation-type-P skos:inScheme asls:soil-profile .
sp:pans-cementation-0 rdfs:isDefinedBy asls:soil-profile .
sp:pans-cementation-0 skos:inScheme asls:soil-profile .
sp:pans-cementation-1 rdfs:isDefinedBy asls:soil-profile .
sp:pans-cementation-1 skos:inScheme asls:soil-profile .
sp:pans-cementation-2 rdfs:isDefinedBy asls:soil-profile .
sp:pans-cementation-2 skos:inScheme asls:soil-profile .
sp:pans-cementation-3 rdfs:isDefinedBy asls:soil-profile .
sp:pans-cementation-3 skos:inScheme asls:soil-profile .
sp:pans-cementation-4 rdfs:isDefinedBy asls:soil-profile .
sp:pans-cementation-4 skos:inScheme asls:soil-profile .
sp:pans-continuity-B rdfs:isDefinedBy asls:soil-profile .
sp:pans-continuity-B skos:inScheme asls:soil-profile .
sp:pans-continuity-C rdfs:isDefinedBy asls:soil-profile .
sp:pans-continuity-C skos:inScheme asls:soil-profile .
sp:pans-continuity-D rdfs:isDefinedBy asls:soil-profile .
sp:pans-continuity-D skos:inScheme asls:soil-profile .
sp:pans-structure-C rdfs:isDefinedBy asls:soil-profile .
sp:pans-structure-C skos:inScheme asls:soil-profile .
sp:pans-structure-L rdfs:isDefinedBy asls:soil-profile .
sp:pans-structure-L skos:inScheme asls:soil-profile .
sp:pans-structure-N rdfs:isDefinedBy asls:soil-profile .
sp:pans-structure-N skos:inScheme asls:soil-profile .
sp:pans-structure-R rdfs:isDefinedBy asls:soil-profile .
sp:pans-structure-R skos:inScheme asls:soil-profile .
sp:pans-structure-S rdfs:isDefinedBy asls:soil-profile .
sp:pans-structure-S skos:inScheme asls:soil-profile .
sp:pans-structure-V rdfs:isDefinedBy asls:soil-profile .
sp:pans-structure-V skos:inScheme asls:soil-profile .
sp:pans-type-A rdfs:isDefinedBy asls:soil-profile .
sp:pans-type-A skos:inScheme asls:soil-profile .
sp:pans-type-C rdfs:isDefinedBy asls:soil-profile .
sp:pans-type-C skos:inScheme asls:soil-profile .
sp:pans-type-D rdfs:isDefinedBy asls:soil-profile .
sp:pans-type-D skos:inScheme asls:soil-profile .
sp:pans-type-E rdfs:isDefinedBy asls:soil-profile .
sp:pans-type-E skos:inScheme asls:soil-profile .
sp:pans-type-F rdfs:isDefinedBy asls:soil-profile .
sp:pans-type-F skos:inScheme asls:soil-profile .
sp:pans-type-I rdfs:isDefinedBy asls:soil-profile .
sp:pans-type-I skos:inScheme asls:soil-profile .
sp:pans-type-K rdfs:isDefinedBy asls:soil-profile .
sp:pans-type-K skos:inScheme asls:soil-profile .
sp:pans-type-L rdfs:isDefinedBy asls:soil-profile .
sp:pans-type-L skos:inScheme asls:soil-profile .
sp:pans-type-M rdfs:isDefinedBy asls:soil-profile .
sp:pans-type-M skos:inScheme asls:soil-profile .
sp:pans-type-N rdfs:isDefinedBy asls:soil-profile .
sp:pans-type-N skos:inScheme asls:soil-profile .
sp:pans-type-O rdfs:isDefinedBy asls:soil-profile .
sp:pans-type-O skos:inScheme asls:soil-profile .
sp:pans-type-R rdfs:isDefinedBy asls:soil-profile .
sp:pans-type-R skos:inScheme asls:soil-profile .
sp:pans-type-T rdfs:isDefinedBy asls:soil-profile .
sp:pans-type-T skos:inScheme asls:soil-profile .
sp:pans-type-V rdfs:isDefinedBy asls:soil-profile .
sp:pans-type-V skos:inScheme asls:soil-profile .
sp:pans-type-Z rdfs:isDefinedBy asls:soil-profile .
sp:pans-type-Z skos:inScheme asls:soil-profile .
sp:particle-size-fraction-boulders rdfs:isDefinedBy asls:soil-profile .
sp:particle-size-fraction-boulders skos:inScheme asls:soil-profile .
sp:particle-size-fraction-clay rdfs:isDefinedBy asls:soil-profile .
sp:particle-size-fraction-clay skos:inScheme asls:soil-profile .
sp:particle-size-fraction-coarse-gravel rdfs:isDefinedBy asls:soil-profile .
sp:particle-size-fraction-coarse-gravel skos:inScheme asls:soil-profile .
sp:particle-size-fraction-coarse-sand rdfs:isDefinedBy asls:soil-profile .
sp:particle-size-fraction-coarse-sand skos:inScheme asls:soil-profile .
sp:particle-size-fraction-cobbles rdfs:isDefinedBy asls:soil-profile .
sp:particle-size-fraction-cobbles skos:inScheme asls:soil-profile .
sp:particle-size-fraction-fine-clay rdfs:isDefinedBy asls:soil-profile .
sp:particle-size-fraction-fine-clay skos:inScheme asls:soil-profile .
sp:particle-size-fraction-fine-gravel rdfs:isDefinedBy asls:soil-profile .
sp:particle-size-fraction-fine-gravel skos:inScheme asls:soil-profile .
sp:particle-size-fraction-fine-sand rdfs:isDefinedBy asls:soil-profile .
sp:particle-size-fraction-fine-sand skos:inScheme asls:soil-profile .
sp:particle-size-fraction-medium-gravel rdfs:isDefinedBy asls:soil-profile .
sp:particle-size-fraction-medium-gravel skos:inScheme asls:soil-profile .
sp:particle-size-fraction-sand rdfs:isDefinedBy asls:soil-profile .
sp:particle-size-fraction-sand skos:inScheme asls:soil-profile .
sp:particle-size-fraction-silt rdfs:isDefinedBy asls:soil-profile .
sp:particle-size-fraction-silt skos:inScheme asls:soil-profile .
sp:particle-size-fraction-stones rdfs:isDefinedBy asls:soil-profile .
sp:particle-size-fraction-stones skos:inScheme asls:soil-profile .
sp:roots-abundance-0 rdfs:isDefinedBy asls:soil-profile .
sp:roots-abundance-0 skos:inScheme asls:soil-profile .
sp:roots-abundance-1 rdfs:isDefinedBy asls:soil-profile .
sp:roots-abundance-1 skos:inScheme asls:soil-profile .
sp:roots-abundance-2 rdfs:isDefinedBy asls:soil-profile .
sp:roots-abundance-2 skos:inScheme asls:soil-profile .
sp:roots-abundance-3 rdfs:isDefinedBy asls:soil-profile .
sp:roots-abundance-3 skos:inScheme asls:soil-profile .
sp:roots-abundance-4 rdfs:isDefinedBy asls:soil-profile .
sp:roots-abundance-4 skos:inScheme asls:soil-profile .
sp:roots-size-1 rdfs:isDefinedBy asls:soil-profile .
sp:roots-size-1 skos:inScheme asls:soil-profile .
sp:roots-size-2 rdfs:isDefinedBy asls:soil-profile .
sp:roots-size-2 skos:inScheme asls:soil-profile .
sp:roots-size-3 rdfs:isDefinedBy asls:soil-profile .
sp:roots-size-3 skos:inScheme asls:soil-profile .
sp:roots-size-4 rdfs:isDefinedBy asls:soil-profile .
sp:roots-size-4 skos:inScheme asls:soil-profile .
sp:segregations-abundance-0 rdfs:isDefinedBy asls:soil-profile .
sp:segregations-abundance-0 skos:inScheme asls:soil-profile .
sp:segregations-abundance-1 rdfs:isDefinedBy asls:soil-profile .
sp:segregations-abundance-1 skos:inScheme asls:soil-profile .
sp:segregations-abundance-2 rdfs:isDefinedBy asls:soil-profile .
sp:segregations-abundance-2 skos:inScheme asls:soil-profile .
sp:segregations-abundance-3 rdfs:isDefinedBy asls:soil-profile .
sp:segregations-abundance-3 skos:inScheme asls:soil-profile .
sp:segregations-abundance-4 rdfs:isDefinedBy asls:soil-profile .
sp:segregations-abundance-4 skos:inScheme asls:soil-profile .
sp:segregations-abundance-5 rdfs:isDefinedBy asls:soil-profile .
sp:segregations-abundance-5 skos:inScheme asls:soil-profile .
sp:segregations-form-C rdfs:isDefinedBy asls:soil-profile .
sp:segregations-form-C skos:inScheme asls:soil-profile .
sp:segregations-form-F rdfs:isDefinedBy asls:soil-profile .
sp:segregations-form-F skos:inScheme asls:soil-profile .
sp:segregations-form-L rdfs:isDefinedBy asls:soil-profile .
sp:segregations-form-L skos:inScheme asls:soil-profile .
sp:segregations-form-N rdfs:isDefinedBy asls:soil-profile .
sp:segregations-form-N skos:inScheme asls:soil-profile .
sp:segregations-form-R rdfs:isDefinedBy asls:soil-profile .
sp:segregations-form-R skos:inScheme asls:soil-profile .
sp:segregations-form-S rdfs:isDefinedBy asls:soil-profile .
sp:segregations-form-S skos:inScheme asls:soil-profile .
sp:segregations-form-T rdfs:isDefinedBy asls:soil-profile .
sp:segregations-form-T skos:inScheme asls:soil-profile .
sp:segregations-form-V rdfs:isDefinedBy asls:soil-profile .
sp:segregations-form-V skos:inScheme asls:soil-profile .
sp:segregations-form-X rdfs:isDefinedBy asls:soil-profile .
sp:segregations-form-X skos:inScheme asls:soil-profile .
sp:segregations-magnetic-M rdfs:isDefinedBy asls:soil-profile .
sp:segregations-magnetic-M skos:inScheme asls:soil-profile .
sp:segregations-magnetic-N rdfs:isDefinedBy asls:soil-profile .
sp:segregations-magnetic-N skos:inScheme asls:soil-profile .
sp:segregations-nature-A rdfs:isDefinedBy asls:soil-profile .
sp:segregations-nature-A skos:inScheme asls:soil-profile .
sp:segregations-nature-E rdfs:isDefinedBy asls:soil-profile .
sp:segregations-nature-E skos:inScheme asls:soil-profile .
sp:segregations-nature-F rdfs:isDefinedBy asls:soil-profile .
sp:segregations-nature-F skos:inScheme asls:soil-profile .
sp:segregations-nature-G rdfs:isDefinedBy asls:soil-profile .
sp:segregations-nature-G skos:inScheme asls:soil-profile .
sp:segregations-nature-H rdfs:isDefinedBy asls:soil-profile .
sp:segregations-nature-H skos:inScheme asls:soil-profile .
sp:segregations-nature-K rdfs:isDefinedBy asls:soil-profile .
sp:segregations-nature-K skos:inScheme asls:soil-profile .
sp:segregations-nature-L rdfs:isDefinedBy asls:soil-profile .
sp:segregations-nature-L skos:inScheme asls:soil-profile .
sp:segregations-nature-M rdfs:isDefinedBy asls:soil-profile .
sp:segregations-nature-M skos:inScheme asls:soil-profile .
sp:segregations-nature-N rdfs:isDefinedBy asls:soil-profile .
sp:segregations-nature-N skos:inScheme asls:soil-profile .
sp:segregations-nature-O rdfs:isDefinedBy asls:soil-profile .
sp:segregations-nature-O skos:inScheme asls:soil-profile .
sp:segregations-nature-S rdfs:isDefinedBy asls:soil-profile .
sp:segregations-nature-S skos:inScheme asls:soil-profile .
sp:segregations-nature-U rdfs:isDefinedBy asls:soil-profile .
sp:segregations-nature-U skos:inScheme asls:soil-profile .
sp:segregations-nature-Y rdfs:isDefinedBy asls:soil-profile .
sp:segregations-nature-Y skos:inScheme asls:soil-profile .
sp:segregations-nature-Z rdfs:isDefinedBy asls:soil-profile .
sp:segregations-nature-Z skos:inScheme asls:soil-profile .
sp:segregations-size-1 rdfs:isDefinedBy asls:soil-profile .
sp:segregations-size-1 skos:inScheme asls:soil-profile .
sp:segregations-size-2 rdfs:isDefinedBy asls:soil-profile .
sp:segregations-size-2 skos:inScheme asls:soil-profile .
sp:segregations-size-3 rdfs:isDefinedBy asls:soil-profile .
sp:segregations-size-3 skos:inScheme asls:soil-profile .
sp:segregations-size-4 rdfs:isDefinedBy asls:soil-profile .
sp:segregations-size-4 skos:inScheme asls:soil-profile .
sp:segregations-size-5 rdfs:isDefinedBy asls:soil-profile .
sp:segregations-size-5 skos:inScheme asls:soil-profile .
sp:segregations-strength-1 rdfs:isDefinedBy asls:soil-profile .
sp:segregations-strength-1 skos:inScheme asls:soil-profile .
sp:segregations-strength-2 rdfs:isDefinedBy asls:soil-profile .
sp:segregations-strength-2 skos:inScheme asls:soil-profile .
sp:soil-water-drainage-1 rdfs:isDefinedBy asls:soil-profile .
sp:soil-water-drainage-1 skos:inScheme asls:soil-profile .
sp:soil-water-drainage-2 rdfs:isDefinedBy asls:soil-profile .
sp:soil-water-drainage-2 skos:inScheme asls:soil-profile .
sp:soil-water-drainage-3 rdfs:isDefinedBy asls:soil-profile .
sp:soil-water-drainage-3 skos:inScheme asls:soil-profile .
sp:soil-water-drainage-4 rdfs:isDefinedBy asls:soil-profile .
sp:soil-water-drainage-4 skos:inScheme asls:soil-profile .
sp:soil-water-drainage-5 rdfs:isDefinedBy asls:soil-profile .
sp:soil-water-drainage-5 skos:inScheme asls:soil-profile .
sp:soil-water-drainage-6 rdfs:isDefinedBy asls:soil-profile .
sp:soil-water-drainage-6 skos:inScheme asls:soil-profile .
sp:soil-water-permeability-1 rdfs:isDefinedBy asls:soil-profile .
sp:soil-water-permeability-1 skos:inScheme asls:soil-profile .
sp:soil-water-permeability-2 rdfs:isDefinedBy asls:soil-profile .
sp:soil-water-permeability-2 skos:inScheme asls:soil-profile .
sp:soil-water-permeability-3 rdfs:isDefinedBy asls:soil-profile .
sp:soil-water-permeability-3 skos:inScheme asls:soil-profile .
sp:soil-water-permeability-4 rdfs:isDefinedBy asls:soil-profile .
sp:soil-water-permeability-4 skos:inScheme asls:soil-profile .
sp:soil-water-status-D rdfs:isDefinedBy asls:soil-profile .
sp:soil-water-status-D skos:inScheme asls:soil-profile .
sp:soil-water-status-M rdfs:isDefinedBy asls:soil-profile .
sp:soil-water-status-M skos:inScheme asls:soil-profile .
sp:soil-water-status-T rdfs:isDefinedBy asls:soil-profile .
sp:soil-water-status-T skos:inScheme asls:soil-profile .
sp:soil-water-status-W rdfs:isDefinedBy asls:soil-profile .
sp:soil-water-status-W skos:inScheme asls:soil-profile .
sp:structure-artificial-CL rdfs:isDefinedBy asls:soil-profile .
sp:structure-artificial-CL skos:inScheme asls:soil-profile .
sp:structure-artificial-FR rdfs:isDefinedBy asls:soil-profile .
sp:structure-artificial-FR skos:inScheme asls:soil-profile .
sp:structure-pedality-grade-G rdfs:isDefinedBy asls:soil-profile .
sp:structure-pedality-grade-G skos:inScheme asls:soil-profile .
sp:structure-pedality-grade-M rdfs:isDefinedBy asls:soil-profile .
sp:structure-pedality-grade-M skos:inScheme asls:soil-profile .
sp:structure-pedality-grade-S rdfs:isDefinedBy asls:soil-profile .
sp:structure-pedality-grade-S skos:inScheme asls:soil-profile .
sp:structure-pedality-grade-V rdfs:isDefinedBy asls:soil-profile .
sp:structure-pedality-grade-V skos:inScheme asls:soil-profile .
sp:structure-pedality-grade-W rdfs:isDefinedBy asls:soil-profile .
sp:structure-pedality-grade-W skos:inScheme asls:soil-profile .
sp:structure-pedality-size-1 rdfs:isDefinedBy asls:soil-profile .
sp:structure-pedality-size-1 skos:inScheme asls:soil-profile .
sp:structure-pedality-size-2 rdfs:isDefinedBy asls:soil-profile .
sp:structure-pedality-size-2 skos:inScheme asls:soil-profile .
sp:structure-pedality-size-3 rdfs:isDefinedBy asls:soil-profile .
sp:structure-pedality-size-3 skos:inScheme asls:soil-profile .
sp:structure-pedality-size-4 rdfs:isDefinedBy asls:soil-profile .
sp:structure-pedality-size-4 skos:inScheme asls:soil-profile .
sp:structure-pedality-size-5 rdfs:isDefinedBy asls:soil-profile .
sp:structure-pedality-size-5 skos:inScheme asls:soil-profile .
sp:structure-pedality-size-6 rdfs:isDefinedBy asls:soil-profile .
sp:structure-pedality-size-6 skos:inScheme asls:soil-profile .
sp:structure-pedality-size-7 rdfs:isDefinedBy asls:soil-profile .
sp:structure-pedality-size-7 skos:inScheme asls:soil-profile .
sp:structure-pedality-size-8 rdfs:isDefinedBy asls:soil-profile .
sp:structure-pedality-size-8 skos:inScheme asls:soil-profile .
sp:structure-pedality-size-9 rdfs:isDefinedBy asls:soil-profile .
sp:structure-pedality-size-9 skos:inScheme asls:soil-profile .
sp:structure-pedality-type-AB rdfs:isDefinedBy asls:soil-profile .
sp:structure-pedality-type-AB skos:inScheme asls:soil-profile .
sp:structure-pedality-type-CA rdfs:isDefinedBy asls:soil-profile .
sp:structure-pedality-type-CA skos:inScheme asls:soil-profile .
sp:structure-pedality-type-CO rdfs:isDefinedBy asls:soil-profile .
sp:structure-pedality-type-CO skos:inScheme asls:soil-profile .
sp:structure-pedality-type-GR rdfs:isDefinedBy asls:soil-profile .
sp:structure-pedality-type-GR skos:inScheme asls:soil-profile .
sp:structure-pedality-type-LE rdfs:isDefinedBy asls:soil-profile .
sp:structure-pedality-type-LE skos:inScheme asls:soil-profile .
sp:structure-pedality-type-PL rdfs:isDefinedBy asls:soil-profile .
sp:structure-pedality-type-PL skos:inScheme asls:soil-profile .
sp:structure-pedality-type-PO rdfs:isDefinedBy asls:soil-profile .
sp:structure-pedality-type-PO skos:inScheme asls:soil-profile .
sp:structure-pedality-type-PR rdfs:isDefinedBy asls:soil-profile .
sp:structure-pedality-type-PR skos:inScheme asls:soil-profile .
sp:structure-pedality-type-SB rdfs:isDefinedBy asls:soil-profile .
sp:structure-pedality-type-SB skos:inScheme asls:soil-profile .
sp:surfacecondition-C rdfs:isDefinedBy asls:soil-profile .
sp:surfacecondition-C skos:inScheme asls:soil-profile .
sp:surfacecondition-F rdfs:isDefinedBy asls:soil-profile .
sp:surfacecondition-F skos:inScheme asls:soil-profile .
sp:surfacecondition-G rdfs:isDefinedBy asls:soil-profile .
sp:surfacecondition-G skos:inScheme asls:soil-profile .
sp:surfacecondition-H rdfs:isDefinedBy asls:soil-profile .
sp:surfacecondition-H skos:inScheme asls:soil-profile .
sp:surfacecondition-L rdfs:isDefinedBy asls:soil-profile .
sp:surfacecondition-L skos:inScheme asls:soil-profile .
sp:surfacecondition-M rdfs:isDefinedBy asls:soil-profile .
sp:surfacecondition-M skos:inScheme asls:soil-profile .
sp:surfacecondition-O rdfs:isDefinedBy asls:soil-profile .
sp:surfacecondition-O skos:inScheme asls:soil-profile .
sp:surfacecondition-P rdfs:isDefinedBy asls:soil-profile .
sp:surfacecondition-P skos:inScheme asls:soil-profile .
sp:surfacecondition-R rdfs:isDefinedBy asls:soil-profile .
sp:surfacecondition-R skos:inScheme asls:soil-profile .
sp:surfacecondition-S rdfs:isDefinedBy asls:soil-profile .
sp:surfacecondition-S skos:inScheme asls:soil-profile .
sp:surfacecondition-T rdfs:isDefinedBy asls:soil-profile .
sp:surfacecondition-T skos:inScheme asls:soil-profile .
sp:surfacecondition-X rdfs:isDefinedBy asls:soil-profile .
sp:surfacecondition-X skos:inScheme asls:soil-profile .
sp:surfacecondition-Y rdfs:isDefinedBy asls:soil-profile .
sp:surfacecondition-Y skos:inScheme asls:soil-profile .
sp:surfacecondition-Z rdfs:isDefinedBy asls:soil-profile .
sp:surfacecondition-Z skos:inScheme asls:soil-profile .
sp:voids-cracks-1 rdfs:isDefinedBy asls:soil-profile .
sp:voids-cracks-1 skos:inScheme asls:soil-profile .
sp:voids-cracks-2 rdfs:isDefinedBy asls:soil-profile .
sp:voids-cracks-2 skos:inScheme asls:soil-profile .
sp:voids-cracks-3 rdfs:isDefinedBy asls:soil-profile .
sp:voids-cracks-3 skos:inScheme asls:soil-profile .
sp:voids-cracks-4 rdfs:isDefinedBy asls:soil-profile .
sp:voids-cracks-4 skos:inScheme asls:soil-profile .
sp:voids-cracks-5 rdfs:isDefinedBy asls:soil-profile .
sp:voids-cracks-5 skos:inScheme asls:soil-profile .
sp:voids-macropores-abundance-0 rdfs:isDefinedBy asls:soil-profile .
sp:voids-macropores-abundance-0 skos:inScheme asls:soil-profile .
sp:voids-macropores-abundance-1 rdfs:isDefinedBy asls:soil-profile .
sp:voids-macropores-abundance-1 skos:inScheme asls:soil-profile .
sp:voids-macropores-abundance-2 rdfs:isDefinedBy asls:soil-profile .
sp:voids-macropores-abundance-2 skos:inScheme asls:soil-profile .
sp:voids-macropores-abundance-3 rdfs:isDefinedBy asls:soil-profile .
sp:voids-macropores-abundance-3 skos:inScheme asls:soil-profile .
sp:voids-macropores-abundance-4 rdfs:isDefinedBy asls:soil-profile .
sp:voids-macropores-abundance-4 skos:inScheme asls:soil-profile .
sp:voids-macropores-abundance-5 rdfs:isDefinedBy asls:soil-profile .
sp:voids-macropores-abundance-5 skos:inScheme asls:soil-profile .
sp:voids-macropores-abundance-6 rdfs:isDefinedBy asls:soil-profile .
sp:voids-macropores-abundance-6 skos:inScheme asls:soil-profile .
sp:voids-macropores-diameter-1 rdfs:isDefinedBy asls:soil-profile .
sp:voids-macropores-diameter-1 skos:inScheme asls:soil-profile .
sp:voids-macropores-diameter-2 rdfs:isDefinedBy asls:soil-profile .
sp:voids-macropores-diameter-2 skos:inScheme asls:soil-profile .
sp:voids-macropores-diameter-3 rdfs:isDefinedBy asls:soil-profile .
sp:voids-macropores-diameter-3 skos:inScheme asls:soil-profile .
sp:voids-macropores-diameter-4 rdfs:isDefinedBy asls:soil-profile .
sp:voids-macropores-diameter-4 skos:inScheme asls:soil-profile .
sp:voids-micropores rdfs:isDefinedBy asls:soil-profile .
sp:voids-micropores skos:inScheme asls:soil-profile .
sp:water-repellence-N rdfs:isDefinedBy asls:soil-profile .
sp:water-repellence-N skos:inScheme asls:soil-profile .
sp:water-repellence-R rdfs:isDefinedBy asls:soil-profile .
sp:water-repellence-R skos:inScheme asls:soil-profile .
sp:water-repellence-S rdfs:isDefinedBy asls:soil-profile .
sp:water-repellence-S skos:inScheme asls:soil-profile .
subst:lithology-AC rdfs:isDefinedBy asls:soil-profile .
subst:lithology-AC skos:inScheme asls:soil-profile .
subst:lithology-AD rdfs:isDefinedBy asls:soil-profile .
subst:lithology-AD skos:inScheme asls:soil-profile .
subst:lithology-AF rdfs:isDefinedBy asls:soil-profile .
subst:lithology-AF skos:inScheme asls:soil-profile .
subst:lithology-AG rdfs:isDefinedBy asls:soil-profile .
subst:lithology-AG skos:inScheme asls:soil-profile .
subst:lithology-AH rdfs:isDefinedBy asls:soil-profile .
subst:lithology-AH skos:inScheme asls:soil-profile .
subst:lithology-AM rdfs:isDefinedBy asls:soil-profile .
subst:lithology-AM skos:inScheme asls:soil-profile .
subst:lithology-AN rdfs:isDefinedBy asls:soil-profile .
subst:lithology-AN skos:inScheme asls:soil-profile .
subst:lithology-AP rdfs:isDefinedBy asls:soil-profile .
subst:lithology-AP skos:inScheme asls:soil-profile .
subst:lithology-AR rdfs:isDefinedBy asls:soil-profile .
subst:lithology-AR skos:inScheme asls:soil-profile .
subst:lithology-AS rdfs:isDefinedBy asls:soil-profile .
subst:lithology-AS skos:inScheme asls:soil-profile .
subst:lithology-BA rdfs:isDefinedBy asls:soil-profile .
subst:lithology-BA skos:inScheme asls:soil-profile .
subst:lithology-BB rdfs:isDefinedBy asls:soil-profile .
subst:lithology-BB skos:inScheme asls:soil-profile .
subst:lithology-BO rdfs:isDefinedBy asls:soil-profile .
subst:lithology-BO skos:inScheme asls:soil-profile .
subst:lithology-BR rdfs:isDefinedBy asls:soil-profile .
subst:lithology-BR skos:inScheme asls:soil-profile .
subst:lithology-C rdfs:isDefinedBy asls:soil-profile .
subst:lithology-C skos:inScheme asls:soil-profile .
subst:lithology-CB rdfs:isDefinedBy asls:soil-profile .
subst:lithology-CB skos:inScheme asls:soil-profile .
subst:lithology-CG rdfs:isDefinedBy asls:soil-profile .
subst:lithology-CG skos:inScheme asls:soil-profile .
subst:lithology-CH rdfs:isDefinedBy asls:soil-profile .
subst:lithology-CH skos:inScheme asls:soil-profile .
subst:lithology-CO rdfs:isDefinedBy asls:soil-profile .
subst:lithology-CO skos:inScheme asls:soil-profile .
subst:lithology-CU rdfs:isDefinedBy asls:soil-profile .
subst:lithology-CU skos:inScheme asls:soil-profile .
subst:lithology-DI rdfs:isDefinedBy asls:soil-profile .
subst:lithology-DI skos:inScheme asls:soil-profile .
subst:lithology-DM rdfs:isDefinedBy asls:soil-profile .
subst:lithology-DM skos:inScheme asls:soil-profile .
subst:lithology-DR rdfs:isDefinedBy asls:soil-profile .
subst:lithology-DR skos:inScheme asls:soil-profile .
subst:lithology-FC rdfs:isDefinedBy asls:soil-profile .
subst:lithology-FC skos:inScheme asls:soil-profile .
subst:lithology-GA rdfs:isDefinedBy asls:soil-profile .
subst:lithology-GA skos:inScheme asls:soil-profile .
subst:lithology-GD rdfs:isDefinedBy asls:soil-profile .
subst:lithology-GD skos:inScheme asls:soil-profile .
subst:lithology-GE rdfs:isDefinedBy asls:soil-profile .
subst:lithology-GE skos:inScheme asls:soil-profile .
subst:lithology-GN rdfs:isDefinedBy asls:soil-profile .
subst:lithology-GN skos:inScheme asls:soil-profile .
subst:lithology-GR rdfs:isDefinedBy asls:soil-profile .
subst:lithology-GR skos:inScheme asls:soil-profile .
subst:lithology-GS rdfs:isDefinedBy asls:soil-profile .
subst:lithology-GS skos:inScheme asls:soil-profile .
subst:lithology-GV rdfs:isDefinedBy asls:soil-profile .
subst:lithology-GV skos:inScheme asls:soil-profile .
subst:lithology-GW rdfs:isDefinedBy asls:soil-profile .
subst:lithology-GW skos:inScheme asls:soil-profile .
subst:lithology-GY rdfs:isDefinedBy asls:soil-profile .
subst:lithology-GY skos:inScheme asls:soil-profile .
subst:lithology-HA rdfs:isDefinedBy asls:soil-profile .
subst:lithology-HA skos:inScheme asls:soil-profile .
subst:lithology-HO rdfs:isDefinedBy asls:soil-profile .
subst:lithology-HO skos:inScheme asls:soil-profile .
subst:lithology-IG rdfs:isDefinedBy asls:soil-profile .
subst:lithology-IG skos:inScheme asls:soil-profile .
subst:lithology-JA rdfs:isDefinedBy asls:soil-profile .
subst:lithology-JA skos:inScheme asls:soil-profile .
subst:lithology-KA rdfs:isDefinedBy asls:soil-profile .
subst:lithology-KA skos:inScheme asls:soil-profile .
subst:lithology-KC rdfs:isDefinedBy asls:soil-profile .
subst:lithology-KC skos:inScheme asls:soil-profile .
subst:lithology-KL rdfs:isDefinedBy asls:soil-profile .
subst:lithology-KL skos:inScheme asls:soil-profile .
subst:lithology-KM rdfs:isDefinedBy asls:soil-profile .
subst:lithology-KM skos:inScheme asls:soil-profile .
subst:lithology-KR rdfs:isDefinedBy asls:soil-profile .
subst:lithology-KR skos:inScheme asls:soil-profile .
subst:lithology-KS rdfs:isDefinedBy asls:soil-profile .
subst:lithology-KS skos:inScheme asls:soil-profile .
subst:lithology-LC rdfs:isDefinedBy asls:soil-profile .
subst:lithology-LC skos:inScheme asls:soil-profile .
subst:lithology-LI rdfs:isDefinedBy asls:soil-profile .
subst:lithology-LI skos:inScheme asls:soil-profile .
subst:lithology-M rdfs:isDefinedBy asls:soil-profile .
subst:lithology-M skos:inScheme asls:soil-profile .
subst:lithology-MB rdfs:isDefinedBy asls:soil-profile .
subst:lithology-MB skos:inScheme asls:soil-profile .
subst:lithology-MD rdfs:isDefinedBy asls:soil-profile .
subst:lithology-MD skos:inScheme asls:soil-profile .
subst:lithology-ME rdfs:isDefinedBy asls:soil-profile .
subst:lithology-ME skos:inScheme asls:soil-profile .
subst:lithology-MG rdfs:isDefinedBy asls:soil-profile .
subst:lithology-MG skos:inScheme asls:soil-profile .
subst:lithology-MI rdfs:isDefinedBy asls:soil-profile .
subst:lithology-MI skos:inScheme asls:soil-profile .
subst:lithology-ML rdfs:isDefinedBy asls:soil-profile .
subst:lithology-ML skos:inScheme asls:soil-profile .
subst:lithology-MS rdfs:isDefinedBy asls:soil-profile .
subst:lithology-MS skos:inScheme asls:soil-profile .
subst:lithology-MU rdfs:isDefinedBy asls:soil-profile .
subst:lithology-MU skos:inScheme asls:soil-profile .
subst:lithology-MY rdfs:isDefinedBy asls:soil-profile .
subst:lithology-MY skos:inScheme asls:soil-profile .
subst:lithology-PC rdfs:isDefinedBy asls:soil-profile .
subst:lithology-PC skos:inScheme asls:soil-profile .
subst:lithology-PE rdfs:isDefinedBy asls:soil-profile .
subst:lithology-PE skos:inScheme asls:soil-profile .
subst:lithology-PG rdfs:isDefinedBy asls:soil-profile .
subst:lithology-PG skos:inScheme asls:soil-profile .
subst:lithology-PH rdfs:isDefinedBy asls:soil-profile .
subst:lithology-PH skos:inScheme asls:soil-profile .
subst:lithology-PL rdfs:isDefinedBy asls:soil-profile .
subst:lithology-PL skos:inScheme asls:soil-profile .
subst:lithology-PO rdfs:isDefinedBy asls:soil-profile .
subst:lithology-PO skos:inScheme asls:soil-profile .
subst:lithology-PY rdfs:isDefinedBy asls:soil-profile .
subst:lithology-PY skos:inScheme asls:soil-profile .
subst:lithology-QP rdfs:isDefinedBy asls:soil-profile .
subst:lithology-QP skos:inScheme asls:soil-profile .
subst:lithology-QS rdfs:isDefinedBy asls:soil-profile .
subst:lithology-QS skos:inScheme asls:soil-profile .
subst:lithology-QU rdfs:isDefinedBy asls:soil-profile .
subst:lithology-QU skos:inScheme asls:soil-profile .
subst:lithology-QZ rdfs:isDefinedBy asls:soil-profile .
subst:lithology-QZ skos:inScheme asls:soil-profile .
subst:lithology-R rdfs:isDefinedBy asls:soil-profile .
subst:lithology-R skos:inScheme asls:soil-profile .
subst:lithology-RB rdfs:isDefinedBy asls:soil-profile .
subst:lithology-RB skos:inScheme asls:soil-profile .
subst:lithology-RH rdfs:isDefinedBy asls:soil-profile .
subst:lithology-RH skos:inScheme asls:soil-profile .
subst:lithology-S rdfs:isDefinedBy asls:soil-profile .
subst:lithology-S skos:inScheme asls:soil-profile .
subst:lithology-SA rdfs:isDefinedBy asls:soil-profile .
subst:lithology-SA skos:inScheme asls:soil-profile .
subst:lithology-SD rdfs:isDefinedBy asls:soil-profile .
subst:lithology-SD skos:inScheme asls:soil-profile .
subst:lithology-SH rdfs:isDefinedBy asls:soil-profile .
subst:lithology-SH skos:inScheme asls:soil-profile .
subst:lithology-SK rdfs:isDefinedBy asls:soil-profile .
subst:lithology-SK skos:inScheme asls:soil-profile .
subst:lithology-SL rdfs:isDefinedBy asls:soil-profile .
subst:lithology-SL skos:inScheme asls:soil-profile .
subst:lithology-SN rdfs:isDefinedBy asls:soil-profile .
subst:lithology-SN skos:inScheme asls:soil-profile .
subst:lithology-SR rdfs:isDefinedBy asls:soil-profile .
subst:lithology-SR skos:inScheme asls:soil-profile .
subst:lithology-ST rdfs:isDefinedBy asls:soil-profile .
subst:lithology-ST skos:inScheme asls:soil-profile .
subst:lithology-SY rdfs:isDefinedBy asls:soil-profile .
subst:lithology-SY skos:inScheme asls:soil-profile .
subst:lithology-TR rdfs:isDefinedBy asls:soil-profile .
subst:lithology-TR skos:inScheme asls:soil-profile .
subst:lithology-TU rdfs:isDefinedBy asls:soil-profile .
subst:lithology-TU skos:inScheme asls:soil-profile .
subst:lithology-UC rdfs:isDefinedBy asls:soil-profile .
subst:lithology-UC skos:inScheme asls:soil-profile .
subst:lithology-VB rdfs:isDefinedBy asls:soil-profile .
subst:lithology-VB skos:inScheme asls:soil-profile .
subst:lithology-VG rdfs:isDefinedBy asls:soil-profile .
subst:lithology-VG skos:inScheme asls:soil-profile .
subst:lithology-Z rdfs:isDefinedBy asls:soil-profile .
subst:lithology-Z skos:inScheme asls:soil-profile .
subst:lithology-ZS rdfs:isDefinedBy asls:soil-profile .
subst:lithology-ZS skos:inScheme asls:soil-profile .
subst:material-strength-M rdfs:isDefinedBy asls:soil-profile .
subst:material-strength-M skos:inScheme asls:soil-profile .
subst:material-strength-S rdfs:isDefinedBy asls:soil-profile .
subst:material-strength-S skos:inScheme asls:soil-profile .
subst:material-strength-VS rdfs:isDefinedBy asls:soil-profile .
subst:material-strength-VS skos:inScheme asls:soil-profile .
subst:material-strength-VW rdfs:isDefinedBy asls:soil-profile .
subst:material-strength-VW skos:inScheme asls:soil-profile .
subst:material-strength-W rdfs:isDefinedBy asls:soil-profile .
subst:material-strength-W skos:inScheme asls:soil-profile .

sp:structure-pedality-compound
  skos:member sp:Pedality-grade-apedal ;
  skos:member sp:Pedality-grade-pedal ;
.

ls:coarse-fragments-abundance-0 skos:topConceptOf asls:soil-profile .
asls:soil-profile skos:hasTopConcept ls:coarse-fragments-abundance-0 .
ls:coarse-fragments-abundance-1 skos:topConceptOf asls:soil-profile .
asls:soil-profile skos:hasTopConcept ls:coarse-fragments-abundance-1 .
ls:coarse-fragments-abundance-2 skos:topConceptOf asls:soil-profile .
asls:soil-profile skos:hasTopConcept ls:coarse-fragments-abundance-2 .
ls:coarse-fragments-abundance-3 skos:topConceptOf asls:soil-profile .
asls:soil-profile skos:hasTopConcept ls:coarse-fragments-abundance-3 .
ls:coarse-fragments-abundance-4 skos:topConceptOf asls:soil-profile .
asls:soil-profile skos:hasTopConcept ls:coarse-fragments-abundance-4 .
ls:coarse-fragments-abundance-5 skos:topConceptOf asls:soil-profile .
asls:soil-profile skos:hasTopConcept ls:coarse-fragments-abundance-5 .
ls:coarse-fragments-abundance-6 skos:topConceptOf asls:soil-profile .
asls:soil-profile skos:hasTopConcept ls:coarse-fragments-abundance-6 .
ls:coarse-fragments-shape-A skos:topConceptOf asls:soil-profile .
asls:soil-profile skos:hasTopConcept ls:coarse-fragments-shape-A .
ls:coarse-fragments-shape-AP skos:topConceptOf asls:soil-profile .
asls:soil-profile skos:hasTopConcept ls:coarse-fragments-shape-AP .
ls:coarse-fragments-shape-AT skos:topConceptOf asls:soil-profile .
asls:soil-profile skos:hasTopConcept ls:coarse-fragments-shape-AT .
ls:coarse-fragments-shape-R skos:topConceptOf asls:soil-profile .
asls:soil-profile skos:hasTopConcept ls:coarse-fragments-shape-R .
ls:coarse-fragments-shape-RP skos:topConceptOf asls:soil-profile .
asls:soil-profile skos:hasTopConcept ls:coarse-fragments-shape-RP .
ls:coarse-fragments-shape-RT skos:topConceptOf asls:soil-profile .
asls:soil-profile skos:hasTopConcept ls:coarse-fragments-shape-RT .
ls:coarse-fragments-shape-S skos:topConceptOf asls:soil-profile .
asls:soil-profile skos:hasTopConcept ls:coarse-fragments-shape-S .
ls:coarse-fragments-shape-SP skos:topConceptOf asls:soil-profile .
asls:soil-profile skos:hasTopConcept ls:coarse-fragments-shape-SP .
ls:coarse-fragments-shape-ST skos:topConceptOf asls:soil-profile .
asls:soil-profile skos:hasTopConcept ls:coarse-fragments-shape-ST .
ls:coarse-fragments-shape-U skos:topConceptOf asls:soil-profile .
asls:soil-profile skos:hasTopConcept ls:coarse-fragments-shape-U .
ls:coarse-fragments-shape-UP skos:topConceptOf asls:soil-profile .
asls:soil-profile skos:hasTopConcept ls:coarse-fragments-shape-UP .
ls:coarse-fragments-shape-UT skos:topConceptOf asls:soil-profile .
asls:soil-profile skos:hasTopConcept ls:coarse-fragments-shape-UT .
ls:coarse-fragments-size-1 skos:topConceptOf asls:soil-profile .
asls:soil-profile skos:hasTopConcept ls:coarse-fragments-size-1 .
ls:coarse-fragments-size-2 skos:topConceptOf asls:soil-profile .
asls:soil-profile skos:hasTopConcept ls:coarse-fragments-size-2 .
ls:coarse-fragments-size-3 skos:topConceptOf asls:soil-profile .
asls:soil-profile skos:hasTopConcept ls:coarse-fragments-size-3 .
ls:coarse-fragments-size-4 skos:topConceptOf asls:soil-profile .
asls:soil-profile skos:hasTopConcept ls:coarse-fragments-size-4 .
ls:coarse-fragments-size-5 skos:topConceptOf asls:soil-profile .
asls:soil-profile skos:hasTopConcept ls:coarse-fragments-size-5 .
ls:coarse-fragments-size-6 skos:topConceptOf asls:soil-profile .
asls:soil-profile skos:hasTopConcept ls:coarse-fragments-size-6 .
ls:coarse-fragments-size-7 skos:topConceptOf asls:soil-profile .
asls:soil-profile skos:hasTopConcept ls:coarse-fragments-size-7 .
ls:lithology-CC skos:topConceptOf asls:soil-profile .
asls:soil-profile skos:hasTopConcept ls:lithology-CC .
ls:lithology-IS skos:topConceptOf asls:soil-profile .
asls:soil-profile skos:hasTopConcept ls:lithology-IS .
ls:lithology-M skos:topConceptOf asls:soil-profile .
asls:soil-profile skos:hasTopConcept ls:lithology-M .
ls:lithology-OT skos:topConceptOf asls:soil-profile .
asls:soil-profile skos:hasTopConcept ls:lithology-OT .
ls:lithology-OW skos:topConceptOf asls:soil-profile .
asls:soil-profile skos:hasTopConcept ls:lithology-OW .
ls:lithology-PU skos:topConceptOf asls:soil-profile .
asls:soil-profile skos:hasTopConcept ls:lithology-PU .
ls:lithology-R skos:topConceptOf asls:soil-profile .
asls:soil-profile skos:hasTopConcept ls:lithology-R .
ls:lithology-SS skos:topConceptOf asls:soil-profile .
asls:soil-profile skos:hasTopConcept ls:lithology-SS .
sp:coarse-fragments-distribution-D skos:topConceptOf asls:soil-profile .
asls:soil-profile skos:hasTopConcept sp:coarse-fragments-distribution-D .
sp:coarse-fragments-distribution-R skos:topConceptOf asls:soil-profile .
asls:soil-profile skos:hasTopConcept sp:coarse-fragments-distribution-R .
sp:coarse-fragments-distribution-S skos:topConceptOf asls:soil-profile .
asls:soil-profile skos:hasTopConcept sp:coarse-fragments-distribution-S .
sp:coarse-fragments-distribution-U skos:topConceptOf asls:soil-profile .
asls:soil-profile skos:hasTopConcept sp:coarse-fragments-distribution-U .
sp:colour-stat-D skos:topConceptOf asls:soil-profile .
asls:soil-profile skos:hasTopConcept sp:colour-stat-D .
sp:colour-stat-M skos:topConceptOf asls:soil-profile .
asls:soil-profile skos:hasTopConcept sp:colour-stat-M .
sp:colour-value skos:topConceptOf asls:soil-profile .
asls:soil-profile skos:hasTopConcept sp:colour-value .
sp:consistence-plasticity-degree-0 skos:topConceptOf asls:soil-profile .
asls:soil-profile skos:hasTopConcept sp:consistence-plasticity-degree-0 .
sp:consistence-plasticity-degree-1 skos:topConceptOf asls:soil-profile .
asls:soil-profile skos:hasTopConcept sp:consistence-plasticity-degree-1 .
sp:consistence-plasticity-degree-2 skos:topConceptOf asls:soil-profile .
asls:soil-profile skos:hasTopConcept sp:consistence-plasticity-degree-2 .
sp:consistence-plasticity-degree-3 skos:topConceptOf asls:soil-profile .
asls:soil-profile skos:hasTopConcept sp:consistence-plasticity-degree-3 .
sp:consistence-plasticity-type-N skos:topConceptOf asls:soil-profile .
asls:soil-profile skos:hasTopConcept sp:consistence-plasticity-type-N .
sp:consistence-plasticity-type-S skos:topConceptOf asls:soil-profile .
asls:soil-profile skos:hasTopConcept sp:consistence-plasticity-type-S .
sp:consistence-plasticity-type-T skos:topConceptOf asls:soil-profile .
asls:soil-profile skos:hasTopConcept sp:consistence-plasticity-type-T .
sp:consistence-plasticity-type-U skos:topConceptOf asls:soil-profile .
asls:soil-profile skos:hasTopConcept sp:consistence-plasticity-type-U .
sp:consistence-stickiness-0 skos:topConceptOf asls:soil-profile .
asls:soil-profile skos:hasTopConcept sp:consistence-stickiness-0 .
sp:consistence-stickiness-1 skos:topConceptOf asls:soil-profile .
asls:soil-profile skos:hasTopConcept sp:consistence-stickiness-1 .
sp:consistence-stickiness-2 skos:topConceptOf asls:soil-profile .
asls:soil-profile skos:hasTopConcept sp:consistence-stickiness-2 .
sp:consistence-stickiness-3 skos:topConceptOf asls:soil-profile .
asls:soil-profile skos:hasTopConcept sp:consistence-stickiness-3 .
sp:consistence-strength-0 skos:topConceptOf asls:soil-profile .
asls:soil-profile skos:hasTopConcept sp:consistence-strength-0 .
sp:consistence-strength-1 skos:topConceptOf asls:soil-profile .
asls:soil-profile skos:hasTopConcept sp:consistence-strength-1 .
sp:consistence-strength-2 skos:topConceptOf asls:soil-profile .
asls:soil-profile skos:hasTopConcept sp:consistence-strength-2 .
sp:consistence-strength-3 skos:topConceptOf asls:soil-profile .
asls:soil-profile skos:hasTopConcept sp:consistence-strength-3 .
sp:consistence-strength-4 skos:topConceptOf asls:soil-profile .
asls:soil-profile skos:hasTopConcept sp:consistence-strength-4 .
sp:consistence-strength-5 skos:topConceptOf asls:soil-profile .
asls:soil-profile skos:hasTopConcept sp:consistence-strength-5 .
sp:consistence-strength-6 skos:topConceptOf asls:soil-profile .
asls:soil-profile skos:hasTopConcept sp:consistence-strength-6 .
sp:consistence-strength-7 skos:topConceptOf asls:soil-profile .
asls:soil-profile skos:hasTopConcept sp:consistence-strength-7 .
sp:cutans-abundance-0 skos:topConceptOf asls:soil-profile .
asls:soil-profile skos:hasTopConcept sp:cutans-abundance-0 .
sp:cutans-abundance-1 skos:topConceptOf asls:soil-profile .
asls:soil-profile skos:hasTopConcept sp:cutans-abundance-1 .
sp:cutans-abundance-2 skos:topConceptOf asls:soil-profile .
asls:soil-profile skos:hasTopConcept sp:cutans-abundance-2 .
sp:cutans-abundance-3 skos:topConceptOf asls:soil-profile .
asls:soil-profile skos:hasTopConcept sp:cutans-abundance-3 .
sp:cutans-distinctness-D skos:topConceptOf asls:soil-profile .
asls:soil-profile skos:hasTopConcept sp:cutans-distinctness-D .
sp:cutans-distinctness-F skos:topConceptOf asls:soil-profile .
asls:soil-profile skos:hasTopConcept sp:cutans-distinctness-F .
sp:cutans-distinctness-P skos:topConceptOf asls:soil-profile .
asls:soil-profile skos:hasTopConcept sp:cutans-distinctness-P .
sp:cutans-type-C skos:topConceptOf asls:soil-profile .
asls:soil-profile skos:hasTopConcept sp:cutans-type-C .
sp:cutans-type-K skos:topConceptOf asls:soil-profile .
asls:soil-profile skos:hasTopConcept sp:cutans-type-K .
sp:cutans-type-M skos:topConceptOf asls:soil-profile .
asls:soil-profile skos:hasTopConcept sp:cutans-type-M .
sp:cutans-type-O skos:topConceptOf asls:soil-profile .
asls:soil-profile skos:hasTopConcept sp:cutans-type-O .
sp:cutans-type-S skos:topConceptOf asls:soil-profile .
asls:soil-profile skos:hasTopConcept sp:cutans-type-S .
sp:cutans-type-U skos:topConceptOf asls:soil-profile .
asls:soil-profile skos:hasTopConcept sp:cutans-type-U .
sp:cutans-type-Z skos:topConceptOf asls:soil-profile .
asls:soil-profile skos:hasTopConcept sp:cutans-type-Z .
sp:depth-of-horizon skos:topConceptOf asls:soil-profile .
asls:soil-profile skos:hasTopConcept sp:depth-of-horizon .
sp:depth-of-horizon-lower skos:topConceptOf asls:soil-profile .
asls:soil-profile skos:hasTopConcept sp:depth-of-horizon-lower .
sp:depth-of-horizon-upper skos:topConceptOf asls:soil-profile .
asls:soil-profile skos:hasTopConcept sp:depth-of-horizon-upper .
sp:depth-to-r-horizon skos:topConceptOf asls:soil-profile .
asls:soil-profile skos:hasTopConcept sp:depth-to-r-horizon .
sp:effervescence-H skos:topConceptOf asls:soil-profile .
asls:soil-profile skos:hasTopConcept sp:effervescence-H .
sp:effervescence-M skos:topConceptOf asls:soil-profile .
asls:soil-profile skos:hasTopConcept sp:effervescence-M .
sp:effervescence-N skos:topConceptOf asls:soil-profile .
asls:soil-profile skos:hasTopConcept sp:effervescence-N .
sp:effervescence-S skos:topConceptOf asls:soil-profile .
asls:soil-profile skos:hasTopConcept sp:effervescence-S .
sp:effervescence-V skos:topConceptOf asls:soil-profile .
asls:soil-profile skos:hasTopConcept sp:effervescence-V .
sp:fabric-E skos:topConceptOf asls:soil-profile .
asls:soil-profile skos:hasTopConcept sp:fabric-E .
sp:fabric-G skos:topConceptOf asls:soil-profile .
asls:soil-profile skos:hasTopConcept sp:fabric-G .
sp:fabric-R skos:topConceptOf asls:soil-profile .
asls:soil-profile skos:hasTopConcept sp:fabric-R .
sp:fabric-S skos:topConceptOf asls:soil-profile .
asls:soil-profile skos:hasTopConcept sp:fabric-S .
sp:field-ph skos:topConceptOf asls:soil-profile .
asls:soil-profile skos:hasTopConcept sp:field-ph .
sp:field-texture-AP skos:topConceptOf asls:soil-profile .
asls:soil-profile skos:hasTopConcept sp:field-texture-AP .
sp:field-texture-C skos:topConceptOf asls:soil-profile .
asls:soil-profile skos:hasTopConcept sp:field-texture-C .
sp:field-texture-CL skos:topConceptOf asls:soil-profile .
asls:soil-profile skos:hasTopConcept sp:field-texture-CL .
sp:field-texture-CLS skos:topConceptOf asls:soil-profile .
asls:soil-profile skos:hasTopConcept sp:field-texture-CLS .
sp:field-texture-CP skos:topConceptOf asls:soil-profile .
asls:soil-profile skos:hasTopConcept sp:field-texture-CP .
sp:field-texture-CS skos:topConceptOf asls:soil-profile .
asls:soil-profile skos:hasTopConcept sp:field-texture-CS .
sp:field-texture-GP skos:topConceptOf asls:soil-profile .
asls:soil-profile skos:hasTopConcept sp:field-texture-GP .
sp:field-texture-HC skos:topConceptOf asls:soil-profile .
asls:soil-profile skos:hasTopConcept sp:field-texture-HC .
sp:field-texture-HP skos:topConceptOf asls:soil-profile .
asls:soil-profile skos:hasTopConcept sp:field-texture-HP .
sp:field-texture-IP skos:topConceptOf asls:soil-profile .
asls:soil-profile skos:hasTopConcept sp:field-texture-IP .
sp:field-texture-L skos:topConceptOf asls:soil-profile .
asls:soil-profile skos:hasTopConcept sp:field-texture-L .
sp:field-texture-LC skos:topConceptOf asls:soil-profile .
asls:soil-profile skos:hasTopConcept sp:field-texture-LC .
sp:field-texture-LMC skos:topConceptOf asls:soil-profile .
asls:soil-profile skos:hasTopConcept sp:field-texture-LMC .
sp:field-texture-LP skos:topConceptOf asls:soil-profile .
asls:soil-profile skos:hasTopConcept sp:field-texture-LP .
sp:field-texture-LS skos:topConceptOf asls:soil-profile .
asls:soil-profile skos:hasTopConcept sp:field-texture-LS .
sp:field-texture-MC skos:topConceptOf asls:soil-profile .
asls:soil-profile skos:hasTopConcept sp:field-texture-MC .
sp:field-texture-MHC skos:topConceptOf asls:soil-profile .
asls:soil-profile skos:hasTopConcept sp:field-texture-MHC .
sp:field-texture-S skos:topConceptOf asls:soil-profile .
asls:soil-profile skos:hasTopConcept sp:field-texture-S .
sp:field-texture-SCL skos:topConceptOf asls:soil-profile .
asls:soil-profile skos:hasTopConcept sp:field-texture-SCL .
sp:field-texture-SL skos:topConceptOf asls:soil-profile .
asls:soil-profile skos:hasTopConcept sp:field-texture-SL .
sp:field-texture-SP skos:topConceptOf asls:soil-profile .
asls:soil-profile skos:hasTopConcept sp:field-texture-SP .
sp:field-texture-ZCL skos:topConceptOf asls:soil-profile .
asls:soil-profile skos:hasTopConcept sp:field-texture-ZCL .
sp:field-texture-ZL skos:topConceptOf asls:soil-profile .
asls:soil-profile skos:hasTopConcept sp:field-texture-ZL .
sp:field-texture-qualifier-fibric skos:topConceptOf asls:soil-profile .
asls:soil-profile skos:hasTopConcept sp:field-texture-qualifier-fibric .
sp:field-texture-qualifier-heavy skos:topConceptOf asls:soil-profile .
asls:soil-profile skos:hasTopConcept sp:field-texture-qualifier-heavy .
sp:field-texture-qualifier-light skos:topConceptOf asls:soil-profile .
asls:soil-profile skos:hasTopConcept sp:field-texture-qualifier-light .
sp:field-texture-qualifier-sapric skos:topConceptOf asls:soil-profile .
asls:soil-profile skos:hasTopConcept sp:field-texture-qualifier-sapric .
sp:horizon-boundary-distinctness-A skos:topConceptOf asls:soil-profile .
asls:soil-profile skos:hasTopConcept sp:horizon-boundary-distinctness-A .
sp:horizon-boundary-distinctness-C skos:topConceptOf asls:soil-profile .
asls:soil-profile skos:hasTopConcept sp:horizon-boundary-distinctness-C .
sp:horizon-boundary-distinctness-D skos:topConceptOf asls:soil-profile .
asls:soil-profile skos:hasTopConcept sp:horizon-boundary-distinctness-D .
sp:horizon-boundary-distinctness-G skos:topConceptOf asls:soil-profile .
asls:soil-profile skos:hasTopConcept sp:horizon-boundary-distinctness-G .
sp:horizon-boundary-distinctness-S skos:topConceptOf asls:soil-profile .
asls:soil-profile skos:hasTopConcept sp:horizon-boundary-distinctness-S .
sp:horizon-boundary-shape-B skos:topConceptOf asls:soil-profile .
asls:soil-profile skos:hasTopConcept sp:horizon-boundary-shape-B .
sp:horizon-boundary-shape-I skos:topConceptOf asls:soil-profile .
asls:soil-profile skos:hasTopConcept sp:horizon-boundary-shape-I .
sp:horizon-boundary-shape-S skos:topConceptOf asls:soil-profile .
asls:soil-profile skos:hasTopConcept sp:horizon-boundary-shape-S .
sp:horizon-boundary-shape-T skos:topConceptOf asls:soil-profile .
asls:soil-profile skos:hasTopConcept sp:horizon-boundary-shape-T .
sp:horizon-boundary-shape-W skos:topConceptOf asls:soil-profile .
asls:soil-profile skos:hasTopConcept sp:horizon-boundary-shape-W .
sp:horizon-prefix skos:topConceptOf asls:soil-profile .
asls:soil-profile skos:hasTopConcept sp:horizon-prefix .
sp:horizon-suffix-b skos:topConceptOf asls:soil-profile .
asls:soil-profile skos:hasTopConcept sp:horizon-suffix-b .
sp:horizon-suffix-c skos:topConceptOf asls:soil-profile .
asls:soil-profile skos:hasTopConcept sp:horizon-suffix-c .
sp:horizon-suffix-d skos:topConceptOf asls:soil-profile .
asls:soil-profile skos:hasTopConcept sp:horizon-suffix-d .
sp:horizon-suffix-e skos:topConceptOf asls:soil-profile .
asls:soil-profile skos:hasTopConcept sp:horizon-suffix-e .
sp:horizon-suffix-f skos:topConceptOf asls:soil-profile .
asls:soil-profile skos:hasTopConcept sp:horizon-suffix-f .
sp:horizon-suffix-g skos:topConceptOf asls:soil-profile .
asls:soil-profile skos:hasTopConcept sp:horizon-suffix-g .
sp:horizon-suffix-h skos:topConceptOf asls:soil-profile .
asls:soil-profile skos:hasTopConcept sp:horizon-suffix-h .
sp:horizon-suffix-j skos:topConceptOf asls:soil-profile .
asls:soil-profile skos:hasTopConcept sp:horizon-suffix-j .
sp:horizon-suffix-k skos:topConceptOf asls:soil-profile .
asls:soil-profile skos:hasTopConcept sp:horizon-suffix-k .
sp:horizon-suffix-m skos:topConceptOf asls:soil-profile .
asls:soil-profile skos:hasTopConcept sp:horizon-suffix-m .
sp:horizon-suffix-p skos:topConceptOf asls:soil-profile .
asls:soil-profile skos:hasTopConcept sp:horizon-suffix-p .
sp:horizon-suffix-q skos:topConceptOf asls:soil-profile .
asls:soil-profile skos:hasTopConcept sp:horizon-suffix-q .
sp:horizon-suffix-r skos:topConceptOf asls:soil-profile .
asls:soil-profile skos:hasTopConcept sp:horizon-suffix-r .
sp:horizon-suffix-s skos:topConceptOf asls:soil-profile .
asls:soil-profile skos:hasTopConcept sp:horizon-suffix-s .
sp:horizon-suffix-t skos:topConceptOf asls:soil-profile .
asls:soil-profile skos:hasTopConcept sp:horizon-suffix-t .
sp:horizon-suffix-w skos:topConceptOf asls:soil-profile .
asls:soil-profile skos:hasTopConcept sp:horizon-suffix-w .
sp:horizon-suffix-x skos:topConceptOf asls:soil-profile .
asls:soil-profile skos:hasTopConcept sp:horizon-suffix-x .
sp:horizon-suffix-y skos:topConceptOf asls:soil-profile .
asls:soil-profile skos:hasTopConcept sp:horizon-suffix-y .
sp:horizon-suffix-z skos:topConceptOf asls:soil-profile .
asls:soil-profile skos:hasTopConcept sp:horizon-suffix-z .
sp:horizons-A skos:topConceptOf asls:soil-profile .
asls:soil-profile skos:hasTopConcept sp:horizons-A .
sp:horizons-B skos:topConceptOf asls:soil-profile .
asls:soil-profile skos:hasTopConcept sp:horizons-B .
sp:horizons-C skos:topConceptOf asls:soil-profile .
asls:soil-profile skos:hasTopConcept sp:horizons-C .
sp:horizons-D skos:topConceptOf asls:soil-profile .
asls:soil-profile skos:hasTopConcept sp:horizons-D .
sp:horizons-O skos:topConceptOf asls:soil-profile .
asls:soil-profile skos:hasTopConcept sp:horizons-O .
sp:horizons-P skos:topConceptOf asls:soil-profile .
asls:soil-profile skos:hasTopConcept sp:horizons-P .
sp:horizons-R skos:topConceptOf asls:soil-profile .
asls:soil-profile skos:hasTopConcept sp:horizons-R .
sp:horizons-bleached skos:topConceptOf asls:soil-profile .
asls:soil-profile skos:hasTopConcept sp:horizons-bleached .
sp:horizons-subdivision skos:topConceptOf asls:soil-profile .
asls:soil-profile skos:hasTopConcept sp:horizons-subdivision .
sp:horizons-transitional skos:topConceptOf asls:soil-profile .
asls:soil-profile skos:hasTopConcept sp:horizons-transitional .
sp:mottle-abundance-0 skos:topConceptOf asls:soil-profile .
asls:soil-profile skos:hasTopConcept sp:mottle-abundance-0 .
sp:mottle-abundance-1 skos:topConceptOf asls:soil-profile .
asls:soil-profile skos:hasTopConcept sp:mottle-abundance-1 .
sp:mottle-abundance-2 skos:topConceptOf asls:soil-profile .
asls:soil-profile skos:hasTopConcept sp:mottle-abundance-2 .
sp:mottle-abundance-3 skos:topConceptOf asls:soil-profile .
asls:soil-profile skos:hasTopConcept sp:mottle-abundance-3 .
sp:mottle-abundance-4 skos:topConceptOf asls:soil-profile .
asls:soil-profile skos:hasTopConcept sp:mottle-abundance-4 .
sp:mottle-boundary-C skos:topConceptOf asls:soil-profile .
asls:soil-profile skos:hasTopConcept sp:mottle-boundary-C .
sp:mottle-boundary-D skos:topConceptOf asls:soil-profile .
asls:soil-profile skos:hasTopConcept sp:mottle-boundary-D .
sp:mottle-boundary-S skos:topConceptOf asls:soil-profile .
asls:soil-profile skos:hasTopConcept sp:mottle-boundary-S .
sp:mottle-colour-B skos:topConceptOf asls:soil-profile .
asls:soil-profile skos:hasTopConcept sp:mottle-colour-B .
sp:mottle-colour-D skos:topConceptOf asls:soil-profile .
asls:soil-profile skos:hasTopConcept sp:mottle-colour-D .
sp:mottle-colour-G skos:topConceptOf asls:soil-profile .
asls:soil-profile skos:hasTopConcept sp:mottle-colour-G .
sp:mottle-colour-L skos:topConceptOf asls:soil-profile .
asls:soil-profile skos:hasTopConcept sp:mottle-colour-L .
sp:mottle-colour-O skos:topConceptOf asls:soil-profile .
asls:soil-profile skos:hasTopConcept sp:mottle-colour-O .
sp:mottle-colour-P skos:topConceptOf asls:soil-profile .
asls:soil-profile skos:hasTopConcept sp:mottle-colour-P .
sp:mottle-colour-R skos:topConceptOf asls:soil-profile .
asls:soil-profile skos:hasTopConcept sp:mottle-colour-R .
sp:mottle-colour-Y skos:topConceptOf asls:soil-profile .
asls:soil-profile skos:hasTopConcept sp:mottle-colour-Y .
sp:mottle-contrast-D skos:topConceptOf asls:soil-profile .
asls:soil-profile skos:hasTopConcept sp:mottle-contrast-D .
sp:mottle-contrast-F skos:topConceptOf asls:soil-profile .
asls:soil-profile skos:hasTopConcept sp:mottle-contrast-F .
sp:mottle-contrast-P skos:topConceptOf asls:soil-profile .
asls:soil-profile skos:hasTopConcept sp:mottle-contrast-P .
sp:mottle-size-1 skos:topConceptOf asls:soil-profile .
asls:soil-profile skos:hasTopConcept sp:mottle-size-1 .
sp:mottle-size-2 skos:topConceptOf asls:soil-profile .
asls:soil-profile skos:hasTopConcept sp:mottle-size-2 .
sp:mottle-size-3 skos:topConceptOf asls:soil-profile .
asls:soil-profile skos:hasTopConcept sp:mottle-size-3 .
sp:mottle-size-4 skos:topConceptOf asls:soil-profile .
asls:soil-profile skos:hasTopConcept sp:mottle-size-4 .
sp:mottle-type-M skos:topConceptOf asls:soil-profile .
asls:soil-profile skos:hasTopConcept sp:mottle-type-M .
sp:mottle-type-X skos:topConceptOf asls:soil-profile .
asls:soil-profile skos:hasTopConcept sp:mottle-type-X .
sp:mottle-type-Y skos:topConceptOf asls:soil-profile .
asls:soil-profile skos:hasTopConcept sp:mottle-type-Y .
sp:mottle-type-Z skos:topConceptOf asls:soil-profile .
asls:soil-profile skos:hasTopConcept sp:mottle-type-Z .
sp:observation-type-A skos:topConceptOf asls:soil-profile .
asls:soil-profile skos:hasTopConcept sp:observation-type-A .
sp:observation-type-C skos:topConceptOf asls:soil-profile .
asls:soil-profile skos:hasTopConcept sp:observation-type-C .
sp:observation-type-E skos:topConceptOf asls:soil-profile .
asls:soil-profile skos:hasTopConcept sp:observation-type-E .
sp:observation-type-P skos:topConceptOf asls:soil-profile .
asls:soil-profile skos:hasTopConcept sp:observation-type-P .
sp:pans-cementation-0 skos:topConceptOf asls:soil-profile .
asls:soil-profile skos:hasTopConcept sp:pans-cementation-0 .
sp:pans-cementation-1 skos:topConceptOf asls:soil-profile .
asls:soil-profile skos:hasTopConcept sp:pans-cementation-1 .
sp:pans-cementation-2 skos:topConceptOf asls:soil-profile .
asls:soil-profile skos:hasTopConcept sp:pans-cementation-2 .
sp:pans-cementation-3 skos:topConceptOf asls:soil-profile .
asls:soil-profile skos:hasTopConcept sp:pans-cementation-3 .
sp:pans-cementation-4 skos:topConceptOf asls:soil-profile .
asls:soil-profile skos:hasTopConcept sp:pans-cementation-4 .
sp:pans-continuity-B skos:topConceptOf asls:soil-profile .
asls:soil-profile skos:hasTopConcept sp:pans-continuity-B .
sp:pans-continuity-C skos:topConceptOf asls:soil-profile .
asls:soil-profile skos:hasTopConcept sp:pans-continuity-C .
sp:pans-continuity-D skos:topConceptOf asls:soil-profile .
asls:soil-profile skos:hasTopConcept sp:pans-continuity-D .
sp:pans-structure-C skos:topConceptOf asls:soil-profile .
asls:soil-profile skos:hasTopConcept sp:pans-structure-C .
sp:pans-structure-L skos:topConceptOf asls:soil-profile .
asls:soil-profile skos:hasTopConcept sp:pans-structure-L .
sp:pans-structure-N skos:topConceptOf asls:soil-profile .
asls:soil-profile skos:hasTopConcept sp:pans-structure-N .
sp:pans-structure-R skos:topConceptOf asls:soil-profile .
asls:soil-profile skos:hasTopConcept sp:pans-structure-R .
sp:pans-structure-S skos:topConceptOf asls:soil-profile .
asls:soil-profile skos:hasTopConcept sp:pans-structure-S .
sp:pans-structure-V skos:topConceptOf asls:soil-profile .
asls:soil-profile skos:hasTopConcept sp:pans-structure-V .
sp:pans-type-A skos:topConceptOf asls:soil-profile .
asls:soil-profile skos:hasTopConcept sp:pans-type-A .
sp:pans-type-C skos:topConceptOf asls:soil-profile .
asls:soil-profile skos:hasTopConcept sp:pans-type-C .
sp:pans-type-D skos:topConceptOf asls:soil-profile .
asls:soil-profile skos:hasTopConcept sp:pans-type-D .
sp:pans-type-E skos:topConceptOf asls:soil-profile .
asls:soil-profile skos:hasTopConcept sp:pans-type-E .
sp:pans-type-F skos:topConceptOf asls:soil-profile .
asls:soil-profile skos:hasTopConcept sp:pans-type-F .
sp:pans-type-I skos:topConceptOf asls:soil-profile .
asls:soil-profile skos:hasTopConcept sp:pans-type-I .
sp:pans-type-K skos:topConceptOf asls:soil-profile .
asls:soil-profile skos:hasTopConcept sp:pans-type-K .
sp:pans-type-L skos:topConceptOf asls:soil-profile .
asls:soil-profile skos:hasTopConcept sp:pans-type-L .
sp:pans-type-M skos:topConceptOf asls:soil-profile .
asls:soil-profile skos:hasTopConcept sp:pans-type-M .
sp:pans-type-N skos:topConceptOf asls:soil-profile .
asls:soil-profile skos:hasTopConcept sp:pans-type-N .
sp:pans-type-O skos:topConceptOf asls:soil-profile .
asls:soil-profile skos:hasTopConcept sp:pans-type-O .
sp:pans-type-R skos:topConceptOf asls:soil-profile .
asls:soil-profile skos:hasTopConcept sp:pans-type-R .
sp:pans-type-T skos:topConceptOf asls:soil-profile .
asls:soil-profile skos:hasTopConcept sp:pans-type-T .
sp:pans-type-V skos:topConceptOf asls:soil-profile .
asls:soil-profile skos:hasTopConcept sp:pans-type-V .
sp:pans-type-Z skos:topConceptOf asls:soil-profile .
asls:soil-profile skos:hasTopConcept sp:pans-type-Z .
sp:particle-size-fraction-boulders skos:topConceptOf asls:soil-profile .
asls:soil-profile skos:hasTopConcept sp:particle-size-fraction-boulders .
sp:particle-size-fraction-clay skos:topConceptOf asls:soil-profile .
asls:soil-profile skos:hasTopConcept sp:particle-size-fraction-clay .
sp:particle-size-fraction-coarse-gravel skos:topConceptOf asls:soil-profile .
asls:soil-profile skos:hasTopConcept sp:particle-size-fraction-coarse-gravel .
sp:particle-size-fraction-cobbles skos:topConceptOf asls:soil-profile .
asls:soil-profile skos:hasTopConcept sp:particle-size-fraction-cobbles .
sp:particle-size-fraction-fine-clay skos:topConceptOf asls:soil-profile .
asls:soil-profile skos:hasTopConcept sp:particle-size-fraction-fine-clay .
sp:particle-size-fraction-fine-gravel skos:topConceptOf asls:soil-profile .
asls:soil-profile skos:hasTopConcept sp:particle-size-fraction-fine-gravel .
sp:particle-size-fraction-medium-gravel skos:topConceptOf asls:soil-profile .
asls:soil-profile skos:hasTopConcept sp:particle-size-fraction-medium-gravel .
sp:particle-size-fraction-sand skos:topConceptOf asls:soil-profile .
asls:soil-profile skos:hasTopConcept sp:particle-size-fraction-sand .
sp:particle-size-fraction-silt skos:topConceptOf asls:soil-profile .
asls:soil-profile skos:hasTopConcept sp:particle-size-fraction-silt .
sp:particle-size-fraction-stones skos:topConceptOf asls:soil-profile .
asls:soil-profile skos:hasTopConcept sp:particle-size-fraction-stones .
sp:roots-abundance-0 skos:topConceptOf asls:soil-profile .
asls:soil-profile skos:hasTopConcept sp:roots-abundance-0 .
sp:roots-abundance-1 skos:topConceptOf asls:soil-profile .
asls:soil-profile skos:hasTopConcept sp:roots-abundance-1 .
sp:roots-abundance-2 skos:topConceptOf asls:soil-profile .
asls:soil-profile skos:hasTopConcept sp:roots-abundance-2 .
sp:roots-abundance-3 skos:topConceptOf asls:soil-profile .
asls:soil-profile skos:hasTopConcept sp:roots-abundance-3 .
sp:roots-abundance-4 skos:topConceptOf asls:soil-profile .
asls:soil-profile skos:hasTopConcept sp:roots-abundance-4 .
sp:roots-size-1 skos:topConceptOf asls:soil-profile .
asls:soil-profile skos:hasTopConcept sp:roots-size-1 .
sp:roots-size-2 skos:topConceptOf asls:soil-profile .
asls:soil-profile skos:hasTopConcept sp:roots-size-2 .
sp:roots-size-3 skos:topConceptOf asls:soil-profile .
asls:soil-profile skos:hasTopConcept sp:roots-size-3 .
sp:roots-size-4 skos:topConceptOf asls:soil-profile .
asls:soil-profile skos:hasTopConcept sp:roots-size-4 .
sp:segregations-abundance-0 skos:topConceptOf asls:soil-profile .
asls:soil-profile skos:hasTopConcept sp:segregations-abundance-0 .
sp:segregations-abundance-1 skos:topConceptOf asls:soil-profile .
asls:soil-profile skos:hasTopConcept sp:segregations-abundance-1 .
sp:segregations-abundance-2 skos:topConceptOf asls:soil-profile .
asls:soil-profile skos:hasTopConcept sp:segregations-abundance-2 .
sp:segregations-abundance-3 skos:topConceptOf asls:soil-profile .
asls:soil-profile skos:hasTopConcept sp:segregations-abundance-3 .
sp:segregations-abundance-4 skos:topConceptOf asls:soil-profile .
asls:soil-profile skos:hasTopConcept sp:segregations-abundance-4 .
sp:segregations-abundance-5 skos:topConceptOf asls:soil-profile .
asls:soil-profile skos:hasTopConcept sp:segregations-abundance-5 .
sp:segregations-form-C skos:topConceptOf asls:soil-profile .
asls:soil-profile skos:hasTopConcept sp:segregations-form-C .
sp:segregations-form-F skos:topConceptOf asls:soil-profile .
asls:soil-profile skos:hasTopConcept sp:segregations-form-F .
sp:segregations-form-L skos:topConceptOf asls:soil-profile .
asls:soil-profile skos:hasTopConcept sp:segregations-form-L .
sp:segregations-form-N skos:topConceptOf asls:soil-profile .
asls:soil-profile skos:hasTopConcept sp:segregations-form-N .
sp:segregations-form-R skos:topConceptOf asls:soil-profile .
asls:soil-profile skos:hasTopConcept sp:segregations-form-R .
sp:segregations-form-S skos:topConceptOf asls:soil-profile .
asls:soil-profile skos:hasTopConcept sp:segregations-form-S .
sp:segregations-form-T skos:topConceptOf asls:soil-profile .
asls:soil-profile skos:hasTopConcept sp:segregations-form-T .
sp:segregations-form-V skos:topConceptOf asls:soil-profile .
asls:soil-profile skos:hasTopConcept sp:segregations-form-V .
sp:segregations-form-X skos:topConceptOf asls:soil-profile .
asls:soil-profile skos:hasTopConcept sp:segregations-form-X .
sp:segregations-magnetic-M skos:topConceptOf asls:soil-profile .
asls:soil-profile skos:hasTopConcept sp:segregations-magnetic-M .
sp:segregations-magnetic-N skos:topConceptOf asls:soil-profile .
asls:soil-profile skos:hasTopConcept sp:segregations-magnetic-N .
sp:segregations-nature-A skos:topConceptOf asls:soil-profile .
asls:soil-profile skos:hasTopConcept sp:segregations-nature-A .
sp:segregations-nature-E skos:topConceptOf asls:soil-profile .
asls:soil-profile skos:hasTopConcept sp:segregations-nature-E .
sp:segregations-nature-F skos:topConceptOf asls:soil-profile .
asls:soil-profile skos:hasTopConcept sp:segregations-nature-F .
sp:segregations-nature-G skos:topConceptOf asls:soil-profile .
asls:soil-profile skos:hasTopConcept sp:segregations-nature-G .
sp:segregations-nature-H skos:topConceptOf asls:soil-profile .
asls:soil-profile skos:hasTopConcept sp:segregations-nature-H .
sp:segregations-nature-K skos:topConceptOf asls:soil-profile .
asls:soil-profile skos:hasTopConcept sp:segregations-nature-K .
sp:segregations-nature-L skos:topConceptOf asls:soil-profile .
asls:soil-profile skos:hasTopConcept sp:segregations-nature-L .
sp:segregations-nature-M skos:topConceptOf asls:soil-profile .
asls:soil-profile skos:hasTopConcept sp:segregations-nature-M .
sp:segregations-nature-N skos:topConceptOf asls:soil-profile .
asls:soil-profile skos:hasTopConcept sp:segregations-nature-N .
sp:segregations-nature-O skos:topConceptOf asls:soil-profile .
asls:soil-profile skos:hasTopConcept sp:segregations-nature-O .
sp:segregations-nature-S skos:topConceptOf asls:soil-profile .
asls:soil-profile skos:hasTopConcept sp:segregations-nature-S .
sp:segregations-nature-U skos:topConceptOf asls:soil-profile .
asls:soil-profile skos:hasTopConcept sp:segregations-nature-U .
sp:segregations-nature-Y skos:topConceptOf asls:soil-profile .
asls:soil-profile skos:hasTopConcept sp:segregations-nature-Y .
sp:segregations-nature-Z skos:topConceptOf asls:soil-profile .
asls:soil-profile skos:hasTopConcept sp:segregations-nature-Z .
sp:segregations-size-1 skos:topConceptOf asls:soil-profile .
asls:soil-profile skos:hasTopConcept sp:segregations-size-1 .
sp:segregations-size-2 skos:topConceptOf asls:soil-profile .
asls:soil-profile skos:hasTopConcept sp:segregations-size-2 .
sp:segregations-size-3 skos:topConceptOf asls:soil-profile .
asls:soil-profile skos:hasTopConcept sp:segregations-size-3 .
sp:segregations-size-4 skos:topConceptOf asls:soil-profile .
asls:soil-profile skos:hasTopConcept sp:segregations-size-4 .
sp:segregations-size-5 skos:topConceptOf asls:soil-profile .
asls:soil-profile skos:hasTopConcept sp:segregations-size-5 .
sp:segregations-strength-1 skos:topConceptOf asls:soil-profile .
asls:soil-profile skos:hasTopConcept sp:segregations-strength-1 .
sp:segregations-strength-2 skos:topConceptOf asls:soil-profile .
asls:soil-profile skos:hasTopConcept sp:segregations-strength-2 .
sp:soil-water-drainage-1 skos:topConceptOf asls:soil-profile .
asls:soil-profile skos:hasTopConcept sp:soil-water-drainage-1 .
sp:soil-water-drainage-2 skos:topConceptOf asls:soil-profile .
asls:soil-profile skos:hasTopConcept sp:soil-water-drainage-2 .
sp:soil-water-drainage-3 skos:topConceptOf asls:soil-profile .
asls:soil-profile skos:hasTopConcept sp:soil-water-drainage-3 .
sp:soil-water-drainage-4 skos:topConceptOf asls:soil-profile .
asls:soil-profile skos:hasTopConcept sp:soil-water-drainage-4 .
sp:soil-water-drainage-5 skos:topConceptOf asls:soil-profile .
asls:soil-profile skos:hasTopConcept sp:soil-water-drainage-5 .
sp:soil-water-drainage-6 skos:topConceptOf asls:soil-profile .
asls:soil-profile skos:hasTopConcept sp:soil-water-drainage-6 .
sp:soil-water-permeability-1 skos:topConceptOf asls:soil-profile .
asls:soil-profile skos:hasTopConcept sp:soil-water-permeability-1 .
sp:soil-water-permeability-2 skos:topConceptOf asls:soil-profile .
asls:soil-profile skos:hasTopConcept sp:soil-water-permeability-2 .
sp:soil-water-permeability-3 skos:topConceptOf asls:soil-profile .
asls:soil-profile skos:hasTopConcept sp:soil-water-permeability-3 .
sp:soil-water-permeability-4 skos:topConceptOf asls:soil-profile .
asls:soil-profile skos:hasTopConcept sp:soil-water-permeability-4 .
sp:soil-water-status-D skos:topConceptOf asls:soil-profile .
asls:soil-profile skos:hasTopConcept sp:soil-water-status-D .
sp:soil-water-status-M skos:topConceptOf asls:soil-profile .
asls:soil-profile skos:hasTopConcept sp:soil-water-status-M .
sp:soil-water-status-T skos:topConceptOf asls:soil-profile .
asls:soil-profile skos:hasTopConcept sp:soil-water-status-T .
sp:soil-water-status-W skos:topConceptOf asls:soil-profile .
asls:soil-profile skos:hasTopConcept sp:soil-water-status-W .
sp:structure-artificial-CL skos:topConceptOf asls:soil-profile .
asls:soil-profile skos:hasTopConcept sp:structure-artificial-CL .
sp:structure-artificial-FR skos:topConceptOf asls:soil-profile .
asls:soil-profile skos:hasTopConcept sp:structure-artificial-FR .
sp:structure-pedality-grade-G skos:topConceptOf asls:soil-profile .
asls:soil-profile skos:hasTopConcept sp:structure-pedality-grade-G .
sp:structure-pedality-grade-M skos:topConceptOf asls:soil-profile .
asls:soil-profile skos:hasTopConcept sp:structure-pedality-grade-M .
sp:structure-pedality-grade-S skos:topConceptOf asls:soil-profile .
asls:soil-profile skos:hasTopConcept sp:structure-pedality-grade-S .
sp:structure-pedality-grade-V skos:topConceptOf asls:soil-profile .
asls:soil-profile skos:hasTopConcept sp:structure-pedality-grade-V .
sp:structure-pedality-grade-W skos:topConceptOf asls:soil-profile .
asls:soil-profile skos:hasTopConcept sp:structure-pedality-grade-W .
sp:structure-pedality-size-1 skos:topConceptOf asls:soil-profile .
asls:soil-profile skos:hasTopConcept sp:structure-pedality-size-1 .
sp:structure-pedality-size-2 skos:topConceptOf asls:soil-profile .
asls:soil-profile skos:hasTopConcept sp:structure-pedality-size-2 .
sp:structure-pedality-size-3 skos:topConceptOf asls:soil-profile .
asls:soil-profile skos:hasTopConcept sp:structure-pedality-size-3 .
sp:structure-pedality-size-4 skos:topConceptOf asls:soil-profile .
asls:soil-profile skos:hasTopConcept sp:structure-pedality-size-4 .
sp:structure-pedality-size-5 skos:topConceptOf asls:soil-profile .
asls:soil-profile skos:hasTopConcept sp:structure-pedality-size-5 .
sp:structure-pedality-size-6 skos:topConceptOf asls:soil-profile .
asls:soil-profile skos:hasTopConcept sp:structure-pedality-size-6 .
sp:structure-pedality-size-7 skos:topConceptOf asls:soil-profile .
asls:soil-profile skos:hasTopConcept sp:structure-pedality-size-7 .
sp:structure-pedality-size-8 skos:topConceptOf asls:soil-profile .
asls:soil-profile skos:hasTopConcept sp:structure-pedality-size-8 .
sp:structure-pedality-size-9 skos:topConceptOf asls:soil-profile .
asls:soil-profile skos:hasTopConcept sp:structure-pedality-size-9 .
sp:structure-pedality-type-AB skos:topConceptOf asls:soil-profile .
asls:soil-profile skos:hasTopConcept sp:structure-pedality-type-AB .
sp:structure-pedality-type-CA skos:topConceptOf asls:soil-profile .
asls:soil-profile skos:hasTopConcept sp:structure-pedality-type-CA .
sp:structure-pedality-type-CO skos:topConceptOf asls:soil-profile .
asls:soil-profile skos:hasTopConcept sp:structure-pedality-type-CO .
sp:structure-pedality-type-GR skos:topConceptOf asls:soil-profile .
asls:soil-profile skos:hasTopConcept sp:structure-pedality-type-GR .
sp:structure-pedality-type-LE skos:topConceptOf asls:soil-profile .
asls:soil-profile skos:hasTopConcept sp:structure-pedality-type-LE .
sp:structure-pedality-type-PL skos:topConceptOf asls:soil-profile .
asls:soil-profile skos:hasTopConcept sp:structure-pedality-type-PL .
sp:structure-pedality-type-PO skos:topConceptOf asls:soil-profile .
asls:soil-profile skos:hasTopConcept sp:structure-pedality-type-PO .
sp:structure-pedality-type-PR skos:topConceptOf asls:soil-profile .
asls:soil-profile skos:hasTopConcept sp:structure-pedality-type-PR .
sp:structure-pedality-type-SB skos:topConceptOf asls:soil-profile .
asls:soil-profile skos:hasTopConcept sp:structure-pedality-type-SB .
sp:surfacecondition-C skos:topConceptOf asls:soil-profile .
asls:soil-profile skos:hasTopConcept sp:surfacecondition-C .
sp:surfacecondition-F skos:topConceptOf asls:soil-profile .
asls:soil-profile skos:hasTopConcept sp:surfacecondition-F .
sp:surfacecondition-G skos:topConceptOf asls:soil-profile .
asls:soil-profile skos:hasTopConcept sp:surfacecondition-G .
sp:surfacecondition-H skos:topConceptOf asls:soil-profile .
asls:soil-profile skos:hasTopConcept sp:surfacecondition-H .
sp:surfacecondition-L skos:topConceptOf asls:soil-profile .
asls:soil-profile skos:hasTopConcept sp:surfacecondition-L .
sp:surfacecondition-M skos:topConceptOf asls:soil-profile .
asls:soil-profile skos:hasTopConcept sp:surfacecondition-M .
sp:surfacecondition-O skos:topConceptOf asls:soil-profile .
asls:soil-profile skos:hasTopConcept sp:surfacecondition-O .
sp:surfacecondition-P skos:topConceptOf asls:soil-profile .
asls:soil-profile skos:hasTopConcept sp:surfacecondition-P .
sp:surfacecondition-R skos:topConceptOf asls:soil-profile .
asls:soil-profile skos:hasTopConcept sp:surfacecondition-R .
sp:surfacecondition-S skos:topConceptOf asls:soil-profile .
asls:soil-profile skos:hasTopConcept sp:surfacecondition-S .
sp:surfacecondition-T skos:topConceptOf asls:soil-profile .
asls:soil-profile skos:hasTopConcept sp:surfacecondition-T .
sp:surfacecondition-X skos:topConceptOf asls:soil-profile .
asls:soil-profile skos:hasTopConcept sp:surfacecondition-X .
sp:surfacecondition-Y skos:topConceptOf asls:soil-profile .
asls:soil-profile skos:hasTopConcept sp:surfacecondition-Y .
sp:surfacecondition-Z skos:topConceptOf asls:soil-profile .
asls:soil-profile skos:hasTopConcept sp:surfacecondition-Z .
sp:voids-cracks-1 skos:topConceptOf asls:soil-profile .
asls:soil-profile skos:hasTopConcept sp:voids-cracks-1 .
sp:voids-cracks-2 skos:topConceptOf asls:soil-profile .
asls:soil-profile skos:hasTopConcept sp:voids-cracks-2 .
sp:voids-cracks-3 skos:topConceptOf asls:soil-profile .
asls:soil-profile skos:hasTopConcept sp:voids-cracks-3 .
sp:voids-cracks-4 skos:topConceptOf asls:soil-profile .
asls:soil-profile skos:hasTopConcept sp:voids-cracks-4 .
sp:voids-cracks-5 skos:topConceptOf asls:soil-profile .
asls:soil-profile skos:hasTopConcept sp:voids-cracks-5 .
sp:voids-macropores-abundance-0 skos:topConceptOf asls:soil-profile .
asls:soil-profile skos:hasTopConcept sp:voids-macropores-abundance-0 .
sp:voids-macropores-abundance-1 skos:topConceptOf asls:soil-profile .
asls:soil-profile skos:hasTopConcept sp:voids-macropores-abundance-1 .
sp:voids-macropores-abundance-2 skos:topConceptOf asls:soil-profile .
asls:soil-profile skos:hasTopConcept sp:voids-macropores-abundance-2 .
sp:voids-macropores-abundance-3 skos:topConceptOf asls:soil-profile .
asls:soil-profile skos:hasTopConcept sp:voids-macropores-abundance-3 .
sp:voids-macropores-abundance-4 skos:topConceptOf asls:soil-profile .
asls:soil-profile skos:hasTopConcept sp:voids-macropores-abundance-4 .
sp:voids-macropores-abundance-5 skos:topConceptOf asls:soil-profile .
asls:soil-profile skos:hasTopConcept sp:voids-macropores-abundance-5 .
sp:voids-macropores-abundance-6 skos:topConceptOf asls:soil-profile .
asls:soil-profile skos:hasTopConcept sp:voids-macropores-abundance-6 .
sp:voids-macropores-diameter-1 skos:topConceptOf asls:soil-profile .
asls:soil-profile skos:hasTopConcept sp:voids-macropores-diameter-1 .
sp:voids-macropores-diameter-2 skos:topConceptOf asls:soil-profile .
asls:soil-profile skos:hasTopConcept sp:voids-macropores-diameter-2 .
sp:voids-macropores-diameter-3 skos:topConceptOf asls:soil-profile .
asls:soil-profile skos:hasTopConcept sp:voids-macropores-diameter-3 .
sp:voids-macropores-diameter-4 skos:topConceptOf asls:soil-profile .
asls:soil-profile skos:hasTopConcept sp:voids-macropores-diameter-4 .
sp:voids-micropores skos:topConceptOf asls:soil-profile .
asls:soil-profile skos:hasTopConcept sp:voids-micropores .
sp:water-repellence-N skos:topConceptOf asls:soil-profile .
asls:soil-profile skos:hasTopConcept sp:water-repellence-N .
sp:water-repellence-R skos:topConceptOf asls:soil-profile .
asls:soil-profile skos:hasTopConcept sp:water-repellence-R .
sp:water-repellence-S skos:topConceptOf asls:soil-profile .
asls:soil-profile skos:hasTopConcept sp:water-repellence-S .
subst:lithology-AC skos:topConceptOf asls:soil-profile .
asls:soil-profile skos:hasTopConcept subst:lithology-AC .
subst:lithology-AD skos:topConceptOf asls:soil-profile .
asls:soil-profile skos:hasTopConcept subst:lithology-AD .
subst:lithology-AF skos:topConceptOf asls:soil-profile .
asls:soil-profile skos:hasTopConcept subst:lithology-AF .
subst:lithology-AG skos:topConceptOf asls:soil-profile .
asls:soil-profile skos:hasTopConcept subst:lithology-AG .
subst:lithology-AH skos:topConceptOf asls:soil-profile .
asls:soil-profile skos:hasTopConcept subst:lithology-AH .
subst:lithology-AM skos:topConceptOf asls:soil-profile .
asls:soil-profile skos:hasTopConcept subst:lithology-AM .
subst:lithology-AN skos:topConceptOf asls:soil-profile .
asls:soil-profile skos:hasTopConcept subst:lithology-AN .
subst:lithology-AP skos:topConceptOf asls:soil-profile .
asls:soil-profile skos:hasTopConcept subst:lithology-AP .
subst:lithology-AR skos:topConceptOf asls:soil-profile .
asls:soil-profile skos:hasTopConcept subst:lithology-AR .
subst:lithology-AS skos:topConceptOf asls:soil-profile .
asls:soil-profile skos:hasTopConcept subst:lithology-AS .
subst:lithology-BA skos:topConceptOf asls:soil-profile .
asls:soil-profile skos:hasTopConcept subst:lithology-BA .
subst:lithology-BB skos:topConceptOf asls:soil-profile .
asls:soil-profile skos:hasTopConcept subst:lithology-BB .
subst:lithology-BO skos:topConceptOf asls:soil-profile .
asls:soil-profile skos:hasTopConcept subst:lithology-BO .
subst:lithology-BR skos:topConceptOf asls:soil-profile .
asls:soil-profile skos:hasTopConcept subst:lithology-BR .
subst:lithology-C skos:topConceptOf asls:soil-profile .
asls:soil-profile skos:hasTopConcept subst:lithology-C .
subst:lithology-CB skos:topConceptOf asls:soil-profile .
asls:soil-profile skos:hasTopConcept subst:lithology-CB .
subst:lithology-CG skos:topConceptOf asls:soil-profile .
asls:soil-profile skos:hasTopConcept subst:lithology-CG .
subst:lithology-CH skos:topConceptOf asls:soil-profile .
asls:soil-profile skos:hasTopConcept subst:lithology-CH .
subst:lithology-CO skos:topConceptOf asls:soil-profile .
asls:soil-profile skos:hasTopConcept subst:lithology-CO .
subst:lithology-CU skos:topConceptOf asls:soil-profile .
asls:soil-profile skos:hasTopConcept subst:lithology-CU .
subst:lithology-DI skos:topConceptOf asls:soil-profile .
asls:soil-profile skos:hasTopConcept subst:lithology-DI .
subst:lithology-DM skos:topConceptOf asls:soil-profile .
asls:soil-profile skos:hasTopConcept subst:lithology-DM .
subst:lithology-DR skos:topConceptOf asls:soil-profile .
asls:soil-profile skos:hasTopConcept subst:lithology-DR .
subst:lithology-FC skos:topConceptOf asls:soil-profile .
asls:soil-profile skos:hasTopConcept subst:lithology-FC .
subst:lithology-GA skos:topConceptOf asls:soil-profile .
asls:soil-profile skos:hasTopConcept subst:lithology-GA .
subst:lithology-GD skos:topConceptOf asls:soil-profile .
asls:soil-profile skos:hasTopConcept subst:lithology-GD .
subst:lithology-GE skos:topConceptOf asls:soil-profile .
asls:soil-profile skos:hasTopConcept subst:lithology-GE .
subst:lithology-GN skos:topConceptOf asls:soil-profile .
asls:soil-profile skos:hasTopConcept subst:lithology-GN .
subst:lithology-GR skos:topConceptOf asls:soil-profile .
asls:soil-profile skos:hasTopConcept subst:lithology-GR .
subst:lithology-GS skos:topConceptOf asls:soil-profile .
asls:soil-profile skos:hasTopConcept subst:lithology-GS .
subst:lithology-GV skos:topConceptOf asls:soil-profile .
asls:soil-profile skos:hasTopConcept subst:lithology-GV .
subst:lithology-GW skos:topConceptOf asls:soil-profile .
asls:soil-profile skos:hasTopConcept subst:lithology-GW .
subst:lithology-GY skos:topConceptOf asls:soil-profile .
asls:soil-profile skos:hasTopConcept subst:lithology-GY .
subst:lithology-HA skos:topConceptOf asls:soil-profile .
asls:soil-profile skos:hasTopConcept subst:lithology-HA .
subst:lithology-HO skos:topConceptOf asls:soil-profile .
asls:soil-profile skos:hasTopConcept subst:lithology-HO .
subst:lithology-IG skos:topConceptOf asls:soil-profile .
asls:soil-profile skos:hasTopConcept subst:lithology-IG .
subst:lithology-JA skos:topConceptOf asls:soil-profile .
asls:soil-profile skos:hasTopConcept subst:lithology-JA .
subst:lithology-KA skos:topConceptOf asls:soil-profile .
asls:soil-profile skos:hasTopConcept subst:lithology-KA .
subst:lithology-KC skos:topConceptOf asls:soil-profile .
asls:soil-profile skos:hasTopConcept subst:lithology-KC .
subst:lithology-KL skos:topConceptOf asls:soil-profile .
asls:soil-profile skos:hasTopConcept subst:lithology-KL .
subst:lithology-KM skos:topConceptOf asls:soil-profile .
asls:soil-profile skos:hasTopConcept subst:lithology-KM .
subst:lithology-KR skos:topConceptOf asls:soil-profile .
asls:soil-profile skos:hasTopConcept subst:lithology-KR .
subst:lithology-KS skos:topConceptOf asls:soil-profile .
asls:soil-profile skos:hasTopConcept subst:lithology-KS .
subst:lithology-LC skos:topConceptOf asls:soil-profile .
asls:soil-profile skos:hasTopConcept subst:lithology-LC .
subst:lithology-LI skos:topConceptOf asls:soil-profile .
asls:soil-profile skos:hasTopConcept subst:lithology-LI .
subst:lithology-M skos:topConceptOf asls:soil-profile .
asls:soil-profile skos:hasTopConcept subst:lithology-M .
subst:lithology-MB skos:topConceptOf asls:soil-profile .
asls:soil-profile skos:hasTopConcept subst:lithology-MB .
subst:lithology-MD skos:topConceptOf asls:soil-profile .
asls:soil-profile skos:hasTopConcept subst:lithology-MD .
subst:lithology-ME skos:topConceptOf asls:soil-profile .
asls:soil-profile skos:hasTopConcept subst:lithology-ME .
subst:lithology-MG skos:topConceptOf asls:soil-profile .
asls:soil-profile skos:hasTopConcept subst:lithology-MG .
subst:lithology-MI skos:topConceptOf asls:soil-profile .
asls:soil-profile skos:hasTopConcept subst:lithology-MI .
subst:lithology-ML skos:topConceptOf asls:soil-profile .
asls:soil-profile skos:hasTopConcept subst:lithology-ML .
subst:lithology-MS skos:topConceptOf asls:soil-profile .
asls:soil-profile skos:hasTopConcept subst:lithology-MS .
subst:lithology-MU skos:topConceptOf asls:soil-profile .
asls:soil-profile skos:hasTopConcept subst:lithology-MU .
subst:lithology-MY skos:topConceptOf asls:soil-profile .
asls:soil-profile skos:hasTopConcept subst:lithology-MY .
subst:lithology-PC skos:topConceptOf asls:soil-profile .
asls:soil-profile skos:hasTopConcept subst:lithology-PC .
subst:lithology-PE skos:topConceptOf asls:soil-profile .
asls:soil-profile skos:hasTopConcept subst:lithology-PE .
subst:lithology-PG skos:topConceptOf asls:soil-profile .
asls:soil-profile skos:hasTopConcept subst:lithology-PG .
subst:lithology-PH skos:topConceptOf asls:soil-profile .
asls:soil-profile skos:hasTopConcept subst:lithology-PH .
subst:lithology-PL skos:topConceptOf asls:soil-profile .
asls:soil-profile skos:hasTopConcept subst:lithology-PL .
subst:lithology-PO skos:topConceptOf asls:soil-profile .
asls:soil-profile skos:hasTopConcept subst:lithology-PO .
subst:lithology-PY skos:topConceptOf asls:soil-profile .
asls:soil-profile skos:hasTopConcept subst:lithology-PY .
subst:lithology-QP skos:topConceptOf asls:soil-profile .
asls:soil-profile skos:hasTopConcept subst:lithology-QP .
subst:lithology-QS skos:topConceptOf asls:soil-profile .
asls:soil-profile skos:hasTopConcept subst:lithology-QS .
subst:lithology-QU skos:topConceptOf asls:soil-profile .
asls:soil-profile skos:hasTopConcept subst:lithology-QU .
subst:lithology-QZ skos:topConceptOf asls:soil-profile .
asls:soil-profile skos:hasTopConcept subst:lithology-QZ .
subst:lithology-R skos:topConceptOf asls:soil-profile .
asls:soil-profile skos:hasTopConcept subst:lithology-R .
subst:lithology-RB skos:topConceptOf asls:soil-profile .
asls:soil-profile skos:hasTopConcept subst:lithology-RB .
subst:lithology-RH skos:topConceptOf asls:soil-profile .
asls:soil-profile skos:hasTopConcept subst:lithology-RH .
subst:lithology-S skos:topConceptOf asls:soil-profile .
asls:soil-profile skos:hasTopConcept subst:lithology-S .
subst:lithology-SA skos:topConceptOf asls:soil-profile .
asls:soil-profile skos:hasTopConcept subst:lithology-SA .
subst:lithology-SD skos:topConceptOf asls:soil-profile .
asls:soil-profile skos:hasTopConcept subst:lithology-SD .
subst:lithology-SH skos:topConceptOf asls:soil-profile .
asls:soil-profile skos:hasTopConcept subst:lithology-SH .
subst:lithology-SK skos:topConceptOf asls:soil-profile .
asls:soil-profile skos:hasTopConcept subst:lithology-SK .
subst:lithology-SL skos:topConceptOf asls:soil-profile .
asls:soil-profile skos:hasTopConcept subst:lithology-SL .
subst:lithology-SN skos:topConceptOf asls:soil-profile .
asls:soil-profile skos:hasTopConcept subst:lithology-SN .
subst:lithology-SR skos:topConceptOf asls:soil-profile .
asls:soil-profile skos:hasTopConcept subst:lithology-SR .
subst:lithology-ST skos:topConceptOf asls:soil-profile .
asls:soil-profile skos:hasTopConcept subst:lithology-ST .
subst:lithology-SY skos:topConceptOf asls:soil-profile .
asls:soil-profile skos:hasTopConcept subst:lithology-SY .
subst:lithology-TR skos:topConceptOf asls:soil-profile .
asls:soil-profile skos:hasTopConcept subst:lithology-TR .
subst:lithology-TU skos:topConceptOf asls:soil-profile .
asls:soil-profile skos:hasTopConcept subst:lithology-TU .
subst:lithology-UC skos:topConceptOf asls:soil-profile .
asls:soil-profile skos:hasTopConcept subst:lithology-UC .
subst:lithology-VB skos:topConceptOf asls:soil-profile .
asls:soil-profile skos:hasTopConcept subst:lithology-VB .
subst:lithology-VG skos:topConceptOf asls:soil-profile .
asls:soil-profile skos:hasTopConcept subst:lithology-VG .
subst:lithology-Z skos:topConceptOf asls:soil-profile .
asls:soil-profile skos:hasTopConcept subst:lithology-Z .
subst:lithology-ZS skos:topConceptOf asls:soil-profile .
asls:soil-profile skos:hasTopConcept subst:lithology-ZS .
subst:material-strength-M skos:topConceptOf asls:soil-profile .
asls:soil-profile skos:hasTopConcept subst:material-strength-M .
subst:material-strength-S skos:topConceptOf asls:soil-profile .
asls:soil-profile skos:hasTopConcept subst:material-strength-S .
subst:material-strength-VS skos:topConceptOf asls:soil-profile .
asls:soil-profile skos:hasTopConcept subst:material-strength-VS .
subst:material-strength-VW skos:topConceptOf asls:soil-profile .
asls:soil-profile skos:hasTopConcept subst:material-strength-VW .
subst:material-strength-W skos:topConceptOf asls:soil-profile .
asls:soil-profile skos:hasTopConcept subst:material-strength-W .